<?xml version="1.0"?>
<rdf:RDF xmlns="https://savage.nps.edu/EthicalControl/ontologies/MissionExecutionOntology"
     xml:base="https://savage.nps.edu/EthicalControl/ontologies/MissionExecutionOntology"
     xmlns:meo="https://savage.nps.edu/EthicalControl/ontologies/MissionExecutionOntology#"
     xmlns:owl="http://www.w3.org/2002/07/owl#"
     xmlns:rdf="http://www.w3.org/1999/02/22-rdf-syntax-ns#"
     xmlns:xml="http://www.w3.org/XML/1998/namespace"
     xmlns:xsd="http://www.w3.org/2001/XMLSchema#"
     xmlns:rdfs="http://www.w3.org/2000/01/rdf-schema#">
    <owl:Ontology rdf:about="https://savage.nps.edu/EthicalControl/ontologies/MissionExecutionOntology"/>
    


    <!-- 
    ///////////////////////////////////////////////////////////////////////////////////////
    //
    // Object Properties
    //
    ///////////////////////////////////////////////////////////////////////////////////////
     -->

    


    <!-- https://savage.nps.edu/EthicalControl/ontologies/MissionExecutionOntology#accomplishes -->

    <owl:ObjectProperty rdf:about="https://savage.nps.edu/EthicalControl/ontologies/MissionExecutionOntology#accomplishes">
        <rdfs:domain rdf:resource="https://savage.nps.edu/EthicalControl/ontologies/MissionExecutionOntology#EndCondition"/>
        <rdfs:range rdf:resource="https://savage.nps.edu/EthicalControl/ontologies/MissionExecutionOntology#IntendedOutcome"/>
        <rdfs:comment>The identified EndCondition must be accomplished to satisfy the identified IntendedOutcome.</rdfs:comment>
    </owl:ObjectProperty>
    


    <!-- https://savage.nps.edu/EthicalControl/ontologies/MissionExecutionOntology#canAchieve -->

    <owl:ObjectProperty rdf:about="https://savage.nps.edu/EthicalControl/ontologies/MissionExecutionOntology#canAchieve">
        <rdfs:domain rdf:resource="https://savage.nps.edu/EthicalControl/ontologies/MissionExecutionOntology#Vehicle"/>
        <rdfs:range rdf:resource="https://savage.nps.edu/EthicalControl/ontologies/MissionExecutionOntology#IntendedOutcome"/>
        <owl:propertyChainAxiom rdf:parseType="Collection">
            <rdf:Description rdf:about="https://savage.nps.edu/EthicalControl/ontologies/MissionExecutionOntology#hasFeature"/>
            <rdf:Description rdf:about="https://savage.nps.edu/EthicalControl/ontologies/MissionExecutionOntology#canFulfill"/>
        </owl:propertyChainAxiom>
        <rdfs:comment>A Vehicle meets one or more IntendedOutcome instances, meaning the Vehicle has at least one VehicleFeature instance that &quot;canFulfill&quot; each IntendedOutcome (&quot;canAchieve&quot; is implied by the composition of &quot;hasFeature&quot; and &quot;canFulfill&quot;).</rdfs:comment>
    </owl:ObjectProperty>
    <owl:Axiom>
        <owl:annotatedSource rdf:resource="https://savage.nps.edu/EthicalControl/ontologies/MissionExecutionOntology#canAchieve"/>
        <owl:annotatedProperty rdf:resource="http://www.w3.org/2002/07/owl#propertyChainAxiom"/>
        <owl:annotatedTarget rdf:parseType="Collection">
            <rdf:Description rdf:about="https://savage.nps.edu/EthicalControl/ontologies/MissionExecutionOntology#hasFeature"/>
            <rdf:Description rdf:about="https://savage.nps.edu/EthicalControl/ontologies/MissionExecutionOntology#canFulfill"/>
        </owl:annotatedTarget>
        <rdfs:comment>A Vehicle meets a GoalRequirement if and only if it has a VehicleFeature that can fulfill that GoalRequirement.

[NOTE: Here we have expressed the chain &quot;hasVehicleFeature o canFulfill&quot; as a SubProptertyOf meetsRequirements . We have not found how to express the reverse assertion in Protege to obtain equivalency. Perhaps it should be acceptable to have a Vehicle that is said to directly meet a GoalRequirement (through relation meetsRequirement] without the added detail of an explicit VehicleFeature that canFulfill that GoalRequirement?]</rdfs:comment>
        <rdfs:label>V3 (partial)</rdfs:label>
    </owl:Axiom>
    


    <!-- https://savage.nps.edu/EthicalControl/ontologies/MissionExecutionOntology#canFulfill -->

    <owl:ObjectProperty rdf:about="https://savage.nps.edu/EthicalControl/ontologies/MissionExecutionOntology#canFulfill">
        <rdfs:domain rdf:resource="https://savage.nps.edu/EthicalControl/ontologies/MissionExecutionOntology#VehicleFeature"/>
        <rdfs:range rdf:resource="https://savage.nps.edu/EthicalControl/ontologies/MissionExecutionOntology#IntendedOutcome"/>
        <rdfs:comment>A VehicleFeature can fulfill one or more IntendedOutcome instances.</rdfs:comment>
    </owl:ObjectProperty>
    <owl:Axiom>
        <owl:annotatedSource rdf:resource="https://savage.nps.edu/EthicalControl/ontologies/MissionExecutionOntology#canFulfill"/>
        <owl:annotatedProperty rdf:resource="http://www.w3.org/2000/01/rdf-schema#range"/>
        <owl:annotatedTarget rdf:resource="https://savage.nps.edu/EthicalControl/ontologies/MissionExecutionOntology#IntendedOutcome"/>
        <rdfs:comment>A VehicleFeature can only fulfill GoalRequirements.</rdfs:comment>
        <rdfs:label>F1</rdfs:label>
    </owl:Axiom>
    


    <!-- https://savage.nps.edu/EthicalControl/ontologies/MissionExecutionOntology#canIdentify -->

    <owl:ObjectProperty rdf:about="https://savage.nps.edu/EthicalControl/ontologies/MissionExecutionOntology#canIdentify">
        <rdfs:domain rdf:resource="https://savage.nps.edu/EthicalControl/ontologies/MissionExecutionOntology#Vehicle"/>
        <rdfs:range rdf:resource="https://savage.nps.edu/EthicalControl/ontologies/MissionExecutionOntology#DADM_Constraints"/>
        <owl:propertyChainAxiom rdf:parseType="Collection">
            <rdf:Description rdf:about="https://savage.nps.edu/EthicalControl/ontologies/MissionExecutionOntology#hasFeature"/>
            <rdf:Description rdf:about="https://savage.nps.edu/EthicalControl/ontologies/MissionExecutionOntology#canMeasure"/>
        </owl:propertyChainAxiom>
        <rdfs:comment>A Vehicle can identify one or more Constraint instances, meaning that the Vehicle has the technical ability to make and discern measurements relating to a Constraint (e.g., an impending position exception, an impending depth exception, etc.).</rdfs:comment>
    </owl:ObjectProperty>
    <owl:Axiom>
        <owl:annotatedSource rdf:resource="https://savage.nps.edu/EthicalControl/ontologies/MissionExecutionOntology#canIdentify"/>
        <owl:annotatedProperty rdf:resource="http://www.w3.org/2002/07/owl#propertyChainAxiom"/>
        <owl:annotatedTarget rdf:parseType="Collection">
            <rdf:Description rdf:about="https://savage.nps.edu/EthicalControl/ontologies/MissionExecutionOntology#hasFeature"/>
            <rdf:Description rdf:about="https://savage.nps.edu/EthicalControl/ontologies/MissionExecutionOntology#canMeasure"/>
        </owl:annotatedTarget>
        <rdfs:comment>If a Vehicle has a VehicleFeature that can test a Constraint, then that Vehicle can identify that Constraint.</rdfs:comment>
        <rdfs:label>V4</rdfs:label>
    </owl:Axiom>
    


    <!-- https://savage.nps.edu/EthicalControl/ontologies/MissionExecutionOntology#canMeasure -->

    <owl:ObjectProperty rdf:about="https://savage.nps.edu/EthicalControl/ontologies/MissionExecutionOntology#canMeasure">
        <rdfs:domain rdf:resource="https://savage.nps.edu/EthicalControl/ontologies/MissionExecutionOntology#VehicleFeature"/>
        <rdfs:range rdf:resource="https://savage.nps.edu/EthicalControl/ontologies/MissionExecutionOntology#EndCondition"/>
        <rdfs:comment>A VehicleFeature can measure phenomena necessary to address one or more EndCondition instances, meaning the VehicleFeature has the capability to measure and discern the conditions stated in each EndCondition.</rdfs:comment>
    </owl:ObjectProperty>
    <owl:Axiom>
        <owl:annotatedSource rdf:resource="https://savage.nps.edu/EthicalControl/ontologies/MissionExecutionOntology#canMeasure"/>
        <owl:annotatedProperty rdf:resource="http://www.w3.org/2000/01/rdf-schema#range"/>
        <owl:annotatedTarget rdf:resource="https://savage.nps.edu/EthicalControl/ontologies/MissionExecutionOntology#EndCondition"/>
        <rdfs:comment>A VehicleFeature can only test Constraints.</rdfs:comment>
        <rdfs:label>F2</rdfs:label>
    </owl:Axiom>
    


    <!-- https://savage.nps.edu/EthicalControl/ontologies/MissionExecutionOntology#canMeet -->

    <owl:ObjectProperty rdf:about="https://savage.nps.edu/EthicalControl/ontologies/MissionExecutionOntology#canMeet">
        <owl:inverseOf rdf:resource="https://savage.nps.edu/EthicalControl/ontologies/MissionExecutionOntology/isMetBy"/>
        <rdfs:domain rdf:resource="https://savage.nps.edu/EthicalControl/ontologies/MissionExecutionOntology#Vehicle"/>
        <rdfs:range rdf:resource="https://savage.nps.edu/EthicalControl/ontologies/MissionExecutionOntology#Goal"/>
        <rdfs:comment>A Vehicle can meet one or more Goal instances, meaning the Vehicle has the physical capabilities to perform actions that can achieve the Goal. This is an indication of achievability, not actual achievement.</rdfs:comment>
    </owl:ObjectProperty>
    


    <!-- https://savage.nps.edu/EthicalControl/ontologies/MissionExecutionOntology#canPerform -->

    <owl:ObjectProperty rdf:about="https://savage.nps.edu/EthicalControl/ontologies/MissionExecutionOntology#canPerform">
        <owl:inverseOf rdf:resource="https://savage.nps.edu/EthicalControl/ontologies/MissionExecutionOntology#isPerformableBy"/>
        <rdfs:domain rdf:resource="https://savage.nps.edu/EthicalControl/ontologies/MissionExecutionOntology#Vehicle"/>
        <rdfs:range rdf:resource="https://savage.nps.edu/EthicalControl/ontologies/MissionExecutionOntology#Mission"/>
        <rdfs:comment>A Vehicle can perform one or more Mission instances, meaning the Vehicle can meet (&quot;canMeet&quot;) all of the Goals associated with the Mission through the &quot;includes&quot; relation.</rdfs:comment>
    </owl:ObjectProperty>
    


    <!-- https://savage.nps.edu/EthicalControl/ontologies/MissionExecutionOntology#constrains -->

    <owl:ObjectProperty rdf:about="https://savage.nps.edu/EthicalControl/ontologies/MissionExecutionOntology#constrains">
        <owl:propertyChainAxiom rdf:parseType="Collection">
            <rdf:Description rdf:about="https://savage.nps.edu/EthicalControl/ontologies/MissionExecutionOntology#constrains"/>
            <rdf:Description rdf:about="https://savage.nps.edu/EthicalControl/ontologies/MissionExecutionOntology#includes"/>
        </owl:propertyChainAxiom>
        <rdfs:comment>A Constraint applies to one or more Missions and/or one or more Goals.</rdfs:comment>
    </owl:ObjectProperty>
    <owl:Axiom>
        <owl:annotatedSource rdf:resource="https://savage.nps.edu/EthicalControl/ontologies/MissionExecutionOntology#constrains"/>
        <owl:annotatedProperty rdf:resource="http://www.w3.org/2002/07/owl#propertyChainAxiom"/>
        <owl:annotatedTarget rdf:parseType="Collection">
            <rdf:Description rdf:about="https://savage.nps.edu/EthicalControl/ontologies/MissionExecutionOntology#constrains"/>
            <rdf:Description rdf:about="https://savage.nps.edu/EthicalControl/ontologies/MissionExecutionOntology#includes"/>
        </owl:annotatedTarget>
        <rdfs:comment>A Constraint that applies to a Mission must also apply to all of the Goals that Mission includes.</rdfs:comment>
        <rdfs:label>C3</rdfs:label>
    </owl:Axiom>
    


    <!-- https://savage.nps.edu/EthicalControl/ontologies/MissionExecutionOntology#constrainsGoal -->

    <owl:ObjectProperty rdf:about="https://savage.nps.edu/EthicalControl/ontologies/MissionExecutionOntology#constrainsGoal">
        <rdfs:subPropertyOf rdf:resource="https://savage.nps.edu/EthicalControl/ontologies/MissionExecutionOntology#constrains"/>
        <owl:inverseOf rdf:resource="https://savage.nps.edu/EthicalControl/ontologies/MissionExecutionOntology#hasGoalConstraint"/>
        <rdfs:domain rdf:resource="https://savage.nps.edu/EthicalControl/ontologies/MissionExecutionOntology#DADM_Constraints"/>
        <rdfs:range rdf:resource="https://savage.nps.edu/EthicalControl/ontologies/MissionExecutionOntology#Goal"/>
    </owl:ObjectProperty>
    


    <!-- https://savage.nps.edu/EthicalControl/ontologies/MissionExecutionOntology#constrainsMission -->

    <owl:ObjectProperty rdf:about="https://savage.nps.edu/EthicalControl/ontologies/MissionExecutionOntology#constrainsMission">
        <rdfs:subPropertyOf rdf:resource="https://savage.nps.edu/EthicalControl/ontologies/MissionExecutionOntology#constrains"/>
        <owl:inverseOf rdf:resource="https://savage.nps.edu/EthicalControl/ontologies/MissionExecutionOntology#hasMissionConstraint"/>
        <rdfs:domain rdf:resource="https://savage.nps.edu/EthicalControl/ontologies/MissionExecutionOntology#DADM_Constraints"/>
        <rdfs:range rdf:resource="https://savage.nps.edu/EthicalControl/ontologies/MissionExecutionOntology#Mission"/>
    </owl:ObjectProperty>
    


    <!-- https://savage.nps.edu/EthicalControl/ontologies/MissionExecutionOntology#hasConstraint -->

    <owl:ObjectProperty rdf:about="https://savage.nps.edu/EthicalControl/ontologies/MissionExecutionOntology#hasConstraint">
        <rdfs:range rdf:resource="https://savage.nps.edu/EthicalControl/ontologies/MissionExecutionOntology#DADM_Constraints"/>
        <owl:propertyChainAxiom rdf:parseType="Collection">
            <rdf:Description rdf:about="https://savage.nps.edu/EthicalControl/ontologies/MissionExecutionOntology#includes"/>
            <rdf:Description>
                <owl:inverseOf rdf:resource="https://savage.nps.edu/EthicalControl/ontologies/MissionExecutionOntology#constrains"/>
            </rdf:Description>
        </owl:propertyChainAxiom>
        <rdfs:comment>A Mission or Goal has one or more Constraint instances, meaning the Mission or Goal must be concerned about the conditions expressed in the Constraint instances in the execution of the associated mission or goal..</rdfs:comment>
    </owl:ObjectProperty>
    <owl:Axiom>
        <owl:annotatedSource rdf:resource="https://savage.nps.edu/EthicalControl/ontologies/MissionExecutionOntology#hasConstraint"/>
        <owl:annotatedProperty rdf:resource="http://www.w3.org/2000/01/rdf-schema#range"/>
        <owl:annotatedTarget rdf:resource="https://savage.nps.edu/EthicalControl/ontologies/MissionExecutionOntology#DADM_Constraints"/>
        <rdfs:comment>A Mission can be constrained only by Constraints.</rdfs:comment>
        <rdfs:label>M3</rdfs:label>
    </owl:Axiom>
    


    <!-- https://savage.nps.edu/EthicalControl/ontologies/MissionExecutionOntology#hasDimensionsAutonomousDecisionMaking -->

    <owl:ObjectProperty rdf:about="https://savage.nps.edu/EthicalControl/ontologies/MissionExecutionOntology#hasDimensionsAutonomousDecisionMaking">
        <rdfs:domain rdf:resource="https://savage.nps.edu/EthicalControl/ontologies/MissionExecutionOntology#DADM_Constraints"/>
        <rdfs:range rdf:resource="https://savage.nps.edu/EthicalControl/ontologies/MissionExecutionOntology#DimensionsAutonomousDecisionMaking"/>
    </owl:ObjectProperty>
    


    <!-- https://savage.nps.edu/EthicalControl/ontologies/MissionExecutionOntology#hasEndCondition -->

    <owl:ObjectProperty rdf:about="https://savage.nps.edu/EthicalControl/ontologies/MissionExecutionOntology#hasEndCondition">
        <rdfs:domain rdf:resource="https://savage.nps.edu/EthicalControl/ontologies/MissionExecutionOntology#Goal"/>
        <rdfs:range rdf:resource="https://savage.nps.edu/EthicalControl/ontologies/MissionExecutionOntology#EndCondition"/>
        <rdfs:comment>Every Goal has a specific EndCondition, which results in either SUCCESS FAILURE or EXCEPTION, based on execution of actions associated with Goal achievement, under any associated Constraint instances.</rdfs:comment>
    </owl:ObjectProperty>
    <owl:Axiom>
        <owl:annotatedSource rdf:resource="https://savage.nps.edu/EthicalControl/ontologies/MissionExecutionOntology#hasEndCondition"/>
        <owl:annotatedProperty rdf:resource="http://www.w3.org/2000/01/rdf-schema#range"/>
        <owl:annotatedTarget rdf:resource="https://savage.nps.edu/EthicalControl/ontologies/MissionExecutionOntology#EndCondition"/>
        <rdfs:comment>A Goal&apos;s end condition (ending state) must be an EndCondition.

[NOTE: In planning, this represents *possible* end conditions for a Goal; the actual end condition will not be known until mission execution.]</rdfs:comment>
        <rdfs:label>G2</rdfs:label>
    </owl:Axiom>
    


    <!-- https://savage.nps.edu/EthicalControl/ontologies/MissionExecutionOntology#hasFeature -->

    <owl:ObjectProperty rdf:about="https://savage.nps.edu/EthicalControl/ontologies/MissionExecutionOntology#hasFeature">
        <rdfs:domain rdf:resource="https://savage.nps.edu/EthicalControl/ontologies/MissionExecutionOntology#Vehicle"/>
        <rdfs:range rdf:resource="https://savage.nps.edu/EthicalControl/ontologies/MissionExecutionOntology#VehicleFeature"/>
        <rdfs:comment>A Vehicle has one or more VehicleFeature instances.</rdfs:comment>
    </owl:ObjectProperty>
    <owl:Axiom>
        <owl:annotatedSource rdf:resource="https://savage.nps.edu/EthicalControl/ontologies/MissionExecutionOntology#hasFeature"/>
        <owl:annotatedProperty rdf:resource="http://www.w3.org/2000/01/rdf-schema#range"/>
        <owl:annotatedTarget rdf:resource="https://savage.nps.edu/EthicalControl/ontologies/MissionExecutionOntology#VehicleFeature"/>
        <rdfs:comment>The only allowable features of a Vehicle are VehicleFeature.</rdfs:comment>
        <rdfs:label>V1</rdfs:label>
    </owl:Axiom>
    


    <!-- https://savage.nps.edu/EthicalControl/ontologies/MissionExecutionOntology#hasGoalConstraint -->

    <owl:ObjectProperty rdf:about="https://savage.nps.edu/EthicalControl/ontologies/MissionExecutionOntology#hasGoalConstraint">
        <rdfs:subPropertyOf rdf:resource="https://savage.nps.edu/EthicalControl/ontologies/MissionExecutionOntology#hasConstraint"/>
        <rdfs:domain rdf:resource="https://savage.nps.edu/EthicalControl/ontologies/MissionExecutionOntology#Goal"/>
        <rdfs:range rdf:resource="https://savage.nps.edu/EthicalControl/ontologies/MissionExecutionOntology#DADM_Constraints"/>
        <rdfs:comment>The hasGoalConstraint property relates a Goal instance to one or more Constraint instances.</rdfs:comment>
    </owl:ObjectProperty>
    


    <!-- https://savage.nps.edu/EthicalControl/ontologies/MissionExecutionOntology#hasIntendedOutcome -->

    <owl:ObjectProperty rdf:about="https://savage.nps.edu/EthicalControl/ontologies/MissionExecutionOntology#hasIntendedOutcome"/>
    


    <!-- https://savage.nps.edu/EthicalControl/ontologies/MissionExecutionOntology#hasMissionConstraint -->

    <owl:ObjectProperty rdf:about="https://savage.nps.edu/EthicalControl/ontologies/MissionExecutionOntology#hasMissionConstraint">
        <rdfs:subPropertyOf rdf:resource="https://savage.nps.edu/EthicalControl/ontologies/MissionExecutionOntology#hasConstraint"/>
        <rdfs:domain rdf:resource="https://savage.nps.edu/EthicalControl/ontologies/MissionExecutionOntology#Mission"/>
        <rdfs:range rdf:resource="https://savage.nps.edu/EthicalControl/ontologies/MissionExecutionOntology#DADM_Constraints"/>
        <rdfs:comment>The hasMissionConstraint property relates a Mission instance to one or more Constraint instances.</rdfs:comment>
    </owl:ObjectProperty>
    


    <!-- https://savage.nps.edu/EthicalControl/ontologies/MissionExecutionOntology#hasNextGoal -->

    <owl:ObjectProperty rdf:about="https://savage.nps.edu/EthicalControl/ontologies/MissionExecutionOntology#hasNextGoal">
        <rdfs:subPropertyOf rdf:resource="https://savage.nps.edu/EthicalControl/ontologies/MissionExecutionOntology#isFollowedBy"/>
        <rdf:type rdf:resource="http://www.w3.org/2002/07/owl#IrreflexiveProperty"/>
        <rdfs:domain rdf:resource="https://savage.nps.edu/EthicalControl/ontologies/MissionExecutionOntology#Goal"/>
        <rdfs:range rdf:resource="https://savage.nps.edu/EthicalControl/ontologies/MissionExecutionOntology#Goal"/>
        <rdfs:comment>Goal &apos;B&apos; is the next goal for Goal &apos;A&apos; when &apos;A&apos; directly precedes &apos;A&apos; in the Mission goal tree. This property is  irreflexive; a Goal cannot return to itself (a weak form of Rule G7).</rdfs:comment>
    </owl:ObjectProperty>
    <owl:Axiom>
        <owl:annotatedSource rdf:resource="https://savage.nps.edu/EthicalControl/ontologies/MissionExecutionOntology#hasNextGoal"/>
        <owl:annotatedProperty rdf:resource="http://www.w3.org/2000/01/rdf-schema#subPropertyOf"/>
        <owl:annotatedTarget rdf:resource="https://savage.nps.edu/EthicalControl/ontologies/MissionExecutionOntology#isFollowedBy"/>
        <rdfs:comment>A Goal follows another Goal if it is the next Goal.</rdfs:comment>
        <rdfs:label>G8</rdfs:label>
    </owl:Axiom>
    <owl:Axiom>
        <owl:annotatedSource rdf:resource="https://savage.nps.edu/EthicalControl/ontologies/MissionExecutionOntology#hasNextGoal"/>
        <owl:annotatedProperty rdf:resource="http://www.w3.org/2000/01/rdf-schema#range"/>
        <owl:annotatedTarget rdf:resource="https://savage.nps.edu/EthicalControl/ontologies/MissionExecutionOntology#Goal"/>
        <rdfs:comment>A Goal can only have other Goals next.</rdfs:comment>
        <rdfs:label>G3</rdfs:label>
    </owl:Axiom>
    


    <!-- https://savage.nps.edu/EthicalControl/ontologies/MissionExecutionOntology#hasNextGoalOnException -->

    <owl:ObjectProperty rdf:about="https://savage.nps.edu/EthicalControl/ontologies/MissionExecutionOntology#hasNextGoalOnException">
        <rdfs:subPropertyOf rdf:resource="https://savage.nps.edu/EthicalControl/ontologies/MissionExecutionOntology#hasNextGoal"/>
        <rdfs:domain rdf:resource="https://savage.nps.edu/EthicalControl/ontologies/MissionExecutionOntology#Goal"/>
        <rdfs:range rdf:resource="https://savage.nps.edu/EthicalControl/ontologies/MissionExecutionOntology#Goal"/>
        <rdfs:comment>The Goal to perform following a EXCEPTION EndCondition on the current Goal.</rdfs:comment>
    </owl:ObjectProperty>
    


    <!-- https://savage.nps.edu/EthicalControl/ontologies/MissionExecutionOntology#hasNextGoalOnFailure -->

    <owl:ObjectProperty rdf:about="https://savage.nps.edu/EthicalControl/ontologies/MissionExecutionOntology#hasNextGoalOnFailure">
        <rdfs:subPropertyOf rdf:resource="https://savage.nps.edu/EthicalControl/ontologies/MissionExecutionOntology#hasNextGoal"/>
        <rdfs:domain rdf:resource="https://savage.nps.edu/EthicalControl/ontologies/MissionExecutionOntology#Goal"/>
        <rdfs:range rdf:resource="https://savage.nps.edu/EthicalControl/ontologies/MissionExecutionOntology#Goal"/>
        <rdfs:comment>The Goal to perform following a FAILURE EndCondition on the current Goal.</rdfs:comment>
    </owl:ObjectProperty>
    


    <!-- https://savage.nps.edu/EthicalControl/ontologies/MissionExecutionOntology#hasNextGoalOnSuccess -->

    <owl:ObjectProperty rdf:about="https://savage.nps.edu/EthicalControl/ontologies/MissionExecutionOntology#hasNextGoalOnSuccess">
        <rdfs:subPropertyOf rdf:resource="https://savage.nps.edu/EthicalControl/ontologies/MissionExecutionOntology#hasNextGoal"/>
        <rdfs:domain rdf:resource="https://savage.nps.edu/EthicalControl/ontologies/MissionExecutionOntology#Goal"/>
        <rdfs:range rdf:resource="https://savage.nps.edu/EthicalControl/ontologies/MissionExecutionOntology#Goal"/>
        <rdfs:comment>The Goal to perform following a SUCCESS EndCondition on the current Goal.</rdfs:comment>
    </owl:ObjectProperty>
    


    <!-- https://savage.nps.edu/EthicalControl/ontologies/MissionExecutionOntology#includes -->

    <owl:ObjectProperty rdf:about="https://savage.nps.edu/EthicalControl/ontologies/MissionExecutionOntology#includes">
        <rdfs:domain rdf:resource="https://savage.nps.edu/EthicalControl/ontologies/MissionExecutionOntology#Mission"/>
        <rdfs:range rdf:resource="https://savage.nps.edu/EthicalControl/ontologies/MissionExecutionOntology#Goal"/>
        <owl:propertyChainAxiom rdf:parseType="Collection">
            <rdf:Description rdf:about="https://savage.nps.edu/EthicalControl/ontologies/MissionExecutionOntology#startsWith"/>
            <rdf:Description rdf:about="https://savage.nps.edu/EthicalControl/ontologies/MissionExecutionOntology#isFollowedBy"/>
        </owl:propertyChainAxiom>
        <rdfs:comment>A Mission &quot;includes&quot; one or more Goal instances. An initial Goal instance is linked to the mission through the &quot;startsWith&quot; relation. The Goals are linked to each other through the &quot;hasNext&quot; set of properties (hasNextOnSuccess, hasNextOnFailure, hasNextOnException), describing a goal tree for the Mission.</rdfs:comment>
    </owl:ObjectProperty>
    <owl:Axiom>
        <owl:annotatedSource rdf:resource="https://savage.nps.edu/EthicalControl/ontologies/MissionExecutionOntology#includes"/>
        <owl:annotatedProperty rdf:resource="http://www.w3.org/2000/01/rdf-schema#range"/>
        <owl:annotatedTarget rdf:resource="https://savage.nps.edu/EthicalControl/ontologies/MissionExecutionOntology#Goal"/>
        <rdfs:comment>A Mission can only include Goals.</rdfs:comment>
        <rdfs:label>M2</rdfs:label>
    </owl:Axiom>
    <owl:Axiom>
        <owl:annotatedSource rdf:resource="https://savage.nps.edu/EthicalControl/ontologies/MissionExecutionOntology#includes"/>
        <owl:annotatedProperty rdf:resource="http://www.w3.org/2002/07/owl#propertyChainAxiom"/>
        <owl:annotatedTarget rdf:parseType="Collection">
            <rdf:Description rdf:about="https://savage.nps.edu/EthicalControl/ontologies/MissionExecutionOntology#startsWith"/>
            <rdf:Description rdf:about="https://savage.nps.edu/EthicalControl/ontologies/MissionExecutionOntology#isFollowedBy"/>
        </owl:annotatedTarget>
        <rdfs:comment>All Goals in a Mission must *potentially* follow the starting Goal (satisfiability vice entailment).

[NOTE: Here we express that the property chain &quot;startsWith o follows&quot; implies includes. Need to see if there is a way to express the reverse containment for equivalency.]</rdfs:comment>
        <rdfs:label>G10 (partial)</rdfs:label>
    </owl:Axiom>
    


    <!-- https://savage.nps.edu/EthicalControl/ontologies/MissionExecutionOntology#isFollowedBy -->

    <owl:ObjectProperty rdf:about="https://savage.nps.edu/EthicalControl/ontologies/MissionExecutionOntology#isFollowedBy">
        <rdf:type rdf:resource="http://www.w3.org/2002/07/owl#TransitiveProperty"/>
        <rdfs:domain rdf:resource="https://savage.nps.edu/EthicalControl/ontologies/MissionExecutionOntology#Goal"/>
        <rdfs:range rdf:resource="https://savage.nps.edu/EthicalControl/ontologies/MissionExecutionOntology#Goal"/>
        <rdfs:comment>A Goal &apos;B&apos; follows another Goal &apos;A&apos; if it occurs below Goal &apos;A&apos; in the Mission goal tree. A Goal instance cannot occur in its set of &quot;follows&quot; goals (the tree of goals must be acyclic). Property &quot;follows&quot; is transitive [ontology rule G9].

TODO: Make isFollowedBy a synonym for hasNextGoal (except, we want isFollowedBy to be transitive and subproperty hasNextGoal to be irreflexive -- the reasoners will not handle a single property being both irreflexive and transitive)..</rdfs:comment>
    </owl:ObjectProperty>
    <owl:Axiom>
        <owl:annotatedSource rdf:resource="https://savage.nps.edu/EthicalControl/ontologies/MissionExecutionOntology#isFollowedBy"/>
        <owl:annotatedProperty rdf:resource="http://www.w3.org/2000/01/rdf-schema#range"/>
        <owl:annotatedTarget rdf:resource="https://savage.nps.edu/EthicalControl/ontologies/MissionExecutionOntology#Goal"/>
        <rdfs:comment>A Goal can only be followed by another Goal.</rdfs:comment>
        <rdfs:label>G6</rdfs:label>
    </owl:Axiom>
    


    <!-- https://savage.nps.edu/EthicalControl/ontologies/MissionExecutionOntology#isInitialGoal -->

    <owl:ObjectProperty rdf:about="https://savage.nps.edu/EthicalControl/ontologies/MissionExecutionOntology#isInitialGoal">
        <rdfs:domain rdf:resource="https://savage.nps.edu/EthicalControl/ontologies/MissionExecutionOntology#Goal"/>
        <rdfs:range rdf:resource="https://savage.nps.edu/EthicalControl/ontologies/MissionExecutionOntology#Mission"/>
        <rdfs:comment>A Goal is identified as the first goal of a Mission (i.e., the initial tasking to be performed by the assigned vehicle).</rdfs:comment>
    </owl:ObjectProperty>
    


    <!-- https://savage.nps.edu/EthicalControl/ontologies/MissionExecutionOntology#isPerformableBy -->

    <owl:ObjectProperty rdf:about="https://savage.nps.edu/EthicalControl/ontologies/MissionExecutionOntology#isPerformableBy">
        <rdfs:domain rdf:resource="https://savage.nps.edu/EthicalControl/ontologies/MissionExecutionOntology#Mission"/>
        <rdfs:range rdf:resource="https://savage.nps.edu/EthicalControl/ontologies/MissionExecutionOntology#Vehicle"/>
        <rdfs:comment>A Mission can be performed by a Vehicle if the Vehicle &quot;canPerform&quot; the Mission or, equivalently, that the Vehicle &quot;canMeet&quot; all of the Goal instances in the &quot;includes&quot; relation for the Mission or, equivalently, that the Vehicle &quot;hasFeature&quot; VehicleFeature instances that &quot;canFulfill&quot; all of the IntendedOutcome instances required by all of the Goal instances in the &quot;includes&quot; relation for the mission. This is an indication of possibility of successful performance, not necessarily achievement of the intended outcomes of each goal in the mission.</rdfs:comment>
    </owl:ObjectProperty>
    <owl:Axiom>
        <owl:annotatedSource rdf:resource="https://savage.nps.edu/EthicalControl/ontologies/MissionExecutionOntology#isPerformableBy"/>
        <owl:annotatedProperty rdf:resource="http://www.w3.org/2000/01/rdf-schema#range"/>
        <owl:annotatedTarget rdf:resource="https://savage.nps.edu/EthicalControl/ontologies/MissionExecutionOntology#Vehicle"/>
        <rdfs:comment>A Mission can only be performed by a Vehicle.</rdfs:comment>
        <rdfs:label>M5</rdfs:label>
    </owl:Axiom>
    


    <!-- https://savage.nps.edu/EthicalControl/ontologies/MissionExecutionOntology#mustSatisfy -->

    <owl:ObjectProperty rdf:about="https://savage.nps.edu/EthicalControl/ontologies/MissionExecutionOntology#mustSatisfy">
        <rdfs:domain rdf:resource="https://savage.nps.edu/EthicalControl/ontologies/MissionExecutionOntology#Goal"/>
        <rdfs:range rdf:resource="https://savage.nps.edu/EthicalControl/ontologies/MissionExecutionOntology#IntendedOutcome"/>
        <rdfs:comment>A Goal must satisfy one or more IntendedOutcome instances for the Goal to be achieved successfully.</rdfs:comment>
    </owl:ObjectProperty>
    <owl:Axiom>
        <owl:annotatedSource rdf:resource="https://savage.nps.edu/EthicalControl/ontologies/MissionExecutionOntology#mustSatisfy"/>
        <owl:annotatedProperty rdf:resource="http://www.w3.org/2000/01/rdf-schema#range"/>
        <owl:annotatedTarget rdf:resource="https://savage.nps.edu/EthicalControl/ontologies/MissionExecutionOntology#IntendedOutcome"/>
        <rdfs:comment>A Goal can only require a GoalRequirement.</rdfs:comment>
        <rdfs:label>G1</rdfs:label>
    </owl:Axiom>
    


    <!-- https://savage.nps.edu/EthicalControl/ontologies/MissionExecutionOntology#startsWith -->

    <owl:ObjectProperty rdf:about="https://savage.nps.edu/EthicalControl/ontologies/MissionExecutionOntology#startsWith">
        <rdfs:subPropertyOf rdf:resource="https://savage.nps.edu/EthicalControl/ontologies/MissionExecutionOntology#includes"/>
        <rdfs:domain rdf:resource="https://savage.nps.edu/EthicalControl/ontologies/MissionExecutionOntology#Mission"/>
        <rdfs:range rdf:resource="https://savage.nps.edu/EthicalControl/ontologies/MissionExecutionOntology#Goal"/>
        <rdfs:comment>A Mission &quot;startsWith&quot; a specific Goal instance. A Mission must have at least one Goal in its goal tree.</rdfs:comment>
    </owl:ObjectProperty>
    <owl:Axiom>
        <owl:annotatedSource rdf:resource="https://savage.nps.edu/EthicalControl/ontologies/MissionExecutionOntology#startsWith"/>
        <owl:annotatedProperty rdf:resource="http://www.w3.org/2000/01/rdf-schema#subPropertyOf"/>
        <owl:annotatedTarget rdf:resource="https://savage.nps.edu/EthicalControl/ontologies/MissionExecutionOntology#includes"/>
        <rdfs:comment>A Mission must include the Goal that it starts with.</rdfs:comment>
        <rdfs:label>M4</rdfs:label>
    </owl:Axiom>
    <owl:Axiom>
        <owl:annotatedSource rdf:resource="https://savage.nps.edu/EthicalControl/ontologies/MissionExecutionOntology#startsWith"/>
        <owl:annotatedProperty rdf:resource="http://www.w3.org/2000/01/rdf-schema#range"/>
        <owl:annotatedTarget rdf:resource="https://savage.nps.edu/EthicalControl/ontologies/MissionExecutionOntology#Goal"/>
        <rdfs:comment>A Mission can only start with a Goal.</rdfs:comment>
        <rdfs:label>M1</rdfs:label>
    </owl:Axiom>
    


    <!-- https://savage.nps.edu/EthicalControl/ontologies/MissionExecutionOntology/canPerformAllGoals -->

    <owl:ObjectProperty rdf:about="https://savage.nps.edu/EthicalControl/ontologies/MissionExecutionOntology/canPerformAllGoals">
        <owl:versionInfo>TODO</owl:versionInfo>
    </owl:ObjectProperty>
    


    <!-- https://savage.nps.edu/EthicalControl/ontologies/MissionExecutionOntology/isMetBy -->

    <owl:ObjectProperty rdf:about="https://savage.nps.edu/EthicalControl/ontologies/MissionExecutionOntology/isMetBy"/>
    


    <!-- 
    ///////////////////////////////////////////////////////////////////////////////////////
    //
    // Data properties
    //
    ///////////////////////////////////////////////////////////////////////////////////////
     -->

    


    <!-- https://savage.nps.edu/EthicalControl/ontologies/MissionExecutionOntology#isTerminalGoal -->

    <owl:DatatypeProperty rdf:about="https://savage.nps.edu/EthicalControl/ontologies/MissionExecutionOntology#isTerminalGoal">
        <rdfs:range rdf:resource="http://www.w3.org/2001/XMLSchema#boolean"/>
        <rdfs:comment>Indicates if a Goal instance has follow-on goals (true or false) indicated by one or more hasNextGoal properties. I.e., if a Goal instance has no hasNextGoal properties, then it is a terminal goal.</rdfs:comment>
    </owl:DatatypeProperty>
    


    <!-- https://savage.nps.edu/EthicalControl/ontologies/MissionExecutionOntology/isPartOfPhase -->

    <owl:DatatypeProperty rdf:about="https://savage.nps.edu/EthicalControl/ontologies/MissionExecutionOntology/isPartOfPhase">
        <rdfs:range rdf:resource="http://www.w3.org/2001/XMLSchema#string"/>
        <rdfs:comment>Mission phase associated with this agenda goal.</rdfs:comment>
    </owl:DatatypeProperty>
    


    <!-- https://savage.nps.edu/EthicalControl/ontologies/MissionExecutionOntology/version -->

    <owl:DatatypeProperty rdf:about="https://savage.nps.edu/EthicalControl/ontologies/MissionExecutionOntology/version">
        <rdfs:range rdf:resource="http://www.w3.org/2001/XMLSchema#string"/>
        <owl:versionInfo>TODO define versioning scheme</owl:versionInfo>
    </owl:DatatypeProperty>
    


    <!-- 
    ///////////////////////////////////////////////////////////////////////////////////////
    //
    // Classes
    //
    ///////////////////////////////////////////////////////////////////////////////////////
     -->

    


    <!-- https://savage.nps.edu/EthicalControl/ontologies/MissionExecutionOntology#AI -->

    <owl:Class rdf:about="https://savage.nps.edu/EthicalControl/ontologies/MissionExecutionOntology#AI">
        <rdfs:subClassOf rdf:resource="https://savage.nps.edu/EthicalControl/ontologies/MissionExecutionOntology#DADM_Abbreviations"/>
        <rdfs:label>Artificial Intelligence (AI)</rdfs:label>
        <owl:versionInfo>page 100</owl:versionInfo>
    </owl:Class>
    


    <!-- https://savage.nps.edu/EthicalControl/ontologies/MissionExecutionOntology#APB -->

    <owl:Class rdf:about="https://savage.nps.edu/EthicalControl/ontologies/MissionExecutionOntology#APB">
        <rdfs:subClassOf rdf:resource="https://savage.nps.edu/EthicalControl/ontologies/MissionExecutionOntology#DADM_Abbreviations"/>
        <rdfs:label>Acquisition Program Baseline (APB)</rdfs:label>
        <owl:versionInfo>page 100</owl:versionInfo>
    </owl:Class>
    


    <!-- https://savage.nps.edu/EthicalControl/ontologies/MissionExecutionOntology#CDD -->

    <owl:Class rdf:about="https://savage.nps.edu/EthicalControl/ontologies/MissionExecutionOntology#CDD">
        <rdfs:subClassOf rdf:resource="https://savage.nps.edu/EthicalControl/ontologies/MissionExecutionOntology#DADM_Abbreviations"/>
        <rdfs:label>Capability Development Document (CDD)</rdfs:label>
        <owl:versionInfo>page 100</owl:versionInfo>
    </owl:Class>
    


    <!-- https://savage.nps.edu/EthicalControl/ontologies/MissionExecutionOntology#CNA -->

    <owl:Class rdf:about="https://savage.nps.edu/EthicalControl/ontologies/MissionExecutionOntology#CNA">
        <rdfs:subClassOf rdf:resource="https://savage.nps.edu/EthicalControl/ontologies/MissionExecutionOntology#DADM_Abbreviations"/>
        <rdfs:label>Center for Naval Analyses (CNA)</rdfs:label>
        <owl:versionInfo>page 100</owl:versionInfo>
    </owl:Class>
    


    <!-- https://savage.nps.edu/EthicalControl/ontologies/MissionExecutionOntology#DADM01 -->

    <owl:Class rdf:about="https://savage.nps.edu/EthicalControl/ontologies/MissionExecutionOntology#DADM01">
        <rdfs:subClassOf rdf:resource="https://savage.nps.edu/EthicalControl/ontologies/MissionExecutionOntology#DimensionsAutonomousDecisionMaking"/>
        <rdfs:comment>Are all parties (developers, decision-makers, commanders, and operators) using a common and agreed-upon IAS lexicon so as not to inadvertently introduce risk via miscommunication?
As the number of organizations developing IAS grows, the need for common definitions and consistency in the semantics that characterize IAS concepts also grows. The main objective of this DADM is to identify terms that, if misunderstood or miscommunicated, could lead to increased risk in the use of an IAS. It is especially important for all persons involved in the life cycle of an IAS (e.g., designers, developers, operators) to take a consistent approach in defining the terms to prevent risks that can inadvertently result in mishaps. Terms that require particular attention are those that are highly subjective and strongly depend on user interpretation and situational context. Consistency is not only important among the different people involved but also across the different phases of military operations. Having standard semantics and concepts may not completely eliminate risk, but reduces the risk of the operator misusing an IAS because of a miscommunication of the designer&apos;s original intention.</rdfs:comment>
        <rdfs:label>DADM01_StandardSemanticsConcepts</rdfs:label>
        <owl:versionInfo>page 16, page 59</owl:versionInfo>
    </owl:Class>
    


    <!-- https://savage.nps.edu/EthicalControl/ontologies/MissionExecutionOntology#DADM02 -->

    <owl:Class rdf:about="https://savage.nps.edu/EthicalControl/ontologies/MissionExecutionOntology#DADM02">
        <rdfs:subClassOf rdf:resource="https://savage.nps.edu/EthicalControl/ontologies/MissionExecutionOntology#DimensionsAutonomousDecisionMaking"/>
        <rdfs:comment>For every point in time during an operation, and for every component that may be used16 during that operation, is there a human who understands how the component functions, is aware of any autonomous functionality within the component, understands the risks associated with its use, and is legally accountable for authorizing its use?
Autonomous functionality can exist in every link of the kill chain, not just at the pinnacle of the decision to apply lethal force. Similarly, autonomous functionality can exist in every precursor activity of a nonlethal autonomous decision aid. Perceived gaps in accountability magnify legal and ethical concerns in the debate on IAS. Ensuring the continuity of legal accountability through every phase of an operation and amongst every interaction between the subcomponents of the overall IAS can help alleviate these concerns.</rdfs:comment>
        <rdfs:label>DADM02_ContinuityLegalAccountability</rdfs:label>
        <owl:versionInfo>page 16, page 60</owl:versionInfo>
    </owl:Class>
    


    <!-- https://savage.nps.edu/EthicalControl/ontologies/MissionExecutionOntology#DADM02.1 -->

    <owl:Class rdf:about="https://savage.nps.edu/EthicalControl/ontologies/MissionExecutionOntology#DADM02.1">
        <rdfs:subClassOf rdf:resource="https://savage.nps.edu/EthicalControl/ontologies/MissionExecutionOntology#DADM02"/>
        <rdfs:comment>Pre-operational phase considerations</rdfs:comment>
        <rdfs:label>DADM02.1_PreoperationalPhaseConsiderations</rdfs:label>
        <owl:versionInfo>page 60</owl:versionInfo>
    </owl:Class>
    


    <!-- https://savage.nps.edu/EthicalControl/ontologies/MissionExecutionOntology#DADM02.2 -->

    <owl:Class rdf:about="https://savage.nps.edu/EthicalControl/ontologies/MissionExecutionOntology#DADM02.2">
        <rdfs:subClassOf rdf:resource="https://savage.nps.edu/EthicalControl/ontologies/MissionExecutionOntology#DADM02"/>
        <rdfs:comment>Considerations for all eleven operational phases</rdfs:comment>
        <rdfs:label>DADM02.2_GeneralConsiderations</rdfs:label>
        <owl:versionInfo>page 61</owl:versionInfo>
    </owl:Class>
    


    <!-- https://savage.nps.edu/EthicalControl/ontologies/MissionExecutionOntology#DADM02.3 -->

    <owl:Class rdf:about="https://savage.nps.edu/EthicalControl/ontologies/MissionExecutionOntology#DADM02.3">
        <rdfs:subClassOf rdf:resource="https://savage.nps.edu/EthicalControl/ontologies/MissionExecutionOntology#DADM02"/>
        <rdfs:comment>Transfer of command and control</rdfs:comment>
        <rdfs:label>DADM02.3_ControlChanges</rdfs:label>
        <owl:versionInfo>page 61</owl:versionInfo>
    </owl:Class>
    


    <!-- https://savage.nps.edu/EthicalControl/ontologies/MissionExecutionOntology#DADM02.4 -->

    <owl:Class rdf:about="https://savage.nps.edu/EthicalControl/ontologies/MissionExecutionOntology#DADM02.4">
        <rdfs:subClassOf rdf:resource="https://savage.nps.edu/EthicalControl/ontologies/MissionExecutionOntology#DADM02"/>
        <rdfs:comment>General considerations</rdfs:comment>
        <rdfs:label>DADM02.4_GeneralConsiderations</rdfs:label>
        <owl:versionInfo>page 62</owl:versionInfo>
    </owl:Class>
    


    <!-- https://savage.nps.edu/EthicalControl/ontologies/MissionExecutionOntology#DADM03 -->

    <owl:Class rdf:about="https://savage.nps.edu/EthicalControl/ontologies/MissionExecutionOntology#DADM03">
        <rdfs:subClassOf rdf:resource="https://savage.nps.edu/EthicalControl/ontologies/MissionExecutionOntology#DimensionsAutonomousDecisionMaking"/>
        <rdfs:comment>Can the degree of autonomous functionality be adjusted to accommodate different or changing degrees of risk tolerance?
The degree of autonomy exists on a spectrum from zero autonomy, in which a human executes all functions, up to full autonomy, in which an IAS executes all functions. Increasing the degree of a system&apos;s autonomy can increase the risk of an unintended negative consequence. Additionally, changes in risk tolerance come with changing situations, conditions, and commanders in any dynamic operational environment. Thus, it is advantageous to have the ability to adjust the degree of autonomous functionality to match different risk tolerances, reducing it when risk tolerance is low and increasing it when risk tolerance is high.</rdfs:comment>
        <rdfs:label>DADM03_DegreeAutonomy</rdfs:label>
        <owl:versionInfo>page 17, page 62</owl:versionInfo>
    </owl:Class>
    


    <!-- https://savage.nps.edu/EthicalControl/ontologies/MissionExecutionOntology#DADM04 -->

    <owl:Class rdf:about="https://savage.nps.edu/EthicalControl/ontologies/MissionExecutionOntology#DADM04">
        <rdfs:subClassOf rdf:resource="https://savage.nps.edu/EthicalControl/ontologies/MissionExecutionOntology#DimensionsAutonomousDecisionMaking"/>
        <rdfs:comment>Does use of the IAS impart a military advantage over a non-autonomous alternative system, to include reducing the probability of collateral damage, that justifies accepting the potential risks associated with the use of the IAS?

The role of autonomy is to extend and complement human capabilities, and it is especially valuable in situations that are &quot;dull, dirty, or dangerous.&quot; Autonomous functionalities also become necessary when an IAS can perform tasks more effectively, such as decision-making at speeds beyond human capability, and when an IAS can help prevent cognitive overload. Ultimately, the potential risks that come with the use of an IAS are justified if an IAS provides a clear advantage over a non-autonomous alternative system. However, if both perform similarly, then the user may opt to use the non-autonomous system to reduce the risks regarding legal and ethical concerns associated with the use of an IAS (when and if these risks are not also present in the non-autonomous alternative).</rdfs:comment>
        <rdfs:label>DADM04_NecessityAutonomy</rdfs:label>
        <owl:versionInfo>page 17, page 64</owl:versionInfo>
    </owl:Class>
    


    <!-- https://savage.nps.edu/EthicalControl/ontologies/MissionExecutionOntology#DADM04.1 -->

    <owl:Class rdf:about="https://savage.nps.edu/EthicalControl/ontologies/MissionExecutionOntology#DADM04.1">
        <rdfs:subClassOf rdf:resource="https://savage.nps.edu/EthicalControl/ontologies/MissionExecutionOntology#DADM04"/>
        <rdfs:comment>General considerations</rdfs:comment>
        <rdfs:label>DADM04.1_GeneralConsiderations</rdfs:label>
        <owl:versionInfo>page 64</owl:versionInfo>
    </owl:Class>
    


    <!-- https://savage.nps.edu/EthicalControl/ontologies/MissionExecutionOntology#DADM04.2 -->

    <owl:Class rdf:about="https://savage.nps.edu/EthicalControl/ontologies/MissionExecutionOntology#DADM04.2">
        <rdfs:subClassOf rdf:resource="https://savage.nps.edu/EthicalControl/ontologies/MissionExecutionOntology#DADM04"/>
        <rdfs:comment>IAS capabilities are clearly superior</rdfs:comment>
        <rdfs:label>DADM04.2_SuperiorCabilities</rdfs:label>
        <owl:versionInfo>page 64</owl:versionInfo>
    </owl:Class>
    


    <!-- https://savage.nps.edu/EthicalControl/ontologies/MissionExecutionOntology#DADM04.3 -->

    <owl:Class rdf:about="https://savage.nps.edu/EthicalControl/ontologies/MissionExecutionOntology#DADM04.3">
        <rdfs:subClassOf rdf:resource="https://savage.nps.edu/EthicalControl/ontologies/MissionExecutionOntology#DADM04"/>
        <rdfs:comment>Distinction</rdfs:comment>
        <rdfs:label>DADM04.3_Distinction</rdfs:label>
        <owl:versionInfo>page 65</owl:versionInfo>
    </owl:Class>
    


    <!-- https://savage.nps.edu/EthicalControl/ontologies/MissionExecutionOntology#DADM04.4 -->

    <owl:Class rdf:about="https://savage.nps.edu/EthicalControl/ontologies/MissionExecutionOntology#DADM04.4">
        <rdfs:subClassOf rdf:resource="https://savage.nps.edu/EthicalControl/ontologies/MissionExecutionOntology#DADM04"/>
        <rdfs:comment>Proportionality</rdfs:comment>
        <rdfs:label>DADM04.4_Proportionality</rdfs:label>
        <owl:versionInfo>page 65</owl:versionInfo>
    </owl:Class>
    


    <!-- https://savage.nps.edu/EthicalControl/ontologies/MissionExecutionOntology#DADM04.5 -->

    <owl:Class rdf:about="https://savage.nps.edu/EthicalControl/ontologies/MissionExecutionOntology#DADM04.5">
        <rdfs:subClassOf rdf:resource="https://savage.nps.edu/EthicalControl/ontologies/MissionExecutionOntology#DADM04"/>
        <rdfs:comment>Decision speed</rdfs:comment>
        <rdfs:label>DADM04.5_DecisionSpeed</rdfs:label>
        <owl:versionInfo>page 65</owl:versionInfo>
    </owl:Class>
    


    <!-- https://savage.nps.edu/EthicalControl/ontologies/MissionExecutionOntology#DADM04.6 -->

    <owl:Class rdf:about="https://savage.nps.edu/EthicalControl/ontologies/MissionExecutionOntology#DADM04.6">
        <rdfs:subClassOf rdf:resource="https://savage.nps.edu/EthicalControl/ontologies/MissionExecutionOntology#DADM04"/>
        <rdfs:comment>Preventing cognitive overload</rdfs:comment>
        <rdfs:label>DADM04.6_PreventingCognitiveOverload</rdfs:label>
        <owl:versionInfo>page 66</owl:versionInfo>
    </owl:Class>
    


    <!-- https://savage.nps.edu/EthicalControl/ontologies/MissionExecutionOntology#DADM04.7 -->

    <owl:Class rdf:about="https://savage.nps.edu/EthicalControl/ontologies/MissionExecutionOntology#DADM04.7">
        <rdfs:subClassOf rdf:resource="https://savage.nps.edu/EthicalControl/ontologies/MissionExecutionOntology#DADM04"/>
        <rdfs:comment>Imposing dilemmas on the enemy</rdfs:comment>
        <rdfs:label>DADM04.7_ImposingAdversaryDilemmas</rdfs:label>
        <owl:versionInfo>page 66</owl:versionInfo>
    </owl:Class>
    


    <!-- https://savage.nps.edu/EthicalControl/ontologies/MissionExecutionOntology#DADM05 -->

    <owl:Class rdf:about="https://savage.nps.edu/EthicalControl/ontologies/MissionExecutionOntology#DADM05">
        <rdfs:subClassOf rdf:resource="https://savage.nps.edu/EthicalControl/ontologies/MissionExecutionOntology#DimensionsAutonomousDecisionMaking"/>
        <rdfs:comment>Has every available and practicable measure been taken by the commander to; prevent loss of command and control, relinquish command and control (but not accountability) only in the most dire of circumstances where no other option is available, ensure transfer of command and control without its loss, detect and prevent unintended behaviors, deactivate systems that demonstrate unintended behavior, i.e. to fail safe when command and control is lost, and re-establish command and control as quickly and safely as possible when it is lost due to error, miscommunication, malfunction or enemy action?

One major concern with IAS is that in some critical circumstances command and control may be difficult or impossible. This DAD seeks to maintain command and control of the IAS to the greatest extent possible and practicable, mitigate against negative consequences when command and control is lost, and minimize but accept the situations where the commander must transfer decision-making capabilities to an IAS. The risk elements under this DAD allow the commander to make a risk-informed decision to transfer decision-making capabilities to an IAS. The commander thus remains accountable for any negative consequences that may result.</rdfs:comment>
        <rdfs:isDefinedBy>Michael Holihan</rdfs:isDefinedBy>
        <rdfs:label>DADM05_CommandControl</rdfs:label>
        <owl:versionInfo>page 18, page 67</owl:versionInfo>
    </owl:Class>
    


    <!-- https://savage.nps.edu/EthicalControl/ontologies/MissionExecutionOntology#DADM05.1 -->

    <owl:Class rdf:about="https://savage.nps.edu/EthicalControl/ontologies/MissionExecutionOntology#DADM05.1">
        <rdfs:subClassOf rdf:resource="https://savage.nps.edu/EthicalControl/ontologies/MissionExecutionOntology#DADM05"/>
        <rdfs:comment>Preventing loss of command and control</rdfs:comment>
        <rdfs:label>DADM05.1_PreventingLossC2</rdfs:label>
        <owl:versionInfo>page 67</owl:versionInfo>
    </owl:Class>
    


    <!-- https://savage.nps.edu/EthicalControl/ontologies/MissionExecutionOntology#DADM05.2 -->

    <owl:Class rdf:about="https://savage.nps.edu/EthicalControl/ontologies/MissionExecutionOntology#DADM05.2">
        <rdfs:subClassOf rdf:resource="https://savage.nps.edu/EthicalControl/ontologies/MissionExecutionOntology#DADM05"/>
        <rdfs:comment>Relinquishing command and control to the IAS (but not accountability)</rdfs:comment>
        <rdfs:label>DADM05.2_RelinquishC2RetainAccountability</rdfs:label>
        <owl:versionInfo>page 68</owl:versionInfo>
    </owl:Class>
    


    <!-- https://savage.nps.edu/EthicalControl/ontologies/MissionExecutionOntology#DADM05.3 -->

    <owl:Class rdf:about="https://savage.nps.edu/EthicalControl/ontologies/MissionExecutionOntology#DADM05.3">
        <rdfs:subClassOf rdf:resource="https://savage.nps.edu/EthicalControl/ontologies/MissionExecutionOntology#DADM05"/>
        <rdfs:comment>Transferring command and control</rdfs:comment>
        <rdfs:label>DADM05.3_TransferC2</rdfs:label>
        <owl:versionInfo>page 68</owl:versionInfo>
    </owl:Class>
    


    <!-- https://savage.nps.edu/EthicalControl/ontologies/MissionExecutionOntology#DADM05.4 -->

    <owl:Class rdf:about="https://savage.nps.edu/EthicalControl/ontologies/MissionExecutionOntology#DADM05.4">
        <rdfs:subClassOf rdf:resource="https://savage.nps.edu/EthicalControl/ontologies/MissionExecutionOntology#DADM05"/>
        <rdfs:comment>Recognizing (uncontrollable) emergent behavior</rdfs:comment>
        <rdfs:label>DADM05.4_RecognizingUncontrollableEmergentBehavior</rdfs:label>
        <owl:versionInfo>page 69</owl:versionInfo>
    </owl:Class>
    


    <!-- https://savage.nps.edu/EthicalControl/ontologies/MissionExecutionOntology#DADM05.5 -->

    <owl:Class rdf:about="https://savage.nps.edu/EthicalControl/ontologies/MissionExecutionOntology#DADM05.5">
        <rdfs:subClassOf rdf:resource="https://savage.nps.edu/EthicalControl/ontologies/MissionExecutionOntology#DADM05"/>
        <rdfs:comment>Failing safe when command and control is lost</rdfs:comment>
        <rdfs:label>DADM05.5_C2LossSafety</rdfs:label>
        <owl:versionInfo>page 70</owl:versionInfo>
    </owl:Class>
    


    <!-- https://savage.nps.edu/EthicalControl/ontologies/MissionExecutionOntology#DADM05.6 -->

    <owl:Class rdf:about="https://savage.nps.edu/EthicalControl/ontologies/MissionExecutionOntology#DADM05.6">
        <rdfs:subClassOf rdf:resource="https://savage.nps.edu/EthicalControl/ontologies/MissionExecutionOntology#DADM05"/>
        <rdfs:comment>Re-establishing command and control</rdfs:comment>
        <rdfs:label>DADM05.6_ReestablishC2</rdfs:label>
        <owl:versionInfo>page 71</owl:versionInfo>
    </owl:Class>
    


    <!-- https://savage.nps.edu/EthicalControl/ontologies/MissionExecutionOntology#DADM06 -->

    <owl:Class rdf:about="https://savage.nps.edu/EthicalControl/ontologies/MissionExecutionOntology#DADM06">
        <rdfs:subClassOf rdf:resource="https://savage.nps.edu/EthicalControl/ontologies/MissionExecutionOntology#DimensionsAutonomousDecisionMaking"/>
        <rdfs:comment>Will there be persons or objects present that cannot be subjected to the effects of the IAS, or that require justification in accordance with applicable laws, policies, and rules of engagement before being subjected to the effects of the IAS?

IAS use must comply with the LOAC, which requires distinction, proportionality, military necessity, and reducing unnecessary suffering in military operations [30]. LOAC applies to all forms and all instruments of warfare, including IAS. It obliges commanders to consider the presence of certain persons and objects in the operational environment. This DAD addresses specific classes of persons and objects protected from the use of force that use of an IAS must be able to identify and not intentionally harm (in a manner that would violate laws, policies, or the rules of engagement). This DAD specifically does not address the use of IAS that do not use force but can still cause harm, such as an automated or autonomous decision aids. We address those systems in DAD#13: Civil and natural rights.</rdfs:comment>
        <rdfs:label>DADM06_PresenceProtectedPersonsObjects</rdfs:label>
        <owl:versionInfo>page 18, page 71</owl:versionInfo>
    </owl:Class>
    


    <!-- https://savage.nps.edu/EthicalControl/ontologies/MissionExecutionOntology#DADM06.1 -->

    <owl:Class rdf:about="https://savage.nps.edu/EthicalControl/ontologies/MissionExecutionOntology#DADM06.1">
        <rdfs:subClassOf rdf:resource="https://savage.nps.edu/EthicalControl/ontologies/MissionExecutionOntology#DADM06"/>
        <rdfs:comment>General considerations pertaining to both persons and objects</rdfs:comment>
        <rdfs:label>DADM06.1_GeneralPersonObject</rdfs:label>
        <owl:versionInfo>page 71</owl:versionInfo>
    </owl:Class>
    


    <!-- https://savage.nps.edu/EthicalControl/ontologies/MissionExecutionOntology#DADM06.10 -->

    <owl:Class rdf:about="https://savage.nps.edu/EthicalControl/ontologies/MissionExecutionOntology#DADM06.10">
        <rdfs:subClassOf rdf:resource="https://savage.nps.edu/EthicalControl/ontologies/MissionExecutionOntology#DADM06"/>
        <rdfs:comment>Perfidy</rdfs:comment>
        <rdfs:label>DADM06.10_Perfidy</rdfs:label>
        <owl:versionInfo>page 74</owl:versionInfo>
    </owl:Class>
    


    <!-- https://savage.nps.edu/EthicalControl/ontologies/MissionExecutionOntology#DADM06.11 -->

    <owl:Class rdf:about="https://savage.nps.edu/EthicalControl/ontologies/MissionExecutionOntology#DADM06.11">
        <rdfs:subClassOf rdf:resource="https://savage.nps.edu/EthicalControl/ontologies/MissionExecutionOntology#DADM06"/>
        <rdfs:comment>Specific classes of persons protected from the use of force</rdfs:comment>
        <rdfs:label>DADM06.11_PerceptionProtectedPerson</rdfs:label>
        <owl:versionInfo>page 75</owl:versionInfo>
    </owl:Class>
    


    <!-- https://savage.nps.edu/EthicalControl/ontologies/MissionExecutionOntology#DADM06.11.1 -->

    <owl:Class rdf:about="https://savage.nps.edu/EthicalControl/ontologies/MissionExecutionOntology#DADM06.11.1">
        <rdfs:subClassOf rdf:resource="https://savage.nps.edu/EthicalControl/ontologies/MissionExecutionOntology#DADM06.11"/>
        <rdfs:comment>Noncombatants</rdfs:comment>
        <rdfs:label>DADM06.11.1_Noncombatants</rdfs:label>
        <owl:versionInfo>page 75</owl:versionInfo>
    </owl:Class>
    


    <!-- https://savage.nps.edu/EthicalControl/ontologies/MissionExecutionOntology#DADM06.11.2 -->

    <owl:Class rdf:about="https://savage.nps.edu/EthicalControl/ontologies/MissionExecutionOntology#DADM06.11.2">
        <rdfs:subClassOf rdf:resource="https://savage.nps.edu/EthicalControl/ontologies/MissionExecutionOntology#DADM06.11"/>
        <rdfs:comment>Surrendering enemy troops</rdfs:comment>
        <rdfs:label>DADM06.11.2_AdversarySurrender</rdfs:label>
        <owl:versionInfo>page 75</owl:versionInfo>
    </owl:Class>
    


    <!-- https://savage.nps.edu/EthicalControl/ontologies/MissionExecutionOntology#DADM06.11.3 -->

    <owl:Class rdf:about="https://savage.nps.edu/EthicalControl/ontologies/MissionExecutionOntology#DADM06.11.3">
        <rdfs:subClassOf rdf:resource="https://savage.nps.edu/EthicalControl/ontologies/MissionExecutionOntology#DADM06.11"/>
        <rdfs:comment>Constitutionally protected US citizens</rdfs:comment>
        <rdfs:label>DADM06.11.3_ProtectedPersons</rdfs:label>
        <owl:versionInfo>page 75</owl:versionInfo>
    </owl:Class>
    


    <!-- https://savage.nps.edu/EthicalControl/ontologies/MissionExecutionOntology#DADM06.11.4 -->

    <owl:Class rdf:about="https://savage.nps.edu/EthicalControl/ontologies/MissionExecutionOntology#DADM06.11.4">
        <rdfs:subClassOf rdf:resource="https://savage.nps.edu/EthicalControl/ontologies/MissionExecutionOntology#DADM06.11"/>
        <rdfs:comment>US and friendly force troops</rdfs:comment>
        <rdfs:label>DADM06.11.4_USFriendlyForceTroops</rdfs:label>
        <owl:versionInfo>page 75</owl:versionInfo>
    </owl:Class>
    


    <!-- https://savage.nps.edu/EthicalControl/ontologies/MissionExecutionOntology#DADM06.12 -->

    <owl:Class rdf:about="https://savage.nps.edu/EthicalControl/ontologies/MissionExecutionOntology#DADM06.12">
        <rdfs:subClassOf rdf:resource="https://savage.nps.edu/EthicalControl/ontologies/MissionExecutionOntology#DADM06"/>
        <rdfs:comment>General considerations pertaining only to objects protected from the use of force</rdfs:comment>
        <rdfs:label>DADM06.12_ProtectedObjects</rdfs:label>
        <owl:versionInfo>page 76</owl:versionInfo>
    </owl:Class>
    


    <!-- https://savage.nps.edu/EthicalControl/ontologies/MissionExecutionOntology#DADM06.13 -->

    <owl:Class rdf:about="https://savage.nps.edu/EthicalControl/ontologies/MissionExecutionOntology#DADM06.13">
        <rdfs:subClassOf rdf:resource="https://savage.nps.edu/EthicalControl/ontologies/MissionExecutionOntology#DADM06"/>
        <rdfs:comment>Distinction</rdfs:comment>
        <rdfs:label>DADM06.13_Distinction</rdfs:label>
        <owl:versionInfo>page 76</owl:versionInfo>
    </owl:Class>
    


    <!-- https://savage.nps.edu/EthicalControl/ontologies/MissionExecutionOntology#DADM06.14 -->

    <owl:Class rdf:about="https://savage.nps.edu/EthicalControl/ontologies/MissionExecutionOntology#DADM06.14">
        <rdfs:subClassOf rdf:resource="https://savage.nps.edu/EthicalControl/ontologies/MissionExecutionOntology#DADM06"/>
        <rdfs:comment>Military necessity</rdfs:comment>
        <rdfs:label>DADM06.14_MilitaryNecessity</rdfs:label>
        <owl:versionInfo>page 76</owl:versionInfo>
    </owl:Class>
    


    <!-- https://savage.nps.edu/EthicalControl/ontologies/MissionExecutionOntology#DADM06.15 -->

    <owl:Class rdf:about="https://savage.nps.edu/EthicalControl/ontologies/MissionExecutionOntology#DADM06.15">
        <rdfs:subClassOf rdf:resource="https://savage.nps.edu/EthicalControl/ontologies/MissionExecutionOntology#DADM06"/>
        <rdfs:comment>Unnecessary suffering</rdfs:comment>
        <rdfs:label>DADM06.15_UnnecessarySuffering</rdfs:label>
        <owl:versionInfo>page 77</owl:versionInfo>
    </owl:Class>
    


    <!-- https://savage.nps.edu/EthicalControl/ontologies/MissionExecutionOntology#DADM06.16 -->

    <owl:Class rdf:about="https://savage.nps.edu/EthicalControl/ontologies/MissionExecutionOntology#DADM06.16">
        <rdfs:subClassOf rdf:resource="https://savage.nps.edu/EthicalControl/ontologies/MissionExecutionOntology#DADM06"/>
        <rdfs:comment>Perfidy</rdfs:comment>
        <rdfs:label>DADM06.16_Perfidy</rdfs:label>
        <owl:versionInfo>page 77</owl:versionInfo>
    </owl:Class>
    


    <!-- https://savage.nps.edu/EthicalControl/ontologies/MissionExecutionOntology#DADM06.17 -->

    <owl:Class rdf:about="https://savage.nps.edu/EthicalControl/ontologies/MissionExecutionOntology#DADM06.17">
        <rdfs:subClassOf rdf:resource="https://savage.nps.edu/EthicalControl/ontologies/MissionExecutionOntology#DADM06"/>
        <rdfs:comment>Specific objects</rdfs:comment>
        <rdfs:label>DADM06.17_SafeObjects</rdfs:label>
        <owl:versionInfo>page 77</owl:versionInfo>
    </owl:Class>
    


    <!-- https://savage.nps.edu/EthicalControl/ontologies/MissionExecutionOntology#DADM06.2 -->

    <owl:Class rdf:about="https://savage.nps.edu/EthicalControl/ontologies/MissionExecutionOntology#DADM06.2">
        <rdfs:subClassOf rdf:resource="https://savage.nps.edu/EthicalControl/ontologies/MissionExecutionOntology#DADM06"/>
        <rdfs:comment>Distinction</rdfs:comment>
        <rdfs:label>DADM06.2_Distinction</rdfs:label>
        <owl:versionInfo>page 71</owl:versionInfo>
    </owl:Class>
    


    <!-- https://savage.nps.edu/EthicalControl/ontologies/MissionExecutionOntology#DADM06.3 -->

    <owl:Class rdf:about="https://savage.nps.edu/EthicalControl/ontologies/MissionExecutionOntology#DADM06.3">
        <rdfs:subClassOf rdf:resource="https://savage.nps.edu/EthicalControl/ontologies/MissionExecutionOntology#DADM06"/>
        <rdfs:comment>Proportionality</rdfs:comment>
        <rdfs:label>DADM06.3_Proportionality</rdfs:label>
        <owl:versionInfo>page 72</owl:versionInfo>
    </owl:Class>
    


    <!-- https://savage.nps.edu/EthicalControl/ontologies/MissionExecutionOntology#DADM06.4 -->

    <owl:Class rdf:about="https://savage.nps.edu/EthicalControl/ontologies/MissionExecutionOntology#DADM06.4">
        <rdfs:subClassOf rdf:resource="https://savage.nps.edu/EthicalControl/ontologies/MissionExecutionOntology#DADM06"/>
        <rdfs:comment>Military necessity</rdfs:comment>
        <rdfs:label>DADM06.4_MilitaryNecessity</rdfs:label>
        <owl:versionInfo>page 72</owl:versionInfo>
    </owl:Class>
    


    <!-- https://savage.nps.edu/EthicalControl/ontologies/MissionExecutionOntology#DADM06.5 -->

    <owl:Class rdf:about="https://savage.nps.edu/EthicalControl/ontologies/MissionExecutionOntology#DADM06.5">
        <rdfs:subClassOf rdf:resource="https://savage.nps.edu/EthicalControl/ontologies/MissionExecutionOntology#DADM06"/>
        <rdfs:comment>Unnecessary suffering</rdfs:comment>
        <rdfs:label>DADM06.5_UnnecessarySuffering</rdfs:label>
        <owl:versionInfo>page 73</owl:versionInfo>
    </owl:Class>
    


    <!-- https://savage.nps.edu/EthicalControl/ontologies/MissionExecutionOntology#DADM06.6 -->

    <owl:Class rdf:about="https://savage.nps.edu/EthicalControl/ontologies/MissionExecutionOntology#DADM06.6">
        <rdfs:subClassOf rdf:resource="https://savage.nps.edu/EthicalControl/ontologies/MissionExecutionOntology#DADM06"/>
        <rdfs:comment>General considerations pertaining only to persons protected from the use of force</rdfs:comment>
        <rdfs:label>DADM06.6_ProtectedPersons</rdfs:label>
        <owl:versionInfo>page 73</owl:versionInfo>
    </owl:Class>
    


    <!-- https://savage.nps.edu/EthicalControl/ontologies/MissionExecutionOntology#DADM06.7 -->

    <owl:Class rdf:about="https://savage.nps.edu/EthicalControl/ontologies/MissionExecutionOntology#DADM06.7">
        <rdfs:subClassOf rdf:resource="https://savage.nps.edu/EthicalControl/ontologies/MissionExecutionOntology#DADM06"/>
        <rdfs:comment>Distinction</rdfs:comment>
        <rdfs:label>DADM06.7_Distinction</rdfs:label>
        <owl:versionInfo>page 73</owl:versionInfo>
    </owl:Class>
    


    <!-- https://savage.nps.edu/EthicalControl/ontologies/MissionExecutionOntology#DADM06.8 -->

    <owl:Class rdf:about="https://savage.nps.edu/EthicalControl/ontologies/MissionExecutionOntology#DADM06.8">
        <rdfs:subClassOf rdf:resource="https://savage.nps.edu/EthicalControl/ontologies/MissionExecutionOntology#DADM06"/>
        <rdfs:comment>Military necessity</rdfs:comment>
        <rdfs:label>DADM06.8_MilitaryNecessity</rdfs:label>
        <owl:versionInfo>page 74</owl:versionInfo>
    </owl:Class>
    


    <!-- https://savage.nps.edu/EthicalControl/ontologies/MissionExecutionOntology#DADM06.9 -->

    <owl:Class rdf:about="https://savage.nps.edu/EthicalControl/ontologies/MissionExecutionOntology#DADM06.9">
        <rdfs:subClassOf rdf:resource="https://savage.nps.edu/EthicalControl/ontologies/MissionExecutionOntology#DADM06"/>
        <rdfs:comment>Unnecessary suffering</rdfs:comment>
        <rdfs:label>DADM06.9_UnnecessarySuffering</rdfs:label>
        <owl:versionInfo>page 74</owl:versionInfo>
    </owl:Class>
    


    <!-- https://savage.nps.edu/EthicalControl/ontologies/MissionExecutionOntology#DADM07 -->

    <owl:Class rdf:about="https://savage.nps.edu/EthicalControl/ontologies/MissionExecutionOntology#DADM07">
        <rdfs:subClassOf rdf:resource="https://savage.nps.edu/EthicalControl/ontologies/MissionExecutionOntology#DimensionsAutonomousDecisionMaking"/>
        <rdfs:comment>Has positive control been retained over all components, and all processes used to develop the IAS, from the time of its pre-acquisition inception to its delivery to the fleet?

The purpose of pre-operational audit logs is provenance in the data, software (algorithms), hardware, personnel activities, and processes that are involved in creating an IAS. In order to take action or make a decision, an IAS depends on all of these, but most heavily on the data. Thus, it is critical to ensure that the data are not manipulated, or improperly deleted, and pre-operational audit logs do so by keeping track of authorized users who accesses and processes the data in much the same way as chain of custody is established and maintained in legal proceedings. It is also important to ensure that pre-operational audit logs have detailed descriptions of the origin and trace the development of the algorithms. Pre-operational audit logs also have information on inspecting computer hardware for repairs and modifications. Proper and complete documentation has an important role in establishing a reliable IAS by helping to retain positive control over all aspects of an IAS during its acquisition.</rdfs:comment>
        <rdfs:label>DADM07_PreOperationalAuditLogs</rdfs:label>
        <owl:versionInfo>page 19, page 78</owl:versionInfo>
    </owl:Class>
    


    <!-- https://savage.nps.edu/EthicalControl/ontologies/MissionExecutionOntology#DADM07.1 -->

    <owl:Class rdf:about="https://savage.nps.edu/EthicalControl/ontologies/MissionExecutionOntology#DADM07.1">
        <rdfs:subClassOf rdf:resource="https://savage.nps.edu/EthicalControl/ontologies/MissionExecutionOntology#DADM07"/>
        <rdfs:comment>General considerations</rdfs:comment>
        <rdfs:label>DADM07.1_GeneralConsiderations</rdfs:label>
        <owl:versionInfo>page 78</owl:versionInfo>
    </owl:Class>
    


    <!-- https://savage.nps.edu/EthicalControl/ontologies/MissionExecutionOntology#DADM07.2 -->

    <owl:Class rdf:about="https://savage.nps.edu/EthicalControl/ontologies/MissionExecutionOntology#DADM07.2">
        <rdfs:subClassOf rdf:resource="https://savage.nps.edu/EthicalControl/ontologies/MissionExecutionOntology#DADM07"/>
        <rdfs:comment>Training data provenance</rdfs:comment>
        <rdfs:label>DADM07.2_TrainingDataProvenance</rdfs:label>
        <owl:versionInfo>page 79</owl:versionInfo>
    </owl:Class>
    


    <!-- https://savage.nps.edu/EthicalControl/ontologies/MissionExecutionOntology#DADM07.3 -->

    <owl:Class rdf:about="https://savage.nps.edu/EthicalControl/ontologies/MissionExecutionOntology#DADM07.3">
        <rdfs:subClassOf rdf:resource="https://savage.nps.edu/EthicalControl/ontologies/MissionExecutionOntology#DADM07"/>
        <rdfs:comment>Algorithm provenance</rdfs:comment>
        <rdfs:label>DADM07.3_AlgorithmProvenance</rdfs:label>
        <owl:versionInfo>page 79</owl:versionInfo>
    </owl:Class>
    


    <!-- https://savage.nps.edu/EthicalControl/ontologies/MissionExecutionOntology#DADM07.4 -->

    <owl:Class rdf:about="https://savage.nps.edu/EthicalControl/ontologies/MissionExecutionOntology#DADM07.4">
        <rdfs:subClassOf rdf:resource="https://savage.nps.edu/EthicalControl/ontologies/MissionExecutionOntology#DADM07"/>
        <rdfs:comment>Computer hardware provenance</rdfs:comment>
        <rdfs:label>DADM07.4_ComputerHardwareProvenance</rdfs:label>
        <owl:versionInfo>page 80</owl:versionInfo>
    </owl:Class>
    


    <!-- https://savage.nps.edu/EthicalControl/ontologies/MissionExecutionOntology#DADM07.5 -->

    <owl:Class rdf:about="https://savage.nps.edu/EthicalControl/ontologies/MissionExecutionOntology#DADM07.5">
        <rdfs:subClassOf rdf:resource="https://savage.nps.edu/EthicalControl/ontologies/MissionExecutionOntology#DADM07"/>
        <rdfs:comment>Acquisition and development</rdfs:comment>
        <rdfs:label>DADM07.5_AcquisitionDevelopment</rdfs:label>
        <owl:versionInfo>page 81</owl:versionInfo>
    </owl:Class>
    


    <!-- https://savage.nps.edu/EthicalControl/ontologies/MissionExecutionOntology#DADM07.6 -->

    <owl:Class rdf:about="https://savage.nps.edu/EthicalControl/ontologies/MissionExecutionOntology#DADM07.6">
        <rdfs:subClassOf rdf:resource="https://savage.nps.edu/EthicalControl/ontologies/MissionExecutionOntology#DADM07"/>
        <rdfs:comment>Authorization</rdfs:comment>
        <rdfs:label>DADM07.6_Authorization</rdfs:label>
        <owl:versionInfo>page 81</owl:versionInfo>
    </owl:Class>
    


    <!-- https://savage.nps.edu/EthicalControl/ontologies/MissionExecutionOntology#DADM08 -->

    <owl:Class rdf:about="https://savage.nps.edu/EthicalControl/ontologies/MissionExecutionOntology#DADM08">
        <rdfs:subClassOf rdf:resource="https://savage.nps.edu/EthicalControl/ontologies/MissionExecutionOntology#DimensionsAutonomousDecisionMaking"/>
        <rdfs:comment>Are all environmental conditions, sensor inputs, operator interactions, internal processes, IAS actions, and operational outcomes recorded for post-operation reconstruction and analyses to support accountability and improvements to tactics, techniques, and procedures (TTP) and technology?

An important consideration in establishing confidence in, and acceptance of an IAS is transparency. Documenting inputs, actions, interactions, and outcomes will help create a transparent IAS. The documentation must be detailed and clear enough to promote confidence and acceptance and to enable post-operation reconstruction and analyses. Proper documentation enables users to share suggestions on improvements and lessons learned from previous systems. It also promotes ethical use of an IAS because the traceability created by these logs create the records required to enforce accountability.</rdfs:comment>
        <rdfs:label>DADM08_OperationalAuditLogs</rdfs:label>
        <owl:versionInfo>page 19, page 82</owl:versionInfo>
    </owl:Class>
    


    <!-- https://savage.nps.edu/EthicalControl/ontologies/MissionExecutionOntology#DADM08.1 -->

    <owl:Class rdf:about="https://savage.nps.edu/EthicalControl/ontologies/MissionExecutionOntology#DADM08.1">
        <rdfs:subClassOf rdf:resource="https://savage.nps.edu/EthicalControl/ontologies/MissionExecutionOntology#DADM08"/>
        <rdfs:comment>General considerations</rdfs:comment>
        <rdfs:label>DADM08.1_GeneralConsiderations</rdfs:label>
        <owl:versionInfo>page 82</owl:versionInfo>
    </owl:Class>
    


    <!-- https://savage.nps.edu/EthicalControl/ontologies/MissionExecutionOntology#DADM08.2 -->

    <owl:Class rdf:about="https://savage.nps.edu/EthicalControl/ontologies/MissionExecutionOntology#DADM08.2">
        <rdfs:subClassOf rdf:resource="https://savage.nps.edu/EthicalControl/ontologies/MissionExecutionOntology#DADM08"/>
        <rdfs:comment>Traceability of audit log data elements</rdfs:comment>
        <rdfs:label>DADM08.2_TraceabilityAuditLogDataElements</rdfs:label>
        <owl:versionInfo>page 83</owl:versionInfo>
    </owl:Class>
    


    <!-- https://savage.nps.edu/EthicalControl/ontologies/MissionExecutionOntology#DADM08.3 -->

    <owl:Class rdf:about="https://savage.nps.edu/EthicalControl/ontologies/MissionExecutionOntology#DADM08.3">
        <rdfs:subClassOf rdf:resource="https://savage.nps.edu/EthicalControl/ontologies/MissionExecutionOntology#DADM08"/>
        <rdfs:comment>Operational audit log retention</rdfs:comment>
        <rdfs:label>DADM08.3_OperationalAuditLogRetention</rdfs:label>
        <owl:versionInfo>page 84</owl:versionInfo>
    </owl:Class>
    


    <!-- https://savage.nps.edu/EthicalControl/ontologies/MissionExecutionOntology#DADM08.4 -->

    <owl:Class rdf:about="https://savage.nps.edu/EthicalControl/ontologies/MissionExecutionOntology#DADM08.4">
        <rdfs:subClassOf rdf:resource="https://savage.nps.edu/EthicalControl/ontologies/MissionExecutionOntology#DADM08"/>
        <rdfs:comment>Operational audit log uses</rdfs:comment>
        <rdfs:label>DADM08.4_OperationalAuditLogUses</rdfs:label>
        <owl:versionInfo>page 84</owl:versionInfo>
    </owl:Class>
    


    <!-- https://savage.nps.edu/EthicalControl/ontologies/MissionExecutionOntology#DADM09 -->

    <owl:Class rdf:about="https://savage.nps.edu/EthicalControl/ontologies/MissionExecutionOntology#DADM09">
        <rdfs:subClassOf rdf:resource="https://savage.nps.edu/EthicalControl/ontologies/MissionExecutionOntology#DimensionsAutonomousDecisionMaking"/>
        <rdfs:comment>Does design of the human-machine team (particularly when the use of force is involved) leverage the human’s superior ability to exercise judgment in the use of the IAS in order to reduce the risks associated with its use?

A common theme running through the literature regarding IAS is that the risks of its use come from its inability to adapt, generalize, or put information into a wider context - thus the concepts of &quot;narrow artificial intelligence&quot; [31] and &quot;brittleness&quot; [32]. It is unfortunate then that warfare (and many other application domains where IAS are used) occurs in an unforgiving environment replete with thinking adversaries that actively seek to push enemy commanders out of their tested and preferred concepts of operation and seek to push the technologies they depend on beyond their original design parameters.

One solution to this problem is to put a human operator &quot;back&quot; into or on the loop. This creates a conundrum in that doing so must not reintroduce the negative characteristics of human performance that the IAS was intended to remove in the first place. Human-machine teaming attempts to design system interactions whereby the respective strengths of the human and the machine are retained, and the weaknesses of each are not. IAS weaknesses can introduce additional legal and ethical risks. Human weaknesses can introduce additional operational risk. (18 We do recognize that humans are not legally or ethically infallible.) Therefore, human-machine team designs provide an opportunity to balance legal and ethical risks against operational risks. The objective of this study was to identify and mitigate the legal and ethical risks, but this must be balanced against operational risk. Hence the inclusion of human-machine teaming as a DAD.</rdfs:comment>
        <rdfs:isDefinedBy>Garrett Cookson</rdfs:isDefinedBy>
        <rdfs:label>DADM09_HumanMachineTeaming</rdfs:label>
        <owl:versionInfo>page 19, page 85</owl:versionInfo>
    </owl:Class>
    


    <!-- https://savage.nps.edu/EthicalControl/ontologies/MissionExecutionOntology#DADM09.1 -->

    <owl:Class rdf:about="https://savage.nps.edu/EthicalControl/ontologies/MissionExecutionOntology#DADM09.1">
        <rdfs:subClassOf rdf:resource="https://savage.nps.edu/EthicalControl/ontologies/MissionExecutionOntology#DADM09"/>
        <rdfs:comment>General considerations</rdfs:comment>
        <rdfs:label>DADM09.1_GeneralConsiderations</rdfs:label>
        <owl:versionInfo>page 85</owl:versionInfo>
    </owl:Class>
    


    <!-- https://savage.nps.edu/EthicalControl/ontologies/MissionExecutionOntology#DADM09.2 -->

    <owl:Class rdf:about="https://savage.nps.edu/EthicalControl/ontologies/MissionExecutionOntology#DADM09.2">
        <rdfs:subClassOf rdf:resource="https://savage.nps.edu/EthicalControl/ontologies/MissionExecutionOntology#DADM09"/>
        <rdfs:comment>Conforming and nonconforming human behavior</rdfs:comment>
        <rdfs:label>DADM09.2_ConformingNonconformingHumanBehavior</rdfs:label>
        <owl:versionInfo>page 87</owl:versionInfo>
    </owl:Class>
    


    <!-- https://savage.nps.edu/EthicalControl/ontologies/MissionExecutionOntology#DADM09.3 -->

    <owl:Class rdf:about="https://savage.nps.edu/EthicalControl/ontologies/MissionExecutionOntology#DADM09.3">
        <rdfs:subClassOf rdf:resource="https://savage.nps.edu/EthicalControl/ontologies/MissionExecutionOntology#DADM09"/>
        <rdfs:comment>Managing interactions</rdfs:comment>
        <rdfs:label>DADM09.3_ManagingInstructions</rdfs:label>
        <owl:versionInfo>page 87</owl:versionInfo>
    </owl:Class>
    


    <!-- https://savage.nps.edu/EthicalControl/ontologies/MissionExecutionOntology#DADM10 -->

    <owl:Class rdf:about="https://savage.nps.edu/EthicalControl/ontologies/MissionExecutionOntology#DADM10">
        <rdfs:subClassOf rdf:resource="https://savage.nps.edu/EthicalControl/ontologies/MissionExecutionOntology#DimensionsAutonomousDecisionMaking"/>
        <rdfs:comment>Will/did the IAS test and evaluation procedure reflect the breadth, depth, and complexity of the contemplated operational environment to test and evaluate the system attributes unique to the use of autonomy technologies to the greatest extent practicable?

The potential negative results of systems used by the DOD include unintended deaths. Such high stakes demand an exhaustive approach for test and evaluation to reduce the risk of these negative consequences. Nondeterministic IAS present a situation where the potential configurations are practically infinite in number, negating any attempt to test each and every possible IAS configuration exhaustively in each and every scenario.
Since there is little hope of eliminating all risk, ways must be found to minimize it to the greatest extent possible within the confines of time and funding constraints. Test and evaluation of IAS is further complicated by subjective terminology in the policy documents that mandate it [1, 5].

This DAD aids the development community in the maximization of test and evaluation, and the minimization of risk, to provide a balance between the depth, breadth, and complexity of testing conditions, recognizing that exhaustively testing along all three axes is certainly not practicable and may not be possible.</rdfs:comment>
        <rdfs:label>DADM10_TestEvaluationAdequacy</rdfs:label>
        <owl:versionInfo>page 20, page 88</owl:versionInfo>
    </owl:Class>
    


    <!-- https://savage.nps.edu/EthicalControl/ontologies/MissionExecutionOntology#DADM10.1 -->

    <owl:Class rdf:about="https://savage.nps.edu/EthicalControl/ontologies/MissionExecutionOntology#DADM10.1">
        <rdfs:subClassOf rdf:resource="https://savage.nps.edu/EthicalControl/ontologies/MissionExecutionOntology#DADM10"/>
        <rdfs:comment>General considerations</rdfs:comment>
        <rdfs:label>DADM10.1_GeneralConsiderations</rdfs:label>
        <owl:versionInfo>page 88</owl:versionInfo>
    </owl:Class>
    


    <!-- https://savage.nps.edu/EthicalControl/ontologies/MissionExecutionOntology#DADM10.2 -->

    <owl:Class rdf:about="https://savage.nps.edu/EthicalControl/ontologies/MissionExecutionOntology#DADM10.2">
        <rdfs:subClassOf rdf:resource="https://savage.nps.edu/EthicalControl/ontologies/MissionExecutionOntology#DADM10"/>
        <rdfs:comment>Simulated replication of the operational environment</rdfs:comment>
        <rdfs:label>DADM10.2_SimulatedReplicationOperationalEnvironment</rdfs:label>
        <owl:versionInfo>page 89</owl:versionInfo>
    </owl:Class>
    


    <!-- https://savage.nps.edu/EthicalControl/ontologies/MissionExecutionOntology#DADM10.3 -->

    <owl:Class rdf:about="https://savage.nps.edu/EthicalControl/ontologies/MissionExecutionOntology#DADM10.3">
        <rdfs:subClassOf rdf:resource="https://savage.nps.edu/EthicalControl/ontologies/MissionExecutionOntology#DADM10"/>
        <rdfs:comment>Depth of testing in the replicated environment</rdfs:comment>
        <rdfs:label>DADM10.3_DepthTestingReplicatedEnvironment</rdfs:label>
        <owl:versionInfo>page 90</owl:versionInfo>
    </owl:Class>
    


    <!-- https://savage.nps.edu/EthicalControl/ontologies/MissionExecutionOntology#DADM11 -->

    <owl:Class rdf:about="https://savage.nps.edu/EthicalControl/ontologies/MissionExecutionOntology#DADM11">
        <rdfs:subClassOf rdf:resource="https://savage.nps.edu/EthicalControl/ontologies/MissionExecutionOntology#DADM12"/>
        <rdfs:comment>Does everyone associated with the use of IAS - developers, civilian and military leaders, and operators - understand the attributes of IAS enough to avoid illegal or unethical use?

Initial and continuing training and education prepares developers, operators, and commanders to establish competence in recognizing the characteristics of an IAS that can lead to illegal or unethical use. Also, through training, human operators prepare for situations that require them to be more active and reestablish command and control for safety or security reasons. Training and education also illuminate the limitations of an IAS, the central role of its data and algorithms, and AI-specific failure modes so that the user can clearly understand the IAS technologies and avoid their misuse.</rdfs:comment>
        <rdfs:label>DADM11_AutonomyTrainingEducation</rdfs:label>
        <owl:versionInfo>page 21, page 90</owl:versionInfo>
    </owl:Class>
    


    <!-- https://savage.nps.edu/EthicalControl/ontologies/MissionExecutionOntology#DADM11.1 -->

    <owl:Class rdf:about="https://savage.nps.edu/EthicalControl/ontologies/MissionExecutionOntology#DADM11.1">
        <rdfs:subClassOf rdf:resource="https://savage.nps.edu/EthicalControl/ontologies/MissionExecutionOntology#DADM11"/>
        <rdfs:comment>Ensuring legal and ethical use</rdfs:comment>
        <rdfs:label>DADM11.1_EnsuringLegalEthicalUse</rdfs:label>
        <owl:versionInfo>page 90</owl:versionInfo>
    </owl:Class>
    


    <!-- https://savage.nps.edu/EthicalControl/ontologies/MissionExecutionOntology#DADM11.2 -->

    <owl:Class rdf:about="https://savage.nps.edu/EthicalControl/ontologies/MissionExecutionOntology#DADM11.2">
        <rdfs:subClassOf rdf:resource="https://savage.nps.edu/EthicalControl/ontologies/MissionExecutionOntology#DADM11"/>
        <rdfs:comment>Certifications</rdfs:comment>
        <rdfs:label>DADM11.2_Certifications</rdfs:label>
        <owl:versionInfo>page 91</owl:versionInfo>
    </owl:Class>
    


    <!-- https://savage.nps.edu/EthicalControl/ontologies/MissionExecutionOntology#DADM11.3 -->

    <owl:Class rdf:about="https://savage.nps.edu/EthicalControl/ontologies/MissionExecutionOntology#DADM11.3">
        <rdfs:subClassOf rdf:resource="https://savage.nps.edu/EthicalControl/ontologies/MissionExecutionOntology#DADM11"/>
        <rdfs:comment>Recognizing IAS limitations</rdfs:comment>
        <rdfs:label>DADM11.3_IASLimitations</rdfs:label>
        <owl:versionInfo>page 91</owl:versionInfo>
    </owl:Class>
    


    <!-- https://savage.nps.edu/EthicalControl/ontologies/MissionExecutionOntology#DADM11.4 -->

    <owl:Class rdf:about="https://savage.nps.edu/EthicalControl/ontologies/MissionExecutionOntology#DADM11.4">
        <rdfs:subClassOf rdf:resource="https://savage.nps.edu/EthicalControl/ontologies/MissionExecutionOntology#DADM11"/>
        <rdfs:comment>Understanding the algorithms</rdfs:comment>
        <rdfs:label>DADM11.4_AlgorithmUnderstanding</rdfs:label>
        <owl:versionInfo>page 92</owl:versionInfo>
    </owl:Class>
    


    <!-- https://savage.nps.edu/EthicalControl/ontologies/MissionExecutionOntology#DADM11.5 -->

    <owl:Class rdf:about="https://savage.nps.edu/EthicalControl/ontologies/MissionExecutionOntology#DADM11.5">
        <rdfs:subClassOf rdf:resource="https://savage.nps.edu/EthicalControl/ontologies/MissionExecutionOntology#DADM11"/>
        <rdfs:comment>Recognizing AI-specific failure modes</rdfs:comment>
        <rdfs:label>DADM11.5_RecognizeAIFailureModes</rdfs:label>
        <owl:versionInfo>page 92</owl:versionInfo>
    </owl:Class>
    


    <!-- https://savage.nps.edu/EthicalControl/ontologies/MissionExecutionOntology#DADM12 -->

    <owl:Class rdf:about="https://savage.nps.edu/EthicalControl/ontologies/MissionExecutionOntology#DADM12">
        <rdfs:subClassOf rdf:resource="https://savage.nps.edu/EthicalControl/ontologies/MissionExecutionOntology#DimensionsAutonomousDecisionMaking"/>
        <rdfs:comment>Will the time required to conduct the contemplated mission be so long, and/or the geographic extent of the IAS’ operating envelope so extensive, that pre-mission risk mitigation conditions and planning factors will change to an extent that might increase risk?

The conditions at the beginning of a long-term mission may change with time. They may also change as the geographic range increases and possibly becomes different from what the IAS design calls for. Thus, initial risk assessments and preprogrammed plans may become invalid by the time an IAS needs to execute its task. Considering an IAS’ performance with respect to time and space is crucial in preventing misconstrued confidence that an IAS will execute its task with appropriate risk. In response to changing risk mitigation conditions and planning factors, it is important that an IAS be able to operate effectively and be equipped to disable autonomous functionalities.</rdfs:comment>
        <rdfs:label>DADM12_MissionDurationGeographicExtent</rdfs:label>
        <owl:versionInfo>page 21, page 93</owl:versionInfo>
    </owl:Class>
    


    <!-- https://savage.nps.edu/EthicalControl/ontologies/MissionExecutionOntology#DADM12.1 -->

    <owl:Class rdf:about="https://savage.nps.edu/EthicalControl/ontologies/MissionExecutionOntology#DADM12.1">
        <rdfs:subClassOf rdf:resource="https://savage.nps.edu/EthicalControl/ontologies/MissionExecutionOntology#DADM12"/>
        <rdfs:comment>Temporal subdivision</rdfs:comment>
        <rdfs:label>DADM12.1_TemporalSubdivision</rdfs:label>
        <owl:versionInfo>page 93</owl:versionInfo>
    </owl:Class>
    


    <!-- https://savage.nps.edu/EthicalControl/ontologies/MissionExecutionOntology#DADM12.2 -->

    <owl:Class rdf:about="https://savage.nps.edu/EthicalControl/ontologies/MissionExecutionOntology#DADM12.2">
        <rdfs:subClassOf rdf:resource="https://savage.nps.edu/EthicalControl/ontologies/MissionExecutionOntology#DADM12"/>
        <rdfs:comment>Spatial subdivision</rdfs:comment>
        <rdfs:label>DADM12.2_SpatialSubdivision</rdfs:label>
        <owl:versionInfo>page 93</owl:versionInfo>
    </owl:Class>
    


    <!-- https://savage.nps.edu/EthicalControl/ontologies/MissionExecutionOntology#DADM12.3 -->

    <owl:Class rdf:about="https://savage.nps.edu/EthicalControl/ontologies/MissionExecutionOntology#DADM12.3">
        <rdfs:subClassOf rdf:resource="https://savage.nps.edu/EthicalControl/ontologies/MissionExecutionOntology#DADM12"/>
        <rdfs:comment>Preprogrammed disablement</rdfs:comment>
        <rdfs:label>DADM12.3_PreprogrammedDisablement</rdfs:label>
        <owl:versionInfo>page 94</owl:versionInfo>
    </owl:Class>
    


    <!-- https://savage.nps.edu/EthicalControl/ontologies/MissionExecutionOntology#DADM13 -->

    <owl:Class rdf:about="https://savage.nps.edu/EthicalControl/ontologies/MissionExecutionOntology#DADM13">
        <rdfs:subClassOf rdf:resource="https://savage.nps.edu/EthicalControl/ontologies/MissionExecutionOntology#DimensionsAutonomousDecisionMaking"/>
        <rdfs:comment>Have all available measures been taken to ensure that the IAS algorithms and/or machine learning (ML) training data employed in automated and autonomous decision aids do not contain any biases that might incorrectly, disproportionately, or otherwise unfairly affect an individual or a group of persons?

An IAS must be engineered to safeguard human rights - civil rights, which are explicitly codified in law, and natural rights, which are implicitly accepted to be self-evident by most freedom-loving persons and nations. This DAD contains natural rights that some public policy advocacy groups assert should be codified in law to become civil rights.

DOD intends to develop IAS as LAWS for use against enemy combatants, but also as non-lethal autonomous decision aids that can affect enemy combatants, US servicemembers and their dependents, DOD civilian employees, and third parties (including civilian populations). Clearly, each group has different expectations and protections with respect to civil and natural rights. Enemy combatants, for example, are not protected by many of the civil rights listed in this DAD.

A primary (but by no means only) source of risk to human rights infringement is bias. Therefore, IAS developers must be able to recognize algorithms and data that contain biases that will unfairly affect an individual or a group. Initial mitigation of bias in the software itself involves the developers being aware of a large variety of potential bias sources that can bias an IAS’ decisions against a particular individual or group of persons. This includes sources of &quot;analytical&quot; bias that are not inherently biased against any group or person but could become so if not identified and addressed.

Notifications of when an IAS is in use further mitigate the effects of bias, as they bring awareness to the persons affected by the IAS’ actions and decisions. Not all persons enjoy this right to notification. It is clearly not practical to extend this right to suspected criminals in law enforcement or some homeland security applications. This DAD also addresses the bias that occurs when operating in coalition and allied environments, such as bias that stems from different sets of treaties, ROE, or cultural norms. Overall, it is important for all persons involved - the developer, operator, commander, affected person, and oversight specialists - to be vigilant in detecting bias that may result in human rights violations.</rdfs:comment>
        <rdfs:label>DADM13_CivilNaturalRights</rdfs:label>
        <owl:versionInfo>page 21, page 94</owl:versionInfo>
    </owl:Class>
    


    <!-- https://savage.nps.edu/EthicalControl/ontologies/MissionExecutionOntology#DADM13.1 -->

    <owl:Class rdf:about="https://savage.nps.edu/EthicalControl/ontologies/MissionExecutionOntology#DADM13.1">
        <rdfs:subClassOf rdf:resource="https://savage.nps.edu/EthicalControl/ontologies/MissionExecutionOntology#DADM13"/>
        <rdfs:comment>Rights of potentially affected persons</rdfs:comment>
        <rdfs:label>DADM13.1_RightsPotentiallyAffectedPersons</rdfs:label>
        <owl:versionInfo>page 94</owl:versionInfo>
    </owl:Class>
    


    <!-- https://savage.nps.edu/EthicalControl/ontologies/MissionExecutionOntology#DADM13.2 -->

    <owl:Class rdf:about="https://savage.nps.edu/EthicalControl/ontologies/MissionExecutionOntology#DADM13.2">
        <rdfs:subClassOf rdf:resource="https://savage.nps.edu/EthicalControl/ontologies/MissionExecutionOntology#DADM13"/>
        <rdfs:comment>Rights of persons affected by the actions or decisions of an IAS</rdfs:comment>
        <rdfs:label>DADM13.2_IASDecisionAffectPersonsRights</rdfs:label>
        <owl:versionInfo>page 95</owl:versionInfo>
    </owl:Class>
    


    <!-- https://savage.nps.edu/EthicalControl/ontologies/MissionExecutionOntology#DADM13.3 -->

    <owl:Class rdf:about="https://savage.nps.edu/EthicalControl/ontologies/MissionExecutionOntology#DADM13.3">
        <rdfs:subClassOf rdf:resource="https://savage.nps.edu/EthicalControl/ontologies/MissionExecutionOntology#DADM13"/>
        <rdfs:comment>Guarding against bias and rights violations</rdfs:comment>
        <rdfs:label>DADM13.3_GuardingAgainstBiasRightsViolations</rdfs:label>
        <owl:versionInfo>page 96</owl:versionInfo>
    </owl:Class>
    


    <!-- https://savage.nps.edu/EthicalControl/ontologies/MissionExecutionOntology#DADM13.3.1 -->

    <owl:Class rdf:about="https://savage.nps.edu/EthicalControl/ontologies/MissionExecutionOntology#DADM13.3.1">
        <rdfs:subClassOf rdf:resource="https://savage.nps.edu/EthicalControl/ontologies/MissionExecutionOntology#DADM13.3"/>
        <rdfs:comment>Development phase search for sources of bias</rdfs:comment>
        <rdfs:label>DADM13.3.1_DevelopmentPhaseSearchSourceBias</rdfs:label>
        <owl:versionInfo>page 96</owl:versionInfo>
    </owl:Class>
    


    <!-- https://savage.nps.edu/EthicalControl/ontologies/MissionExecutionOntology#DADM13.3.2 -->

    <owl:Class rdf:about="https://savage.nps.edu/EthicalControl/ontologies/MissionExecutionOntology#DADM13.3.2">
        <rdfs:subClassOf rdf:resource="https://savage.nps.edu/EthicalControl/ontologies/MissionExecutionOntology#DADM13.3"/>
        <rdfs:comment>Post-operational human-on-the-loop oversight</rdfs:comment>
        <rdfs:label>DADM13.3.2_PostoperationalHumanOnTheLoopOversight</rdfs:label>
        <owl:versionInfo>page 99</owl:versionInfo>
    </owl:Class>
    


    <!-- https://savage.nps.edu/EthicalControl/ontologies/MissionExecutionOntology#DADM_Abbreviations -->

    <owl:Class rdf:about="https://savage.nps.edu/EthicalControl/ontologies/MissionExecutionOntology#DADM_Abbreviations">
        <rdfs:subClassOf rdf:resource="https://savage.nps.edu/EthicalControl/ontologies/MissionExecutionOntology#DimensionsAutonomousDecisionMaking"/>
        <rdfs:comment>Abbreviations which detail the acronyms used throughout the document and ontology.

TODO: Figure out how to make abbreviations linkable from the ontology risk elements to the section.</rdfs:comment>
        <rdfs:label>DADM_Abbreviations</rdfs:label>
        <owl:versionInfo>page 100</owl:versionInfo>
    </owl:Class>
    


    <!-- https://savage.nps.edu/EthicalControl/ontologies/MissionExecutionOntology#DADM_Constraints -->

    <owl:Class rdf:about="https://savage.nps.edu/EthicalControl/ontologies/MissionExecutionOntology#DADM_Constraints">
        <rdfs:subClassOf rdf:resource="https://savage.nps.edu/EthicalControl/ontologies/MissionExecutionOntology#DimensionsAutonomousDecisionMaking"/>
        <rdfs:comment>A Constraint is a condition placed on a Mission or a Goal. The Constraint must be satisfied for the associated Mission or Goal to be achievable. A Mission may have multiple Constraint instances. A Constraint on a Mission applies to all of the Goals in the Mission. A Constraint on a Goal applies only to that Goal.</rdfs:comment>
        <rdfs:label>DADM_Constraints</rdfs:label>
    </owl:Class>
    


    <!-- https://savage.nps.edu/EthicalControl/ontologies/MissionExecutionOntology#DADM_OperationalPhases -->

    <owl:Class rdf:about="https://savage.nps.edu/EthicalControl/ontologies/MissionExecutionOntology#DADM_OperationalPhases">
        <rdfs:subClassOf rdf:resource="https://savage.nps.edu/EthicalControl/ontologies/MissionExecutionOntology#DimensionsAutonomousDecisionMaking"/>
        <rdfs:comment>TODO -- correlations to NATO terminology and Duane Davis ontology</rdfs:comment>
        <rdfs:label>DADM_OperationalPhases</rdfs:label>
        <owl:versionInfo>page 60 DADM</owl:versionInfo>
    </owl:Class>
    


    <!-- https://savage.nps.edu/EthicalControl/ontologies/MissionExecutionOntology#DADM_References -->

    <owl:Class rdf:about="https://savage.nps.edu/EthicalControl/ontologies/MissionExecutionOntology#DADM_References">
        <rdfs:subClassOf rdf:resource="https://savage.nps.edu/EthicalControl/ontologies/MissionExecutionOntology#DimensionsAutonomousDecisionMaking"/>
        <rdfs:comment>References are key documents defining principles and concepts of content used throughout the ontology. TODO: Figure out how to make references linkable from the ontology risk elements to the section.</rdfs:comment>
        <rdfs:label>DADM_References</rdfs:label>
        <owl:versionInfo>pages 101-104</owl:versionInfo>
    </owl:Class>
    


    <!-- https://savage.nps.edu/EthicalControl/ontologies/MissionExecutionOntology#DEVRON -->

    <owl:Class rdf:about="https://savage.nps.edu/EthicalControl/ontologies/MissionExecutionOntology#DEVRON">
        <rdfs:subClassOf rdf:resource="https://savage.nps.edu/EthicalControl/ontologies/MissionExecutionOntology#DADM_Abbreviations"/>
        <rdfs:label>Development Squadron (DEVRON)</rdfs:label>
        <owl:versionInfo>page 100</owl:versionInfo>
    </owl:Class>
    


    <!-- https://savage.nps.edu/EthicalControl/ontologies/MissionExecutionOntology#DHS -->

    <owl:Class rdf:about="https://savage.nps.edu/EthicalControl/ontologies/MissionExecutionOntology#DHS">
        <rdfs:subClassOf rdf:resource="https://savage.nps.edu/EthicalControl/ontologies/MissionExecutionOntology#DADM_Abbreviations"/>
        <rdfs:label>Department of Homeland Security (DHS)</rdfs:label>
        <owl:versionInfo>page 100</owl:versionInfo>
    </owl:Class>
    


    <!-- https://savage.nps.edu/EthicalControl/ontologies/MissionExecutionOntology#DRAID -->

    <owl:Class rdf:about="https://savage.nps.edu/EthicalControl/ontologies/MissionExecutionOntology#DRAID">
        <rdfs:subClassOf rdf:resource="https://savage.nps.edu/EthicalControl/ontologies/MissionExecutionOntology#DADM_Abbreviations"/>
        <rdfs:label>Joint AI Center’s Data Readiness for AI Data (DRAID)</rdfs:label>
        <owl:versionInfo>page 100</owl:versionInfo>
    </owl:Class>
    


    <!-- https://savage.nps.edu/EthicalControl/ontologies/MissionExecutionOntology#DimensionsAutonomousDecisionMaking -->

    <owl:Class rdf:about="https://savage.nps.edu/EthicalControl/ontologies/MissionExecutionOntology#DimensionsAutonomousDecisionMaking">
        <rdfs:comment>Abstract
This study identifies the dimensions of autonomous decision-making (DADMs), namely the categories and causes of potential risk that one should consider before transferring decision-making capabilities to an intelligent autonomous system (IAS). The objective of this study was to provide some of the tools needed to implement existing policies with respect to the legal, ethical, and militarily effective use of IAS. These tools help to identify and either mitigate or accept the risks associated with the use of IAS that might result in a negative outcome. The 13 identified DADMs were developed from a comprehensive list of 565 &quot;risk elements&quot; drawn from hundreds of documents authored by parties in favor of, and opposed to, the use of autonomy technology in weapons systems. We record these elements in the form of a question so that they can be used by the acquisition community to develop requirements documents that ensure the ethical use of autonomous systems, and be used by military commanders as a risk assessment checklist to ensure that autonomous systems are not used in an unethical manner. In this way, the Department of Defense can make fully-informed risk assessment decisions before developing or deploying autonomous systems.</rdfs:comment>
        <owl:versionInfo>DRM-2021-U-030642-1Rev</owl:versionInfo>
    </owl:Class>
    


    <!-- https://savage.nps.edu/EthicalControl/ontologies/MissionExecutionOntology#DoD -->

    <owl:Class rdf:about="https://savage.nps.edu/EthicalControl/ontologies/MissionExecutionOntology#DoD">
        <rdfs:subClassOf rdf:resource="https://savage.nps.edu/EthicalControl/ontologies/MissionExecutionOntology#DADM_Abbreviations"/>
        <rdfs:label>Department of Defense (DoD)</rdfs:label>
        <owl:versionInfo>page 100</owl:versionInfo>
    </owl:Class>
    


    <!-- https://savage.nps.edu/EthicalControl/ontologies/MissionExecutionOntology#DoN -->

    <owl:Class rdf:about="https://savage.nps.edu/EthicalControl/ontologies/MissionExecutionOntology#DoN">
        <rdfs:subClassOf rdf:resource="https://savage.nps.edu/EthicalControl/ontologies/MissionExecutionOntology#DADM_Abbreviations"/>
        <rdfs:label>Department of the Navy (DoN)</rdfs:label>
        <owl:versionInfo>page 100</owl:versionInfo>
    </owl:Class>
    


    <!-- https://savage.nps.edu/EthicalControl/ontologies/MissionExecutionOntology#EXCEPTION -->

    <owl:Class rdf:about="https://savage.nps.edu/EthicalControl/ontologies/MissionExecutionOntology#EXCEPTION">
        <rdfs:subClassOf rdf:resource="https://savage.nps.edu/EthicalControl/ontologies/MissionExecutionOntology#EndCondition"/>
        <rdfs:comment>The EXCEPTION EndCondition indicates a Goal did not complete due to run-time determination that an associated Constraint was not satisfied.</rdfs:comment>
    </owl:Class>
    


    <!-- https://savage.nps.edu/EthicalControl/ontologies/MissionExecutionOntology#EndCondition -->

    <owl:Class rdf:about="https://savage.nps.edu/EthicalControl/ontologies/MissionExecutionOntology#EndCondition">
        <owl:equivalentClass>
            <owl:Class>
                <owl:unionOf rdf:parseType="Collection">
                    <rdf:Description rdf:about="https://savage.nps.edu/EthicalControl/ontologies/MissionExecutionOntology#EXCEPTION"/>
                    <rdf:Description rdf:about="https://savage.nps.edu/EthicalControl/ontologies/MissionExecutionOntology#FAILURE"/>
                    <rdf:Description rdf:about="https://savage.nps.edu/EthicalControl/ontologies/MissionExecutionOntology#SUCCESS"/>
                </owl:unionOf>
            </owl:Class>
        </owl:equivalentClass>
        <rdfs:comment>EndCondition describes termination state upon finishing a Goal. Enumeration values describe the result of executing a Goal instance in a mission.  An allowed value is either SUCCESS, FAILURE, or EXCEPTION. Such ternary logic for connecting goals appears to be fully capable of describing any mission decision tree.</rdfs:comment>
    </owl:Class>
    


    <!-- https://savage.nps.edu/EthicalControl/ontologies/MissionExecutionOntology#FAILURE -->

    <owl:Class rdf:about="https://savage.nps.edu/EthicalControl/ontologies/MissionExecutionOntology#FAILURE">
        <rdfs:subClassOf rdf:resource="https://savage.nps.edu/EthicalControl/ontologies/MissionExecutionOntology#EndCondition"/>
        <rdfs:comment>The FAILURE EndCondition indicates that a Goal instance completed but failed to meet one or more associated IntendedOutcome requirements.</rdfs:comment>
    </owl:Class>
    


    <!-- https://savage.nps.edu/EthicalControl/ontologies/MissionExecutionOntology#FFRDC -->

    <owl:Class rdf:about="https://savage.nps.edu/EthicalControl/ontologies/MissionExecutionOntology#FFRDC">
        <rdfs:subClassOf rdf:resource="https://savage.nps.edu/EthicalControl/ontologies/MissionExecutionOntology#DADM_Abbreviations"/>
        <rdfs:label>Federally Funded Research and Development Center (FFRDC)</rdfs:label>
        <owl:versionInfo>page 100</owl:versionInfo>
    </owl:Class>
    


    <!-- https://savage.nps.edu/EthicalControl/ontologies/MissionExecutionOntology#GeospatialConstraint -->

    <owl:Class rdf:about="https://savage.nps.edu/EthicalControl/ontologies/MissionExecutionOntology#GeospatialConstraint">
        <rdfs:subClassOf rdf:resource="https://savage.nps.edu/EthicalControl/ontologies/MissionExecutionOntology#OperationalConstraint"/>
        <rdfs:subClassOf rdf:resource="https://savage.nps.edu/EthicalControl/ontologies/MissionExecutionOntology#PolicyConstraint"/>
    </owl:Class>
    


    <!-- https://savage.nps.edu/EthicalControl/ontologies/MissionExecutionOntology#Goal -->

    <owl:Class rdf:about="https://savage.nps.edu/EthicalControl/ontologies/MissionExecutionOntology#Goal">
        <rdfs:subClassOf>
            <owl:Class>
                <owl:unionOf rdf:parseType="Collection">
                    <owl:Class>
                        <owl:intersectionOf rdf:parseType="Collection">
                            <owl:Restriction>
                                <owl:onProperty rdf:resource="https://savage.nps.edu/EthicalControl/ontologies/MissionExecutionOntology#hasEndCondition"/>
                                <owl:allValuesFrom rdf:resource="https://savage.nps.edu/EthicalControl/ontologies/MissionExecutionOntology#EXCEPTION"/>
                            </owl:Restriction>
                            <owl:Restriction>
                                <owl:onProperty rdf:resource="https://savage.nps.edu/EthicalControl/ontologies/MissionExecutionOntology#hasNextGoalOnException"/>
                                <owl:qualifiedCardinality rdf:datatype="http://www.w3.org/2001/XMLSchema#nonNegativeInteger">1</owl:qualifiedCardinality>
                                <owl:onClass rdf:resource="https://savage.nps.edu/EthicalControl/ontologies/MissionExecutionOntology#Goal"/>
                            </owl:Restriction>
                        </owl:intersectionOf>
                    </owl:Class>
                    <owl:Class>
                        <owl:intersectionOf rdf:parseType="Collection">
                            <owl:Restriction>
                                <owl:onProperty rdf:resource="https://savage.nps.edu/EthicalControl/ontologies/MissionExecutionOntology#hasEndCondition"/>
                                <owl:allValuesFrom rdf:resource="https://savage.nps.edu/EthicalControl/ontologies/MissionExecutionOntology#FAILURE"/>
                            </owl:Restriction>
                            <owl:Restriction>
                                <owl:onProperty rdf:resource="https://savage.nps.edu/EthicalControl/ontologies/MissionExecutionOntology#hasNextGoalOnFailure"/>
                                <owl:qualifiedCardinality rdf:datatype="http://www.w3.org/2001/XMLSchema#nonNegativeInteger">1</owl:qualifiedCardinality>
                                <owl:onClass rdf:resource="https://savage.nps.edu/EthicalControl/ontologies/MissionExecutionOntology#Goal"/>
                            </owl:Restriction>
                        </owl:intersectionOf>
                    </owl:Class>
                    <owl:Class>
                        <owl:intersectionOf rdf:parseType="Collection">
                            <owl:Restriction>
                                <owl:onProperty rdf:resource="https://savage.nps.edu/EthicalControl/ontologies/MissionExecutionOntology#hasEndCondition"/>
                                <owl:allValuesFrom rdf:resource="https://savage.nps.edu/EthicalControl/ontologies/MissionExecutionOntology#SUCCESS"/>
                            </owl:Restriction>
                            <owl:Restriction>
                                <owl:onProperty rdf:resource="https://savage.nps.edu/EthicalControl/ontologies/MissionExecutionOntology#hasNextGoalOnSuccess"/>
                                <owl:qualifiedCardinality rdf:datatype="http://www.w3.org/2001/XMLSchema#nonNegativeInteger">1</owl:qualifiedCardinality>
                                <owl:onClass rdf:resource="https://savage.nps.edu/EthicalControl/ontologies/MissionExecutionOntology#Goal"/>
                            </owl:Restriction>
                        </owl:intersectionOf>
                    </owl:Class>
                </owl:unionOf>
            </owl:Class>
        </rdfs:subClassOf>
        <rdfs:subClassOf>
            <owl:Restriction>
                <owl:onProperty rdf:resource="https://savage.nps.edu/EthicalControl/ontologies/MissionExecutionOntology#hasConstraint"/>
                <owl:allValuesFrom rdf:resource="https://savage.nps.edu/EthicalControl/ontologies/MissionExecutionOntology#DADM_Constraints"/>
            </owl:Restriction>
        </rdfs:subClassOf>
        <rdfs:subClassOf>
            <owl:Restriction>
                <owl:onProperty rdf:resource="https://savage.nps.edu/EthicalControl/ontologies/MissionExecutionOntology#hasEndCondition"/>
                <owl:allValuesFrom rdf:resource="https://savage.nps.edu/EthicalControl/ontologies/MissionExecutionOntology#EndCondition"/>
            </owl:Restriction>
        </rdfs:subClassOf>
        <rdfs:subClassOf>
            <owl:Restriction>
                <owl:onProperty rdf:resource="https://savage.nps.edu/EthicalControl/ontologies/MissionExecutionOntology#isFollowedBy"/>
                <owl:allValuesFrom rdf:resource="https://savage.nps.edu/EthicalControl/ontologies/MissionExecutionOntology#Goal"/>
            </owl:Restriction>
        </rdfs:subClassOf>
        <rdfs:subClassOf>
            <owl:Restriction>
                <owl:onProperty rdf:resource="https://savage.nps.edu/EthicalControl/ontologies/MissionExecutionOntology#mustSatisfy"/>
                <owl:allValuesFrom rdf:resource="https://savage.nps.edu/EthicalControl/ontologies/MissionExecutionOntology#IntendedOutcome"/>
            </owl:Restriction>
        </rdfs:subClassOf>
        <rdfs:subClassOf>
            <owl:Restriction>
                <owl:onProperty rdf:resource="https://savage.nps.edu/EthicalControl/ontologies/MissionExecutionOntology#hasEndCondition"/>
                <owl:maxQualifiedCardinality rdf:datatype="http://www.w3.org/2001/XMLSchema#nonNegativeInteger">1</owl:maxQualifiedCardinality>
                <owl:onClass rdf:resource="https://savage.nps.edu/EthicalControl/ontologies/MissionExecutionOntology#EndCondition"/>
            </owl:Restriction>
        </rdfs:subClassOf>
        <rdfs:subClassOf>
            <owl:Restriction>
                <owl:onProperty rdf:resource="https://savage.nps.edu/EthicalControl/ontologies/MissionExecutionOntology/isPartOfPhase"/>
                <owl:maxQualifiedCardinality rdf:datatype="http://www.w3.org/2001/XMLSchema#nonNegativeInteger">1</owl:maxQualifiedCardinality>
                <owl:onDataRange rdf:resource="http://www.w3.org/2001/XMLSchema#string"/>
            </owl:Restriction>
        </rdfs:subClassOf>
        <rdfs:comment>A Goal is an operational objective the mission is intended to achieve.</rdfs:comment>
    </owl:Class>
    <owl:Axiom>
        <owl:annotatedSource rdf:resource="https://savage.nps.edu/EthicalControl/ontologies/MissionExecutionOntology#Goal"/>
        <owl:annotatedProperty rdf:resource="http://www.w3.org/2000/01/rdf-schema#subClassOf"/>
        <owl:annotatedTarget>
            <owl:Restriction>
                <owl:onProperty rdf:resource="https://savage.nps.edu/EthicalControl/ontologies/MissionExecutionOntology#mustSatisfy"/>
                <owl:allValuesFrom rdf:resource="https://savage.nps.edu/EthicalControl/ontologies/MissionExecutionOntology#IntendedOutcome"/>
            </owl:Restriction>
        </owl:annotatedTarget>
        <rdfs:comment>A Goal may require 0 or more GoalRequirements.</rdfs:comment>
        <rdfs:label>G1</rdfs:label>
    </owl:Axiom>
    <owl:Axiom>
        <owl:annotatedSource rdf:resource="https://savage.nps.edu/EthicalControl/ontologies/MissionExecutionOntology#Goal"/>
        <owl:annotatedProperty rdf:resource="http://www.w3.org/2000/01/rdf-schema#subClassOf"/>
        <owl:annotatedTarget>
            <owl:Restriction>
                <owl:onProperty rdf:resource="https://savage.nps.edu/EthicalControl/ontologies/MissionExecutionOntology#hasEndCondition"/>
                <owl:maxQualifiedCardinality rdf:datatype="http://www.w3.org/2001/XMLSchema#nonNegativeInteger">1</owl:maxQualifiedCardinality>
                <owl:onClass rdf:resource="https://savage.nps.edu/EthicalControl/ontologies/MissionExecutionOntology#EndCondition"/>
            </owl:Restriction>
        </owl:annotatedTarget>
        <rdfs:comment>A Goal&apos;s ending condition (state) can end with at most one EndCondition.

[NOTE: This statement would seem to apply more to the final state of the Goal during Mission execution. In planning, there must be consideration of what happens following Goal success, failure, or faces an imminent exception. That is, what is the next Goal for the Vehicle to perform under each of those end conditions?]</rdfs:comment>
        <rdfs:label>G2</rdfs:label>
    </owl:Axiom>
    


    <!-- https://savage.nps.edu/EthicalControl/ontologies/MissionExecutionOntology#IAS -->

    <owl:Class rdf:about="https://savage.nps.edu/EthicalControl/ontologies/MissionExecutionOntology#IAS">
        <rdfs:subClassOf rdf:resource="https://savage.nps.edu/EthicalControl/ontologies/MissionExecutionOntology#DADM_Abbreviations"/>
        <rdfs:label>Intelligent Autonomous System (IAS)</rdfs:label>
        <owl:versionInfo>page 100</owl:versionInfo>
    </owl:Class>
    


    <!-- https://savage.nps.edu/EthicalControl/ontologies/MissionExecutionOntology#IntendedOutcome -->

    <owl:Class rdf:about="https://savage.nps.edu/EthicalControl/ontologies/MissionExecutionOntology#IntendedOutcome">
        <rdfs:comment>IntendedOutcome is a condition that must be met for the associated Goal to be achieved successfully.</rdfs:comment>
    </owl:Class>
    


    <!-- https://savage.nps.edu/EthicalControl/ontologies/MissionExecutionOntology#InternationalHumanitarianLaw -->

    <owl:Class rdf:about="https://savage.nps.edu/EthicalControl/ontologies/MissionExecutionOntology#InternationalHumanitarianLaw">
        <rdfs:subClassOf rdf:resource="https://savage.nps.edu/EthicalControl/ontologies/MissionExecutionOntology#LegalConstraint"/>
    </owl:Class>
    


    <!-- https://savage.nps.edu/EthicalControl/ontologies/MissionExecutionOntology#JAREL -->

    <owl:Class rdf:about="https://savage.nps.edu/EthicalControl/ontologies/MissionExecutionOntology#JAREL">
        <rdfs:subClassOf rdf:resource="https://savage.nps.edu/EthicalControl/ontologies/MissionExecutionOntology#DADM_Abbreviations"/>
        <rdfs:label>Joint Autonomy Risk Elements List (JAREL)</rdfs:label>
        <owl:versionInfo>page 100</owl:versionInfo>
    </owl:Class>
    


    <!-- https://savage.nps.edu/EthicalControl/ontologies/MissionExecutionOntology#KPP -->

    <owl:Class rdf:about="https://savage.nps.edu/EthicalControl/ontologies/MissionExecutionOntology#KPP">
        <rdfs:subClassOf rdf:resource="https://savage.nps.edu/EthicalControl/ontologies/MissionExecutionOntology#DADM_Abbreviations"/>
        <rdfs:label>Key Performance Parameter (KPP)</rdfs:label>
        <owl:versionInfo>page 100</owl:versionInfo>
    </owl:Class>
    


    <!-- https://savage.nps.edu/EthicalControl/ontologies/MissionExecutionOntology#KSA -->

    <owl:Class rdf:about="https://savage.nps.edu/EthicalControl/ontologies/MissionExecutionOntology#KSA">
        <rdfs:subClassOf rdf:resource="https://savage.nps.edu/EthicalControl/ontologies/MissionExecutionOntology#DADM_Abbreviations"/>
        <rdfs:label>Key System Attribute (KSA)</rdfs:label>
        <owl:versionInfo>page 100</owl:versionInfo>
    </owl:Class>
    


    <!-- https://savage.nps.edu/EthicalControl/ontologies/MissionExecutionOntology#LAWS -->

    <owl:Class rdf:about="https://savage.nps.edu/EthicalControl/ontologies/MissionExecutionOntology#LAWS">
        <rdfs:subClassOf rdf:resource="https://savage.nps.edu/EthicalControl/ontologies/MissionExecutionOntology#DADM_Abbreviations"/>
        <rdfs:label>Lethal Autonomous Weapons System (LAWS)</rdfs:label>
        <owl:versionInfo>page 100</owl:versionInfo>
    </owl:Class>
    


    <!-- https://savage.nps.edu/EthicalControl/ontologies/MissionExecutionOntology#LOAC -->

    <owl:Class rdf:about="https://savage.nps.edu/EthicalControl/ontologies/MissionExecutionOntology#LOAC">
        <rdfs:subClassOf rdf:resource="https://savage.nps.edu/EthicalControl/ontologies/MissionExecutionOntology#DADM_Abbreviations"/>
        <rdfs:label>Laws of Armed Conflict ((LOAC)</rdfs:label>
        <owl:versionInfo>page 100</owl:versionInfo>
    </owl:Class>
    


    <!-- https://savage.nps.edu/EthicalControl/ontologies/MissionExecutionOntology#LawOfArmedConflict -->

    <owl:Class rdf:about="https://savage.nps.edu/EthicalControl/ontologies/MissionExecutionOntology#LawOfArmedConflict">
        <rdfs:subClassOf rdf:resource="https://savage.nps.edu/EthicalControl/ontologies/MissionExecutionOntology#LegalConstraint"/>
    </owl:Class>
    


    <!-- https://savage.nps.edu/EthicalControl/ontologies/MissionExecutionOntology#LegalConstraint -->

    <owl:Class rdf:about="https://savage.nps.edu/EthicalControl/ontologies/MissionExecutionOntology#LegalConstraint">
        <rdfs:subClassOf rdf:resource="https://savage.nps.edu/EthicalControl/ontologies/MissionExecutionOntology#PolicyConstraint"/>
    </owl:Class>
    


    <!-- https://savage.nps.edu/EthicalControl/ontologies/MissionExecutionOntology#METL -->

    <owl:Class rdf:about="https://savage.nps.edu/EthicalControl/ontologies/MissionExecutionOntology#METL">
        <rdfs:subClassOf rdf:resource="https://savage.nps.edu/EthicalControl/ontologies/MissionExecutionOntology#DADM_Abbreviations"/>
        <rdfs:label>Mission Essential Task List (METL)</rdfs:label>
        <owl:versionInfo>page 100</owl:versionInfo>
    </owl:Class>
    


    <!-- https://savage.nps.edu/EthicalControl/ontologies/MissionExecutionOntology#MOP -->

    <owl:Class rdf:about="https://savage.nps.edu/EthicalControl/ontologies/MissionExecutionOntology#MOP">
        <rdfs:subClassOf rdf:resource="https://savage.nps.edu/EthicalControl/ontologies/MissionExecutionOntology#DADM_Abbreviations"/>
        <rdfs:label>Measure of Performance (MOP)</rdfs:label>
        <owl:versionInfo>page 100</owl:versionInfo>
    </owl:Class>
    


    <!-- https://savage.nps.edu/EthicalControl/ontologies/MissionExecutionOntology#Mission -->

    <owl:Class rdf:about="https://savage.nps.edu/EthicalControl/ontologies/MissionExecutionOntology#Mission">
        <rdfs:subClassOf>
            <owl:Restriction>
                <owl:onProperty rdf:resource="https://savage.nps.edu/EthicalControl/ontologies/MissionExecutionOntology#hasIntendedOutcome"/>
                <owl:someValuesFrom rdf:resource="https://savage.nps.edu/EthicalControl/ontologies/MissionExecutionOntology#IntendedOutcome"/>
            </owl:Restriction>
        </rdfs:subClassOf>
        <rdfs:subClassOf>
            <owl:Restriction>
                <owl:onProperty rdf:resource="https://savage.nps.edu/EthicalControl/ontologies/MissionExecutionOntology#hasConstraint"/>
                <owl:allValuesFrom rdf:resource="https://savage.nps.edu/EthicalControl/ontologies/MissionExecutionOntology#DADM_Constraints"/>
            </owl:Restriction>
        </rdfs:subClassOf>
        <rdfs:subClassOf>
            <owl:Restriction>
                <owl:onProperty rdf:resource="https://savage.nps.edu/EthicalControl/ontologies/MissionExecutionOntology#isPerformableBy"/>
                <owl:allValuesFrom rdf:resource="https://savage.nps.edu/EthicalControl/ontologies/MissionExecutionOntology#Vehicle"/>
            </owl:Restriction>
        </rdfs:subClassOf>
        <rdfs:subClassOf>
            <owl:Restriction>
                <owl:onProperty rdf:resource="https://savage.nps.edu/EthicalControl/ontologies/MissionExecutionOntology#includes"/>
                <owl:minQualifiedCardinality rdf:datatype="http://www.w3.org/2001/XMLSchema#nonNegativeInteger">1</owl:minQualifiedCardinality>
                <owl:onClass rdf:resource="https://savage.nps.edu/EthicalControl/ontologies/MissionExecutionOntology#Goal"/>
            </owl:Restriction>
        </rdfs:subClassOf>
        <rdfs:subClassOf>
            <owl:Restriction>
                <owl:onProperty rdf:resource="https://savage.nps.edu/EthicalControl/ontologies/MissionExecutionOntology#startsWith"/>
                <owl:qualifiedCardinality rdf:datatype="http://www.w3.org/2001/XMLSchema#nonNegativeInteger">1</owl:qualifiedCardinality>
                <owl:onClass rdf:resource="https://savage.nps.edu/EthicalControl/ontologies/MissionExecutionOntology#Goal"/>
            </owl:Restriction>
        </rdfs:subClassOf>
        <rdfs:comment>Mission is a set of Goals to be performed by a Vehicle, under one or more Constraint instances associated with the Mission or with individual Goals in the Mission.</rdfs:comment>
    </owl:Class>
    <owl:Axiom>
        <owl:annotatedSource rdf:resource="https://savage.nps.edu/EthicalControl/ontologies/MissionExecutionOntology#Mission"/>
        <owl:annotatedProperty rdf:resource="http://www.w3.org/2000/01/rdf-schema#subClassOf"/>
        <owl:annotatedTarget>
            <owl:Restriction>
                <owl:onProperty rdf:resource="https://savage.nps.edu/EthicalControl/ontologies/MissionExecutionOntology#hasConstraint"/>
                <owl:allValuesFrom rdf:resource="https://savage.nps.edu/EthicalControl/ontologies/MissionExecutionOntology#DADM_Constraints"/>
            </owl:Restriction>
        </owl:annotatedTarget>
        <rdfs:comment>A Mission can have 0 or more Constraints.</rdfs:comment>
        <rdfs:label>M3</rdfs:label>
    </owl:Axiom>
    <owl:Axiom>
        <owl:annotatedSource rdf:resource="https://savage.nps.edu/EthicalControl/ontologies/MissionExecutionOntology#Mission"/>
        <owl:annotatedProperty rdf:resource="http://www.w3.org/2000/01/rdf-schema#subClassOf"/>
        <owl:annotatedTarget>
            <owl:Restriction>
                <owl:onProperty rdf:resource="https://savage.nps.edu/EthicalControl/ontologies/MissionExecutionOntology#isPerformableBy"/>
                <owl:allValuesFrom rdf:resource="https://savage.nps.edu/EthicalControl/ontologies/MissionExecutionOntology#Vehicle"/>
            </owl:Restriction>
        </owl:annotatedTarget>
        <rdfs:comment>A Mission can be performable by 0 or more Vehicles.</rdfs:comment>
        <rdfs:label>M5</rdfs:label>
    </owl:Axiom>
    <owl:Axiom>
        <owl:annotatedSource rdf:resource="https://savage.nps.edu/EthicalControl/ontologies/MissionExecutionOntology#Mission"/>
        <owl:annotatedProperty rdf:resource="http://www.w3.org/2000/01/rdf-schema#subClassOf"/>
        <owl:annotatedTarget>
            <owl:Restriction>
                <owl:onProperty rdf:resource="https://savage.nps.edu/EthicalControl/ontologies/MissionExecutionOntology#includes"/>
                <owl:minQualifiedCardinality rdf:datatype="http://www.w3.org/2001/XMLSchema#nonNegativeInteger">1</owl:minQualifiedCardinality>
                <owl:onClass rdf:resource="https://savage.nps.edu/EthicalControl/ontologies/MissionExecutionOntology#Goal"/>
            </owl:Restriction>
        </owl:annotatedTarget>
        <rdfs:comment>A Mission must include one or more goals.</rdfs:comment>
        <rdfs:label>M2</rdfs:label>
    </owl:Axiom>
    <owl:Axiom>
        <owl:annotatedSource rdf:resource="https://savage.nps.edu/EthicalControl/ontologies/MissionExecutionOntology#Mission"/>
        <owl:annotatedProperty rdf:resource="http://www.w3.org/2000/01/rdf-schema#subClassOf"/>
        <owl:annotatedTarget>
            <owl:Restriction>
                <owl:onProperty rdf:resource="https://savage.nps.edu/EthicalControl/ontologies/MissionExecutionOntology#startsWith"/>
                <owl:qualifiedCardinality rdf:datatype="http://www.w3.org/2001/XMLSchema#nonNegativeInteger">1</owl:qualifiedCardinality>
                <owl:onClass rdf:resource="https://savage.nps.edu/EthicalControl/ontologies/MissionExecutionOntology#Goal"/>
            </owl:Restriction>
        </owl:annotatedTarget>
        <rdfs:comment>A Mission must start with exactly one Goal.</rdfs:comment>
        <rdfs:label>M1</rdfs:label>
    </owl:Axiom>
    


    <!-- https://savage.nps.edu/EthicalControl/ontologies/MissionExecutionOntology#NATOPolicy -->

    <owl:Class rdf:about="https://savage.nps.edu/EthicalControl/ontologies/MissionExecutionOntology#NATOPolicy">
        <rdfs:subClassOf rdf:resource="https://savage.nps.edu/EthicalControl/ontologies/MissionExecutionOntology#LegalConstraint"/>
    </owl:Class>
    


    <!-- https://savage.nps.edu/EthicalControl/ontologies/MissionExecutionOntology#OP01_Search -->

    <owl:Class rdf:about="https://savage.nps.edu/EthicalControl/ontologies/MissionExecutionOntology#OP01_Search">
        <rdfs:subClassOf rdf:resource="https://savage.nps.edu/EthicalControl/ontologies/MissionExecutionOntology#DADM_OperationalPhases"/>
        <rdfs:seeAlso></rdfs:seeAlso>
        <owl:versionInfo>page 60 DADM</owl:versionInfo>
    </owl:Class>
    


    <!-- https://savage.nps.edu/EthicalControl/ontologies/MissionExecutionOntology#OP02_Detection -->

    <owl:Class rdf:about="https://savage.nps.edu/EthicalControl/ontologies/MissionExecutionOntology#OP02_Detection">
        <rdfs:subClassOf rdf:resource="https://savage.nps.edu/EthicalControl/ontologies/MissionExecutionOntology#DADM_OperationalPhases"/>
        <owl:versionInfo>page 60 DADM</owl:versionInfo>
    </owl:Class>
    


    <!-- https://savage.nps.edu/EthicalControl/ontologies/MissionExecutionOntology#OP03_Tracking -->

    <owl:Class rdf:about="https://savage.nps.edu/EthicalControl/ontologies/MissionExecutionOntology#OP03_Tracking">
        <rdfs:subClassOf rdf:resource="https://savage.nps.edu/EthicalControl/ontologies/MissionExecutionOntology#DADM_OperationalPhases"/>
        <owl:versionInfo>page 60 DADM</owl:versionInfo>
    </owl:Class>
    


    <!-- https://savage.nps.edu/EthicalControl/ontologies/MissionExecutionOntology#OP04_Identification -->

    <owl:Class rdf:about="https://savage.nps.edu/EthicalControl/ontologies/MissionExecutionOntology#OP04_Identification">
        <rdfs:subClassOf rdf:resource="https://savage.nps.edu/EthicalControl/ontologies/MissionExecutionOntology#DADM_OperationalPhases"/>
        <owl:versionInfo>page 60 DADM</owl:versionInfo>
    </owl:Class>
    


    <!-- https://savage.nps.edu/EthicalControl/ontologies/MissionExecutionOntology#OP05_Cueing -->

    <owl:Class rdf:about="https://savage.nps.edu/EthicalControl/ontologies/MissionExecutionOntology#OP05_Cueing">
        <rdfs:subClassOf rdf:resource="https://savage.nps.edu/EthicalControl/ontologies/MissionExecutionOntology#DADM_OperationalPhases"/>
        <owl:versionInfo>page 60 DADM</owl:versionInfo>
    </owl:Class>
    


    <!-- https://savage.nps.edu/EthicalControl/ontologies/MissionExecutionOntology#OP06_Prioritization -->

    <owl:Class rdf:about="https://savage.nps.edu/EthicalControl/ontologies/MissionExecutionOntology#OP06_Prioritization">
        <rdfs:subClassOf rdf:resource="https://savage.nps.edu/EthicalControl/ontologies/MissionExecutionOntology#DADM_OperationalPhases"/>
        <owl:versionInfo>page 60 DADM</owl:versionInfo>
    </owl:Class>
    


    <!-- https://savage.nps.edu/EthicalControl/ontologies/MissionExecutionOntology#OP07_Selection -->

    <owl:Class rdf:about="https://savage.nps.edu/EthicalControl/ontologies/MissionExecutionOntology#OP07_Selection">
        <rdfs:subClassOf rdf:resource="https://savage.nps.edu/EthicalControl/ontologies/MissionExecutionOntology#DADM_OperationalPhases"/>
        <owl:versionInfo>page 60 DADM</owl:versionInfo>
    </owl:Class>
    


    <!-- https://savage.nps.edu/EthicalControl/ontologies/MissionExecutionOntology#OP08_EngagementTiming -->

    <owl:Class rdf:about="https://savage.nps.edu/EthicalControl/ontologies/MissionExecutionOntology#OP08_EngagementTiming">
        <rdfs:subClassOf rdf:resource="https://savage.nps.edu/EthicalControl/ontologies/MissionExecutionOntology#DADM_OperationalPhases"/>
        <owl:versionInfo>page 60 DADM</owl:versionInfo>
    </owl:Class>
    


    <!-- https://savage.nps.edu/EthicalControl/ontologies/MissionExecutionOntology#OP09_TerminalGuidance -->

    <owl:Class rdf:about="https://savage.nps.edu/EthicalControl/ontologies/MissionExecutionOntology#OP09_TerminalGuidance">
        <rdfs:subClassOf rdf:resource="https://savage.nps.edu/EthicalControl/ontologies/MissionExecutionOntology#DADM_OperationalPhases"/>
        <owl:versionInfo>page 60 DADM</owl:versionInfo>
    </owl:Class>
    


    <!-- https://savage.nps.edu/EthicalControl/ontologies/MissionExecutionOntology#OP10_Engagement -->

    <owl:Class rdf:about="https://savage.nps.edu/EthicalControl/ontologies/MissionExecutionOntology#OP10_Engagement">
        <rdfs:subClassOf rdf:resource="https://savage.nps.edu/EthicalControl/ontologies/MissionExecutionOntology#DADM_OperationalPhases"/>
        <owl:versionInfo>page 60 DADM</owl:versionInfo>
    </owl:Class>
    


    <!-- https://savage.nps.edu/EthicalControl/ontologies/MissionExecutionOntology#OP11_BattleDamageAssessment -->

    <owl:Class rdf:about="https://savage.nps.edu/EthicalControl/ontologies/MissionExecutionOntology#OP11_BattleDamageAssessment">
        <rdfs:subClassOf rdf:resource="https://savage.nps.edu/EthicalControl/ontologies/MissionExecutionOntology#DADM_OperationalPhases"/>
        <owl:versionInfo>page 60 DADM</owl:versionInfo>
    </owl:Class>
    


    <!-- https://savage.nps.edu/EthicalControl/ontologies/MissionExecutionOntology#OperationalConstraint -->

    <owl:Class rdf:about="https://savage.nps.edu/EthicalControl/ontologies/MissionExecutionOntology#OperationalConstraint">
        <rdfs:subClassOf rdf:resource="https://savage.nps.edu/EthicalControl/ontologies/MissionExecutionOntology#DADM_Constraints"/>
    </owl:Class>
    


    <!-- https://savage.nps.edu/EthicalControl/ontologies/MissionExecutionOntology#PlanningConstraint -->

    <owl:Class rdf:about="https://savage.nps.edu/EthicalControl/ontologies/MissionExecutionOntology#PlanningConstraint">
        <rdfs:subClassOf rdf:resource="https://savage.nps.edu/EthicalControl/ontologies/MissionExecutionOntology#DADM_Constraints"/>
    </owl:Class>
    


    <!-- https://savage.nps.edu/EthicalControl/ontologies/MissionExecutionOntology#PolicyConstraint -->

    <owl:Class rdf:about="https://savage.nps.edu/EthicalControl/ontologies/MissionExecutionOntology#PolicyConstraint">
        <rdfs:subClassOf rdf:resource="https://savage.nps.edu/EthicalControl/ontologies/MissionExecutionOntology#DADM_Constraints"/>
    </owl:Class>
    


    <!-- https://savage.nps.edu/EthicalControl/ontologies/MissionExecutionOntology#PostOperationAnalyticsConstraint -->

    <owl:Class rdf:about="https://savage.nps.edu/EthicalControl/ontologies/MissionExecutionOntology#PostOperationAnalyticsConstraint">
        <rdfs:subClassOf rdf:resource="https://savage.nps.edu/EthicalControl/ontologies/MissionExecutionOntology#DADM_Constraints"/>
    </owl:Class>
    


    <!-- https://savage.nps.edu/EthicalControl/ontologies/MissionExecutionOntology#RE -->

    <owl:Class rdf:about="https://savage.nps.edu/EthicalControl/ontologies/MissionExecutionOntology#RE">
        <rdfs:subClassOf rdf:resource="https://savage.nps.edu/EthicalControl/ontologies/MissionExecutionOntology#DADM_Abbreviations"/>
        <rdfs:comment>Risk Element definitions are fundamentally important to determine risk mitigation</rdfs:comment>
        <rdfs:label>Risk Element (RE)</rdfs:label>
        <owl:versionInfo>page 100</owl:versionInfo>
    </owl:Class>
    


    <!-- https://savage.nps.edu/EthicalControl/ontologies/MissionExecutionOntology#RE01.1 -->

    <owl:Class rdf:about="https://savage.nps.edu/EthicalControl/ontologies/MissionExecutionOntology#RE01.1">
        <rdfs:subClassOf rdf:resource="https://savage.nps.edu/EthicalControl/ontologies/MissionExecutionOntology#DADM01"/>
        <rdfs:comment>Have all parties identified all the important terms being used in the development and use of the IAS that require definition?</rdfs:comment>
        <rdfs:label>RE01.1_IdentifiedTermsDevelopmentUse</rdfs:label>
        <owl:versionInfo>page 59</owl:versionInfo>
    </owl:Class>
    


    <!-- https://savage.nps.edu/EthicalControl/ontologies/MissionExecutionOntology#RE01.10 -->

    <owl:Class rdf:about="https://savage.nps.edu/EthicalControl/ontologies/MissionExecutionOntology#RE01.10">
        <rdfs:subClassOf rdf:resource="https://savage.nps.edu/EthicalControl/ontologies/MissionExecutionOntology#DADM01"/>
        <rdfs:comment>Are all parties using the same risk management framework?</rdfs:comment>
        <rdfs:label>RE01.10_SameDefinitionRiskFramework</rdfs:label>
        <owl:versionInfo>page 59</owl:versionInfo>
    </owl:Class>
    


    <!-- https://savage.nps.edu/EthicalControl/ontologies/MissionExecutionOntology#RE01.11 -->

    <owl:Class rdf:about="https://savage.nps.edu/EthicalControl/ontologies/MissionExecutionOntology#RE01.11">
        <rdfs:subClassOf rdf:resource="https://savage.nps.edu/EthicalControl/ontologies/MissionExecutionOntology#DADM01"/>
        <rdfs:comment>Are all parties using the same technical standards throughout the entire lifecycle of the IAS?</rdfs:comment>
        <rdfs:label>RE01.11_SameDefinitionsLifecycleTechnicalStandards</rdfs:label>
        <owl:versionInfo>page 59</owl:versionInfo>
    </owl:Class>
    


    <!-- https://savage.nps.edu/EthicalControl/ontologies/MissionExecutionOntology#RE01.12 -->

    <owl:Class rdf:about="https://savage.nps.edu/EthicalControl/ontologies/MissionExecutionOntology#RE01.12">
        <rdfs:subClassOf rdf:resource="https://savage.nps.edu/EthicalControl/ontologies/MissionExecutionOntology#DADM01"/>
        <rdfs:comment>Are all parties using the same metrics for quantitative analysis (e.g., analyzing confidence levels, comparing similarities, measuring differences)?</rdfs:comment>
        <rdfs:label>RE01.12_SameDefinitionsQuantitativeAnalysis</rdfs:label>
        <owl:versionInfo>page 59</owl:versionInfo>
    </owl:Class>
    


    <!-- https://savage.nps.edu/EthicalControl/ontologies/MissionExecutionOntology#RE01.2 -->

    <owl:Class rdf:about="https://savage.nps.edu/EthicalControl/ontologies/MissionExecutionOntology#RE01.2">
        <rdfs:subClassOf rdf:resource="https://savage.nps.edu/EthicalControl/ontologies/MissionExecutionOntology#DADM01"/>
        <rdfs:comment>Are all parties (when they come from different organizations with different doctrine with respect to IAS use) using consistent and non-conflicting doctrinal terminology?</rdfs:comment>
        <rdfs:label>RE01.2_ConsistentDoctrinalTerminology</rdfs:label>
        <owl:versionInfo>page 59</owl:versionInfo>
    </owl:Class>
    


    <!-- https://savage.nps.edu/EthicalControl/ontologies/MissionExecutionOntology#RE01.3 -->

    <owl:Class rdf:about="https://savage.nps.edu/EthicalControl/ontologies/MissionExecutionOntology#RE01.3">
        <rdfs:subClassOf rdf:resource="https://savage.nps.edu/EthicalControl/ontologies/MissionExecutionOntology#DADM01"/>
        <rdfs:comment>Does IAS use require the use of rapidly emerging terminology that must be defined and agreed upon before use?</rdfs:comment>
        <rdfs:label>RE01.3_RapidlyEmergingTerminology</rdfs:label>
        <owl:versionInfo>page 59</owl:versionInfo>
    </owl:Class>
    


    <!-- https://savage.nps.edu/EthicalControl/ontologies/MissionExecutionOntology#RE01.4 -->

    <owl:Class rdf:about="https://savage.nps.edu/EthicalControl/ontologies/MissionExecutionOntology#RE01.4">
        <rdfs:subClassOf rdf:resource="https://savage.nps.edu/EthicalControl/ontologies/MissionExecutionOntology#DADM01"/>
        <rdfs:comment>Are all parties using the same definitions for &quot;artificial intelligence,&quot; &quot;intelligent autonomous systems,&quot; &quot;autonomy,&quot; &quot;automatic,&quot; and &quot;autonomous functionality?&quot;</rdfs:comment>
        <rdfs:label>RE01.4_SameDefinitionsAI</rdfs:label>
        <owl:versionInfo>page 59</owl:versionInfo>
    </owl:Class>
    


    <!-- https://savage.nps.edu/EthicalControl/ontologies/MissionExecutionOntology#RE01.5 -->

    <owl:Class rdf:about="https://savage.nps.edu/EthicalControl/ontologies/MissionExecutionOntology#RE01.5">
        <rdfs:subClassOf rdf:resource="https://savage.nps.edu/EthicalControl/ontologies/MissionExecutionOntology#DADM01"/>
        <rdfs:comment>Are all parties using the same definitions for &quot;peacetime status&quot; and wartime status?&quot;</rdfs:comment>
        <rdfs:label>RE01.5_SameDefinitionsPeaceWar</rdfs:label>
        <owl:versionInfo>page 59</owl:versionInfo>
    </owl:Class>
    


    <!-- https://savage.nps.edu/EthicalControl/ontologies/MissionExecutionOntology#RE01.6 -->

    <owl:Class rdf:about="https://savage.nps.edu/EthicalControl/ontologies/MissionExecutionOntology#RE01.6">
        <rdfs:subClassOf rdf:resource="https://savage.nps.edu/EthicalControl/ontologies/MissionExecutionOntology#DADM01"/>
        <rdfs:comment>Are all parties using the same definitions for IAS &quot;degree of autonomy?&quot;</rdfs:comment>
        <rdfs:label>RE01.6_SameDefinitionDegreeAutonomy</rdfs:label>
        <owl:versionInfo>page 59</owl:versionInfo>
    </owl:Class>
    


    <!-- https://savage.nps.edu/EthicalControl/ontologies/MissionExecutionOntology#RE01.7 -->

    <owl:Class rdf:about="https://savage.nps.edu/EthicalControl/ontologies/MissionExecutionOntology#RE01.7">
        <rdfs:subClassOf rdf:resource="https://savage.nps.edu/EthicalControl/ontologies/MissionExecutionOntology#DADM01"/>
        <rdfs:comment>Are all parties using the same definition for &quot;realistic operational environment&quot; for IAS developmental and operational test and evaluation purposes?</rdfs:comment>
        <rdfs:label>RE01.7_SameDefinitionRealisticOperationalEnvironment</rdfs:label>
        <owl:versionInfo>page 59</owl:versionInfo>
    </owl:Class>
    


    <!-- https://savage.nps.edu/EthicalControl/ontologies/MissionExecutionOntology#RE01.8 -->

    <owl:Class rdf:about="https://savage.nps.edu/EthicalControl/ontologies/MissionExecutionOntology#RE01.8">
        <rdfs:subClassOf rdf:resource="https://savage.nps.edu/EthicalControl/ontologies/MissionExecutionOntology#DADM01"/>
        <rdfs:comment>Are all parties using the same definitions for &quot;training data, input data and feedback data?&quot;</rdfs:comment>
        <rdfs:label>RE01.8_SameDefinitionsModelTestTrainValidate</rdfs:label>
        <owl:versionInfo>page 59</owl:versionInfo>
    </owl:Class>
    


    <!-- https://savage.nps.edu/EthicalControl/ontologies/MissionExecutionOntology#RE01.9 -->

    <owl:Class rdf:about="https://savage.nps.edu/EthicalControl/ontologies/MissionExecutionOntology#RE01.9">
        <rdfs:subClassOf rdf:resource="https://savage.nps.edu/EthicalControl/ontologies/MissionExecutionOntology#DADM01"/>
        <rdfs:comment>Are all parties using the same definitions for the several and distinct operational phases?</rdfs:comment>
        <rdfs:label>RE01.9_SameDefinitionsOperationalPhases</rdfs:label>
        <owl:versionInfo>page 59</owl:versionInfo>
    </owl:Class>
    


    <!-- https://savage.nps.edu/EthicalControl/ontologies/MissionExecutionOntology#RE02.1.1 -->

    <owl:Class rdf:about="https://savage.nps.edu/EthicalControl/ontologies/MissionExecutionOntology#RE02.1.1">
        <rdfs:subClassOf rdf:resource="https://savage.nps.edu/EthicalControl/ontologies/MissionExecutionOntology#DADM02.1"/>
        <rdfs:comment>Has the concept of operation been analyzed to verify that no temporal or spatial accountability gaps exist regarding the use of IAS?</rdfs:comment>
        <rdfs:label>RE02.1.1_ConsiderationsOperationalPhases</rdfs:label>
        <owl:versionInfo>page 60</owl:versionInfo>
    </owl:Class>
    


    <!-- https://savage.nps.edu/EthicalControl/ontologies/MissionExecutionOntology#RE02.1.2 -->

    <owl:Class rdf:about="https://savage.nps.edu/EthicalControl/ontologies/MissionExecutionOntology#RE02.1.2">
        <rdfs:subClassOf rdf:resource="https://savage.nps.edu/EthicalControl/ontologies/MissionExecutionOntology#DADM02.1"/>
        <rdfs:comment>Has the concept of operation been analyzed to verify that no transfer of command and control over the IAS can occur without specific authorization by the person(s) designated to be accountable for the use of the IAS?</rdfs:comment>
        <rdfs:label>RE02.1.2_TransferCommandControl</rdfs:label>
        <owl:versionInfo>page 60</owl:versionInfo>
    </owl:Class>
    


    <!-- https://savage.nps.edu/EthicalControl/ontologies/MissionExecutionOntology#RE02.1.3 -->

    <owl:Class rdf:about="https://savage.nps.edu/EthicalControl/ontologies/MissionExecutionOntology#RE02.1.3">
        <rdfs:subClassOf rdf:resource="https://savage.nps.edu/EthicalControl/ontologies/MissionExecutionOntology#DADM02.1"/>
        <rdfs:comment>Is/are the person(s) designated to be accountable for the use of an IAS the only person(s) with the physical ability to transfer decision-making capability to the IAS?</rdfs:comment>
        <rdfs:label>RE02.1.3_SingleDecisionAuthority</rdfs:label>
        <owl:versionInfo>page 60</owl:versionInfo>
    </owl:Class>
    


    <!-- https://savage.nps.edu/EthicalControl/ontologies/MissionExecutionOntology#RE02.1.4 -->

    <owl:Class rdf:about="https://savage.nps.edu/EthicalControl/ontologies/MissionExecutionOntology#RE02.1.4">
        <rdfs:subClassOf rdf:resource="https://savage.nps.edu/EthicalControl/ontologies/MissionExecutionOntology#DADM02.1"/>
        <rdfs:comment>Is/are the person(s) designated to be accountable for the use of an IAS the only person(s) able to authorize in situ changes to the IAS’s configuration created by exposure to incoming data streams?</rdfs:comment>
        <rdfs:label>RE02.1.4_DesignatedChangeAuthority</rdfs:label>
        <owl:versionInfo>page 60</owl:versionInfo>
    </owl:Class>
    


    <!-- https://savage.nps.edu/EthicalControl/ontologies/MissionExecutionOntology#RE02.1.5 -->

    <owl:Class rdf:about="https://savage.nps.edu/EthicalControl/ontologies/MissionExecutionOntology#RE02.1.5">
        <rdfs:subClassOf rdf:resource="https://savage.nps.edu/EthicalControl/ontologies/MissionExecutionOntology#DADM02.1"/>
        <rdfs:comment>Have all persons who may be designated to be accountable for the use of an IAS received training on the Law of Armed Conflict and ethics policies?</rdfs:comment>
        <rdfs:label>RE02.1.5_ArmedConflictEthicsPolicyTraining</rdfs:label>
        <owl:versionInfo>page 60</owl:versionInfo>
    </owl:Class>
    


    <!-- https://savage.nps.edu/EthicalControl/ontologies/MissionExecutionOntology#RE02.1.6 -->

    <owl:Class rdf:about="https://savage.nps.edu/EthicalControl/ontologies/MissionExecutionOntology#RE02.1.6">
        <rdfs:subClassOf rdf:resource="https://savage.nps.edu/EthicalControl/ontologies/MissionExecutionOntology#DADM02.1"/>
        <rdfs:comment>Have all persons who may be designated to be accountable for the use of an IAS been briefed on the current and prevailing rules of engagement?</rdfs:comment>
        <rdfs:label>RE02.1.6_UnderstandRulesEngagement</rdfs:label>
        <owl:versionInfo>page 60</owl:versionInfo>
    </owl:Class>
    


    <!-- https://savage.nps.edu/EthicalControl/ontologies/MissionExecutionOntology#RE02.1.7 -->

    <owl:Class rdf:about="https://savage.nps.edu/EthicalControl/ontologies/MissionExecutionOntology#RE02.1.7">
        <rdfs:subClassOf rdf:resource="https://savage.nps.edu/EthicalControl/ontologies/MissionExecutionOntology#DADM02.1"/>
        <rdfs:comment>Have all persons who may be designated to be accountable for the use of an IAS understand that transfer of decision-making capabilities to an IAS does not transfer accountability for the results of any decisions made by that IAS?</rdfs:comment>
        <rdfs:label>RE02.1.7_UnderstandingDecisionAccountability</rdfs:label>
        <owl:versionInfo>page 60</owl:versionInfo>
    </owl:Class>
    


    <!-- https://savage.nps.edu/EthicalControl/ontologies/MissionExecutionOntology#RE02.1.8 -->

    <owl:Class rdf:about="https://savage.nps.edu/EthicalControl/ontologies/MissionExecutionOntology#RE02.1.8">
        <rdfs:subClassOf rdf:resource="https://savage.nps.edu/EthicalControl/ontologies/MissionExecutionOntology#DADM02.1"/>
        <rdfs:comment>Can IAS lethal capabilities (or other capabilities authorized only for use during wartime) be disabled during peacetime and only be activated after a verifiable transmission is received from an accountable (military or civilian) authority?</rdfs:comment>
        <rdfs:label>RE02.1.8_SecureWartimeModes</rdfs:label>
        <owl:versionInfo>page 60</owl:versionInfo>
    </owl:Class>
    


    <!-- https://savage.nps.edu/EthicalControl/ontologies/MissionExecutionOntology#RE02.1.9 -->

    <owl:Class rdf:about="https://savage.nps.edu/EthicalControl/ontologies/MissionExecutionOntology#RE02.1.9">
        <rdfs:subClassOf rdf:resource="https://savage.nps.edu/EthicalControl/ontologies/MissionExecutionOntology#DADM02.1"/>
        <rdfs:comment>Can the IAS engagement parameters be pre-set to either allow or prohibit it from developing its own target selection, discrimination, or engagement criteria?</rdfs:comment>
        <rdfs:label>RE02.1.9_PreconfigurationFullAuto</rdfs:label>
        <owl:versionInfo>page 60</owl:versionInfo>
    </owl:Class>
    


    <!-- https://savage.nps.edu/EthicalControl/ontologies/MissionExecutionOntology#RE02.2.1 -->

    <owl:Class rdf:about="https://savage.nps.edu/EthicalControl/ontologies/MissionExecutionOntology#RE02.2.1">
        <rdfs:subClassOf rdf:resource="https://savage.nps.edu/EthicalControl/ontologies/MissionExecutionOntology#DADM02.2"/>
        <rdfs:comment>Does the IAS allow for human judgment to be exercised over the IAS during this phase while complying with the relevant rules of engagement?</rdfs:comment>
        <rdfs:label>RE02.2.1_HumanOveridesROEPerson</rdfs:label>
        <owl:versionInfo>page 61</owl:versionInfo>
    </owl:Class>
    


    <!-- https://savage.nps.edu/EthicalControl/ontologies/MissionExecutionOntology#RE02.2.2 -->

    <owl:Class rdf:about="https://savage.nps.edu/EthicalControl/ontologies/MissionExecutionOntology#RE02.2.2">
        <rdfs:subClassOf rdf:resource="https://savage.nps.edu/EthicalControl/ontologies/MissionExecutionOntology#DADM02.2"/>
        <rdfs:comment>If one is required, has the commander designated someone to be accountable for exercising human judgement over any IAS in use during this phase?</rdfs:comment>
        <rdfs:label>RE02.2.2_DesignatedHumanOversightPerson</rdfs:label>
        <owl:versionInfo>page 61</owl:versionInfo>
    </owl:Class>
    


    <!-- https://savage.nps.edu/EthicalControl/ontologies/MissionExecutionOntology#RE02.2.3 -->

    <owl:Class rdf:about="https://savage.nps.edu/EthicalControl/ontologies/MissionExecutionOntology#RE02.2.3">
        <rdfs:subClassOf rdf:resource="https://savage.nps.edu/EthicalControl/ontologies/MissionExecutionOntology#DADM02.2"/>
        <rdfs:comment>Is/are the accountable person(s) able to disable, redirect or recall the IAS if they obtain evidence that it may be operating in a manner contrary to law, policy, rules of engagement, or outside of expected technical parameters?</rdfs:comment>
        <rdfs:label>RE02.2.3_EndOpUseAccountablePerson</rdfs:label>
        <owl:versionInfo>page 61</owl:versionInfo>
    </owl:Class>
    


    <!-- https://savage.nps.edu/EthicalControl/ontologies/MissionExecutionOntology#RE02.2.4 -->

    <owl:Class rdf:about="https://savage.nps.edu/EthicalControl/ontologies/MissionExecutionOntology#RE02.2.4">
        <rdfs:subClassOf rdf:resource="https://savage.nps.edu/EthicalControl/ontologies/MissionExecutionOntology#DADM02.2"/>
        <rdfs:comment>Are there multiple connected IAS involved in the mission?</rdfs:comment>
        <rdfs:label>RE02.2.4_MultipleSystemsComplexity</rdfs:label>
        <owl:versionInfo>page 61</owl:versionInfo>
    </owl:Class>
    


    <!-- https://savage.nps.edu/EthicalControl/ontologies/MissionExecutionOntology#RE02.2.5 -->

    <owl:Class rdf:about="https://savage.nps.edu/EthicalControl/ontologies/MissionExecutionOntology#RE02.2.5">
        <rdfs:subClassOf rdf:resource="https://savage.nps.edu/EthicalControl/ontologies/MissionExecutionOntology#DADM02.2"/>
        <rdfs:comment>Have all systems assessed as having no autonomous functionality been certified to that affect?</rdfs:comment>
        <rdfs:label>RE02.2.5_CertifiedUnknownAutonomy</rdfs:label>
        <owl:versionInfo>page 61</owl:versionInfo>
    </owl:Class>
    


    <!-- https://savage.nps.edu/EthicalControl/ontologies/MissionExecutionOntology#RE02.2.6 -->

    <owl:Class rdf:about="https://savage.nps.edu/EthicalControl/ontologies/MissionExecutionOntology#RE02.2.6">
        <rdfs:subClassOf rdf:resource="https://savage.nps.edu/EthicalControl/ontologies/MissionExecutionOntology#DADM02.2"/>
        <rdfs:comment>Is/are the person(s) accountable for executing the tasks in this phase aware of all IAS available for use?</rdfs:comment>
        <rdfs:label>RE02.2.6_IASSystemFullScopePerson</rdfs:label>
        <owl:versionInfo>page 61</owl:versionInfo>
    </owl:Class>
    


    <!-- https://savage.nps.edu/EthicalControl/ontologies/MissionExecutionOntology#RE02.2.7 -->

    <owl:Class rdf:about="https://savage.nps.edu/EthicalControl/ontologies/MissionExecutionOntology#RE02.2.7">
        <rdfs:subClassOf rdf:resource="https://savage.nps.edu/EthicalControl/ontologies/MissionExecutionOntology#DADM02.2"/>
        <rdfs:comment>Is/are the person(s) accountable for executing the tasks in this phase trained and certified in the use of all IAS available for use?</rdfs:comment>
        <rdfs:label>RE02.2.7_IASSystemCertifiedPerson</rdfs:label>
        <owl:versionInfo>page 61</owl:versionInfo>
    </owl:Class>
    


    <!-- https://savage.nps.edu/EthicalControl/ontologies/MissionExecutionOntology#RE02.2.8 -->

    <owl:Class rdf:about="https://savage.nps.edu/EthicalControl/ontologies/MissionExecutionOntology#RE02.2.8">
        <rdfs:subClassOf rdf:resource="https://savage.nps.edu/EthicalControl/ontologies/MissionExecutionOntology#DADM02.2"/>
        <rdfs:comment>Will the IAS respond to instructions only from the person(s) designated to be accountable for the use of the IAS?</rdfs:comment>
        <rdfs:label>RE02.2.8_SingleControlPersonAccountable</rdfs:label>
        <owl:versionInfo>page 61</owl:versionInfo>
    </owl:Class>
    


    <!-- https://savage.nps.edu/EthicalControl/ontologies/MissionExecutionOntology#RE02.2.9 -->

    <owl:Class rdf:about="https://savage.nps.edu/EthicalControl/ontologies/MissionExecutionOntology#RE02.2.9">
        <rdfs:subClassOf rdf:resource="https://savage.nps.edu/EthicalControl/ontologies/MissionExecutionOntology#DADM02.2"/>
        <rdfs:comment>Will the IAS respond only to instructions that follow the commander’s intent or equivalent authoritative statement of the overarching mission objectives?</rdfs:comment>
        <rdfs:label>RE02.2.9_ControlWithinMissionObjectives</rdfs:label>
        <owl:versionInfo>page 61</owl:versionInfo>
    </owl:Class>
    


    <!-- https://savage.nps.edu/EthicalControl/ontologies/MissionExecutionOntology#RE02.3.1 -->

    <owl:Class rdf:about="https://savage.nps.edu/EthicalControl/ontologies/MissionExecutionOntology#RE02.3.1">
        <rdfs:subClassOf rdf:resource="https://savage.nps.edu/EthicalControl/ontologies/MissionExecutionOntology#DADM02.3"/>
        <rdfs:comment>Can the IAS transfer command and control between entities authorized to exercise this command and control without creating any temporal gaps in accountability?</rdfs:comment>
        <rdfs:label>RE02.3.1_TimeGapsControlChanges</rdfs:label>
        <owl:versionInfo>page 61</owl:versionInfo>
    </owl:Class>
    


    <!-- https://savage.nps.edu/EthicalControl/ontologies/MissionExecutionOntology#RE02.3.2 -->

    <owl:Class rdf:about="https://savage.nps.edu/EthicalControl/ontologies/MissionExecutionOntology#RE02.3.2">
        <rdfs:subClassOf rdf:resource="https://savage.nps.edu/EthicalControl/ontologies/MissionExecutionOntology#DADM02.3"/>
        <rdfs:comment>Is there a process by which the person(s) designated to be accountable for the use of an IAS in any particular phase are made aware of any decisions made by an IAS in a previous phase that they have &quot;inherited&quot; and are now accountable for?</rdfs:comment>
        <rdfs:label>RE02.3.2_InheritedControlAccountabilityDebt</rdfs:label>
        <owl:versionInfo>page 61</owl:versionInfo>
    </owl:Class>
    


    <!-- https://savage.nps.edu/EthicalControl/ontologies/MissionExecutionOntology#RE02.3.3 -->

    <owl:Class rdf:about="https://savage.nps.edu/EthicalControl/ontologies/MissionExecutionOntology#RE02.3.3">
        <rdfs:subClassOf rdf:resource="https://savage.nps.edu/EthicalControl/ontologies/MissionExecutionOntology#DADM02.3"/>
        <rdfs:comment>Does the IAS clearly communicate the transfer of command and control to and/or from the human operator?</rdfs:comment>
        <rdfs:label>RE02.3.3_SystemIndicatesPositiveChangeControls</rdfs:label>
        <owl:versionInfo>page 61</owl:versionInfo>
    </owl:Class>
    


    <!-- https://savage.nps.edu/EthicalControl/ontologies/MissionExecutionOntology#RE02.3.4 -->

    <owl:Class rdf:about="https://savage.nps.edu/EthicalControl/ontologies/MissionExecutionOntology#RE02.3.4">
        <rdfs:subClassOf rdf:resource="https://savage.nps.edu/EthicalControl/ontologies/MissionExecutionOntology#DADM02.3"/>
        <rdfs:comment>Is accountability for the use of the IAS, to include knowledge of what actions may transfer accountability to others or to themselves, understood by all participants in the operation?</rdfs:comment>
        <rdfs:label>RE02.3.4_OperationalBriefingControlAuthorities</rdfs:label>
        <owl:versionInfo>page 61</owl:versionInfo>
    </owl:Class>
    


    <!-- https://savage.nps.edu/EthicalControl/ontologies/MissionExecutionOntology#RE02.3.5 -->

    <owl:Class rdf:about="https://savage.nps.edu/EthicalControl/ontologies/MissionExecutionOntology#RE02.3.5">
        <rdfs:subClassOf rdf:resource="https://savage.nps.edu/EthicalControl/ontologies/MissionExecutionOntology#DADM02.3"/>
        <rdfs:comment>Can the human operator take command and control of just the use of force functions and allow the IAS to continue to execute other tasks (i.e., navigation, sensor data ingest) autonomously?</rdfs:comment>
        <rdfs:label>RE02.3.5_PersonControlForceFunctions</rdfs:label>
        <owl:versionInfo>page 62</owl:versionInfo>
    </owl:Class>
    


    <!-- https://savage.nps.edu/EthicalControl/ontologies/MissionExecutionOntology#RE02.3.6 -->

    <owl:Class rdf:about="https://savage.nps.edu/EthicalControl/ontologies/MissionExecutionOntology#RE02.3.6">
        <rdfs:subClassOf rdf:resource="https://savage.nps.edu/EthicalControl/ontologies/MissionExecutionOntology#DADM02.3"/>
        <rdfs:comment>Are there subsystems in the IAS that can continue to operate with full autonomy, while other subsystems need human judgment?</rdfs:comment>
        <rdfs:label>RE02.3.6_PartialAutonomyRequiresHuman</rdfs:label>
        <owl:versionInfo>page 62</owl:versionInfo>
    </owl:Class>
    


    <!-- https://savage.nps.edu/EthicalControl/ontologies/MissionExecutionOntology#RE02.3.7 -->

    <owl:Class rdf:about="https://savage.nps.edu/EthicalControl/ontologies/MissionExecutionOntology#RE02.3.7">
        <rdfs:subClassOf rdf:resource="https://savage.nps.edu/EthicalControl/ontologies/MissionExecutionOntology#DADM02.3"/>
        <rdfs:comment>Will the transfer of command and control between (culturally different) coalition and allied forces be subject to any cultural biases in training data sets that might affect IAS functions?</rdfs:comment>
        <rdfs:label>RE02.3.7_JointOperationalBiasSystem</rdfs:label>
        <owl:versionInfo>page 62</owl:versionInfo>
    </owl:Class>
    


    <!-- https://savage.nps.edu/EthicalControl/ontologies/MissionExecutionOntology#RE02.3.8 -->

    <owl:Class rdf:about="https://savage.nps.edu/EthicalControl/ontologies/MissionExecutionOntology#RE02.3.8">
        <rdfs:subClassOf rdf:resource="https://savage.nps.edu/EthicalControl/ontologies/MissionExecutionOntology#DADM02.3"/>
        <rdfs:comment>Do the commander and human operators understand the implications of sharing accountability when transferring command and control in coalition and allied operations?</rdfs:comment>
        <rdfs:label>RE02.3.8_SharedAccountabilityJointOperations</rdfs:label>
        <owl:versionInfo>page 62</owl:versionInfo>
    </owl:Class>
    


    <!-- https://savage.nps.edu/EthicalControl/ontologies/MissionExecutionOntology#RE02.3.9 -->

    <owl:Class rdf:about="https://savage.nps.edu/EthicalControl/ontologies/MissionExecutionOntology#RE02.3.9">
        <rdfs:subClassOf rdf:resource="https://savage.nps.edu/EthicalControl/ontologies/MissionExecutionOntology#DADM02.3"/>
        <rdfs:comment>Is the human operator sufficiently trained to appropriately judge when to take command and control even when the IAS does not recommend it?</rdfs:comment>
        <rdfs:label>RE02.3.9_HumanJudgementTakeControls</rdfs:label>
        <owl:versionInfo>page 62</owl:versionInfo>
    </owl:Class>
    


    <!-- https://savage.nps.edu/EthicalControl/ontologies/MissionExecutionOntology#RE02.4.1 -->

    <owl:Class rdf:about="https://savage.nps.edu/EthicalControl/ontologies/MissionExecutionOntology#RE02.4.1">
        <rdfs:subClassOf rdf:resource="https://savage.nps.edu/EthicalControl/ontologies/MissionExecutionOntology#DADM02.4"/>
        <rdfs:comment>Are protections in place to prevent the problem of the &quot;moral buffer,&quot; where the user mentally transfers accountability for negative consequences to the machine?</rdfs:comment>
        <rdfs:label>RE02.4.1_MoralBufferHuman</rdfs:label>
        <owl:versionInfo>page 62</owl:versionInfo>
    </owl:Class>
    


    <!-- https://savage.nps.edu/EthicalControl/ontologies/MissionExecutionOntology#RE02.4.2 -->

    <owl:Class rdf:about="https://savage.nps.edu/EthicalControl/ontologies/MissionExecutionOntology#RE02.4.2">
        <rdfs:subClassOf rdf:resource="https://savage.nps.edu/EthicalControl/ontologies/MissionExecutionOntology#DADM02.4"/>
        <rdfs:comment>Has/have an accountable person(s) been identified for the inadvertent use of force (to include friendly-fire incidents) caused by the IAS?</rdfs:comment>
        <rdfs:label>RE02.4.2_PersonAccountableFriendlyFire</rdfs:label>
        <owl:versionInfo>page 62</owl:versionInfo>
    </owl:Class>
    


    <!-- https://savage.nps.edu/EthicalControl/ontologies/MissionExecutionOntology#RE02.4.3 -->

    <owl:Class rdf:about="https://savage.nps.edu/EthicalControl/ontologies/MissionExecutionOntology#RE02.4.3">
        <rdfs:subClassOf rdf:resource="https://savage.nps.edu/EthicalControl/ontologies/MissionExecutionOntology#DADM02.4"/>
        <rdfs:comment>Are enemy actions that result in loss of IAS command and control and subsequent negative outcomes sensed, communicated, and recorded?</rdfs:comment>
        <rdfs:label>RE02.4.3_AwarenessAdversaryC2Loss</rdfs:label>
        <owl:versionInfo>page 62</owl:versionInfo>
    </owl:Class>
    


    <!-- https://savage.nps.edu/EthicalControl/ontologies/MissionExecutionOntology#RE02.4.4 -->

    <owl:Class rdf:about="https://savage.nps.edu/EthicalControl/ontologies/MissionExecutionOntology#RE02.4.4">
        <rdfs:subClassOf rdf:resource="https://savage.nps.edu/EthicalControl/ontologies/MissionExecutionOntology#DADM02.4"/>
        <rdfs:comment>Are communications between the IAS and the person(s) designated to be accountable for its use reliable enough (e.g., consistent, frequent) to support this accountability?</rdfs:comment>
        <rdfs:label>RE02.4.4_ReliableCommunicationsAccountability</rdfs:label>
        <owl:versionInfo>page 62</owl:versionInfo>
    </owl:Class>
    


    <!-- https://savage.nps.edu/EthicalControl/ontologies/MissionExecutionOntology#RE02.4.5 -->

    <owl:Class rdf:about="https://savage.nps.edu/EthicalControl/ontologies/MissionExecutionOntology#RE02.4.5">
        <rdfs:subClassOf rdf:resource="https://savage.nps.edu/EthicalControl/ontologies/MissionExecutionOntology#DADM02.4"/>
        <rdfs:comment>Is command and control over the IAS limited to a human (mindlessly) pressing a &quot;fire&quot; button in response to indications from an IAS?</rdfs:comment>
        <rdfs:label>RE02.4.5_MicromanagedFirePerson</rdfs:label>
        <owl:versionInfo>page 62</owl:versionInfo>
    </owl:Class>
    


    <!-- https://savage.nps.edu/EthicalControl/ontologies/MissionExecutionOntology#RE02.4.6 -->

    <owl:Class rdf:about="https://savage.nps.edu/EthicalControl/ontologies/MissionExecutionOntology#RE02.4.6">
        <rdfs:subClassOf rdf:resource="https://savage.nps.edu/EthicalControl/ontologies/MissionExecutionOntology#DADM02.4"/>
        <rdfs:comment>Is there communication between the human operators who are each accountable for understanding their individual functions of the IAS that they operate?</rdfs:comment>
        <rdfs:label>RE02.4.6_OpsTeamCommunicationConstructive</rdfs:label>
        <owl:versionInfo>page 62</owl:versionInfo>
    </owl:Class>
    


    <!-- https://savage.nps.edu/EthicalControl/ontologies/MissionExecutionOntology#RE02.4.7 -->

    <owl:Class rdf:about="https://savage.nps.edu/EthicalControl/ontologies/MissionExecutionOntology#RE02.4.7">
        <rdfs:subClassOf rdf:resource="https://savage.nps.edu/EthicalControl/ontologies/MissionExecutionOntology#DADM02.4"/>
        <rdfs:comment>Are all human operators accountable for the outcome of IAS use, even if they were only involved in a subcomponent of the overall mission?</rdfs:comment>
        <rdfs:label>RE02.4.7_AllOpsTeamAccountable</rdfs:label>
        <owl:versionInfo>page 62</owl:versionInfo>
    </owl:Class>
    


    <!-- https://savage.nps.edu/EthicalControl/ontologies/MissionExecutionOntology#RE03.1 -->

    <owl:Class rdf:about="https://savage.nps.edu/EthicalControl/ontologies/MissionExecutionOntology#RE03.1">
        <rdfs:subClassOf rdf:resource="https://savage.nps.edu/EthicalControl/ontologies/MissionExecutionOntology#DADM03"/>
        <rdfs:comment>Can the degree of IAS autonomy be adjusted?</rdfs:comment>
        <rdfs:label>RE03.1_DegreeAutonomyAdjustable</rdfs:label>
        <owl:versionInfo>page 62</owl:versionInfo>
    </owl:Class>
    


    <!-- https://savage.nps.edu/EthicalControl/ontologies/MissionExecutionOntology#RE03.10 -->

    <owl:Class rdf:about="https://savage.nps.edu/EthicalControl/ontologies/MissionExecutionOntology#RE03.10">
        <rdfs:subClassOf rdf:resource="https://savage.nps.edu/EthicalControl/ontologies/MissionExecutionOntology#DADM03"/>
        <rdfs:comment>Can the degree of IAS autonomy be chosen to allow the IAS to calculate probable enemy losses for a candidate action, compare these losses to how the candidate action contributes to the success of the mission, and make a &quot;return on investment&quot; assessment before taking the action?</rdfs:comment>
        <rdfs:label>RE03.10_IASDetermineAdversaryLoss</rdfs:label>
        <owl:versionInfo>page 63</owl:versionInfo>
    </owl:Class>
    


    <!-- https://savage.nps.edu/EthicalControl/ontologies/MissionExecutionOntology#RE03.11 -->

    <owl:Class rdf:about="https://savage.nps.edu/EthicalControl/ontologies/MissionExecutionOntology#RE03.11">
        <rdfs:subClassOf rdf:resource="https://savage.nps.edu/EthicalControl/ontologies/MissionExecutionOntology#DADM03"/>
        <rdfs:comment>Can the degree of IAS autonomy be adjusted downward for platforms with larger magazines in consideration of the increased level of risk that the larger magazine presumably entails?</rdfs:comment>
        <rdfs:label>RE03.11_DegreeAutonomyModifiableViaMagazine</rdfs:label>
        <owl:versionInfo>page 63</owl:versionInfo>
    </owl:Class>
    


    <!-- https://savage.nps.edu/EthicalControl/ontologies/MissionExecutionOntology#RE03.12 -->

    <owl:Class rdf:about="https://savage.nps.edu/EthicalControl/ontologies/MissionExecutionOntology#RE03.12">
        <rdfs:subClassOf rdf:resource="https://savage.nps.edu/EthicalControl/ontologies/MissionExecutionOntology#DADM03"/>
        <rdfs:comment>Can the degree of IAS autonomy be adjusted downward to reduce risk when operational conditions are such that there is a higher perceived risk to the IAS from either enemy action, environmental factors or malfunction?</rdfs:comment>
        <rdfs:label>RE03.12_DegreeAutonomyModifiableViaEnvironmentRisks</rdfs:label>
        <owl:versionInfo>page 63</owl:versionInfo>
    </owl:Class>
    


    <!-- https://savage.nps.edu/EthicalControl/ontologies/MissionExecutionOntology#RE03.13 -->

    <owl:Class rdf:about="https://savage.nps.edu/EthicalControl/ontologies/MissionExecutionOntology#RE03.13">
        <rdfs:subClassOf rdf:resource="https://savage.nps.edu/EthicalControl/ontologies/MissionExecutionOntology#DADM03"/>
        <rdfs:comment>Is the human operator fully equipped and prepared to take over if the IAS malfunctions or breaks down mid-operation?</rdfs:comment>
        <rdfs:label>RE03.13_DegreeAutonomyMissionDependent</rdfs:label>
        <owl:versionInfo>page 63</owl:versionInfo>
    </owl:Class>
    


    <!-- https://savage.nps.edu/EthicalControl/ontologies/MissionExecutionOntology#RE03.14 -->

    <owl:Class rdf:about="https://savage.nps.edu/EthicalControl/ontologies/MissionExecutionOntology#RE03.14">
        <rdfs:subClassOf rdf:resource="https://savage.nps.edu/EthicalControl/ontologies/MissionExecutionOntology#DADM03"/>
        <rdfs:comment>Does the human operator fully understand the differences between an automatic system and an autonomous system?</rdfs:comment>
        <rdfs:label>RE03.14_DegreeAutonomyAdustableIndividually</rdfs:label>
        <owl:versionInfo>page 63</owl:versionInfo>
    </owl:Class>
    


    <!-- https://savage.nps.edu/EthicalControl/ontologies/MissionExecutionOntology#RE03.15 -->

    <owl:Class rdf:about="https://savage.nps.edu/EthicalControl/ontologies/MissionExecutionOntology#RE03.15">
        <rdfs:subClassOf rdf:resource="https://savage.nps.edu/EthicalControl/ontologies/MissionExecutionOntology#DADM03"/>
        <rdfs:comment>Can the degree of autonomy be adjusted based on various levels of abstraction (e.g., task, function, or mission)?</rdfs:comment>
        <rdfs:label>RE03.15_DegreeAutonomyLowestSelectable</rdfs:label>
        <owl:versionInfo>page 63</owl:versionInfo>
    </owl:Class>
    


    <!-- https://savage.nps.edu/EthicalControl/ontologies/MissionExecutionOntology#RE03.2 -->

    <owl:Class rdf:about="https://savage.nps.edu/EthicalControl/ontologies/MissionExecutionOntology#RE03.2">
        <rdfs:subClassOf rdf:resource="https://savage.nps.edu/EthicalControl/ontologies/MissionExecutionOntology#DADM03"/>
        <rdfs:comment>Can the degree of IAS autonomy be made known (through markings or public communications such as a notice to mariners) to supported friendly forces, to noncombatants, and/or to enemy combatants at the discretion of the operator or commander?</rdfs:comment>
        <rdfs:label>RE03.2_DegreeAutonomySharable</rdfs:label>
        <owl:versionInfo>page 63</owl:versionInfo>
    </owl:Class>
    


    <!-- https://savage.nps.edu/EthicalControl/ontologies/MissionExecutionOntology#RE03.3 -->

    <owl:Class rdf:about="https://savage.nps.edu/EthicalControl/ontologies/MissionExecutionOntology#RE03.3">
        <rdfs:subClassOf rdf:resource="https://savage.nps.edu/EthicalControl/ontologies/MissionExecutionOntology#DADM03"/>
        <rdfs:comment>Can the IAS make it known to anyone who might be in a position to disable, board, or seize it that it has - and will exercise - its universal right to self-defense?</rdfs:comment>
        <rdfs:label>RE03.3_ReportsRightSelfDefense</rdfs:label>
        <owl:versionInfo>page 63</owl:versionInfo>
    </owl:Class>
    


    <!-- https://savage.nps.edu/EthicalControl/ontologies/MissionExecutionOntology#RE03.4 -->

    <owl:Class rdf:about="https://savage.nps.edu/EthicalControl/ontologies/MissionExecutionOntology#RE03.4">
        <rdfs:subClassOf rdf:resource="https://savage.nps.edu/EthicalControl/ontologies/MissionExecutionOntology#DADM03"/>
        <rdfs:comment>Can the commander or operator throttle the IAS to dynamically increase or decrease the degree of autonomy to adjust to the dynamics of the operational situation?</rdfs:comment>
        <rdfs:label>RE03.4_DegreeAutonomyAdjustableDynamically</rdfs:label>
        <owl:versionInfo>page 63</owl:versionInfo>
    </owl:Class>
    


    <!-- https://savage.nps.edu/EthicalControl/ontologies/MissionExecutionOntology#RE03.5 -->

    <owl:Class rdf:about="https://savage.nps.edu/EthicalControl/ontologies/MissionExecutionOntology#RE03.5">
        <rdfs:subClassOf rdf:resource="https://savage.nps.edu/EthicalControl/ontologies/MissionExecutionOntology#DADM03"/>
        <rdfs:comment>Is there an established and accepted threshold degree of autonomy, that when exceeded, the IAS becomes a LAWS, where a human no longer selects the target?</rdfs:comment>
        <rdfs:label>RE03.5_AutonomyThresholdLethalForceWeaponSystem</rdfs:label>
        <owl:versionInfo>page 63</owl:versionInfo>
    </owl:Class>
    


    <!-- https://savage.nps.edu/EthicalControl/ontologies/MissionExecutionOntology#RE03.6 -->

    <owl:Class rdf:about="https://savage.nps.edu/EthicalControl/ontologies/MissionExecutionOntology#RE03.6">
        <rdfs:subClassOf rdf:resource="https://savage.nps.edu/EthicalControl/ontologies/MissionExecutionOntology#DADM03"/>
        <rdfs:comment>Can the degree of IAS autonomy be conditionally changed, either through predetermined rule sets, or resulting from emergent information not covered by the predetermined rules, such as the elevation of the defense condition (DEFCON)?</rdfs:comment>
        <rdfs:label>RE03.6_DegreeAutonomyModifiableViaRuleSets</rdfs:label>
        <owl:versionInfo>page 63</owl:versionInfo>
    </owl:Class>
    


    <!-- https://savage.nps.edu/EthicalControl/ontologies/MissionExecutionOntology#RE03.7 -->

    <owl:Class rdf:about="https://savage.nps.edu/EthicalControl/ontologies/MissionExecutionOntology#RE03.7">
        <rdfs:subClassOf rdf:resource="https://savage.nps.edu/EthicalControl/ontologies/MissionExecutionOntology#DADM03"/>
        <rdfs:comment>Can the degree of IAS autonomy for a multi-mission capable platform be chosen and/or adjusted independently for each mission?</rdfs:comment>
        <rdfs:label>RE03.7_DegreeAutonomyMissionDependent</rdfs:label>
        <owl:versionInfo>page 63</owl:versionInfo>
    </owl:Class>
    


    <!-- https://savage.nps.edu/EthicalControl/ontologies/MissionExecutionOntology#RE03.8 -->

    <owl:Class rdf:about="https://savage.nps.edu/EthicalControl/ontologies/MissionExecutionOntology#RE03.8">
        <rdfs:subClassOf rdf:resource="https://savage.nps.edu/EthicalControl/ontologies/MissionExecutionOntology#DADM03"/>
        <rdfs:comment>Can the degree of autonomy for each autonomous function of an IAS be adjusted individually?</rdfs:comment>
        <rdfs:label>RE03.8_DegreeAutonomyAdustableIndividually</rdfs:label>
        <owl:versionInfo>page 63</owl:versionInfo>
    </owl:Class>
    


    <!-- https://savage.nps.edu/EthicalControl/ontologies/MissionExecutionOntology#RE03.9 -->

    <owl:Class rdf:about="https://savage.nps.edu/EthicalControl/ontologies/MissionExecutionOntology#RE03.9">
        <rdfs:subClassOf rdf:resource="https://savage.nps.edu/EthicalControl/ontologies/MissionExecutionOntology#DADM03"/>
        <rdfs:comment>Can the degree of IAS autonomy be selected by the IAS such that it is the lowest degree of autonomy required to accomplish the mission?</rdfs:comment>
        <rdfs:label>RE03.9_DegreeAutonomyLowestSelectable</rdfs:label>
        <owl:versionInfo>page 63</owl:versionInfo>
    </owl:Class>
    


    <!-- https://savage.nps.edu/EthicalControl/ontologies/MissionExecutionOntology#RE04.1.1 -->

    <owl:Class rdf:about="https://savage.nps.edu/EthicalControl/ontologies/MissionExecutionOntology#RE04.1.1">
        <rdfs:subClassOf rdf:resource="https://savage.nps.edu/EthicalControl/ontologies/MissionExecutionOntology#DADM04.1"/>
        <rdfs:comment>Can the contemplated operation be executed with a non-autonomous alternative?</rdfs:comment>
        <rdfs:label>RE04.1.1_AlternativesAutonomousSystems</rdfs:label>
        <owl:versionInfo>page 64</owl:versionInfo>
    </owl:Class>
    


    <!-- https://savage.nps.edu/EthicalControl/ontologies/MissionExecutionOntology#RE04.1.10 -->

    <owl:Class rdf:about="https://savage.nps.edu/EthicalControl/ontologies/MissionExecutionOntology#RE04.1.10">
        <rdfs:subClassOf rdf:resource="https://savage.nps.edu/EthicalControl/ontologies/MissionExecutionOntology#DADM04.1"/>
        <rdfs:comment>Does the existing force structure and manning necessitate the use of IAS?</rdfs:comment>
        <rdfs:label>RE04.1.10_OrganizationManningNecessitity</rdfs:label>
        <owl:versionInfo>page 64</owl:versionInfo>
    </owl:Class>
    


    <!-- https://savage.nps.edu/EthicalControl/ontologies/MissionExecutionOntology#RE04.1.11 -->

    <owl:Class rdf:about="https://savage.nps.edu/EthicalControl/ontologies/MissionExecutionOntology#RE04.1.11">
        <rdfs:subClassOf rdf:resource="https://savage.nps.edu/EthicalControl/ontologies/MissionExecutionOntology#DADM04.1"/>
        <rdfs:comment>Can the IAS help determine whether to use autonomous, semi-autonomous, or non- autonomous functional modes based on current circumstances and conditions?</rdfs:comment>
        <rdfs:label>RE04.1.11_PlatformRecommendsAutonomyLevel</rdfs:label>
        <owl:versionInfo>page 64</owl:versionInfo>
    </owl:Class>
    


    <!-- https://savage.nps.edu/EthicalControl/ontologies/MissionExecutionOntology#RE04.1.12 -->

    <owl:Class rdf:about="https://savage.nps.edu/EthicalControl/ontologies/MissionExecutionOntology#RE04.1.12">
        <rdfs:subClassOf rdf:resource="https://savage.nps.edu/EthicalControl/ontologies/MissionExecutionOntology#DADM04.1"/>
        <rdfs:comment>Can the use of IAS improve military capabilities?</rdfs:comment>
        <rdfs:label>RE04.1.12_OrganizationImprovedOutcomes</rdfs:label>
        <owl:versionInfo>page 64</owl:versionInfo>
    </owl:Class>
    


    <!-- https://savage.nps.edu/EthicalControl/ontologies/MissionExecutionOntology#RE04.1.13 -->

    <owl:Class rdf:about="https://savage.nps.edu/EthicalControl/ontologies/MissionExecutionOntology#RE04.1.13">
        <rdfs:subClassOf rdf:resource="https://savage.nps.edu/EthicalControl/ontologies/MissionExecutionOntology#DADM04.1"/>
        <rdfs:comment>Can the use of IAS reduce loss of human life?</rdfs:comment>
        <rdfs:label>RE04.1.13_UseReducesLossHumanLife</rdfs:label>
        <owl:versionInfo>page 64</owl:versionInfo>
    </owl:Class>
    


    <!-- https://savage.nps.edu/EthicalControl/ontologies/MissionExecutionOntology#RE04.1.2 -->

    <owl:Class rdf:about="https://savage.nps.edu/EthicalControl/ontologies/MissionExecutionOntology#RE04.1.2">
        <rdfs:subClassOf rdf:resource="https://savage.nps.edu/EthicalControl/ontologies/MissionExecutionOntology#DADM04.1"/>
        <rdfs:comment>Do rules of engagement or policy require the commander to consider all available non-autonomous alternatives before employing an IAS?</rdfs:comment>
        <rdfs:label>RE04.1.2_RulesAlternativeAutonomousSystems</rdfs:label>
        <owl:versionInfo>page 64</owl:versionInfo>
    </owl:Class>
    


    <!-- https://savage.nps.edu/EthicalControl/ontologies/MissionExecutionOntology#RE04.1.3 -->

    <owl:Class rdf:about="https://savage.nps.edu/EthicalControl/ontologies/MissionExecutionOntology#RE04.1.3">
        <rdfs:subClassOf rdf:resource="https://savage.nps.edu/EthicalControl/ontologies/MissionExecutionOntology#DADM04.1"/>
        <rdfs:comment>Will failure to transfer decision-making capabilities to the IAS result in a military disadvantage?</rdfs:comment>
        <rdfs:label>RE04.1.3_AdvantageAutonomousSystem</rdfs:label>
        <owl:versionInfo>page 64</owl:versionInfo>
    </owl:Class>
    


    <!-- https://savage.nps.edu/EthicalControl/ontologies/MissionExecutionOntology#RE04.1.4 -->

    <owl:Class rdf:about="https://savage.nps.edu/EthicalControl/ontologies/MissionExecutionOntology#RE04.1.4">
        <rdfs:subClassOf rdf:resource="https://savage.nps.edu/EthicalControl/ontologies/MissionExecutionOntology#DADM04.1"/>
        <rdfs:comment>Is the contemplated task monotonous or fatiguing (i.e., &quot;dull&quot;) to the point that human performance will degrade but IAS performance will not?</rdfs:comment>
        <rdfs:label>RE04.1.4_HumanFactorBoringTasking</rdfs:label>
        <owl:versionInfo>page 64</owl:versionInfo>
    </owl:Class>
    


    <!-- https://savage.nps.edu/EthicalControl/ontologies/MissionExecutionOntology#RE04.1.5 -->

    <owl:Class rdf:about="https://savage.nps.edu/EthicalControl/ontologies/MissionExecutionOntology#RE04.1.5">
        <rdfs:subClassOf rdf:resource="https://savage.nps.edu/EthicalControl/ontologies/MissionExecutionOntology#DADM04.1"/>
        <rdfs:comment>Does the contemplated task put humans in harm’s way by exposing them to (dirty) hazardous materials?</rdfs:comment>
        <rdfs:label>RE04.1.5_HumanFactorDirtyHazardousMaterial</rdfs:label>
        <owl:versionInfo>page 64</owl:versionInfo>
    </owl:Class>
    


    <!-- https://savage.nps.edu/EthicalControl/ontologies/MissionExecutionOntology#RE04.1.6 -->

    <owl:Class rdf:about="https://savage.nps.edu/EthicalControl/ontologies/MissionExecutionOntology#RE04.1.6">
        <rdfs:subClassOf rdf:resource="https://savage.nps.edu/EthicalControl/ontologies/MissionExecutionOntology#DADM04.1"/>
        <rdfs:comment>Does the contemplated task put humans in harm’s way by exposing them to (dangerous) enemy action or violent weather conditions?</rdfs:comment>
        <rdfs:label>RE04.1.6_HumanExposureAdversary</rdfs:label>
        <owl:versionInfo>page 64</owl:versionInfo>
    </owl:Class>
    


    <!-- https://savage.nps.edu/EthicalControl/ontologies/MissionExecutionOntology#RE04.1.7 -->

    <owl:Class rdf:about="https://savage.nps.edu/EthicalControl/ontologies/MissionExecutionOntology#RE04.1.7">
        <rdfs:subClassOf rdf:resource="https://savage.nps.edu/EthicalControl/ontologies/MissionExecutionOntology#DADM04.1"/>
        <rdfs:comment>Does the use of the IAS deprive the commander of human ingenuity, creativity, flexibility, or (operational) art capabilities that makes the force less capable?</rdfs:comment>
        <rdfs:label>RE04.1.7_HumanFactorLossOperationalEffectiveness</rdfs:label>
        <owl:versionInfo>page 64</owl:versionInfo>
    </owl:Class>
    


    <!-- https://savage.nps.edu/EthicalControl/ontologies/MissionExecutionOntology#RE04.1.8 -->

    <owl:Class rdf:about="https://savage.nps.edu/EthicalControl/ontologies/MissionExecutionOntology#RE04.1.8">
        <rdfs:subClassOf rdf:resource="https://savage.nps.edu/EthicalControl/ontologies/MissionExecutionOntology#DADM04.1"/>
        <rdfs:comment>Can the IAS conduct an operation more safely than a human can?</rdfs:comment>
        <rdfs:label>RE04.1.8_AutonomousSystemSafer</rdfs:label>
        <owl:versionInfo>page 64</owl:versionInfo>
    </owl:Class>
    


    <!-- https://savage.nps.edu/EthicalControl/ontologies/MissionExecutionOntology#RE04.1.9 -->

    <owl:Class rdf:about="https://savage.nps.edu/EthicalControl/ontologies/MissionExecutionOntology#RE04.1.9">
        <rdfs:subClassOf rdf:resource="https://savage.nps.edu/EthicalControl/ontologies/MissionExecutionOntology#DADM04.1"/>
        <rdfs:comment>Does the commander have any systems that provide the same capability as the IAS, but do not depend on AI or autonomy?</rdfs:comment>
        <rdfs:label>RE04.1.9_FunctionalNonAutomousSystemsAvailable</rdfs:label>
        <owl:versionInfo>page 64</owl:versionInfo>
    </owl:Class>
    


    <!-- https://savage.nps.edu/EthicalControl/ontologies/MissionExecutionOntology#RE04.2.1 -->

    <owl:Class rdf:about="https://savage.nps.edu/EthicalControl/ontologies/MissionExecutionOntology#RE04.2.1">
        <rdfs:subClassOf rdf:resource="https://savage.nps.edu/EthicalControl/ontologies/MissionExecutionOntology#DADM04.2"/>
        <rdfs:comment>Is the perceptual space of the IAS clearly superior to that of the nonautonomous alternative (i.e., infrared or radio frequency emission detection)?</rdfs:comment>
        <rdfs:label>RE04.2.1_SensorPerceptualSpace</rdfs:label>
        <owl:versionInfo>page 64</owl:versionInfo>
    </owl:Class>
    


    <!-- https://savage.nps.edu/EthicalControl/ontologies/MissionExecutionOntology#RE04.2.2 -->

    <owl:Class rdf:about="https://savage.nps.edu/EthicalControl/ontologies/MissionExecutionOntology#RE04.2.2">
        <rdfs:subClassOf rdf:resource="https://savage.nps.edu/EthicalControl/ontologies/MissionExecutionOntology#DADM04.2"/>
        <rdfs:comment>Can the IAS consistently catch important clues that human operators would miss or misconstrue?</rdfs:comment>
        <rdfs:label>RE04.2.2_SceneUnderstandingPerceptualDetail</rdfs:label>
        <owl:versionInfo>page 64</owl:versionInfo>
    </owl:Class>
    


    <!-- https://savage.nps.edu/EthicalControl/ontologies/MissionExecutionOntology#RE04.2.3 -->

    <owl:Class rdf:about="https://savage.nps.edu/EthicalControl/ontologies/MissionExecutionOntology#RE04.2.3">
        <rdfs:subClassOf rdf:resource="https://savage.nps.edu/EthicalControl/ontologies/MissionExecutionOntology#DADM04.2"/>
        <rdfs:comment>Does the IAS consistently have greater operational range or longer time on station than the nonautonomous alternative?</rdfs:comment>
        <rdfs:label>RE04.2.3_GreaterOperationalPersistance</rdfs:label>
        <owl:versionInfo>page 64</owl:versionInfo>
    </owl:Class>
    


    <!-- https://savage.nps.edu/EthicalControl/ontologies/MissionExecutionOntology#RE04.2.4 -->

    <owl:Class rdf:about="https://savage.nps.edu/EthicalControl/ontologies/MissionExecutionOntology#RE04.2.4">
        <rdfs:subClassOf rdf:resource="https://savage.nps.edu/EthicalControl/ontologies/MissionExecutionOntology#DADM04.2"/>
        <rdfs:comment>Can the IAS physically outmaneuver any enemy platforms it might face, for which the nonautonomous alternative cannot?</rdfs:comment>
        <rdfs:label>RE04.2.4_GreaterManeuverability</rdfs:label>
        <owl:versionInfo>page 64</owl:versionInfo>
    </owl:Class>
    


    <!-- https://savage.nps.edu/EthicalControl/ontologies/MissionExecutionOntology#RE04.2.5 -->

    <owl:Class rdf:about="https://savage.nps.edu/EthicalControl/ontologies/MissionExecutionOntology#RE04.2.5">
        <rdfs:subClassOf rdf:resource="https://savage.nps.edu/EthicalControl/ontologies/MissionExecutionOntology#DADM04.2"/>
        <rdfs:comment>Can the IAS consistently service targets that are inaccessible to the nonautonomous alternative?</rdfs:comment>
        <rdfs:label>RE04.2.5_GreaterTargetAccess</rdfs:label>
        <owl:versionInfo>page 65</owl:versionInfo>
    </owl:Class>
    


    <!-- https://savage.nps.edu/EthicalControl/ontologies/MissionExecutionOntology#RE04.2.6 -->

    <owl:Class rdf:about="https://savage.nps.edu/EthicalControl/ontologies/MissionExecutionOntology#RE04.2.6">
        <rdfs:subClassOf rdf:resource="https://savage.nps.edu/EthicalControl/ontologies/MissionExecutionOntology#DADM04.2"/>
        <rdfs:comment>Can the IAS consistently conduct multiple tasks simultaneously, freeing up humans for other tasks that the human is better suited to than the IAS?</rdfs:comment>
        <rdfs:label>RE04.2.6_MultitargetTasking</rdfs:label>
        <owl:versionInfo>page 65</owl:versionInfo>
    </owl:Class>
    


    <!-- https://savage.nps.edu/EthicalControl/ontologies/MissionExecutionOntology#RE04.3.1 -->

    <owl:Class rdf:about="https://savage.nps.edu/EthicalControl/ontologies/MissionExecutionOntology#RE04.3.1">
        <rdfs:subClassOf rdf:resource="https://savage.nps.edu/EthicalControl/ontologies/MissionExecutionOntology#DADM04.3"/>
        <rdfs:comment>Can the IAS create a model of a given object and differentiate the object (military versus civilian) as well or better than the nonautonomous alternative can?</rdfs:comment>
        <rdfs:label>RE04.3.1_OperationalPerceptualModelingEquipmentAdvantage</rdfs:label>
        <owl:versionInfo>page 65</owl:versionInfo>
    </owl:Class>
    


    <!-- https://savage.nps.edu/EthicalControl/ontologies/MissionExecutionOntology#RE04.3.2 -->

    <owl:Class rdf:about="https://savage.nps.edu/EthicalControl/ontologies/MissionExecutionOntology#RE04.3.2">
        <rdfs:subClassOf rdf:resource="https://savage.nps.edu/EthicalControl/ontologies/MissionExecutionOntology#DADM04.3"/>
        <rdfs:comment>Can the IAS create a model of a person and differentiate enemy combatants, friendly combatants, and noncombatants as well as, or better than, than the nonautonomous alternative can?</rdfs:comment>
        <rdfs:label>RE04.3.2_OperationalPerceptualModelingPeopleAdvantage</rdfs:label>
        <owl:versionInfo>page 65</owl:versionInfo>
    </owl:Class>
    


    <!-- https://savage.nps.edu/EthicalControl/ontologies/MissionExecutionOntology#RE04.3.3 -->

    <owl:Class rdf:about="https://savage.nps.edu/EthicalControl/ontologies/MissionExecutionOntology#RE04.3.3">
        <rdfs:subClassOf rdf:resource="https://savage.nps.edu/EthicalControl/ontologies/MissionExecutionOntology#DADM04.3"/>
        <rdfs:comment>Is a level of confidence required to be established for the IAS to distinguish a target in different operational situations?</rdfs:comment>
        <rdfs:label>RE04.3.3_DifferentConfidenceLevels</rdfs:label>
        <owl:versionInfo>page 65</owl:versionInfo>
    </owl:Class>
    


    <!-- https://savage.nps.edu/EthicalControl/ontologies/MissionExecutionOntology#RE04.3.4 -->

    <owl:Class rdf:about="https://savage.nps.edu/EthicalControl/ontologies/MissionExecutionOntology#RE04.3.4">
        <rdfs:subClassOf rdf:resource="https://savage.nps.edu/EthicalControl/ontologies/MissionExecutionOntology#DADM04.3"/>
        <rdfs:comment>Does the IAS know when a given object is outside of its training set (i.e., out-of-distribution detection)?</rdfs:comment>
        <rdfs:label>RE04.3.4_OutOfDistributionDetection</rdfs:label>
        <owl:versionInfo>page 65</owl:versionInfo>
    </owl:Class>
    


    <!-- https://savage.nps.edu/EthicalControl/ontologies/MissionExecutionOntology#RE04.4.1 -->

    <owl:Class rdf:about="https://savage.nps.edu/EthicalControl/ontologies/MissionExecutionOntology#RE04.4.1">
        <rdfs:subClassOf rdf:resource="https://savage.nps.edu/EthicalControl/ontologies/MissionExecutionOntology#DADM04.4"/>
        <rdfs:comment>Would the use of IAS allow the commander to use more precise munitions to minimize collateral damage?</rdfs:comment>
        <rdfs:label>RE04.4.1_RelativeTargetingMinimizeCollateralDamage</rdfs:label>
        <owl:versionInfo>page 65</owl:versionInfo>
    </owl:Class>
    


    <!-- https://savage.nps.edu/EthicalControl/ontologies/MissionExecutionOntology#RE04.4.2 -->

    <owl:Class rdf:about="https://savage.nps.edu/EthicalControl/ontologies/MissionExecutionOntology#RE04.4.2">
        <rdfs:subClassOf rdf:resource="https://savage.nps.edu/EthicalControl/ontologies/MissionExecutionOntology#DADM04.4"/>
        <rdfs:comment>Can the IAS determine the appropriate level of proportionality in attack during the conduct of a mission (e.g., when to continue, when to cease action)?</rdfs:comment>
        <rdfs:label>RE04.4.2_StopAttacking</rdfs:label>
        <owl:versionInfo>page 65</owl:versionInfo>
    </owl:Class>
    


    <!-- https://savage.nps.edu/EthicalControl/ontologies/MissionExecutionOntology#RE04.4.3 -->

    <owl:Class rdf:about="https://savage.nps.edu/EthicalControl/ontologies/MissionExecutionOntology#RE04.4.3">
        <rdfs:subClassOf rdf:resource="https://savage.nps.edu/EthicalControl/ontologies/MissionExecutionOntology#DADM04.4"/>
        <rdfs:comment>Can the IAS provide better identification and more accurately strike a specific location on a target with smaller munition and reduced blast radius?</rdfs:comment>
        <rdfs:label>RE04.4.3_RelativeTargetIdentificationMinimizeBlast</rdfs:label>
        <owl:versionInfo>page 65</owl:versionInfo>
    </owl:Class>
    


    <!-- https://savage.nps.edu/EthicalControl/ontologies/MissionExecutionOntology#RE04.4.4 -->

    <owl:Class rdf:about="https://savage.nps.edu/EthicalControl/ontologies/MissionExecutionOntology#RE04.4.4">
        <rdfs:subClassOf rdf:resource="https://savage.nps.edu/EthicalControl/ontologies/MissionExecutionOntology#DADM04.4"/>
        <rdfs:comment>Can the IAS discern whether or not the target is sufficiently valuable to risk collateral damage?</rdfs:comment>
        <rdfs:label>RE04.4.4_HighValueTargetIdentification</rdfs:label>
        <owl:versionInfo>page 65</owl:versionInfo>
    </owl:Class>
    


    <!-- https://savage.nps.edu/EthicalControl/ontologies/MissionExecutionOntology#RE04.5.1 -->

    <owl:Class rdf:about="https://savage.nps.edu/EthicalControl/ontologies/MissionExecutionOntology#RE04.5.1">
        <rdfs:subClassOf rdf:resource="https://savage.nps.edu/EthicalControl/ontologies/MissionExecutionOntology#DADM04.5"/>
        <rdfs:comment>Is the speed of operation of the IAS in synch with the speed of the situational assessment?</rdfs:comment>
        <rdfs:label>RE04.5.1_DominatesEnvironmentOperationalPerception</rdfs:label>
        <owl:versionInfo>page 65</owl:versionInfo>
    </owl:Class>
    


    <!-- https://savage.nps.edu/EthicalControl/ontologies/MissionExecutionOntology#RE04.5.2 -->

    <owl:Class rdf:about="https://savage.nps.edu/EthicalControl/ontologies/MissionExecutionOntology#RE04.5.2">
        <rdfs:subClassOf rdf:resource="https://savage.nps.edu/EthicalControl/ontologies/MissionExecutionOntology#DADM04.5"/>
        <rdfs:comment>Does the superior decision speed of the IAS over the human justify the risk of an incorrect decision by the IAS that a human would not likely make incorrectly?</rdfs:comment>
        <rdfs:label>RE04.5.2_ActionSpeedErrorRates</rdfs:label>
        <owl:versionInfo>page 65</owl:versionInfo>
    </owl:Class>
    


    <!-- https://savage.nps.edu/EthicalControl/ontologies/MissionExecutionOntology#RE04.5.3 -->

    <owl:Class rdf:about="https://savage.nps.edu/EthicalControl/ontologies/MissionExecutionOntology#RE04.5.3">
        <rdfs:subClassOf rdf:resource="https://savage.nps.edu/EthicalControl/ontologies/MissionExecutionOntology#DADM04.5"/>
        <rdfs:comment>Will the IAS be used for situations where human reactions are too slow for an effective response?</rdfs:comment>
        <rdfs:label>RE04.5.3_FunctionSpeedNecessatesUse</rdfs:label>
        <owl:versionInfo>page 65</owl:versionInfo>
    </owl:Class>
    


    <!-- https://savage.nps.edu/EthicalControl/ontologies/MissionExecutionOntology#RE04.5.4 -->

    <owl:Class rdf:about="https://savage.nps.edu/EthicalControl/ontologies/MissionExecutionOntology#RE04.5.4">
        <rdfs:subClassOf rdf:resource="https://savage.nps.edu/EthicalControl/ontologies/MissionExecutionOntology#DADM04.5"/>
        <rdfs:comment>Will IAS decision-making speed decrease if it must allow human operators to oversee and approve its actions?</rdfs:comment>
        <rdfs:label>RE04.5.4_HumanInLoopSlowsSystem</rdfs:label>
        <owl:versionInfo>page 65</owl:versionInfo>
    </owl:Class>
    


    <!-- https://savage.nps.edu/EthicalControl/ontologies/MissionExecutionOntology#RE04.5.5 -->

    <owl:Class rdf:about="https://savage.nps.edu/EthicalControl/ontologies/MissionExecutionOntology#RE04.5.5">
        <rdfs:subClassOf rdf:resource="https://savage.nps.edu/EthicalControl/ontologies/MissionExecutionOntology#DADM04.5"/>
        <rdfs:comment>Does the mission require action in windows of opportunity too short for effective human intervention/action?</rdfs:comment>
        <rdfs:label>RE04.5.5_OperationalWindowJustifiesUse</rdfs:label>
        <owl:versionInfo>page 66</owl:versionInfo>
    </owl:Class>
    


    <!-- https://savage.nps.edu/EthicalControl/ontologies/MissionExecutionOntology#RE04.5.6 -->

    <owl:Class rdf:about="https://savage.nps.edu/EthicalControl/ontologies/MissionExecutionOntology#RE04.5.6">
        <rdfs:subClassOf rdf:resource="https://savage.nps.edu/EthicalControl/ontologies/MissionExecutionOntology#DADM04.5"/>
        <rdfs:comment>Will the failure to transfer decision-making capabilities to the IAS result in the enemy having a faster OODA loop?</rdfs:comment>
        <rdfs:label>RE04.5.6_AdversaryAdvantageWithoutDecisionAutonomy</rdfs:label>
        <owl:versionInfo>page 66</owl:versionInfo>
    </owl:Class>
    


    <!-- https://savage.nps.edu/EthicalControl/ontologies/MissionExecutionOntology#RE04.6.1 -->

    <owl:Class rdf:about="https://savage.nps.edu/EthicalControl/ontologies/MissionExecutionOntology#RE04.6.1">
        <rdfs:subClassOf rdf:resource="https://savage.nps.edu/EthicalControl/ontologies/MissionExecutionOntology#DADM04.6"/>
        <rdfs:comment>Are battlefield information flows so fast as to justify a reliance on an IAS instead of a human decision maker?</rdfs:comment>
        <rdfs:label>RE04.6.1_EnvironmentChangeQuick</rdfs:label>
        <owl:versionInfo>page 66</owl:versionInfo>
    </owl:Class>
    


    <!-- https://savage.nps.edu/EthicalControl/ontologies/MissionExecutionOntology#RE04.6.2 -->

    <owl:Class rdf:about="https://savage.nps.edu/EthicalControl/ontologies/MissionExecutionOntology#RE04.6.2">
        <rdfs:subClassOf rdf:resource="https://savage.nps.edu/EthicalControl/ontologies/MissionExecutionOntology#DADM04.6"/>
        <rdfs:comment>Are battlefield information flows so large as to justify a reliance on an IAS instead of a human decision maker?</rdfs:comment>
        <rdfs:label>RE04.6.2_EnvironmentChangeLarge</rdfs:label>
        <owl:versionInfo>page 66</owl:versionInfo>
    </owl:Class>
    


    <!-- https://savage.nps.edu/EthicalControl/ontologies/MissionExecutionOntology#RE04.6.3 -->

    <owl:Class rdf:about="https://savage.nps.edu/EthicalControl/ontologies/MissionExecutionOntology#RE04.6.3">
        <rdfs:subClassOf rdf:resource="https://savage.nps.edu/EthicalControl/ontologies/MissionExecutionOntology#DADM04.6"/>
        <rdfs:comment>Are battlefield information flows so varied as to justify a reliance on an IAS instead of a human decision maker?</rdfs:comment>
        <rdfs:label>RE04.6.3_EnvironmentChangeNumerous</rdfs:label>
        <owl:versionInfo>page 66</owl:versionInfo>
    </owl:Class>
    


    <!-- https://savage.nps.edu/EthicalControl/ontologies/MissionExecutionOntology#RE04.6.4 -->

    <owl:Class rdf:about="https://savage.nps.edu/EthicalControl/ontologies/MissionExecutionOntology#RE04.6.4">
        <rdfs:subClassOf rdf:resource="https://savage.nps.edu/EthicalControl/ontologies/MissionExecutionOntology#DADM04.6"/>
        <rdfs:comment>Will the use of the IAS cause the pace of events on the battlefield to accelerate beyond the point that the commander can comprehend the events and take decisive action?</rdfs:comment>
        <rdfs:label>RE04.6.4_AdversaryIASSystemAccelerateEnvironmentDominance</rdfs:label>
        <owl:versionInfo>page 66</owl:versionInfo>
    </owl:Class>
    


    <!-- https://savage.nps.edu/EthicalControl/ontologies/MissionExecutionOntology#RE04.6.5 -->

    <owl:Class rdf:about="https://savage.nps.edu/EthicalControl/ontologies/MissionExecutionOntology#RE04.6.5">
        <rdfs:subClassOf rdf:resource="https://savage.nps.edu/EthicalControl/ontologies/MissionExecutionOntology#DADM04.6"/>
        <rdfs:comment>Will the enemy use of the IAS cause the pace of events on the battlefield to accelerate beyond the point that the commander can comprehend and control these events?</rdfs:comment>
        <rdfs:label>RE04.6.5_AdversaryIASRequiresIAS</rdfs:label>
        <owl:versionInfo>page 66</owl:versionInfo>
    </owl:Class>
    


    <!-- https://savage.nps.edu/EthicalControl/ontologies/MissionExecutionOntology#RE04.7.1 -->

    <owl:Class rdf:about="https://savage.nps.edu/EthicalControl/ontologies/MissionExecutionOntology#RE04.7.1">
        <rdfs:subClassOf rdf:resource="https://savage.nps.edu/EthicalControl/ontologies/MissionExecutionOntology#DADM04.7"/>
        <rdfs:comment>Can the decisions of the IAS overwhelm the adversary’s decision-making process?</rdfs:comment>
        <rdfs:label>RE04.7.1_OverwhelmAdversaryDecisionMaking</rdfs:label>
        <owl:versionInfo>page 66</owl:versionInfo>
    </owl:Class>
    


    <!-- https://savage.nps.edu/EthicalControl/ontologies/MissionExecutionOntology#RE04.7.2 -->

    <owl:Class rdf:about="https://savage.nps.edu/EthicalControl/ontologies/MissionExecutionOntology#RE04.7.2">
        <rdfs:subClassOf rdf:resource="https://savage.nps.edu/EthicalControl/ontologies/MissionExecutionOntology#DADM04.7"/>
        <rdfs:comment>Can the decisions of the IAS complicate the adversary’s decision-making process by being less predictable than the decisions of a human operator?</rdfs:comment>
        <rdfs:label>RE04.7.2_ComplicateAdversaryLessPredictable</rdfs:label>
        <owl:versionInfo>page 66</owl:versionInfo>
    </owl:Class>
    


    <!-- https://savage.nps.edu/EthicalControl/ontologies/MissionExecutionOntology#RE04.7.3 -->

    <owl:Class rdf:about="https://savage.nps.edu/EthicalControl/ontologies/MissionExecutionOntology#RE04.7.3">
        <rdfs:subClassOf rdf:resource="https://savage.nps.edu/EthicalControl/ontologies/MissionExecutionOntology#DADM04.7"/>
        <rdfs:comment>Can the IAS provide both speed and scale of action to impose multiple dilemmas on the enemy?</rdfs:comment>
        <rdfs:label>RE04.7.3_IASFunctionalMultipleAdversaryDilemmas</rdfs:label>
        <owl:versionInfo>page 66</owl:versionInfo>
    </owl:Class>
    


    <!-- https://savage.nps.edu/EthicalControl/ontologies/MissionExecutionOntology#RE04.7.4 -->

    <owl:Class rdf:about="https://savage.nps.edu/EthicalControl/ontologies/MissionExecutionOntology#RE04.7.4">
        <rdfs:subClassOf rdf:resource="https://savage.nps.edu/EthicalControl/ontologies/MissionExecutionOntology#DADM04.7"/>
        <rdfs:comment>Will the IAS enable superposition of multiple, fluidly composed and independent kill chains (or webs) that eliminate, or at least severely curtail, response options available to the enemy?</rdfs:comment>
        <rdfs:label>RE04.7.4_IASFunctionalMultipleFluidKillChains</rdfs:label>
        <owl:versionInfo>page 66</owl:versionInfo>
    </owl:Class>
    


    <!-- https://savage.nps.edu/EthicalControl/ontologies/MissionExecutionOntology#RE04.7.5 -->

    <owl:Class rdf:about="https://savage.nps.edu/EthicalControl/ontologies/MissionExecutionOntology#RE04.7.5">
        <rdfs:subClassOf rdf:resource="https://savage.nps.edu/EthicalControl/ontologies/MissionExecutionOntology#DADM04.7"/>
        <rdfs:comment>Can the IAS create an operational tempo that does not permit the adversary to regroup or concentrate?</rdfs:comment>
        <rdfs:label>RE04.7.5_IASFunctionalOverwhelmAdversary</rdfs:label>
        <owl:versionInfo>page 66</owl:versionInfo>
    </owl:Class>
    


    <!-- https://savage.nps.edu/EthicalControl/ontologies/MissionExecutionOntology#RE05.1.1 -->

    <owl:Class rdf:about="https://savage.nps.edu/EthicalControl/ontologies/MissionExecutionOntology#RE05.1.1">
        <rdfs:subClassOf rdf:resource="https://savage.nps.edu/EthicalControl/ontologies/MissionExecutionOntology#DADM05.1"/>
        <rdfs:comment>Can the IAS determine if its (possibly changing) operational environment requires &quot;human-in-the-loop,&quot; &quot;human-on-the-loop&quot;, or &quot;human-out-of-the-loop&quot; control and make that requirement known to a human operator?</rdfs:comment>
        <rdfs:label>RE05.1.1_IASDetermineHumanControl</rdfs:label>
        <owl:versionInfo>page 67</owl:versionInfo>
    </owl:Class>
    


    <!-- https://savage.nps.edu/EthicalControl/ontologies/MissionExecutionOntology#RE05.1.10 -->

    <owl:Class rdf:about="https://savage.nps.edu/EthicalControl/ontologies/MissionExecutionOntology#RE05.1.10">
        <rdfs:subClassOf rdf:resource="https://savage.nps.edu/EthicalControl/ontologies/MissionExecutionOntology#DADM05.1"/>
        <rdfs:comment>Are the number of human operators available sufficient to the number of IAS requiring command and control?</rdfs:comment>
        <rdfs:label>RE05.1.10_NumberOperatorsSufficient</rdfs:label>
        <owl:versionInfo>page 67</owl:versionInfo>
    </owl:Class>
    


    <!-- https://savage.nps.edu/EthicalControl/ontologies/MissionExecutionOntology#RE05.1.11 -->

    <owl:Class rdf:about="https://savage.nps.edu/EthicalControl/ontologies/MissionExecutionOntology#RE05.1.11">
        <rdfs:subClassOf rdf:resource="https://savage.nps.edu/EthicalControl/ontologies/MissionExecutionOntology#DADM05.1"/>
        <rdfs:comment>Can the IAS detect enemy attempts to wrest command and control away and notify the human operator?</rdfs:comment>
        <rdfs:label>RE05.1.11_IASDetectEnemyControl</rdfs:label>
        <owl:versionInfo>page 67</owl:versionInfo>
    </owl:Class>
    


    <!-- https://savage.nps.edu/EthicalControl/ontologies/MissionExecutionOntology#RE05.1.12 -->

    <owl:Class rdf:about="https://savage.nps.edu/EthicalControl/ontologies/MissionExecutionOntology#RE05.1.12">
        <rdfs:subClassOf rdf:resource="https://savage.nps.edu/EthicalControl/ontologies/MissionExecutionOntology#DADM05.1"/>
        <rdfs:comment>Can the IAS detect malfunctions or out of tolerance performance conditions that could result in a loss of command and control and notify the human operator?</rdfs:comment>
        <rdfs:label>RE05.1.12_IASDetectMalfunctions</rdfs:label>
        <owl:versionInfo>page 67</owl:versionInfo>
    </owl:Class>
    


    <!-- https://savage.nps.edu/EthicalControl/ontologies/MissionExecutionOntology#RE05.1.13 -->

    <owl:Class rdf:about="https://savage.nps.edu/EthicalControl/ontologies/MissionExecutionOntology#RE05.1.13">
        <rdfs:subClassOf rdf:resource="https://savage.nps.edu/EthicalControl/ontologies/MissionExecutionOntology#DADM05.1"/>
        <rdfs:comment>Can the IAS constantly monitor the availability of a control link, even when not under the direct and immediate direction of the human operator?</rdfs:comment>
        <rdfs:label>RE05.1.13_IASMonitorControlLink</rdfs:label>
        <owl:versionInfo>page 67</owl:versionInfo>
    </owl:Class>
    


    <!-- https://savage.nps.edu/EthicalControl/ontologies/MissionExecutionOntology#RE05.1.14 -->

    <owl:Class rdf:about="https://savage.nps.edu/EthicalControl/ontologies/MissionExecutionOntology#RE05.1.14">
        <rdfs:subClassOf rdf:resource="https://savage.nps.edu/EthicalControl/ontologies/MissionExecutionOntology#DADM05.1"/>
        <rdfs:comment>Can an IAS operating in a passive mode be prohibited from changing to an active mode of operation absent a direct instruction to do so by a human operator?</rdfs:comment>
        <rdfs:label>RE05.1.14_IASProhibitedActiveMode</rdfs:label>
        <owl:versionInfo>page 67</owl:versionInfo>
    </owl:Class>
    


    <!-- https://savage.nps.edu/EthicalControl/ontologies/MissionExecutionOntology#RE05.1.15 -->

    <owl:Class rdf:about="https://savage.nps.edu/EthicalControl/ontologies/MissionExecutionOntology#RE05.1.15">
        <rdfs:subClassOf rdf:resource="https://savage.nps.edu/EthicalControl/ontologies/MissionExecutionOntology#DADM05.1"/>
        <rdfs:comment>Can the IAS engage an emergent target, not on any preplanned list, without validation from a human operator?</rdfs:comment>
        <rdfs:label>RE05.1.15_IASEngageEmergentTarget</rdfs:label>
        <owl:versionInfo>page 68</owl:versionInfo>
    </owl:Class>
    


    <!-- https://savage.nps.edu/EthicalControl/ontologies/MissionExecutionOntology#RE05.1.16 -->

    <owl:Class rdf:about="https://savage.nps.edu/EthicalControl/ontologies/MissionExecutionOntology#RE05.1.16">
        <rdfs:subClassOf rdf:resource="https://savage.nps.edu/EthicalControl/ontologies/MissionExecutionOntology#DADM05.1"/>
        <rdfs:comment>Can the human operator choose to reject automated decision-making capabilities at their own discretion and at any time?</rdfs:comment>
        <rdfs:label>RE05.1.16_HumanRejectAutonomousDecision</rdfs:label>
        <owl:versionInfo>page 68</owl:versionInfo>
    </owl:Class>
    


    <!-- https://savage.nps.edu/EthicalControl/ontologies/MissionExecutionOntology#RE05.1.17 -->

    <owl:Class rdf:about="https://savage.nps.edu/EthicalControl/ontologies/MissionExecutionOntology#RE05.1.17">
        <rdfs:subClassOf rdf:resource="https://savage.nps.edu/EthicalControl/ontologies/MissionExecutionOntology#DADM05.1"/>
        <rdfs:comment>Can the human operator select a minimum confidence level that must be attained before the IAS can act without approval?</rdfs:comment>
        <rdfs:label>RE05.1.17_HumanSelectMinConfidence</rdfs:label>
        <owl:versionInfo>page 68</owl:versionInfo>
    </owl:Class>
    


    <!-- https://savage.nps.edu/EthicalControl/ontologies/MissionExecutionOntology#RE05.1.18 -->

    <owl:Class rdf:about="https://savage.nps.edu/EthicalControl/ontologies/MissionExecutionOntology#RE05.1.18">
        <rdfs:subClassOf rdf:resource="https://savage.nps.edu/EthicalControl/ontologies/MissionExecutionOntology#DADM05.1"/>
        <rdfs:comment>Can the IAS be made to have to check in with a human operator and be in receipt of an acknowledgement before proceeding with further actions?</rdfs:comment>
        <rdfs:label>RE05.1.18_IASForcedCheckIn</rdfs:label>
        <owl:versionInfo>page 68</owl:versionInfo>
    </owl:Class>
    


    <!-- https://savage.nps.edu/EthicalControl/ontologies/MissionExecutionOntology#RE05.1.19 -->

    <owl:Class rdf:about="https://savage.nps.edu/EthicalControl/ontologies/MissionExecutionOntology#RE05.1.19">
        <rdfs:subClassOf rdf:resource="https://savage.nps.edu/EthicalControl/ontologies/MissionExecutionOntology#DADM05.1"/>
        <rdfs:comment>Can the IAS identify conditions that might cause it to lose access to the control link with the human operator?</rdfs:comment>
        <rdfs:label>RE05.1.19_IASIdentifyLostLink</rdfs:label>
        <owl:versionInfo>page 68</owl:versionInfo>
    </owl:Class>
    


    <!-- https://savage.nps.edu/EthicalControl/ontologies/MissionExecutionOntology#RE05.1.2 -->

    <owl:Class rdf:about="https://savage.nps.edu/EthicalControl/ontologies/MissionExecutionOntology#RE05.1.2">
        <rdfs:subClassOf rdf:resource="https://savage.nps.edu/EthicalControl/ontologies/MissionExecutionOntology#DADM05.1"/>
        <rdfs:comment>Is the IAS prohibited from learning and executing new behaviors based on sensor inputs or data feeds received once decision-making capabilities have been transferred to it?</rdfs:comment>
        <rdfs:label>RE05.1.2_IASNewBehaviorsProhibited</rdfs:label>
        <owl:versionInfo>page 67</owl:versionInfo>
    </owl:Class>
    


    <!-- https://savage.nps.edu/EthicalControl/ontologies/MissionExecutionOntology#RE05.1.3 -->

    <owl:Class rdf:about="https://savage.nps.edu/EthicalControl/ontologies/MissionExecutionOntology#RE05.1.3">
        <rdfs:subClassOf rdf:resource="https://savage.nps.edu/EthicalControl/ontologies/MissionExecutionOntology#DADM05.1"/>
        <rdfs:comment>If the IAS is allowed to modify its behavior, does it consult the human operator beforehand?</rdfs:comment>
        <rdfs:label>RE05.1.3_IASConsultHuman</rdfs:label>
        <owl:versionInfo>page 67</owl:versionInfo>
    </owl:Class>
    


    <!-- https://savage.nps.edu/EthicalControl/ontologies/MissionExecutionOntology#RE05.1.4 -->

    <owl:Class rdf:about="https://savage.nps.edu/EthicalControl/ontologies/MissionExecutionOntology#RE05.1.4">
        <rdfs:subClassOf rdf:resource="https://savage.nps.edu/EthicalControl/ontologies/MissionExecutionOntology#DADM05.1"/>
        <rdfs:comment>Is the IAS prohibited from initiating operation in the absence of a control link to a human operator?</rdfs:comment>
        <rdfs:label>RE05.1.4_IASOperationInitiationProhibited</rdfs:label>
        <owl:versionInfo>page 67</owl:versionInfo>
    </owl:Class>
    


    <!-- https://savage.nps.edu/EthicalControl/ontologies/MissionExecutionOntology#RE05.1.5 -->

    <owl:Class rdf:about="https://savage.nps.edu/EthicalControl/ontologies/MissionExecutionOntology#RE05.1.5">
        <rdfs:subClassOf rdf:resource="https://savage.nps.edu/EthicalControl/ontologies/MissionExecutionOntology#DADM05.1"/>
        <rdfs:comment>Is the IAS prohibited from moving to a location where the control link to a human operator can be degraded or lost?</rdfs:comment>
        <rdfs:label>RE05.1.5_IASMovingProhibited</rdfs:label>
        <owl:versionInfo>page 67</owl:versionInfo>
    </owl:Class>
    


    <!-- https://savage.nps.edu/EthicalControl/ontologies/MissionExecutionOntology#RE05.1.6 -->

    <owl:Class rdf:about="https://savage.nps.edu/EthicalControl/ontologies/MissionExecutionOntology#RE05.1.6">
        <rdfs:subClassOf rdf:resource="https://savage.nps.edu/EthicalControl/ontologies/MissionExecutionOntology#DADM05.1"/>
        <rdfs:comment>Is the human operator still able to provide command and control over the actions of the IAS when it is employed as part of, and can act based on the conditions within, a swarm of other IAS?</rdfs:comment>
        <rdfs:label>RE05.1.6_HumanControlSwarm</rdfs:label>
        <owl:versionInfo>page 67</owl:versionInfo>
    </owl:Class>
    


    <!-- https://savage.nps.edu/EthicalControl/ontologies/MissionExecutionOntology#RE05.1.7 -->

    <owl:Class rdf:about="https://savage.nps.edu/EthicalControl/ontologies/MissionExecutionOntology#RE05.1.7">
        <rdfs:subClassOf rdf:resource="https://savage.nps.edu/EthicalControl/ontologies/MissionExecutionOntology#DADM05.1"/>
        <rdfs:comment>Is the human operator able to choose between a &quot;human in, on, or out of the loop?&quot;</rdfs:comment>
        <rdfs:label>RE05.1.7_HumanChooseInLoop</rdfs:label>
        <owl:versionInfo>page 67</owl:versionInfo>
    </owl:Class>
    


    <!-- https://savage.nps.edu/EthicalControl/ontologies/MissionExecutionOntology#RE05.1.8 -->

    <owl:Class rdf:about="https://savage.nps.edu/EthicalControl/ontologies/MissionExecutionOntology#RE05.1.8">
        <rdfs:subClassOf rdf:resource="https://savage.nps.edu/EthicalControl/ontologies/MissionExecutionOntology#DADM05.1"/>
        <rdfs:comment>Does the IAS enable the commander to determine and/or manage the symmetries/asymmetries in the level of complexity between own forces and enemy forces?</rdfs:comment>
        <rdfs:label>RE05.1.8_CommanderManageComplexity</rdfs:label>
        <owl:versionInfo>page 67</owl:versionInfo>
    </owl:Class>
    


    <!-- https://savage.nps.edu/EthicalControl/ontologies/MissionExecutionOntology#RE05.1.9 -->

    <owl:Class rdf:about="https://savage.nps.edu/EthicalControl/ontologies/MissionExecutionOntology#RE05.1.9">
        <rdfs:subClassOf rdf:resource="https://savage.nps.edu/EthicalControl/ontologies/MissionExecutionOntology#DADM05.1"/>
        <rdfs:comment>If a situation becomes too complex or unfolds too rapidly for the human operator to comprehend, can the human operator terminate an engagement?</rdfs:comment>
        <rdfs:label>RE05.1.9_HumanTerminateEngagement</rdfs:label>
        <owl:versionInfo>page 67</owl:versionInfo>
    </owl:Class>
    


    <!-- https://savage.nps.edu/EthicalControl/ontologies/MissionExecutionOntology#RE05.2.1 -->

    <owl:Class rdf:about="https://savage.nps.edu/EthicalControl/ontologies/MissionExecutionOntology#RE05.2.1">
        <rdfs:subClassOf rdf:resource="https://savage.nps.edu/EthicalControl/ontologies/MissionExecutionOntology#DADM05.2"/>
        <rdfs:comment>Can the commander selectively limit the actions that an IAS can take before relinquishing command and control over it?</rdfs:comment>
        <rdfs:label>RE05.2.1_IASActionsLimited</rdfs:label>
        <owl:versionInfo>page 68</owl:versionInfo>
    </owl:Class>
    


    <!-- https://savage.nps.edu/EthicalControl/ontologies/MissionExecutionOntology#RE05.2.2 -->

    <owl:Class rdf:about="https://savage.nps.edu/EthicalControl/ontologies/MissionExecutionOntology#RE05.2.2">
        <rdfs:subClassOf rdf:resource="https://savage.nps.edu/EthicalControl/ontologies/MissionExecutionOntology#DADM05.2"/>
        <rdfs:comment>Does the commander have a checklist of conditions that must be met, risk mitigation steps that have been taken, and an understanding of the risks being incurred, before relinquishing command and control over an IAS which possesses no lethal force capabilities, but whose autonomous operation could result in a lethal outcome via some secondary affect?</rdfs:comment>
        <rdfs:label>RE05.2.2_CommanderUnderstandRisk</rdfs:label>
        <owl:versionInfo>page 68</owl:versionInfo>
    </owl:Class>
    


    <!-- https://savage.nps.edu/EthicalControl/ontologies/MissionExecutionOntology#RE05.2.3 -->

    <owl:Class rdf:about="https://savage.nps.edu/EthicalControl/ontologies/MissionExecutionOntology#RE05.2.3">
        <rdfs:subClassOf rdf:resource="https://savage.nps.edu/EthicalControl/ontologies/MissionExecutionOntology#DADM05.2"/>
        <rdfs:comment>Has the commander acknowledged to his or her supporting Staff Judge Advocate, before relinquishing command and control of the IAS, that by doing so he or she is not relinquishing accountability for the outcomes of its actions?</rdfs:comment>
        <rdfs:label>RE05.2.3_CommanderAcknowledgeAccountabilityNonLethal</rdfs:label>
        <owl:versionInfo>page 68</owl:versionInfo>
    </owl:Class>
    


    <!-- https://savage.nps.edu/EthicalControl/ontologies/MissionExecutionOntology#RE05.2.4 -->

    <owl:Class rdf:about="https://savage.nps.edu/EthicalControl/ontologies/MissionExecutionOntology#RE05.2.4">
        <rdfs:subClassOf rdf:resource="https://savage.nps.edu/EthicalControl/ontologies/MissionExecutionOntology#DADM05.2"/>
        <rdfs:comment>Does the commander have a checklist of conditions that must be met, risk mitigation steps that have been taken, and an understanding of the risks being incurred, before relinquishing command and control over an IAS capable of selecting targets and applying lethal force to them?</rdfs:comment>
        <rdfs:label>RE05.2.4_CommanderAcknowledgeAccountabilityLethal</rdfs:label>
        <owl:versionInfo>page 68</owl:versionInfo>
    </owl:Class>
    


    <!-- https://savage.nps.edu/EthicalControl/ontologies/MissionExecutionOntology#RE05.3.1 -->

    <owl:Class rdf:about="https://savage.nps.edu/EthicalControl/ontologies/MissionExecutionOntology#RE05.3.1">
        <rdfs:subClassOf rdf:resource="https://savage.nps.edu/EthicalControl/ontologies/MissionExecutionOntology#DADM05.3"/>
        <rdfs:comment>Can the IAS verify that a request for transfer of command and control is from a human operator who is authorized to do so?</rdfs:comment>
        <rdfs:label>RE05.3.1_IASVerifyRequest</rdfs:label>
        <owl:versionInfo>page 68</owl:versionInfo>
    </owl:Class>
    


    <!-- https://savage.nps.edu/EthicalControl/ontologies/MissionExecutionOntology#RE05.3.2 -->

    <owl:Class rdf:about="https://savage.nps.edu/EthicalControl/ontologies/MissionExecutionOntology#RE05.3.2">
        <rdfs:subClassOf rdf:resource="https://savage.nps.edu/EthicalControl/ontologies/MissionExecutionOntology#DADM05.3"/>
        <rdfs:comment>Can the IAS determine when command and control has been transferred?</rdfs:comment>
        <rdfs:label>RE05.3.2_IASDetermineControlTransferred</rdfs:label>
        <owl:versionInfo>page 68</owl:versionInfo>
    </owl:Class>
    


    <!-- https://savage.nps.edu/EthicalControl/ontologies/MissionExecutionOntology#RE05.3.3 -->

    <owl:Class rdf:about="https://savage.nps.edu/EthicalControl/ontologies/MissionExecutionOntology#RE05.3.3">
        <rdfs:subClassOf rdf:resource="https://savage.nps.edu/EthicalControl/ontologies/MissionExecutionOntology#DADM05.3"/>
        <rdfs:comment>Is the IAS notified when the commander delegates control, to include target engagement authority, to a subordinate commander?</rdfs:comment>
        <rdfs:label>RE05.3.3_IASNotifiedControlDelegated</rdfs:label>
        <owl:versionInfo>page 68</owl:versionInfo>
    </owl:Class>
    


    <!-- https://savage.nps.edu/EthicalControl/ontologies/MissionExecutionOntology#RE05.3.4 -->

    <owl:Class rdf:about="https://savage.nps.edu/EthicalControl/ontologies/MissionExecutionOntology#RE05.3.4">
        <rdfs:subClassOf rdf:resource="https://savage.nps.edu/EthicalControl/ontologies/MissionExecutionOntology#DADM05.3"/>
        <rdfs:comment>Can the IAS transfer control back to a commander, or between commanders safely and in a manner that does not result in any lapses?</rdfs:comment>
        <rdfs:label>RE05.3.4_IASTransferControlSafely</rdfs:label>
        <owl:versionInfo>page 69</owl:versionInfo>
    </owl:Class>
    


    <!-- https://savage.nps.edu/EthicalControl/ontologies/MissionExecutionOntology#RE05.3.5 -->

    <owl:Class rdf:about="https://savage.nps.edu/EthicalControl/ontologies/MissionExecutionOntology#RE05.3.5">
        <rdfs:subClassOf rdf:resource="https://savage.nps.edu/EthicalControl/ontologies/MissionExecutionOntology#DADM05.3"/>
        <rdfs:comment>Can transfer of IAS control result in a loss of command and control, and can the transfer be delayed until a time when that possibility is at an acceptable minimum?</rdfs:comment>
        <rdfs:label>RE05.3.5_TransferCausedLossC2</rdfs:label>
        <owl:versionInfo>page 69</owl:versionInfo>
    </owl:Class>
    


    <!-- https://savage.nps.edu/EthicalControl/ontologies/MissionExecutionOntology#RE05.3.6 -->

    <owl:Class rdf:about="https://savage.nps.edu/EthicalControl/ontologies/MissionExecutionOntology#RE05.3.6">
        <rdfs:subClassOf rdf:resource="https://savage.nps.edu/EthicalControl/ontologies/MissionExecutionOntology#DADM05.3"/>
        <rdfs:comment>Can the IAS default to a minimal risk operating condition in the event that transfer of command and control was not successful?</rdfs:comment>
        <rdfs:label>RE05.3.6_IASDefaultMinimumRisk</rdfs:label>
        <owl:versionInfo>page 69</owl:versionInfo>
    </owl:Class>
    


    <!-- https://savage.nps.edu/EthicalControl/ontologies/MissionExecutionOntology#RE05.3.7 -->

    <owl:Class rdf:about="https://savage.nps.edu/EthicalControl/ontologies/MissionExecutionOntology#RE05.3.7">
        <rdfs:subClassOf rdf:resource="https://savage.nps.edu/EthicalControl/ontologies/MissionExecutionOntology#DADM05.3"/>
        <rdfs:comment>Can the IAS detect the absence or unavailability of a human operator before transferring command and control and default to a minimal risk operating condition until the human operator becomes available?</rdfs:comment>
        <rdfs:label>RE05.3.7_IASDetectAbsentOperator</rdfs:label>
        <owl:versionInfo>page 69</owl:versionInfo>
    </owl:Class>
    


    <!-- https://savage.nps.edu/EthicalControl/ontologies/MissionExecutionOntology#RE05.3.8 -->

    <owl:Class rdf:about="https://savage.nps.edu/EthicalControl/ontologies/MissionExecutionOntology#RE05.3.8">
        <rdfs:subClassOf rdf:resource="https://savage.nps.edu/EthicalControl/ontologies/MissionExecutionOntology#DADM05.3"/>
        <rdfs:comment>Can transfer of command and control of the IAS occur between coalition and allied forces?</rdfs:comment>
        <rdfs:label>RE05.3.8_IASControlledByAllies</rdfs:label>
        <owl:versionInfo>page 69</owl:versionInfo>
    </owl:Class>
    


    <!-- https://savage.nps.edu/EthicalControl/ontologies/MissionExecutionOntology#RE05.4.1 -->

    <owl:Class rdf:about="https://savage.nps.edu/EthicalControl/ontologies/MissionExecutionOntology#RE05.4.1">
        <rdfs:subClassOf rdf:resource="https://savage.nps.edu/EthicalControl/ontologies/MissionExecutionOntology#DADM05.4"/>
        <rdfs:comment>Can the IAS recognize and cease the conduct of emergent behaviors?</rdfs:comment>
        <rdfs:label>RE05.4.1_IASRecognizeEmergence</rdfs:label>
        <owl:versionInfo>page 69</owl:versionInfo>
    </owl:Class>
    


    <!-- https://savage.nps.edu/EthicalControl/ontologies/MissionExecutionOntology#RE05.4.10 -->

    <owl:Class rdf:about="https://savage.nps.edu/EthicalControl/ontologies/MissionExecutionOntology#RE05.4.10">
        <rdfs:subClassOf rdf:resource="https://savage.nps.edu/EthicalControl/ontologies/MissionExecutionOntology#DADM05.4"/>
        <rdfs:comment>Is the IAS susceptible to misread the environment and mismatch the appropriate action (e.g., come across a different environment but take the same action it has done before)?</rdfs:comment>
        <rdfs:label>RE05.4.10_IASMisreadEnvironment</rdfs:label>
        <owl:versionInfo>page 69</owl:versionInfo>
    </owl:Class>
    


    <!-- https://savage.nps.edu/EthicalControl/ontologies/MissionExecutionOntology#RE05.4.2 -->

    <owl:Class rdf:about="https://savage.nps.edu/EthicalControl/ontologies/MissionExecutionOntology#RE05.4.2">
        <rdfs:subClassOf rdf:resource="https://savage.nps.edu/EthicalControl/ontologies/MissionExecutionOntology#DADM05.4"/>
        <rdfs:comment>Is the IAS prohibited from learning during operations where there is no human in the loop?</rdfs:comment>
        <rdfs:label>RE05.4.2_IASLearningProhibited</rdfs:label>
        <owl:versionInfo>page 69</owl:versionInfo>
    </owl:Class>
    


    <!-- https://savage.nps.edu/EthicalControl/ontologies/MissionExecutionOntology#RE05.4.3 -->

    <owl:Class rdf:about="https://savage.nps.edu/EthicalControl/ontologies/MissionExecutionOntology#RE05.4.3">
        <rdfs:subClassOf rdf:resource="https://savage.nps.edu/EthicalControl/ontologies/MissionExecutionOntology#DADM05.4"/>
        <rdfs:comment>Can the IAS still learn but refrain from modifying behavior until evaluated by a human operator?</rdfs:comment>
        <rdfs:label>RE05.4.3_IASModifyBehavior</rdfs:label>
        <owl:versionInfo>page 69</owl:versionInfo>
    </owl:Class>
    


    <!-- https://savage.nps.edu/EthicalControl/ontologies/MissionExecutionOntology#RE05.4.4 -->

    <owl:Class rdf:about="https://savage.nps.edu/EthicalControl/ontologies/MissionExecutionOntology#RE05.4.4">
        <rdfs:subClassOf rdf:resource="https://savage.nps.edu/EthicalControl/ontologies/MissionExecutionOntology#DADM05.4"/>
        <rdfs:comment>Are commanders made aware of IAS under their command that have the ability to learn during operations and execute emergent behaviors based on incoming sensor data?</rdfs:comment>
        <rdfs:label>RE05.4.4_CommandersAwareIASEmergence</rdfs:label>
        <owl:versionInfo>page 69</owl:versionInfo>
    </owl:Class>
    


    <!-- https://savage.nps.edu/EthicalControl/ontologies/MissionExecutionOntology#RE05.4.5 -->

    <owl:Class rdf:about="https://savage.nps.edu/EthicalControl/ontologies/MissionExecutionOntology#RE05.4.5">
        <rdfs:subClassOf rdf:resource="https://savage.nps.edu/EthicalControl/ontologies/MissionExecutionOntology#DADM05.4"/>
        <rdfs:comment>Do commanders understand the potential occurrence of emergent behaviors with the IAS, based on its type and implementation of autonomous decisions?</rdfs:comment>
        <rdfs:label>RE05.4.5_CommandersUnderstandEmergence</rdfs:label>
        <owl:versionInfo>page 69</owl:versionInfo>
    </owl:Class>
    


    <!-- https://savage.nps.edu/EthicalControl/ontologies/MissionExecutionOntology#RE05.4.6 -->

    <owl:Class rdf:about="https://savage.nps.edu/EthicalControl/ontologies/MissionExecutionOntology#RE05.4.6">
        <rdfs:subClassOf rdf:resource="https://savage.nps.edu/EthicalControl/ontologies/MissionExecutionOntology#DADM05.4"/>
        <rdfs:comment>Are thresholds identified and set to alert the commander to the existence and nature of emergent behaviors?</rdfs:comment>
        <rdfs:label>RE05.4.6_EmergenceThresholdsSet</rdfs:label>
        <owl:versionInfo>page 69</owl:versionInfo>
    </owl:Class>
    


    <!-- https://savage.nps.edu/EthicalControl/ontologies/MissionExecutionOntology#RE05.4.7 -->

    <owl:Class rdf:about="https://savage.nps.edu/EthicalControl/ontologies/MissionExecutionOntology#RE05.4.7">
        <rdfs:subClassOf rdf:resource="https://savage.nps.edu/EthicalControl/ontologies/MissionExecutionOntology#DADM05.4"/>
        <rdfs:comment>Can the commander limit the ability of the IAS to learn during operations and exhibit emergent behavior?</rdfs:comment>
        <rdfs:label>RE05.4.7_IASEmergenceLimitable</rdfs:label>
        <owl:versionInfo>page 69</owl:versionInfo>
    </owl:Class>
    


    <!-- https://savage.nps.edu/EthicalControl/ontologies/MissionExecutionOntology#RE05.4.8 -->

    <owl:Class rdf:about="https://savage.nps.edu/EthicalControl/ontologies/MissionExecutionOntology#RE05.4.8">
        <rdfs:subClassOf rdf:resource="https://savage.nps.edu/EthicalControl/ontologies/MissionExecutionOntology#DADM05.4"/>
        <rdfs:comment>Can the IAS notify the commander when it alters its operating code?</rdfs:comment>
        <rdfs:label>RE05.4.8_IASAlertsCodeChanges</rdfs:label>
        <owl:versionInfo>page 69</owl:versionInfo>
    </owl:Class>
    


    <!-- https://savage.nps.edu/EthicalControl/ontologies/MissionExecutionOntology#RE05.4.9 -->

    <owl:Class rdf:about="https://savage.nps.edu/EthicalControl/ontologies/MissionExecutionOntology#RE05.4.9">
        <rdfs:subClassOf rdf:resource="https://savage.nps.edu/EthicalControl/ontologies/MissionExecutionOntology#DADM05.4"/>
        <rdfs:comment>Can the IAS retain a record of every action it has ever taken and notify the commander when it is about to take an action that deviates from previous actions by a predefined threshold or standard?</rdfs:comment>
        <rdfs:label>RE05.4.9_IASAlertActionsDeviate</rdfs:label>
        <owl:versionInfo>page 69</owl:versionInfo>
    </owl:Class>
    


    <!-- https://savage.nps.edu/EthicalControl/ontologies/MissionExecutionOntology#RE05.5.1 -->

    <owl:Class rdf:about="https://savage.nps.edu/EthicalControl/ontologies/MissionExecutionOntology#RE05.5.1">
        <rdfs:subClassOf rdf:resource="https://savage.nps.edu/EthicalControl/ontologies/MissionExecutionOntology#DADM05.5"/>
        <rdfs:comment>Can the IAS, in the event that command and control is lost for any reason (and based on pre-determined criteria), continue autonomously to execute the most recent mission or task instruction if that is the safest option?</rdfs:comment>
        <rdfs:label>RE05.5.1_IASContinueSafely</rdfs:label>
        <owl:versionInfo>page 70</owl:versionInfo>
    </owl:Class>
    


    <!-- https://savage.nps.edu/EthicalControl/ontologies/MissionExecutionOntology#RE05.5.10 -->

    <owl:Class rdf:about="https://savage.nps.edu/EthicalControl/ontologies/MissionExecutionOntology#RE05.5.10">
        <rdfs:subClassOf rdf:resource="https://savage.nps.edu/EthicalControl/ontologies/MissionExecutionOntology#DADM05.5"/>
        <rdfs:comment>Does the IAS have multiple redundancies in critical systems that enable graceful degradation of performance instead of a catastrophic loss of command and control?</rdfs:comment>
        <rdfs:label>RE05.5.10_IASReduntantCCSystems</rdfs:label>
        <owl:versionInfo>page 70</owl:versionInfo>
    </owl:Class>
    


    <!-- https://savage.nps.edu/EthicalControl/ontologies/MissionExecutionOntology#RE05.5.11 -->

    <owl:Class rdf:about="https://savage.nps.edu/EthicalControl/ontologies/MissionExecutionOntology#RE05.5.11">
        <rdfs:subClassOf rdf:resource="https://savage.nps.edu/EthicalControl/ontologies/MissionExecutionOntology#DADM05.5"/>
        <rdfs:comment>Does the IAS have internal sensors capable of detecting current or impending system failures or battle damage such that it can autonomously switch to an appropriate redundant backup system?</rdfs:comment>
        <rdfs:label>RE05.5.11_IASSwitchBackupSystems</rdfs:label>
        <owl:versionInfo>page 70</owl:versionInfo>
    </owl:Class>
    


    <!-- https://savage.nps.edu/EthicalControl/ontologies/MissionExecutionOntology#RE05.5.2 -->

    <owl:Class rdf:about="https://savage.nps.edu/EthicalControl/ontologies/MissionExecutionOntology#RE05.5.2">
        <rdfs:subClassOf rdf:resource="https://savage.nps.edu/EthicalControl/ontologies/MissionExecutionOntology#DADM05.5"/>
        <rdfs:comment>Can the IAS, in the event that command and control is lost for any reason (and based on pre-determined criteria), hold speed and course or loiter to await re-establishment of command and control?</rdfs:comment>
        <rdfs:label>RE05.5.2_IASMaintainMotion</rdfs:label>
        <owl:versionInfo>page 70</owl:versionInfo>
    </owl:Class>
    


    <!-- https://savage.nps.edu/EthicalControl/ontologies/MissionExecutionOntology#RE05.5.3 -->

    <owl:Class rdf:about="https://savage.nps.edu/EthicalControl/ontologies/MissionExecutionOntology#RE05.5.3">
        <rdfs:subClassOf rdf:resource="https://savage.nps.edu/EthicalControl/ontologies/MissionExecutionOntology#DADM05.5"/>
        <rdfs:comment>Can the IAS, in the event that command and control is lost for any reason (and based on pre-determined criteria), abort mission and return to base?</rdfs:comment>
        <rdfs:label>RE05.5.3_IASAbortMission</rdfs:label>
        <owl:versionInfo>page 70</owl:versionInfo>
    </owl:Class>
    


    <!-- https://savage.nps.edu/EthicalControl/ontologies/MissionExecutionOntology#RE05.5.4 -->

    <owl:Class rdf:about="https://savage.nps.edu/EthicalControl/ontologies/MissionExecutionOntology#RE05.5.4">
        <rdfs:subClassOf rdf:resource="https://savage.nps.edu/EthicalControl/ontologies/MissionExecutionOntology#DADM05.5"/>
        <rdfs:comment>Can the IAS, in the event that command and control is lost for any reason (and based on pre-determined criteria), initiate emergency (and possibly non-secure) communications to receive further instructions?</rdfs:comment>
        <rdfs:label>RE05.5.4_IASInitiateEmergencyComms</rdfs:label>
        <owl:versionInfo>page 70</owl:versionInfo>
    </owl:Class>
    


    <!-- https://savage.nps.edu/EthicalControl/ontologies/MissionExecutionOntology#RE05.5.5 -->

    <owl:Class rdf:about="https://savage.nps.edu/EthicalControl/ontologies/MissionExecutionOntology#RE05.5.5">
        <rdfs:subClassOf rdf:resource="https://savage.nps.edu/EthicalControl/ontologies/MissionExecutionOntology#DADM05.5"/>
        <rdfs:comment>Can the IAS, in the event that command and control is lost for any reason (and based on pre-determined criteria), destroy itself?</rdfs:comment>
        <rdfs:label>RE05.5.5_IASSelfDestruct</rdfs:label>
        <owl:versionInfo>page 70</owl:versionInfo>
    </owl:Class>
    


    <!-- https://savage.nps.edu/EthicalControl/ontologies/MissionExecutionOntology#RE05.5.6 -->

    <owl:Class rdf:about="https://savage.nps.edu/EthicalControl/ontologies/MissionExecutionOntology#RE05.5.6">
        <rdfs:subClassOf rdf:resource="https://savage.nps.edu/EthicalControl/ontologies/MissionExecutionOntology#DADM05.5"/>
        <rdfs:comment>Can the IAS, in the event that command and control is lost for any reason (and based on pre-determined criteria), be prohibited from autonomous selection and engagement of individual targets that have not been previously selected by an authorized human operator?</rdfs:comment>
        <rdfs:label>RE05.5.6_IASProhibitedSelectingTargets</rdfs:label>
        <owl:versionInfo>page 70</owl:versionInfo>
    </owl:Class>
    


    <!-- https://savage.nps.edu/EthicalControl/ontologies/MissionExecutionOntology#RE05.5.7 -->

    <owl:Class rdf:about="https://savage.nps.edu/EthicalControl/ontologies/MissionExecutionOntology#RE05.5.7">
        <rdfs:subClassOf rdf:resource="https://savage.nps.edu/EthicalControl/ontologies/MissionExecutionOntology#DADM05.5"/>
        <rdfs:comment>Can the IAS, in the event that command and control is lost for any reason (and based on pre-determined criteria), be prohibited from autonomous selection and engagement of specific target groups that have not been previously selected by an authorized human operator?</rdfs:comment>
        <rdfs:label>RE05.5.7_IASProhibitedSelectingTargetGroups</rdfs:label>
        <owl:versionInfo>page 70</owl:versionInfo>
    </owl:Class>
    


    <!-- https://savage.nps.edu/EthicalControl/ontologies/MissionExecutionOntology#RE05.5.8 -->

    <owl:Class rdf:about="https://savage.nps.edu/EthicalControl/ontologies/MissionExecutionOntology#RE05.5.8">
        <rdfs:subClassOf rdf:resource="https://savage.nps.edu/EthicalControl/ontologies/MissionExecutionOntology#DADM05.5"/>
        <rdfs:comment>Can the IAS, in the event that command and control is lost for any reason (and based on pre-determined criteria), be prohibited from autonomously making any hostile and/or targeting decision whatsoever?</rdfs:comment>
        <rdfs:label>RE05.5.8_IASProhibitedTargetingDecisions</rdfs:label>
        <owl:versionInfo>page 70</owl:versionInfo>
    </owl:Class>
    


    <!-- https://savage.nps.edu/EthicalControl/ontologies/MissionExecutionOntology#RE05.5.9 -->

    <owl:Class rdf:about="https://savage.nps.edu/EthicalControl/ontologies/MissionExecutionOntology#RE05.5.9">
        <rdfs:subClassOf rdf:resource="https://savage.nps.edu/EthicalControl/ontologies/MissionExecutionOntology#DADM05.5"/>
        <rdfs:comment>Can the IAS, in the event that command and control is lost for any reason (and based on pre-determined criteria), follow the original human intent regarding target selection?</rdfs:comment>
        <rdfs:label>RE05.5.9_IASFollowHumanIntent</rdfs:label>
        <owl:versionInfo>page 70</owl:versionInfo>
    </owl:Class>
    


    <!-- https://savage.nps.edu/EthicalControl/ontologies/MissionExecutionOntology#RE05.6.1 -->

    <owl:Class rdf:about="https://savage.nps.edu/EthicalControl/ontologies/MissionExecutionOntology#RE05.6.1">
        <rdfs:subClassOf rdf:resource="https://savage.nps.edu/EthicalControl/ontologies/MissionExecutionOntology#DADM05.6"/>
        <rdfs:comment>Can the human operator verify that he/she has re-established command and control to prevent an IAS from continuing to execute failsafe protocols?</rdfs:comment>
        <rdfs:label>RE05.6.1_OperatorVerifyC2</rdfs:label>
        <owl:versionInfo>page 71</owl:versionInfo>
    </owl:Class>
    


    <!-- https://savage.nps.edu/EthicalControl/ontologies/MissionExecutionOntology#RE05.6.2 -->

    <owl:Class rdf:about="https://savage.nps.edu/EthicalControl/ontologies/MissionExecutionOntology#RE05.6.2">
        <rdfs:subClassOf rdf:resource="https://savage.nps.edu/EthicalControl/ontologies/MissionExecutionOntology#DADM05.6"/>
        <rdfs:comment>Does the IAS immediately alert emergency service providers and recovery crews in the event of a collision or malfunction who can verify safe operating condition before returning the IAS to service?</rdfs:comment>
        <rdfs:label>RE05.6.2_IASAlertRecoveryCrew</rdfs:label>
        <owl:versionInfo>page 71</owl:versionInfo>
    </owl:Class>
    


    <!-- https://savage.nps.edu/EthicalControl/ontologies/MissionExecutionOntology#RE06.1.1 -->

    <owl:Class rdf:about="https://savage.nps.edu/EthicalControl/ontologies/MissionExecutionOntology#RE06.1.1">
        <rdfs:subClassOf rdf:resource="https://savage.nps.edu/EthicalControl/ontologies/MissionExecutionOntology#DADM06.1"/>
        <rdfs:comment>Can the IAS calculate a confidence factor for positive identification assessments of persons and objects protected from the use of force and prohibit the use of force if that confidence factor is below a minimum threshold set by the commander?</rdfs:comment>
        <rdfs:label>RE06.1.1_CanCalculateConfidenceFactor</rdfs:label>
        <owl:versionInfo>page 71</owl:versionInfo>
    </owl:Class>
    


    <!-- https://savage.nps.edu/EthicalControl/ontologies/MissionExecutionOntology#RE06.1.2 -->

    <owl:Class rdf:about="https://savage.nps.edu/EthicalControl/ontologies/MissionExecutionOntology#RE06.1.2">
        <rdfs:subClassOf rdf:resource="https://savage.nps.edu/EthicalControl/ontologies/MissionExecutionOntology#DADM06.1"/>
        <rdfs:comment>Can the IAS task own platform or other platform sensors to gather additional data to improve positive identification assessments when the confidence factors are below the minimum threshold set by the commander?</rdfs:comment>
        <rdfs:label>RE06.1.2_CanTaskImprovePerceptionConfidence</rdfs:label>
        <owl:versionInfo>page 71</owl:versionInfo>
    </owl:Class>
    


    <!-- https://savage.nps.edu/EthicalControl/ontologies/MissionExecutionOntology#RE06.1.3 -->

    <owl:Class rdf:about="https://savage.nps.edu/EthicalControl/ontologies/MissionExecutionOntology#RE06.1.3">
        <rdfs:subClassOf rdf:resource="https://savage.nps.edu/EthicalControl/ontologies/MissionExecutionOntology#DADM06.1"/>
        <rdfs:comment>Can the IAS seek additional &quot;reach back&quot; intelligence information to improve positive identification assessments when the confidence factor is below the minimum threshold set by the commander?</rdfs:comment>
        <rdfs:label>RE06.1.3_CanCallbackImproveConfidence</rdfs:label>
        <owl:versionInfo>page 71</owl:versionInfo>
    </owl:Class>
    


    <!-- https://savage.nps.edu/EthicalControl/ontologies/MissionExecutionOntology#RE06.1.4 -->

    <owl:Class rdf:about="https://savage.nps.edu/EthicalControl/ontologies/MissionExecutionOntology#RE06.1.4">
        <rdfs:subClassOf rdf:resource="https://savage.nps.edu/EthicalControl/ontologies/MissionExecutionOntology#DADM06.1"/>
        <rdfs:comment>Can the IAS decision not to act based on a confidence factor below the minimum threshold set by the commander be overridden by that commander?</rdfs:comment>
        <rdfs:label>RE06.1.4_CanCommanderUpdateConfidenceThreshold</rdfs:label>
        <owl:versionInfo>page 71</owl:versionInfo>
    </owl:Class>
    


    <!-- https://savage.nps.edu/EthicalControl/ontologies/MissionExecutionOntology#RE06.1.5 -->

    <owl:Class rdf:about="https://savage.nps.edu/EthicalControl/ontologies/MissionExecutionOntology#RE06.1.5">
        <rdfs:subClassOf rdf:resource="https://savage.nps.edu/EthicalControl/ontologies/MissionExecutionOntology#DADM06.1"/>
        <rdfs:comment>Can the IAS decision not to act based on a confidence factor below the minimum threshold set by the commander be overridden by other commanders who have had that authority delegated to them by the commander?</rdfs:comment>
        <rdfs:label>RE06.1.5_CanOtherCommandersUpdateConfidenceThreshold</rdfs:label>
        <owl:versionInfo>page 71</owl:versionInfo>
    </owl:Class>
    


    <!-- https://savage.nps.edu/EthicalControl/ontologies/MissionExecutionOntology#RE06.1.6 -->

    <owl:Class rdf:about="https://savage.nps.edu/EthicalControl/ontologies/MissionExecutionOntology#RE06.1.6">
        <rdfs:subClassOf rdf:resource="https://savage.nps.edu/EthicalControl/ontologies/MissionExecutionOntology#DADM06.1"/>
        <rdfs:comment>Can the IAS deployment be limited to a well-defined area where only enemy combatants or military objects are present?</rdfs:comment>
        <rdfs:label>RE06.1.6_CanIASBeGeofenced</rdfs:label>
        <owl:versionInfo>page 71</owl:versionInfo>
    </owl:Class>
    


    <!-- https://savage.nps.edu/EthicalControl/ontologies/MissionExecutionOntology#RE06.1.7 -->

    <owl:Class rdf:about="https://savage.nps.edu/EthicalControl/ontologies/MissionExecutionOntology#RE06.1.7">
        <rdfs:subClassOf rdf:resource="https://savage.nps.edu/EthicalControl/ontologies/MissionExecutionOntology#DADM06.1"/>
        <rdfs:comment>Can the IAS detect the presence of (uncategorized) humans near or within a targeted object?</rdfs:comment>
        <rdfs:label>RE06.1.7_CanIASDetectUnknownPeopleInTarget</rdfs:label>
        <owl:versionInfo>page 71</owl:versionInfo>
    </owl:Class>
    


    <!-- https://savage.nps.edu/EthicalControl/ontologies/MissionExecutionOntology#RE06.1.8 -->

    <owl:Class rdf:about="https://savage.nps.edu/EthicalControl/ontologies/MissionExecutionOntology#RE06.1.8">
        <rdfs:subClassOf rdf:resource="https://savage.nps.edu/EthicalControl/ontologies/MissionExecutionOntology#DADM06.1"/>
        <rdfs:comment>Can an IAS, even if unarmed, result in collateral damage in the event of a malfunction (such as a crash)?</rdfs:comment>
        <rdfs:label>RE06.1.8_CanIASYieldCrashDamage</rdfs:label>
        <owl:versionInfo>page 71</owl:versionInfo>
    </owl:Class>
    


    <!-- https://savage.nps.edu/EthicalControl/ontologies/MissionExecutionOntology#RE06.10.1 -->

    <owl:Class rdf:about="https://savage.nps.edu/EthicalControl/ontologies/MissionExecutionOntology#RE06.10.1">
        <rdfs:subClassOf rdf:resource="https://savage.nps.edu/EthicalControl/ontologies/MissionExecutionOntology#DADM06.10"/>
        <rdfs:comment>Can the IAS detect when a surrendering enemy combatant has violated the terms of surrender by attempting to escape?</rdfs:comment>
        <rdfs:label>RE06.10.1_CanDetectSurrenderViolation</rdfs:label>
        <owl:versionInfo>page 74</owl:versionInfo>
    </owl:Class>
    


    <!-- https://savage.nps.edu/EthicalControl/ontologies/MissionExecutionOntology#RE06.10.2 -->

    <owl:Class rdf:about="https://savage.nps.edu/EthicalControl/ontologies/MissionExecutionOntology#RE06.10.2">
        <rdfs:subClassOf rdf:resource="https://savage.nps.edu/EthicalControl/ontologies/MissionExecutionOntology#DADM06.10"/>
        <rdfs:comment>Can the IAS detect when a surrendering enemy combatant has violated the terms of surrender by committing a hostile act?</rdfs:comment>
        <rdfs:label>RE06.10.2_CanDetectHostileActViolation</rdfs:label>
        <owl:versionInfo>page 74</owl:versionInfo>
    </owl:Class>
    


    <!-- https://savage.nps.edu/EthicalControl/ontologies/MissionExecutionOntology#RE06.10.3 -->

    <owl:Class rdf:about="https://savage.nps.edu/EthicalControl/ontologies/MissionExecutionOntology#RE06.10.3">
        <rdfs:subClassOf rdf:resource="https://savage.nps.edu/EthicalControl/ontologies/MissionExecutionOntology#DADM06.10"/>
        <rdfs:comment>Can the IAS detect and communicate perfidious acts to human operators?</rdfs:comment>
        <rdfs:label>RE06.10.3_CanInferPerfidiousActsPeople</rdfs:label>
        <owl:versionInfo>page 74</owl:versionInfo>
    </owl:Class>
    


    <!-- https://savage.nps.edu/EthicalControl/ontologies/MissionExecutionOntology#RE06.11.1.1 -->

    <owl:Class rdf:about="https://savage.nps.edu/EthicalControl/ontologies/MissionExecutionOntology#RE06.11.1.1">
        <rdfs:subClassOf rdf:resource="https://savage.nps.edu/EthicalControl/ontologies/MissionExecutionOntology#DADM06.11.1"/>
        <rdfs:comment>Can the IAS identify and not intentionally harm (in a manner that would violate laws, policies, or the rules of engagement) military medical personnel?</rdfs:comment>
        <rdfs:label>RE06.11.1.1_CanEnsureProtectionMilitaryMedicalPeople</rdfs:label>
        <owl:versionInfo>page 75</owl:versionInfo>
    </owl:Class>
    


    <!-- https://savage.nps.edu/EthicalControl/ontologies/MissionExecutionOntology#RE06.11.1.2 -->

    <owl:Class rdf:about="https://savage.nps.edu/EthicalControl/ontologies/MissionExecutionOntology#RE06.11.1.2">
        <rdfs:subClassOf rdf:resource="https://savage.nps.edu/EthicalControl/ontologies/MissionExecutionOntology#DADM06.11.1"/>
        <rdfs:comment>Can the IAS identify and not intentionally harm (in a manner that would violate laws, policies, or the rules of engagement) military religious personnel?</rdfs:comment>
        <rdfs:label>RE06.11.1.2_CanEnsureProtectionMilitaryReligiousLeader</rdfs:label>
        <owl:versionInfo>page 75</owl:versionInfo>
    </owl:Class>
    


    <!-- https://savage.nps.edu/EthicalControl/ontologies/MissionExecutionOntology#RE06.11.1.3 -->

    <owl:Class rdf:about="https://savage.nps.edu/EthicalControl/ontologies/MissionExecutionOntology#RE06.11.1.3">
        <rdfs:subClassOf rdf:resource="https://savage.nps.edu/EthicalControl/ontologies/MissionExecutionOntology#DADM06.11.1"/>
        <rdfs:comment>Can the IAS identify and not intentionally harm (in a manner that would violate laws, policies, or the rules of engagement) human shields (persons placed around or within valid military target to hinder attack)?</rdfs:comment>
        <rdfs:label>RE06.11.1.3_CanEnsureProtectionHumanShields</rdfs:label>
        <owl:versionInfo>page 75</owl:versionInfo>
    </owl:Class>
    


    <!-- https://savage.nps.edu/EthicalControl/ontologies/MissionExecutionOntology#RE06.11.2.1 -->

    <owl:Class rdf:about="https://savage.nps.edu/EthicalControl/ontologies/MissionExecutionOntology#RE06.11.2.1">
        <rdfs:subClassOf rdf:resource="https://savage.nps.edu/EthicalControl/ontologies/MissionExecutionOntology#DADM06.11.2"/>
        <rdfs:comment>Can the IAS detect and perceive any signal of surrender that all combatant sides have previously agreed to use?</rdfs:comment>
        <rdfs:label>RE06.11.2.1_CanRecognizeAgreedSurrenderSignals</rdfs:label>
        <owl:versionInfo>page 75</owl:versionInfo>
    </owl:Class>
    


    <!-- https://savage.nps.edu/EthicalControl/ontologies/MissionExecutionOntology#RE06.11.2.2 -->

    <owl:Class rdf:about="https://savage.nps.edu/EthicalControl/ontologies/MissionExecutionOntology#RE06.11.2.2">
        <rdfs:subClassOf rdf:resource="https://savage.nps.edu/EthicalControl/ontologies/MissionExecutionOntology#DADM06.11.2"/>
        <rdfs:comment>Can the IAS detect and perceive indications of surrender from enemy combatants that have been trained on how to indicate surrender to the IAS?</rdfs:comment>
        <rdfs:label>RE06.11.2.2_CanRecognizeSurrenderTrainedPeople</rdfs:label>
        <owl:versionInfo>page 75</owl:versionInfo>
    </owl:Class>
    


    <!-- https://savage.nps.edu/EthicalControl/ontologies/MissionExecutionOntology#RE06.11.2.3 -->

    <owl:Class rdf:about="https://savage.nps.edu/EthicalControl/ontologies/MissionExecutionOntology#RE06.11.2.3">
        <rdfs:subClassOf rdf:resource="https://savage.nps.edu/EthicalControl/ontologies/MissionExecutionOntology#DADM06.11.2"/>
        <rdfs:comment>Can the IAS detect and perceive indications of surrender from enemy combatants that have not been trained on how to indicate surrender to the IAS?</rdfs:comment>
        <rdfs:label>RE06.11.2.3_CanRecognizeSurrenderUntrainedPeople</rdfs:label>
        <owl:versionInfo>page 75</owl:versionInfo>
    </owl:Class>
    


    <!-- https://savage.nps.edu/EthicalControl/ontologies/MissionExecutionOntology#RE06.11.2.4 -->

    <owl:Class rdf:about="https://savage.nps.edu/EthicalControl/ontologies/MissionExecutionOntology#RE06.11.2.4">
        <rdfs:subClassOf rdf:resource="https://savage.nps.edu/EthicalControl/ontologies/MissionExecutionOntology#DADM06.11.2"/>
        <rdfs:comment>Can the IAS detect and perceive the changes in orientation and force posture of combatants that are commonly associated with the act of surrender?</rdfs:comment>
        <rdfs:label>RE06.11.2.4_CanIdentifyReadySurrender</rdfs:label>
        <owl:versionInfo>page 75</owl:versionInfo>
    </owl:Class>
    


    <!-- https://savage.nps.edu/EthicalControl/ontologies/MissionExecutionOntology#RE06.11.2.5 -->

    <owl:Class rdf:about="https://savage.nps.edu/EthicalControl/ontologies/MissionExecutionOntology#RE06.11.2.5">
        <rdfs:subClassOf rdf:resource="https://savage.nps.edu/EthicalControl/ontologies/MissionExecutionOntology#DADM06.11.2"/>
        <rdfs:comment>Can the IAS distinguish between retreating and surrendering enemy forces? Incapacitated persons</rdfs:comment>
        <rdfs:label>RE06.11.2.5_CanIdentifyRetreatingSurrenderingIncapacitatedPerson</rdfs:label>
        <owl:versionInfo>page 75</owl:versionInfo>
    </owl:Class>
    


    <!-- https://savage.nps.edu/EthicalControl/ontologies/MissionExecutionOntology#RE06.11.2.6 -->

    <owl:Class rdf:about="https://savage.nps.edu/EthicalControl/ontologies/MissionExecutionOntology#RE06.11.2.6">
        <rdfs:subClassOf rdf:resource="https://savage.nps.edu/EthicalControl/ontologies/MissionExecutionOntology#DADM06.11.2"/>
        <rdfs:comment>Can the IAS identify and not intentionally harm (in a manner that would violate laws, policies, or the rules of engagement) wounded or sick persons?</rdfs:comment>
        <rdfs:label>RE06.11.2.6_CanIdentifyWoundedSickPerson</rdfs:label>
        <owl:versionInfo>page 75</owl:versionInfo>
    </owl:Class>
    


    <!-- https://savage.nps.edu/EthicalControl/ontologies/MissionExecutionOntology#RE06.11.2.7 -->

    <owl:Class rdf:about="https://savage.nps.edu/EthicalControl/ontologies/MissionExecutionOntology#RE06.11.2.7">
        <rdfs:subClassOf rdf:resource="https://savage.nps.edu/EthicalControl/ontologies/MissionExecutionOntology#DADM06.11.2"/>
        <rdfs:comment>Can the IAS identify and not intentionally harm (in a manner that would violate laws, policies, or the rules of engagement) shipwrecked persons?</rdfs:comment>
        <rdfs:label>RE06.11.2.7_CanIdentifyShipwreckedPerson</rdfs:label>
        <owl:versionInfo>page 75</owl:versionInfo>
    </owl:Class>
    


    <!-- https://savage.nps.edu/EthicalControl/ontologies/MissionExecutionOntology#RE06.11.3.1 -->

    <owl:Class rdf:about="https://savage.nps.edu/EthicalControl/ontologies/MissionExecutionOntology#RE06.11.3.1">
        <rdfs:subClassOf rdf:resource="https://savage.nps.edu/EthicalControl/ontologies/MissionExecutionOntology#DADM06.11.3"/>
        <rdfs:comment>Can the IAS detect and not intentionally harm US citizens in a manner that would violate Constitutional protections?</rdfs:comment>
        <rdfs:label>RE06.11.3.1_CanProtectUSCitizen</rdfs:label>
        <owl:versionInfo>page 75</owl:versionInfo>
    </owl:Class>
    


    <!-- https://savage.nps.edu/EthicalControl/ontologies/MissionExecutionOntology#RE06.11.3.2 -->

    <owl:Class rdf:about="https://savage.nps.edu/EthicalControl/ontologies/MissionExecutionOntology#RE06.11.3.2">
        <rdfs:subClassOf rdf:resource="https://savage.nps.edu/EthicalControl/ontologies/MissionExecutionOntology#DADM06.11.3"/>
        <rdfs:comment>Can the IAS detect and distinguish the presence of US citizens who are acting as enemy combatants?</rdfs:comment>
        <rdfs:label>RE06.11.3.2_CanIdentifyUSCitizenEnemyCombatant</rdfs:label>
        <owl:versionInfo>page 75</owl:versionInfo>
    </owl:Class>
    


    <!-- https://savage.nps.edu/EthicalControl/ontologies/MissionExecutionOntology#RE06.11.4.1 -->

    <owl:Class rdf:about="https://savage.nps.edu/EthicalControl/ontologies/MissionExecutionOntology#RE06.11.4.1">
        <rdfs:subClassOf rdf:resource="https://savage.nps.edu/EthicalControl/ontologies/MissionExecutionOntology#DADM06.11.4"/>
        <rdfs:comment>Can the IAS ingest data from all blue force tracker systems?</rdfs:comment>
        <rdfs:label>RE06.11.4.1_CanIngestBlueForceTracker</rdfs:label>
        <owl:versionInfo>page 75</owl:versionInfo>
    </owl:Class>
    


    <!-- https://savage.nps.edu/EthicalControl/ontologies/MissionExecutionOntology#RE06.11.4.2 -->

    <owl:Class rdf:about="https://savage.nps.edu/EthicalControl/ontologies/MissionExecutionOntology#RE06.11.4.2">
        <rdfs:subClassOf rdf:resource="https://savage.nps.edu/EthicalControl/ontologies/MissionExecutionOntology#DADM06.11.4"/>
        <rdfs:comment>Can the IAS obtain, analyze and use information to assess risk to friendly forces and calculate a confidence factor for each assessment?</rdfs:comment>
        <rdfs:label>RE06.11.4.2_CanCalculateConfidenceFactorFriendlyForces</rdfs:label>
        <owl:versionInfo>page 76</owl:versionInfo>
    </owl:Class>
    


    <!-- https://savage.nps.edu/EthicalControl/ontologies/MissionExecutionOntology#RE06.11.4.3 -->

    <owl:Class rdf:about="https://savage.nps.edu/EthicalControl/ontologies/MissionExecutionOntology#RE06.11.4.3">
        <rdfs:subClassOf rdf:resource="https://savage.nps.edu/EthicalControl/ontologies/MissionExecutionOntology#DADM06.11.4"/>
        <rdfs:comment>Can the IAS detect, distinguish and designate (crewed) vessels and aircraft as friendly, neutral, or adversarial and calculate a confidence factor for each designation?</rdfs:comment>
        <rdfs:label>RE06.11.4.3_CanCalculateConfidenceFactorIFFPlatforms</rdfs:label>
        <owl:versionInfo>page 76</owl:versionInfo>
    </owl:Class>
    


    <!-- https://savage.nps.edu/EthicalControl/ontologies/MissionExecutionOntology#RE06.11.4.4 -->

    <owl:Class rdf:about="https://savage.nps.edu/EthicalControl/ontologies/MissionExecutionOntology#RE06.11.4.4">
        <rdfs:subClassOf rdf:resource="https://savage.nps.edu/EthicalControl/ontologies/MissionExecutionOntology#DADM06.11.4"/>
        <rdfs:comment>Can the IAS distinguish between enemy combatants, friendly force personnel, and noncombatant individuals and calculate a confidence factor for each designation?</rdfs:comment>
        <rdfs:label>RE06.11.4.4_CanCalculateConfidenceFactorEnemyFriendlyNoncombatePeople</rdfs:label>
        <owl:versionInfo>page 76</owl:versionInfo>
    </owl:Class>
    


    <!-- https://savage.nps.edu/EthicalControl/ontologies/MissionExecutionOntology#RE06.12.1 -->

    <owl:Class rdf:about="https://savage.nps.edu/EthicalControl/ontologies/MissionExecutionOntology#RE06.12.1">
        <rdfs:subClassOf rdf:resource="https://savage.nps.edu/EthicalControl/ontologies/MissionExecutionOntology#DADM06.12"/>
        <rdfs:comment>Can the IAS detect, or access information regarding, the interdependencies that objects protected from the use of force have with other objects (that may or may not be protected from the use of force)?</rdfs:comment>
        <rdfs:label>RE06.12.1_CanLeverageProtectedObjectInterdependencies</rdfs:label>
        <owl:versionInfo>page 76</owl:versionInfo>
    </owl:Class>
    


    <!-- https://savage.nps.edu/EthicalControl/ontologies/MissionExecutionOntology#RE06.12.2 -->

    <owl:Class rdf:about="https://savage.nps.edu/EthicalControl/ontologies/MissionExecutionOntology#RE06.12.2">
        <rdfs:subClassOf rdf:resource="https://savage.nps.edu/EthicalControl/ontologies/MissionExecutionOntology#DADM06.12"/>
        <rdfs:comment>Can the IAS access an up-to-date and complete list of restricted targets and areas?</rdfs:comment>
        <rdfs:label>RE06.12.2_CanLeverageRestrictedTargetsLocations</rdfs:label>
        <owl:versionInfo>page 76</owl:versionInfo>
    </owl:Class>
    


    <!-- https://savage.nps.edu/EthicalControl/ontologies/MissionExecutionOntology#RE06.12.3 -->

    <owl:Class rdf:about="https://savage.nps.edu/EthicalControl/ontologies/MissionExecutionOntology#RE06.12.3">
        <rdfs:subClassOf rdf:resource="https://savage.nps.edu/EthicalControl/ontologies/MissionExecutionOntology#DADM06.12"/>
        <rdfs:comment>Can the IAS identify and not intentionally harm (in a manner that would violate laws, policies, or the rules of engagement) objects whose destruction might damage relations with local noncombatant populations?</rdfs:comment>
        <rdfs:label>RE06.12.3_CanLeverageAdverseDestructionObjectsList</rdfs:label>
        <owl:versionInfo>page 76</owl:versionInfo>
    </owl:Class>
    


    <!-- https://savage.nps.edu/EthicalControl/ontologies/MissionExecutionOntology#RE06.12.4 -->

    <owl:Class rdf:about="https://savage.nps.edu/EthicalControl/ontologies/MissionExecutionOntology#RE06.12.4">
        <rdfs:subClassOf rdf:resource="https://savage.nps.edu/EthicalControl/ontologies/MissionExecutionOntology#DADM06.12"/>
        <rdfs:comment>Can the IAS identify and not intentionally harm (in a manner that would violate laws, policies, or the rules of engagement) objects whose destruction might provide propaganda value to enemy forces?</rdfs:comment>
        <rdfs:label>RE06.12.4_CanLeverageAdverseDestructionPropagandaList</rdfs:label>
        <owl:versionInfo>page 76</owl:versionInfo>
    </owl:Class>
    


    <!-- https://savage.nps.edu/EthicalControl/ontologies/MissionExecutionOntology#RE06.12.5 -->

    <owl:Class rdf:about="https://savage.nps.edu/EthicalControl/ontologies/MissionExecutionOntology#RE06.12.5">
        <rdfs:subClassOf rdf:resource="https://savage.nps.edu/EthicalControl/ontologies/MissionExecutionOntology#DADM06.12"/>
        <rdfs:comment>Can the IAS provide information regarding objects protected from the use of force that will assist a human operator in making use of force decisions?</rdfs:comment>
        <rdfs:label>RE06.12.5_CanDisseminateIdentifiedProtectedObjects</rdfs:label>
        <owl:versionInfo>page 76</owl:versionInfo>
    </owl:Class>
    


    <!-- https://savage.nps.edu/EthicalControl/ontologies/MissionExecutionOntology#RE06.13.1 -->

    <owl:Class rdf:about="https://savage.nps.edu/EthicalControl/ontologies/MissionExecutionOntology#RE06.13.1">
        <rdfs:subClassOf rdf:resource="https://savage.nps.edu/EthicalControl/ontologies/MissionExecutionOntology#DADM06.13"/>
        <rdfs:comment>Can the IAS determine when enemy combatants have entered into an area or structure that is protected from the use of force?</rdfs:comment>
        <rdfs:label>RE06.13.1_SafeListLocations</rdfs:label>
        <owl:versionInfo>page 76</owl:versionInfo>
    </owl:Class>
    


    <!-- https://savage.nps.edu/EthicalControl/ontologies/MissionExecutionOntology#RE06.13.2 -->

    <owl:Class rdf:about="https://savage.nps.edu/EthicalControl/ontologies/MissionExecutionOntology#RE06.13.2">
        <rdfs:subClassOf rdf:resource="https://savage.nps.edu/EthicalControl/ontologies/MissionExecutionOntology#DADM06.13"/>
        <rdfs:comment>Can the IAS use signatures to distinguish military from civilian objects that are unique to either the military object only or the civilian object only?</rdfs:comment>
        <rdfs:label>RE06.13.2_SafelistObjects</rdfs:label>
        <owl:versionInfo>page 76</owl:versionInfo>
    </owl:Class>
    


    <!-- https://savage.nps.edu/EthicalControl/ontologies/MissionExecutionOntology#RE06.13.3 -->

    <owl:Class rdf:about="https://savage.nps.edu/EthicalControl/ontologies/MissionExecutionOntology#RE06.13.3">
        <rdfs:subClassOf rdf:resource="https://savage.nps.edu/EthicalControl/ontologies/MissionExecutionOntology#DADM06.13"/>
        <rdfs:comment>Can the IAS account for unknown transient civilian or noncombatant personnel and/or equipment near a targetable military object?</rdfs:comment>
        <rdfs:label>RE06.13.3_SafelistPeople</rdfs:label>
        <owl:versionInfo>page 76</owl:versionInfo>
    </owl:Class>
    


    <!-- https://savage.nps.edu/EthicalControl/ontologies/MissionExecutionOntology#RE06.14.1 -->

    <owl:Class rdf:about="https://savage.nps.edu/EthicalControl/ontologies/MissionExecutionOntology#RE06.14.1">
        <rdfs:subClassOf rdf:resource="https://savage.nps.edu/EthicalControl/ontologies/MissionExecutionOntology#DADM06.14"/>
        <rdfs:comment>Can the IAS detect a &quot;mission kill,&quot; where an object has been damaged but not destroyed, to the point that it no longer has military utility and cease further use of force?</rdfs:comment>
        <rdfs:label>RE06.14.1_DetectObjectsFunctionalLoss</rdfs:label>
        <owl:versionInfo>page 76</owl:versionInfo>
    </owl:Class>
    


    <!-- https://savage.nps.edu/EthicalControl/ontologies/MissionExecutionOntology#RE06.15.1 -->

    <owl:Class rdf:about="https://savage.nps.edu/EthicalControl/ontologies/MissionExecutionOntology#RE06.15.1">
        <rdfs:subClassOf rdf:resource="https://savage.nps.edu/EthicalControl/ontologies/MissionExecutionOntology#DADM06.15"/>
        <rdfs:comment>Can the IAS prohibit engagements that would cause widespread, long-term, and/or severe impact to the health of general population (such as the destruction of a power plant that services a hospital or a refugee camp)?</rdfs:comment>
        <rdfs:label>RE06.15.1_TargetingLongtermHealth</rdfs:label>
        <owl:versionInfo>page 77</owl:versionInfo>
    </owl:Class>
    


    <!-- https://savage.nps.edu/EthicalControl/ontologies/MissionExecutionOntology#RE06.16.1 -->

    <owl:Class rdf:about="https://savage.nps.edu/EthicalControl/ontologies/MissionExecutionOntology#RE06.16.1">
        <rdfs:subClassOf rdf:resource="https://savage.nps.edu/EthicalControl/ontologies/MissionExecutionOntology#DADM06.16"/>
        <rdfs:comment>Can the IAS detect perfidious use of objects protected from the use of force (such as using an ambulance for military transport)?</rdfs:comment>
        <rdfs:label>RE06.16.1_ObjectIllIntent</rdfs:label>
        <owl:versionInfo>page 77</owl:versionInfo>
    </owl:Class>
    


    <!-- https://savage.nps.edu/EthicalControl/ontologies/MissionExecutionOntology#RE06.16.2 -->

    <owl:Class rdf:about="https://savage.nps.edu/EthicalControl/ontologies/MissionExecutionOntology#RE06.16.2">
        <rdfs:subClassOf rdf:resource="https://savage.nps.edu/EthicalControl/ontologies/MissionExecutionOntology#DADM06.16"/>
        <rdfs:comment>Can the IAS detect perfidious use of facilities protected from the use of force (such as using a house of worship as a sniper position?</rdfs:comment>
        <rdfs:label>RE06.16.2_LocationIllIntent</rdfs:label>
        <owl:versionInfo>page 77</owl:versionInfo>
    </owl:Class>
    


    <!-- https://savage.nps.edu/EthicalControl/ontologies/MissionExecutionOntology#RE06.17.1 -->

    <owl:Class rdf:about="https://savage.nps.edu/EthicalControl/ontologies/MissionExecutionOntology#RE06.17.1">
        <rdfs:subClassOf rdf:resource="https://savage.nps.edu/EthicalControl/ontologies/MissionExecutionOntology#DADM06.17"/>
        <rdfs:comment>Can the IAS identify and not intentionally harm (in a manner that would violate laws, policies, or the rules of engagement) diplomatic offices, foreign missions, and the sovereign nonmilitary properties of other nations?</rdfs:comment>
        <rdfs:label>RE06.17.1_SafeObjectsSovereignLocations</rdfs:label>
        <owl:versionInfo>page 77</owl:versionInfo>
    </owl:Class>
    


    <!-- https://savage.nps.edu/EthicalControl/ontologies/MissionExecutionOntology#RE06.17.10 -->

    <owl:Class rdf:about="https://savage.nps.edu/EthicalControl/ontologies/MissionExecutionOntology#RE06.17.10">
        <rdfs:subClassOf rdf:resource="https://savage.nps.edu/EthicalControl/ontologies/MissionExecutionOntology#DADM06.17"/>
        <rdfs:comment>Can the IAS identify and not intentionally harm (in a manner that would violate laws, policies, or the rules of engagement) prisoner of war camps and government detention facilities/prisons?</rdfs:comment>
        <rdfs:label>RE06.17.10_SafeObjectsPOWDetentionLocations</rdfs:label>
        <owl:versionInfo>page 78</owl:versionInfo>
    </owl:Class>
    


    <!-- https://savage.nps.edu/EthicalControl/ontologies/MissionExecutionOntology#RE06.17.11 -->

    <owl:Class rdf:about="https://savage.nps.edu/EthicalControl/ontologies/MissionExecutionOntology#RE06.17.11">
        <rdfs:subClassOf rdf:resource="https://savage.nps.edu/EthicalControl/ontologies/MissionExecutionOntology#DADM06.17"/>
        <rdfs:comment>Can the IAS identify and not intentionally initiate (in a manner that would violate laws, policies, or the rules of engagement) engagements that may result in pollution or have potential to release toxic chemicals?</rdfs:comment>
        <rdfs:label>RE06.17.11_SafeObjectsPreventsToxicRelease</rdfs:label>
        <owl:versionInfo>page 78</owl:versionInfo>
    </owl:Class>
    


    <!-- https://savage.nps.edu/EthicalControl/ontologies/MissionExecutionOntology#RE06.17.12 -->

    <owl:Class rdf:about="https://savage.nps.edu/EthicalControl/ontologies/MissionExecutionOntology#RE06.17.12">
        <rdfs:subClassOf rdf:resource="https://savage.nps.edu/EthicalControl/ontologies/MissionExecutionOntology#DADM06.17"/>
        <rdfs:comment>Can the IAS identify and not intentionally harm (in a manner that would violate laws, policies, or the rules of engagement) dams or dikes whose engagement may result in flooding of civilian areas?</rdfs:comment>
        <rdfs:label>RE06.17.12_SafeObjectsPreventsFloodingCivilians</rdfs:label>
        <owl:versionInfo>page 78</owl:versionInfo>
    </owl:Class>
    


    <!-- https://savage.nps.edu/EthicalControl/ontologies/MissionExecutionOntology#RE06.17.13 -->

    <owl:Class rdf:about="https://savage.nps.edu/EthicalControl/ontologies/MissionExecutionOntology#RE06.17.13">
        <rdfs:subClassOf rdf:resource="https://savage.nps.edu/EthicalControl/ontologies/MissionExecutionOntology#DADM06.17"/>
        <rdfs:comment>Can the IAS identify and not intentionally harm (in a manner that would violate laws, policies, or the rules of engagement) facilities whose engagement may threaten astronauts and/or manned space flight missions?</rdfs:comment>
        <rdfs:label>RE06.17.13_SafeObjectsSpace</rdfs:label>
        <owl:versionInfo>page 78</owl:versionInfo>
    </owl:Class>
    


    <!-- https://savage.nps.edu/EthicalControl/ontologies/MissionExecutionOntology#RE06.17.14 -->

    <owl:Class rdf:about="https://savage.nps.edu/EthicalControl/ontologies/MissionExecutionOntology#RE06.17.14">
        <rdfs:subClassOf rdf:resource="https://savage.nps.edu/EthicalControl/ontologies/MissionExecutionOntology#DADM06.17"/>
        <rdfs:comment>Can the IAS identify and not intentionally harm (in a manner that would violate laws, policies, or the rules of engagement) civilian meeting places?</rdfs:comment>
        <rdfs:label>RE06.17.14_SafeObjectsCivilianMeetingPlaces</rdfs:label>
        <owl:versionInfo>page 78</owl:versionInfo>
    </owl:Class>
    


    <!-- https://savage.nps.edu/EthicalControl/ontologies/MissionExecutionOntology#RE06.17.15 -->

    <owl:Class rdf:about="https://savage.nps.edu/EthicalControl/ontologies/MissionExecutionOntology#RE06.17.15">
        <rdfs:subClassOf rdf:resource="https://savage.nps.edu/EthicalControl/ontologies/MissionExecutionOntology#DADM06.17"/>
        <rdfs:comment>Can the IAS identify and not intentionally harm (in a manner that would violate laws, policies, or the rules of engagement) public utilities and facilities?</rdfs:comment>
        <rdfs:label>RE06.17.15_SafeObjectsPublicUtilitiesFacilities</rdfs:label>
        <owl:versionInfo>page 78</owl:versionInfo>
    </owl:Class>
    


    <!-- https://savage.nps.edu/EthicalControl/ontologies/MissionExecutionOntology#RE06.17.16 -->

    <owl:Class rdf:about="https://savage.nps.edu/EthicalControl/ontologies/MissionExecutionOntology#RE06.17.16">
        <rdfs:subClassOf rdf:resource="https://savage.nps.edu/EthicalControl/ontologies/MissionExecutionOntology#DADM06.17"/>
        <rdfs:comment>Can the IAS identify and not intentionally harm (in a manner that would violate laws, policies, or the rules of engagement) facilities and/or structures with unknown functionality/purpose?</rdfs:comment>
        <rdfs:label>RE06.17.16_SafeObjectsUnknown</rdfs:label>
        <owl:versionInfo>page 78</owl:versionInfo>
    </owl:Class>
    


    <!-- https://savage.nps.edu/EthicalControl/ontologies/MissionExecutionOntology#RE06.17.17 -->

    <owl:Class rdf:about="https://savage.nps.edu/EthicalControl/ontologies/MissionExecutionOntology#RE06.17.17">
        <rdfs:subClassOf rdf:resource="https://savage.nps.edu/EthicalControl/ontologies/MissionExecutionOntology#DADM06.17"/>
        <rdfs:comment>Can the IAS identify and not intentionally harm (in a manner that would violate laws, policies, or the rules of engagement) agricultural processing and storage facilities?</rdfs:comment>
        <rdfs:label>RE06.17.17_SafeAgriculturalObjects</rdfs:label>
        <owl:versionInfo>page 78</owl:versionInfo>
    </owl:Class>
    


    <!-- https://savage.nps.edu/EthicalControl/ontologies/MissionExecutionOntology#RE06.17.18 -->

    <owl:Class rdf:about="https://savage.nps.edu/EthicalControl/ontologies/MissionExecutionOntology#RE06.17.18">
        <rdfs:subClassOf rdf:resource="https://savage.nps.edu/EthicalControl/ontologies/MissionExecutionOntology#DADM06.17"/>
        <rdfs:comment>Can the IAS identify and not intentionally harm (in a manner that would violate laws, policies, or the rules of engagement) facilities that provide products or services for both civilian and military use?</rdfs:comment>
        <rdfs:label>RE06.17.18_SafObjectsDualUse</rdfs:label>
        <owl:versionInfo>page 78</owl:versionInfo>
    </owl:Class>
    


    <!-- https://savage.nps.edu/EthicalControl/ontologies/MissionExecutionOntology#RE06.17.2 -->

    <owl:Class rdf:about="https://savage.nps.edu/EthicalControl/ontologies/MissionExecutionOntology#RE06.17.2">
        <rdfs:subClassOf rdf:resource="https://savage.nps.edu/EthicalControl/ontologies/MissionExecutionOntology#DADM06.17"/>
        <rdfs:comment>Can the IAS identify and not intentionally harm (in a manner that would violate laws, policies, or the rules of engagement) religious, cultural, historical institutions, cemeteries, and structures?</rdfs:comment>
        <rdfs:label>RE06.17.2_SafeObjectsSpecialLocations</rdfs:label>
        <owl:versionInfo>page 77</owl:versionInfo>
    </owl:Class>
    


    <!-- https://savage.nps.edu/EthicalControl/ontologies/MissionExecutionOntology#RE06.17.3 -->

    <owl:Class rdf:about="https://savage.nps.edu/EthicalControl/ontologies/MissionExecutionOntology#RE06.17.3">
        <rdfs:subClassOf rdf:resource="https://savage.nps.edu/EthicalControl/ontologies/MissionExecutionOntology#DADM06.17"/>
        <rdfs:comment>Can the IAS identify and not intentionally harm (in a manner that would violate laws, policies, or the rules of engagement) fixed medical facilities?</rdfs:comment>
        <rdfs:label>RE06.17.3_SafeObjectsMixedMedical</rdfs:label>
        <owl:versionInfo>page 77</owl:versionInfo>
    </owl:Class>
    


    <!-- https://savage.nps.edu/EthicalControl/ontologies/MissionExecutionOntology#RE06.17.4 -->

    <owl:Class rdf:about="https://savage.nps.edu/EthicalControl/ontologies/MissionExecutionOntology#RE06.17.4">
        <rdfs:subClassOf rdf:resource="https://savage.nps.edu/EthicalControl/ontologies/MissionExecutionOntology#DADM06.17"/>
        <rdfs:comment>Can the IAS identify and not intentionally harm (in a manner that would violate laws, policies, or the rules of engagement) mobile medical facilities?</rdfs:comment>
        <rdfs:label>RE06.17.4_SafeObjectsMobileMedical</rdfs:label>
        <owl:versionInfo>page 77</owl:versionInfo>
    </owl:Class>
    


    <!-- https://savage.nps.edu/EthicalControl/ontologies/MissionExecutionOntology#RE06.17.5 -->

    <owl:Class rdf:about="https://savage.nps.edu/EthicalControl/ontologies/MissionExecutionOntology#RE06.17.5">
        <rdfs:subClassOf rdf:resource="https://savage.nps.edu/EthicalControl/ontologies/MissionExecutionOntology#DADM06.17"/>
        <rdfs:comment>Can the IAS identify and not intentionally harm (in a manner that would violate laws, policies, or the rules of engagement) ambulances and clearly marked medical ground transport vehicles?</rdfs:comment>
        <rdfs:label>RE06.17.5_SafeObjectsMedicalGroundTransport</rdfs:label>
        <owl:versionInfo>page 77</owl:versionInfo>
    </owl:Class>
    


    <!-- https://savage.nps.edu/EthicalControl/ontologies/MissionExecutionOntology#RE06.17.6 -->

    <owl:Class rdf:about="https://savage.nps.edu/EthicalControl/ontologies/MissionExecutionOntology#RE06.17.6">
        <rdfs:subClassOf rdf:resource="https://savage.nps.edu/EthicalControl/ontologies/MissionExecutionOntology#DADM06.17"/>
        <rdfs:comment>Can the IAS identify and not intentionally harm (in a manner that would violate laws, policies, or the rules of engagement) air ambulances and clearly marked medical aircraft?</rdfs:comment>
        <rdfs:label>RE06.17.6_SafeObjectsMedicalAircraft</rdfs:label>
        <owl:versionInfo>page 77</owl:versionInfo>
    </owl:Class>
    


    <!-- https://savage.nps.edu/EthicalControl/ontologies/MissionExecutionOntology#RE06.17.7 -->

    <owl:Class rdf:about="https://savage.nps.edu/EthicalControl/ontologies/MissionExecutionOntology#RE06.17.7">
        <rdfs:subClassOf rdf:resource="https://savage.nps.edu/EthicalControl/ontologies/MissionExecutionOntology#DADM06.17"/>
        <rdfs:comment>Can the IAS identify and not intentionally harm (in a manner that would violate laws, policies, or the rules of engagement) hospital ships?</rdfs:comment>
        <rdfs:label>RE06.17.7_SafeObjectsHospitalShips</rdfs:label>
        <owl:versionInfo>page 77</owl:versionInfo>
    </owl:Class>
    


    <!-- https://savage.nps.edu/EthicalControl/ontologies/MissionExecutionOntology#RE06.17.8 -->

    <owl:Class rdf:about="https://savage.nps.edu/EthicalControl/ontologies/MissionExecutionOntology#RE06.17.8">
        <rdfs:subClassOf rdf:resource="https://savage.nps.edu/EthicalControl/ontologies/MissionExecutionOntology#DADM06.17"/>
        <rdfs:comment>Can the IAS identify and not intentionally harm (in a manner that would violate laws, policies, or the rules of engagement) public education facilities?</rdfs:comment>
        <rdfs:label>RE06.17.8_SafeObjectsPublicEducationLocations</rdfs:label>
        <owl:versionInfo>page 77</owl:versionInfo>
    </owl:Class>
    


    <!-- https://savage.nps.edu/EthicalControl/ontologies/MissionExecutionOntology#RE06.17.9 -->

    <owl:Class rdf:about="https://savage.nps.edu/EthicalControl/ontologies/MissionExecutionOntology#RE06.17.9">
        <rdfs:subClassOf rdf:resource="https://savage.nps.edu/EthicalControl/ontologies/MissionExecutionOntology#DADM06.17"/>
        <rdfs:comment>Can the IAS identify and not intentionally harm (in a manner that would violate laws, policies, or the rules of engagement) civilian refugee camps?</rdfs:comment>
        <rdfs:label>RE06.17.9_SafeObjectsRefugeeLocations</rdfs:label>
        <owl:versionInfo>page 77</owl:versionInfo>
    </owl:Class>
    


    <!-- https://savage.nps.edu/EthicalControl/ontologies/MissionExecutionOntology#RE06.2.1 -->

    <owl:Class rdf:about="https://savage.nps.edu/EthicalControl/ontologies/MissionExecutionOntology#RE06.2.1">
        <rdfs:subClassOf rdf:resource="https://savage.nps.edu/EthicalControl/ontologies/MissionExecutionOntology#DADM06.2"/>
        <rdfs:comment>Can the IAS recognize symbols that designate persons and objects protected from the use of force, such as a Red Cross or Red Crescent?</rdfs:comment>
        <rdfs:label>RE06.2.1_CanRecognizeSafeSymbols</rdfs:label>
        <owl:versionInfo>page 71</owl:versionInfo>
    </owl:Class>
    


    <!-- https://savage.nps.edu/EthicalControl/ontologies/MissionExecutionOntology#RE06.3.1 -->

    <owl:Class rdf:about="https://savage.nps.edu/EthicalControl/ontologies/MissionExecutionOntology#RE06.3.1">
        <rdfs:subClassOf rdf:resource="https://savage.nps.edu/EthicalControl/ontologies/MissionExecutionOntology#DADM06.3"/>
        <rdfs:comment>Can the IAS estimate potential collateral damage and conduct collateral damage assessments before going forth with force decisions (from either the IAS or a human operator)?</rdfs:comment>
        <rdfs:label>RE06.3.1_CanPredictDamage</rdfs:label>
        <owl:versionInfo>page 72</owl:versionInfo>
    </owl:Class>
    


    <!-- https://savage.nps.edu/EthicalControl/ontologies/MissionExecutionOntology#RE06.3.10 -->

    <owl:Class rdf:about="https://savage.nps.edu/EthicalControl/ontologies/MissionExecutionOntology#RE06.3.10">
        <rdfs:subClassOf rdf:resource="https://savage.nps.edu/EthicalControl/ontologies/MissionExecutionOntology#DADM06.3"/>
        <rdfs:comment>Can the IAS ingest and utilize collateral effects analysis results prepared by the commander’s staff?</rdfs:comment>
        <rdfs:label>RE06.3.10_CanUpdateCollateralEffectModels</rdfs:label>
        <owl:versionInfo>page 72</owl:versionInfo>
    </owl:Class>
    


    <!-- https://savage.nps.edu/EthicalControl/ontologies/MissionExecutionOntology#RE06.3.11 -->

    <owl:Class rdf:about="https://savage.nps.edu/EthicalControl/ontologies/MissionExecutionOntology#RE06.3.11">
        <rdfs:subClassOf rdf:resource="https://savage.nps.edu/EthicalControl/ontologies/MissionExecutionOntology#DADM06.3"/>
        <rdfs:comment>Can the IAS identify any temporal, spatial or technical limits on the accuracy of its collateral damage estimates and convey those to the operator/commander?</rdfs:comment>
        <rdfs:label>RE06.3.11_CanDisseminateCollateralDamageAccuracyUpdates</rdfs:label>
        <owl:versionInfo>page 72</owl:versionInfo>
    </owl:Class>
    


    <!-- https://savage.nps.edu/EthicalControl/ontologies/MissionExecutionOntology#RE06.3.12 -->

    <owl:Class rdf:about="https://savage.nps.edu/EthicalControl/ontologies/MissionExecutionOntology#RE06.3.12">
        <rdfs:subClassOf rdf:resource="https://savage.nps.edu/EthicalControl/ontologies/MissionExecutionOntology#DADM06.3"/>
        <rdfs:comment>Can the IAS determine when its actions might pose a collateral damage hazard to persons or objects protected from the use of force, cease the potentially hazardous action, and communicate its inability to take this action to the commander?</rdfs:comment>
        <rdfs:label>RE06.3.12_CanIdentifyUnacceptableCollageralDamageRisk</rdfs:label>
        <owl:versionInfo>page 72</owl:versionInfo>
    </owl:Class>
    


    <!-- https://savage.nps.edu/EthicalControl/ontologies/MissionExecutionOntology#RE06.3.13 -->

    <owl:Class rdf:about="https://savage.nps.edu/EthicalControl/ontologies/MissionExecutionOntology#RE06.3.13">
        <rdfs:subClassOf rdf:resource="https://savage.nps.edu/EthicalControl/ontologies/MissionExecutionOntology#DADM06.3"/>
        <rdfs:comment>Can the IAS seek approval to use a larger or less precise munition if its supply of smaller and/or more precise munitions is exhausted?</rdfs:comment>
        <rdfs:label>RE06.3.13_CanRequestAvailableMunition</rdfs:label>
        <owl:versionInfo>page 72</owl:versionInfo>
    </owl:Class>
    


    <!-- https://savage.nps.edu/EthicalControl/ontologies/MissionExecutionOntology#RE06.3.2 -->

    <owl:Class rdf:about="https://savage.nps.edu/EthicalControl/ontologies/MissionExecutionOntology#RE06.3.2">
        <rdfs:subClassOf rdf:resource="https://savage.nps.edu/EthicalControl/ontologies/MissionExecutionOntology#DADM06.3"/>
        <rdfs:comment>Can the IAS conduct collateral damage assessments and compare them to the commander’s proportionality assessment for consistency?</rdfs:comment>
        <rdfs:label>RE06.3.2_CanDifferencePredictedDamage</rdfs:label>
        <owl:versionInfo>page 72</owl:versionInfo>
    </owl:Class>
    


    <!-- https://savage.nps.edu/EthicalControl/ontologies/MissionExecutionOntology#RE06.3.3 -->

    <owl:Class rdf:about="https://savage.nps.edu/EthicalControl/ontologies/MissionExecutionOntology#RE06.3.3">
        <rdfs:subClassOf rdf:resource="https://savage.nps.edu/EthicalControl/ontologies/MissionExecutionOntology#DADM06.3"/>
        <rdfs:comment>Can the IAS provide commanders and operators with the information needed to assess proportionality when the IAS cannot do so without human assistance?</rdfs:comment>
        <rdfs:label>RE06.3.3_CanDisseminatePredictedDamage</rdfs:label>
        <owl:versionInfo>page 72</owl:versionInfo>
    </owl:Class>
    


    <!-- https://savage.nps.edu/EthicalControl/ontologies/MissionExecutionOntology#RE06.3.4 -->

    <owl:Class rdf:about="https://savage.nps.edu/EthicalControl/ontologies/MissionExecutionOntology#RE06.3.4">
        <rdfs:subClassOf rdf:resource="https://savage.nps.edu/EthicalControl/ontologies/MissionExecutionOntology#DADM06.3"/>
        <rdfs:comment>Can the IAS obtain, analyze and use information on the effects radii and patterns of munitions to determine if persons or objects protected from the use of force (to include friendly combatants) are within those radii and patterns?</rdfs:comment>
        <rdfs:label>RE06.3.4_CanPredictMunitionDamagePattern</rdfs:label>
        <owl:versionInfo>page 72</owl:versionInfo>
    </owl:Class>
    


    <!-- https://savage.nps.edu/EthicalControl/ontologies/MissionExecutionOntology#RE06.3.5 -->

    <owl:Class rdf:about="https://savage.nps.edu/EthicalControl/ontologies/MissionExecutionOntology#RE06.3.5">
        <rdfs:subClassOf rdf:resource="https://savage.nps.edu/EthicalControl/ontologies/MissionExecutionOntology#DADM06.3"/>
        <rdfs:comment>Can the IAS access the most up-to-date assessments of collateral effects radius assessments prepared by the commander’s staff?</rdfs:comment>
        <rdfs:label>RE06.3.5_CanAcceptCollateralEffectsLimitUpdates</rdfs:label>
        <owl:versionInfo>page 72</owl:versionInfo>
    </owl:Class>
    


    <!-- https://savage.nps.edu/EthicalControl/ontologies/MissionExecutionOntology#RE06.3.6 -->

    <owl:Class rdf:about="https://savage.nps.edu/EthicalControl/ontologies/MissionExecutionOntology#RE06.3.6">
        <rdfs:subClassOf rdf:resource="https://savage.nps.edu/EthicalControl/ontologies/MissionExecutionOntology#DADM06.3"/>
        <rdfs:comment>Can the IAS obtain, analyze and use information on the potential for secondary explosions before delivering a munition?</rdfs:comment>
        <rdfs:label>RE06.3.6_CanPredictSecondaryDamage</rdfs:label>
        <owl:versionInfo>page 72</owl:versionInfo>
    </owl:Class>
    


    <!-- https://savage.nps.edu/EthicalControl/ontologies/MissionExecutionOntology#RE06.3.7 -->

    <owl:Class rdf:about="https://savage.nps.edu/EthicalControl/ontologies/MissionExecutionOntology#RE06.3.7">
        <rdfs:subClassOf rdf:resource="https://savage.nps.edu/EthicalControl/ontologies/MissionExecutionOntology#DADM06.3"/>
        <rdfs:comment>Can the IAS distinguish between actions that cause repairable/reversible harm and actions that cause irreparable/irreversible harm?</rdfs:comment>
        <rdfs:label>RE06.3.7_DamageModelRepairFidelity</rdfs:label>
        <owl:versionInfo>page 72</owl:versionInfo>
    </owl:Class>
    


    <!-- https://savage.nps.edu/EthicalControl/ontologies/MissionExecutionOntology#RE06.3.8 -->

    <owl:Class rdf:about="https://savage.nps.edu/EthicalControl/ontologies/MissionExecutionOntology#RE06.3.8">
        <rdfs:subClassOf rdf:resource="https://savage.nps.edu/EthicalControl/ontologies/MissionExecutionOntology#DADM06.3"/>
        <rdfs:comment>Can the IAS assist the proportionality assessment summary by tracking assessments and the confidence levels thereof?</rdfs:comment>
        <rdfs:label>RE06.3.8_CanUpdateDamageAssessments</rdfs:label>
        <owl:versionInfo>page 72</owl:versionInfo>
    </owl:Class>
    


    <!-- https://savage.nps.edu/EthicalControl/ontologies/MissionExecutionOntology#RE06.3.9 -->

    <owl:Class rdf:about="https://savage.nps.edu/EthicalControl/ontologies/MissionExecutionOntology#RE06.3.9">
        <rdfs:subClassOf rdf:resource="https://savage.nps.edu/EthicalControl/ontologies/MissionExecutionOntology#DADM06.3"/>
        <rdfs:comment>Can the IAS incorporate outcomes of previous operations that resulted in unacceptable collateral damage to prevent a recurrence?</rdfs:comment>
        <rdfs:label>RE06.3.9_CanUpdateDamageModels</rdfs:label>
        <owl:versionInfo>page 72</owl:versionInfo>
    </owl:Class>
    


    <!-- https://savage.nps.edu/EthicalControl/ontologies/MissionExecutionOntology#RE06.4.1 -->

    <owl:Class rdf:about="https://savage.nps.edu/EthicalControl/ontologies/MissionExecutionOntology#RE06.4.1">
        <rdfs:subClassOf rdf:resource="https://savage.nps.edu/EthicalControl/ontologies/MissionExecutionOntology#DADM06.4"/>
        <rdfs:comment>Can the IAS analyze the military necessity and appropriateness of an attack?</rdfs:comment>
        <rdfs:label>RE06.4.1_CanSwitchMilitaryNecessityMode</rdfs:label>
        <owl:versionInfo>page 72</owl:versionInfo>
    </owl:Class>
    


    <!-- https://savage.nps.edu/EthicalControl/ontologies/MissionExecutionOntology#RE06.4.2 -->

    <owl:Class rdf:about="https://savage.nps.edu/EthicalControl/ontologies/MissionExecutionOntology#RE06.4.2">
        <rdfs:subClassOf rdf:resource="https://savage.nps.edu/EthicalControl/ontologies/MissionExecutionOntology#DADM06.4"/>
        <rdfs:comment>Can the IAS assess the contribution that destruction of a target would make toward achieving a legitimate military objective?</rdfs:comment>
        <rdfs:label>RE06.4.2_CanMeasureTargetsDestructionContribution</rdfs:label>
        <owl:versionInfo>page 72</owl:versionInfo>
    </owl:Class>
    


    <!-- https://savage.nps.edu/EthicalControl/ontologies/MissionExecutionOntology#RE06.4.3 -->

    <owl:Class rdf:about="https://savage.nps.edu/EthicalControl/ontologies/MissionExecutionOntology#RE06.4.3">
        <rdfs:subClassOf rdf:resource="https://savage.nps.edu/EthicalControl/ontologies/MissionExecutionOntology#DADM06.4"/>
        <rdfs:comment>Can the IAS deconflict requirements to not intentionally harm persons or objects (in a manner that would violate laws, policies, or the rules of engagement) with its requirement to support achieving the military objective?</rdfs:comment>
        <rdfs:label>RE06.4.3_CanSupportMilitaryObjectives</rdfs:label>
        <owl:versionInfo>page 73</owl:versionInfo>
    </owl:Class>
    


    <!-- https://savage.nps.edu/EthicalControl/ontologies/MissionExecutionOntology#RE06.4.4 -->

    <owl:Class rdf:about="https://savage.nps.edu/EthicalControl/ontologies/MissionExecutionOntology#RE06.4.4">
        <rdfs:subClassOf rdf:resource="https://savage.nps.edu/EthicalControl/ontologies/MissionExecutionOntology#DADM06.4"/>
        <rdfs:comment>Can the IAS cancel or suspend an attack if it becomes apparent that the objective is not a military one?</rdfs:comment>
        <rdfs:label>RE06.4.4_CanAbortNonmilitaryObjective</rdfs:label>
        <owl:versionInfo>page 73</owl:versionInfo>
    </owl:Class>
    


    <!-- https://savage.nps.edu/EthicalControl/ontologies/MissionExecutionOntology#RE06.4.5 -->

    <owl:Class rdf:about="https://savage.nps.edu/EthicalControl/ontologies/MissionExecutionOntology#RE06.4.5">
        <rdfs:subClassOf rdf:resource="https://savage.nps.edu/EthicalControl/ontologies/MissionExecutionOntology#DADM06.4"/>
        <rdfs:comment>Can the IAS abort an attack if the target no longer has military value because some other target that it depends on for its military value has been destroyed?</rdfs:comment>
        <rdfs:label>RE06.4.5_CanAbortTargetsValueChange</rdfs:label>
        <owl:versionInfo>page 73</owl:versionInfo>
    </owl:Class>
    


    <!-- https://savage.nps.edu/EthicalControl/ontologies/MissionExecutionOntology#RE06.5.1 -->

    <owl:Class rdf:about="https://savage.nps.edu/EthicalControl/ontologies/MissionExecutionOntology#RE06.5.1">
        <rdfs:subClassOf rdf:resource="https://savage.nps.edu/EthicalControl/ontologies/MissionExecutionOntology#DADM06.5"/>
        <rdfs:comment>Can the IAS reduce or disable any prompts that would activate the use of force when it is operating in, or transiting through, an uncontested area?</rdfs:comment>
        <rdfs:label>RE06.5.1_CanWeaponsSafeLocations</rdfs:label>
        <owl:versionInfo>page 73</owl:versionInfo>
    </owl:Class>
    


    <!-- https://savage.nps.edu/EthicalControl/ontologies/MissionExecutionOntology#RE06.5.2 -->

    <owl:Class rdf:about="https://savage.nps.edu/EthicalControl/ontologies/MissionExecutionOntology#RE06.5.2">
        <rdfs:subClassOf rdf:resource="https://savage.nps.edu/EthicalControl/ontologies/MissionExecutionOntology#DADM06.5"/>
        <rdfs:comment>Can the IAS determine when the thresholds to authorize the use force by a human commander or operator have lowered over time, due to a growing indifference to taking human life or creating damage?</rdfs:comment>
        <rdfs:label>RE06.5.2_CanIASAcceptWeaponsFree</rdfs:label>
        <owl:versionInfo>page 73</owl:versionInfo>
    </owl:Class>
    


    <!-- https://savage.nps.edu/EthicalControl/ontologies/MissionExecutionOntology#RE06.5.3 -->

    <owl:Class rdf:about="https://savage.nps.edu/EthicalControl/ontologies/MissionExecutionOntology#RE06.5.3">
        <rdfs:subClassOf rdf:resource="https://savage.nps.edu/EthicalControl/ontologies/MissionExecutionOntology#DADM06.5"/>
        <rdfs:comment>Will repeated employment of the IAS as a LAWS numb the human operator or commander to the taking of human life?</rdfs:comment>
        <rdfs:label>RE06.5.3_WillMilitaryPersonBecomeNumb</rdfs:label>
        <owl:versionInfo>page 73</owl:versionInfo>
    </owl:Class>
    


    <!-- https://savage.nps.edu/EthicalControl/ontologies/MissionExecutionOntology#RE06.6.1 -->

    <owl:Class rdf:about="https://savage.nps.edu/EthicalControl/ontologies/MissionExecutionOntology#RE06.6.1">
        <rdfs:subClassOf rdf:resource="https://savage.nps.edu/EthicalControl/ontologies/MissionExecutionOntology#DADM06.6"/>
        <rdfs:comment>Can the IAS determine who receives medical attention?</rdfs:comment>
        <rdfs:label>RE06.6.1_CanDirectMedicalTasking</rdfs:label>
        <owl:versionInfo>page 73</owl:versionInfo>
    </owl:Class>
    


    <!-- https://savage.nps.edu/EthicalControl/ontologies/MissionExecutionOntology#RE06.6.2 -->

    <owl:Class rdf:about="https://savage.nps.edu/EthicalControl/ontologies/MissionExecutionOntology#RE06.6.2">
        <rdfs:subClassOf rdf:resource="https://savage.nps.edu/EthicalControl/ontologies/MissionExecutionOntology#DADM06.6"/>
        <rdfs:comment>Can the IAS make humans present in the operational environment aware of any hazards caused by interacting with it?</rdfs:comment>
        <rdfs:label>RE06.6.2_CanWarnHumansInteractionHazards</rdfs:label>
        <owl:versionInfo>page 73</owl:versionInfo>
    </owl:Class>
    


    <!-- https://savage.nps.edu/EthicalControl/ontologies/MissionExecutionOntology#RE06.7.1 -->

    <owl:Class rdf:about="https://savage.nps.edu/EthicalControl/ontologies/MissionExecutionOntology#RE06.7.1">
        <rdfs:subClassOf rdf:resource="https://savage.nps.edu/EthicalControl/ontologies/MissionExecutionOntology#DADM06.7"/>
        <rdfs:comment>Can the IAS distinguish between enemy combatants, friendly combatants, neutral combatants, and noncombatants?</rdfs:comment>
        <rdfs:label>RE06.7.1_CanDistinguishCurrentHumanCombatantStatus</rdfs:label>
        <owl:versionInfo>page 73</owl:versionInfo>
    </owl:Class>
    


    <!-- https://savage.nps.edu/EthicalControl/ontologies/MissionExecutionOntology#RE06.7.10 -->

    <owl:Class rdf:about="https://savage.nps.edu/EthicalControl/ontologies/MissionExecutionOntology#RE06.7.10">
        <rdfs:subClassOf rdf:resource="https://savage.nps.edu/EthicalControl/ontologies/MissionExecutionOntology#DADM06.7"/>
        <rdfs:comment>Can the IAS distinguish between benign and hostile intentions?</rdfs:comment>
        <rdfs:label>RE06.7.10_CanRecognizeHostileIntention</rdfs:label>
        <owl:versionInfo>page 74</owl:versionInfo>
    </owl:Class>
    


    <!-- https://savage.nps.edu/EthicalControl/ontologies/MissionExecutionOntology#RE06.7.11 -->

    <owl:Class rdf:about="https://savage.nps.edu/EthicalControl/ontologies/MissionExecutionOntology#RE06.7.11">
        <rdfs:subClassOf rdf:resource="https://savage.nps.edu/EthicalControl/ontologies/MissionExecutionOntology#DADM06.7"/>
        <rdfs:comment>Can the IAS distinguish between benign and hostile actions?</rdfs:comment>
        <rdfs:label>RE06.7.11_CanRecognizeHostileActions</rdfs:label>
        <owl:versionInfo>page 74</owl:versionInfo>
    </owl:Class>
    


    <!-- https://savage.nps.edu/EthicalControl/ontologies/MissionExecutionOntology#RE06.7.2 -->

    <owl:Class rdf:about="https://savage.nps.edu/EthicalControl/ontologies/MissionExecutionOntology#RE06.7.2">
        <rdfs:subClassOf rdf:resource="https://savage.nps.edu/EthicalControl/ontologies/MissionExecutionOntology#DADM06.7"/>
        <rdfs:comment> the IAS be prohibited from making determinations regarding who will be harmed - in a situation where harm to someone is unavoidable - based on any intrinsic characteristics of a person such as age, gender, or other physical or mental conditions?</rdfs:comment>
        <rdfs:label>RE06.7.2_CanDistinguishHumanIntrinsicCharacteristics</rdfs:label>
        <owl:versionInfo>page 73</owl:versionInfo>
    </owl:Class>
    


    <!-- https://savage.nps.edu/EthicalControl/ontologies/MissionExecutionOntology#RE06.7.3 -->

    <owl:Class rdf:about="https://savage.nps.edu/EthicalControl/ontologies/MissionExecutionOntology#RE06.7.3">
        <rdfs:subClassOf rdf:resource="https://savage.nps.edu/EthicalControl/ontologies/MissionExecutionOntology#DADM06.7"/>
        <rdfs:comment>Can the IAS make determinations regarding who will be harmed - in a situation where harm to someone is unavoidable - based on an individual’s status as an enemy combatant, a friendly combatant, or a noncombatant person?</rdfs:comment>
        <rdfs:label>RE06.7.3_CanDamageModelUnknownHuman</rdfs:label>
        <owl:versionInfo>page 73</owl:versionInfo>
    </owl:Class>
    


    <!-- https://savage.nps.edu/EthicalControl/ontologies/MissionExecutionOntology#RE06.7.4 -->

    <owl:Class rdf:about="https://savage.nps.edu/EthicalControl/ontologies/MissionExecutionOntology#RE06.7.4">
        <rdfs:subClassOf rdf:resource="https://savage.nps.edu/EthicalControl/ontologies/MissionExecutionOntology#DADM06.7"/>
        <rdfs:comment>Can the IAS account for unknown transient noncombatant personnel in or near a target area?</rdfs:comment>
        <rdfs:label>RE06.7.4_CanIdentifyUnknownPerson</rdfs:label>
        <owl:versionInfo>page 73</owl:versionInfo>
    </owl:Class>
    


    <!-- https://savage.nps.edu/EthicalControl/ontologies/MissionExecutionOntology#RE06.7.5 -->

    <owl:Class rdf:about="https://savage.nps.edu/EthicalControl/ontologies/MissionExecutionOntology#RE06.7.5">
        <rdfs:subClassOf rdf:resource="https://savage.nps.edu/EthicalControl/ontologies/MissionExecutionOntology#DADM06.7"/>
        <rdfs:comment>Can the IAS distinguish between adversarial human combatants and adversarial equipment and adjust the effect accordingly?</rdfs:comment>
        <rdfs:label>RE06.7.5_CanIdentifyAdversarialHumansObjects</rdfs:label>
        <owl:versionInfo>page 74</owl:versionInfo>
    </owl:Class>
    


    <!-- https://savage.nps.edu/EthicalControl/ontologies/MissionExecutionOntology#RE06.7.6 -->

    <owl:Class rdf:about="https://savage.nps.edu/EthicalControl/ontologies/MissionExecutionOntology#RE06.7.6">
        <rdfs:subClassOf rdf:resource="https://savage.nps.edu/EthicalControl/ontologies/MissionExecutionOntology#DADM06.7"/>
        <rdfs:comment>Can the IAS default to categorizing a person as an &quot;unknown,&quot; and not engage in instances where positive identification is below the required confidence level?</rdfs:comment>
        <rdfs:label>RE06.7.6_CanAvoidUnknownStatusPeople</rdfs:label>
        <owl:versionInfo>page 74</owl:versionInfo>
    </owl:Class>
    


    <!-- https://savage.nps.edu/EthicalControl/ontologies/MissionExecutionOntology#RE06.7.7 -->

    <owl:Class rdf:about="https://savage.nps.edu/EthicalControl/ontologies/MissionExecutionOntology#RE06.7.7">
        <rdfs:subClassOf rdf:resource="https://savage.nps.edu/EthicalControl/ontologies/MissionExecutionOntology#DADM06.7"/>
        <rdfs:comment>Can the IAS obtain, analyze and use information on civilian patterns of life to distinguish noncombatants from combatants?</rdfs:comment>
        <rdfs:label>RE06.7.7_CanUsePoLStatusPeople</rdfs:label>
        <owl:versionInfo>page 74</owl:versionInfo>
    </owl:Class>
    


    <!-- https://savage.nps.edu/EthicalControl/ontologies/MissionExecutionOntology#RE06.7.8 -->

    <owl:Class rdf:about="https://savage.nps.edu/EthicalControl/ontologies/MissionExecutionOntology#RE06.7.8">
        <rdfs:subClassOf rdf:resource="https://savage.nps.edu/EthicalControl/ontologies/MissionExecutionOntology#DADM06.7"/>
        <rdfs:comment>Can the IAS determine when enemy combatants have interspersed into a group of noncombatants that cannot be engaged with force?</rdfs:comment>
        <rdfs:label>RE06.7.8_CanBreakEngagementInterspersedNoncombatants</rdfs:label>
        <owl:versionInfo>page 74</owl:versionInfo>
    </owl:Class>
    


    <!-- https://savage.nps.edu/EthicalControl/ontologies/MissionExecutionOntology#RE06.7.9 -->

    <owl:Class rdf:about="https://savage.nps.edu/EthicalControl/ontologies/MissionExecutionOntology#RE06.7.9">
        <rdfs:subClassOf rdf:resource="https://savage.nps.edu/EthicalControl/ontologies/MissionExecutionOntology#DADM06.7"/>
        <rdfs:comment>Can the IAS use signatures to distinguish combatants from noncombatants that are unique to either the combatant only or the noncombatant only?</rdfs:comment>
        <rdfs:label>RE06.7.9_CanUseCombatantOnlySignatures</rdfs:label>
        <owl:versionInfo>page 74</owl:versionInfo>
    </owl:Class>
    


    <!-- https://savage.nps.edu/EthicalControl/ontologies/MissionExecutionOntology#RE06.8.1 -->

    <owl:Class rdf:about="https://savage.nps.edu/EthicalControl/ontologies/MissionExecutionOntology#RE06.8.1">
        <rdfs:subClassOf rdf:resource="https://savage.nps.edu/EthicalControl/ontologies/MissionExecutionOntology#DADM06.8"/>
        <rdfs:comment>Can the IAS detect a &quot;mission kill,&quot; where a person has been incapacitated and rendered hors de combat but not killed, and cease further use of force?</rdfs:comment>
        <rdfs:label>RE06.8.1_CanRecognizeNeutralizedPerson</rdfs:label>
        <owl:versionInfo>page 74</owl:versionInfo>
    </owl:Class>
    


    <!-- https://savage.nps.edu/EthicalControl/ontologies/MissionExecutionOntology#RE06.8.2 -->

    <owl:Class rdf:about="https://savage.nps.edu/EthicalControl/ontologies/MissionExecutionOntology#RE06.8.2">
        <rdfs:subClassOf rdf:resource="https://savage.nps.edu/EthicalControl/ontologies/MissionExecutionOntology#DADM06.8"/>
        <rdfs:comment>Can the IAS detect a &quot;mission kill,&quot; where a crewed vehicle has been damaged but not destroyed, rendering the crew hors de combat, and cease further use of force?</rdfs:comment>
        <rdfs:label>RE06.8.2_CanRecognizeNeutralizedObject</rdfs:label>
        <owl:versionInfo>page 74</owl:versionInfo>
    </owl:Class>
    


    <!-- https://savage.nps.edu/EthicalControl/ontologies/MissionExecutionOntology#RE06.9.1 -->

    <owl:Class rdf:about="https://savage.nps.edu/EthicalControl/ontologies/MissionExecutionOntology#RE06.9.1">
        <rdfs:subClassOf rdf:resource="https://savage.nps.edu/EthicalControl/ontologies/MissionExecutionOntology#DADM06.9"/>
        <rdfs:comment>Can the IAS prohibit the use of any action, method or munition available to it that could conceivably cause collateral injuries or death or cause unnecessary suffering?</rdfs:comment>
        <rdfs:label>RE06.9.1_CanMinimizeCollateralDamage</rdfs:label>
        <owl:versionInfo>page 74</owl:versionInfo>
    </owl:Class>
    


    <!-- https://savage.nps.edu/EthicalControl/ontologies/MissionExecutionOntology#RE06.9.2 -->

    <owl:Class rdf:about="https://savage.nps.edu/EthicalControl/ontologies/MissionExecutionOntology#RE06.9.2">
        <rdfs:subClassOf rdf:resource="https://savage.nps.edu/EthicalControl/ontologies/MissionExecutionOntology#DADM06.9"/>
        <rdfs:comment>Can the IAS prohibit the use of any action, method or munition available to it that could conceivably result in unacceptable amounts of noncombatant casualties?</rdfs:comment>
        <rdfs:label>RE06.9.2_CanModelNoncombatantCasualties</rdfs:label>
        <owl:versionInfo>page 74</owl:versionInfo>
    </owl:Class>
    


    <!-- https://savage.nps.edu/EthicalControl/ontologies/MissionExecutionOntology#RE06.9.3 -->

    <owl:Class rdf:about="https://savage.nps.edu/EthicalControl/ontologies/MissionExecutionOntology#RE06.9.3">
        <rdfs:subClassOf rdf:resource="https://savage.nps.edu/EthicalControl/ontologies/MissionExecutionOntology#DADM06.9"/>
        <rdfs:comment>Can the IAS prohibit engagements that would cause widespread, long-term, and/or severe impact to the health of persons protected from the use of force?</rdfs:comment>
        <rdfs:label>RE06.9.3_CanIdentifyPreventWidespreadLTSevereHealthPeople</rdfs:label>
        <owl:versionInfo>page 74</owl:versionInfo>
    </owl:Class>
    


    <!-- https://savage.nps.edu/EthicalControl/ontologies/MissionExecutionOntology#RE06.9.4 -->

    <owl:Class rdf:about="https://savage.nps.edu/EthicalControl/ontologies/MissionExecutionOntology#RE06.9.4">
        <rdfs:subClassOf rdf:resource="https://savage.nps.edu/EthicalControl/ontologies/MissionExecutionOntology#DADM06.9"/>
        <rdfs:comment>Can the IAS conduct an analysis to minimize the severity of injury, when causing some injury is unavoidable?</rdfs:comment>
        <rdfs:label>RE06.9.4_CanMinimizeInjuryPeople</rdfs:label>
        <owl:versionInfo>page 74</owl:versionInfo>
    </owl:Class>
    


    <!-- https://savage.nps.edu/EthicalControl/ontologies/MissionExecutionOntology#RE07.1.1 -->

    <owl:Class rdf:about="https://savage.nps.edu/EthicalControl/ontologies/MissionExecutionOntology#RE07.1.1">
        <rdfs:subClassOf rdf:resource="https://savage.nps.edu/EthicalControl/ontologies/MissionExecutionOntology#DADM07.1"/>
        <rdfs:comment>Is all pre-operational documentation made visible and accessible to the greatest extent possible, limited only by the potential creation of operational vulnerabilities?</rdfs:comment>
        <rdfs:label>RE07.1.1_PreoperationalDocumentationAvailable</rdfs:label>
        <owl:versionInfo>page 78</owl:versionInfo>
    </owl:Class>
    


    <!-- https://savage.nps.edu/EthicalControl/ontologies/MissionExecutionOntology#RE07.1.2 -->

    <owl:Class rdf:about="https://savage.nps.edu/EthicalControl/ontologies/MissionExecutionOntology#RE07.1.2">
        <rdfs:subClassOf rdf:resource="https://savage.nps.edu/EthicalControl/ontologies/MissionExecutionOntology#DADM07.1"/>
        <rdfs:comment>Is a formal procedure in place whereby individuals with concerns over unethical or illegal application of an IAS can (and are required to) document those concerns without fear of retaliation?</rdfs:comment>
        <rdfs:label>RE07.1.2_OpenChannelUnethicalIllegalApplicationsNoretaliation</rdfs:label>
        <owl:versionInfo>page 78</owl:versionInfo>
    </owl:Class>
    


    <!-- https://savage.nps.edu/EthicalControl/ontologies/MissionExecutionOntology#RE07.1.3 -->

    <owl:Class rdf:about="https://savage.nps.edu/EthicalControl/ontologies/MissionExecutionOntology#RE07.1.3">
        <rdfs:subClassOf rdf:resource="https://savage.nps.edu/EthicalControl/ontologies/MissionExecutionOntology#DADM07.1"/>
        <rdfs:comment>Is positive control of the individual IAS and all of its subcomponents documented as they move from one organization to the next in the research, development, and test and evaluation process?</rdfs:comment>
        <rdfs:label>RE07.1.3_RDTLifecycleDocumentationPersistance</rdfs:label>
        <owl:versionInfo>page 79</owl:versionInfo>
    </owl:Class>
    


    <!-- https://savage.nps.edu/EthicalControl/ontologies/MissionExecutionOntology#RE07.1.4 -->

    <owl:Class rdf:about="https://savage.nps.edu/EthicalControl/ontologies/MissionExecutionOntology#RE07.1.4">
        <rdfs:subClassOf rdf:resource="https://savage.nps.edu/EthicalControl/ontologies/MissionExecutionOntology#DADM07.1"/>
        <rdfs:comment>Are all commercial vendor marketing materials and claims about acquired IAS available for inspection and oversight?</rdfs:comment>
        <rdfs:label>RE07.1.4_IASSystemClaimsMaterialsAvailableInspectionOversight</rdfs:label>
        <owl:versionInfo>page 79</owl:versionInfo>
    </owl:Class>
    


    <!-- https://savage.nps.edu/EthicalControl/ontologies/MissionExecutionOntology#RE07.2.1 -->

    <owl:Class rdf:about="https://savage.nps.edu/EthicalControl/ontologies/MissionExecutionOntology#RE07.2.1">
        <rdfs:subClassOf rdf:resource="https://savage.nps.edu/EthicalControl/ontologies/MissionExecutionOntology#DADM07.2"/>
        <rdfs:comment>Is the chain of custody for all IAS training data documented from creation to final use?</rdfs:comment>
        <rdfs:label>RE07.2.1_TrainingDataProvananceCaptured</rdfs:label>
        <owl:versionInfo>page 79</owl:versionInfo>
    </owl:Class>
    


    <!-- https://savage.nps.edu/EthicalControl/ontologies/MissionExecutionOntology#RE07.2.10 -->

    <owl:Class rdf:about="https://savage.nps.edu/EthicalControl/ontologies/MissionExecutionOntology#RE07.2.10">
        <rdfs:subClassOf rdf:resource="https://savage.nps.edu/EthicalControl/ontologies/MissionExecutionOntology#DADM07.2"/>
        <rdfs:comment>Are the descriptions and labels that describe the IAS training data documented?</rdfs:comment>
        <rdfs:label>RE07.2.10_TrainingDataLabelsDescriptionsDocumented</rdfs:label>
        <owl:versionInfo>page 79</owl:versionInfo>
    </owl:Class>
    


    <!-- https://savage.nps.edu/EthicalControl/ontologies/MissionExecutionOntology#RE07.2.11 -->

    <owl:Class rdf:about="https://savage.nps.edu/EthicalControl/ontologies/MissionExecutionOntology#RE07.2.11">
        <rdfs:subClassOf rdf:resource="https://savage.nps.edu/EthicalControl/ontologies/MissionExecutionOntology#DADM07.2"/>
        <rdfs:comment>Does the IAS use any open-source training data with absent or suspect provenance documentation?</rdfs:comment>
        <rdfs:label>RE07.2.11_TrainingDataSuspect</rdfs:label>
        <owl:versionInfo>page 79</owl:versionInfo>
    </owl:Class>
    


    <!-- https://savage.nps.edu/EthicalControl/ontologies/MissionExecutionOntology#RE07.2.12 -->

    <owl:Class rdf:about="https://savage.nps.edu/EthicalControl/ontologies/MissionExecutionOntology#RE07.2.12">
        <rdfs:subClassOf rdf:resource="https://savage.nps.edu/EthicalControl/ontologies/MissionExecutionOntology#DADM07.2"/>
        <rdfs:comment>Can a higher-level IAS verify the reliability of inputs from its subsystem components that may or may not be autonomous?</rdfs:comment>
        <rdfs:label>RE07.2.12_IASInjestSubsystemVerifications</rdfs:label>
        <owl:versionInfo>page 79</owl:versionInfo>
    </owl:Class>
    


    <!-- https://savage.nps.edu/EthicalControl/ontologies/MissionExecutionOntology#RE07.2.13 -->

    <owl:Class rdf:about="https://savage.nps.edu/EthicalControl/ontologies/MissionExecutionOntology#RE07.2.13">
        <rdfs:subClassOf rdf:resource="https://savage.nps.edu/EthicalControl/ontologies/MissionExecutionOntology#DADM07.2"/>
        <rdfs:comment>Is the training data for the overall IAS the same training data that was used to design and verify the component autonomous subsystems?</rdfs:comment>
        <rdfs:label>RE07.2.13_DataConsistentWithVerificationDesignUse</rdfs:label>
        <owl:versionInfo>page 79</owl:versionInfo>
    </owl:Class>
    


    <!-- https://savage.nps.edu/EthicalControl/ontologies/MissionExecutionOntology#RE07.2.2 -->

    <owl:Class rdf:about="https://savage.nps.edu/EthicalControl/ontologies/MissionExecutionOntology#RE07.2.2">
        <rdfs:subClassOf rdf:resource="https://savage.nps.edu/EthicalControl/ontologies/MissionExecutionOntology#DADM07.2"/>
        <rdfs:comment>Are all requests for sharing of IAS training data documented?</rdfs:comment>
        <rdfs:label>RE07.2.2_TrainingDataAccessDocumented</rdfs:label>
        <owl:versionInfo>page 79</owl:versionInfo>
    </owl:Class>
    


    <!-- https://savage.nps.edu/EthicalControl/ontologies/MissionExecutionOntology#RE07.2.3 -->

    <owl:Class rdf:about="https://savage.nps.edu/EthicalControl/ontologies/MissionExecutionOntology#RE07.2.3">
        <rdfs:subClassOf rdf:resource="https://savage.nps.edu/EthicalControl/ontologies/MissionExecutionOntology#DADM07.2"/>
        <rdfs:comment>Are there access controls and processes in place to ensure that only authorized persons may make modifications to IAS training data?</rdfs:comment>
        <rdfs:label>RE07.2.3_TrainingDataAccessRestrictions</rdfs:label>
        <owl:versionInfo>page 79</owl:versionInfo>
    </owl:Class>
    


    <!-- https://savage.nps.edu/EthicalControl/ontologies/MissionExecutionOntology#RE07.2.4 -->

    <owl:Class rdf:about="https://savage.nps.edu/EthicalControl/ontologies/MissionExecutionOntology#RE07.2.4">
        <rdfs:subClassOf rdf:resource="https://savage.nps.edu/EthicalControl/ontologies/MissionExecutionOntology#DADM07.2"/>
        <rdfs:comment>Is the identity of all persons who accessed, or who authorized access to the IAS training data documented?</rdfs:comment>
        <rdfs:label>RE07.2.4_TrainingDataIdentidyDocumented</rdfs:label>
        <owl:versionInfo>page 79</owl:versionInfo>
    </owl:Class>
    


    <!-- https://savage.nps.edu/EthicalControl/ontologies/MissionExecutionOntology#RE07.2.5 -->

    <owl:Class rdf:about="https://savage.nps.edu/EthicalControl/ontologies/MissionExecutionOntology#RE07.2.5">
        <rdfs:subClassOf rdf:resource="https://savage.nps.edu/EthicalControl/ontologies/MissionExecutionOntology#DADM07.2"/>
        <rdfs:comment>Are the current, and all previous versions of the IAS training data retained for inspection?</rdfs:comment>
        <rdfs:label>RE07.2.5_TrainingDataVersioningCaptured</rdfs:label>
        <owl:versionInfo>page 79</owl:versionInfo>
    </owl:Class>
    


    <!-- https://savage.nps.edu/EthicalControl/ontologies/MissionExecutionOntology#RE07.2.6 -->

    <owl:Class rdf:about="https://savage.nps.edu/EthicalControl/ontologies/MissionExecutionOntology#RE07.2.6">
        <rdfs:subClassOf rdf:resource="https://savage.nps.edu/EthicalControl/ontologies/MissionExecutionOntology#DADM07.2"/>
        <rdfs:comment>Are all modifications to the IAS training data documented?</rdfs:comment>
        <rdfs:label>RE07.2.6_TrainingDataChangesCaptured</rdfs:label>
        <owl:versionInfo>page 79</owl:versionInfo>
    </owl:Class>
    


    <!-- https://savage.nps.edu/EthicalControl/ontologies/MissionExecutionOntology#RE07.2.7 -->

    <owl:Class rdf:about="https://savage.nps.edu/EthicalControl/ontologies/MissionExecutionOntology#RE07.2.7">
        <rdfs:subClassOf rdf:resource="https://savage.nps.edu/EthicalControl/ontologies/MissionExecutionOntology#DADM07.2"/>
        <rdfs:comment>Is the IAS training data available for inspection immediately prior to use?</rdfs:comment>
        <rdfs:label>RE07.2.7_TrainingDataInspectionReady</rdfs:label>
        <owl:versionInfo>page 79</owl:versionInfo>
    </owl:Class>
    


    <!-- https://savage.nps.edu/EthicalControl/ontologies/MissionExecutionOntology#RE07.2.8 -->

    <owl:Class rdf:about="https://savage.nps.edu/EthicalControl/ontologies/MissionExecutionOntology#RE07.2.8">
        <rdfs:subClassOf rdf:resource="https://savage.nps.edu/EthicalControl/ontologies/MissionExecutionOntology#DADM07.2"/>
        <rdfs:comment>Is the IAS training data retention policy documented?</rdfs:comment>
        <rdfs:label>RE07.2.8_TrainingDataRetentionPolicyDocumented</rdfs:label>
        <owl:versionInfo>page 79</owl:versionInfo>
    </owl:Class>
    


    <!-- https://savage.nps.edu/EthicalControl/ontologies/MissionExecutionOntology#RE07.2.9 -->

    <owl:Class rdf:about="https://savage.nps.edu/EthicalControl/ontologies/MissionExecutionOntology#RE07.2.9">
        <rdfs:subClassOf rdf:resource="https://savage.nps.edu/EthicalControl/ontologies/MissionExecutionOntology#DADM07.2"/>
        <rdfs:comment>Is the nature and origin of all IAS training data documented?</rdfs:comment>
        <rdfs:label>RE07.2.9_TrainingDataSourcesCaptured</rdfs:label>
        <owl:versionInfo>page 79</owl:versionInfo>
    </owl:Class>
    


    <!-- https://savage.nps.edu/EthicalControl/ontologies/MissionExecutionOntology#RE07.3.1 -->

    <owl:Class rdf:about="https://savage.nps.edu/EthicalControl/ontologies/MissionExecutionOntology#RE07.3.1">
        <rdfs:subClassOf rdf:resource="https://savage.nps.edu/EthicalControl/ontologies/MissionExecutionOntology#DADM07.3"/>
        <rdfs:comment>Is the chain of custody for all IAS algorithm’s source code documented from creation to final use?</rdfs:comment>
        <rdfs:label>RE07.3.1_SourceCodeLifecycleChangeControlledCaptured</rdfs:label>
        <owl:versionInfo>page 79</owl:versionInfo>
    </owl:Class>
    


    <!-- https://savage.nps.edu/EthicalControl/ontologies/MissionExecutionOntology#RE07.3.10 -->

    <owl:Class rdf:about="https://savage.nps.edu/EthicalControl/ontologies/MissionExecutionOntology#RE07.3.10">
        <rdfs:subClassOf rdf:resource="https://savage.nps.edu/EthicalControl/ontologies/MissionExecutionOntology#DADM07.3"/>
        <rdfs:comment>Are the descriptions and labels that describe the IAS algorithms documented?</rdfs:comment>
        <rdfs:label>RE07.3.10_DataLabelDescriptionsDocumented</rdfs:label>
        <owl:versionInfo>page 80</owl:versionInfo>
    </owl:Class>
    


    <!-- https://savage.nps.edu/EthicalControl/ontologies/MissionExecutionOntology#RE07.3.11 -->

    <owl:Class rdf:about="https://savage.nps.edu/EthicalControl/ontologies/MissionExecutionOntology#RE07.3.11">
        <rdfs:subClassOf rdf:resource="https://savage.nps.edu/EthicalControl/ontologies/MissionExecutionOntology#DADM07.3"/>
        <rdfs:comment>Do the IAS algorithms use any open-source code with absent or suspect provenance documentation?</rdfs:comment>
        <rdfs:label>RE07.3.11_AlgorithmsDependesCodeSuspectProvenanceCaptured</rdfs:label>
        <owl:versionInfo>page 80</owl:versionInfo>
    </owl:Class>
    


    <!-- https://savage.nps.edu/EthicalControl/ontologies/MissionExecutionOntology#RE07.3.12 -->

    <owl:Class rdf:about="https://savage.nps.edu/EthicalControl/ontologies/MissionExecutionOntology#RE07.3.12">
        <rdfs:subClassOf rdf:resource="https://savage.nps.edu/EthicalControl/ontologies/MissionExecutionOntology#DADM07.3"/>
        <rdfs:comment>Is the design documentation describing the IAS algorithms technical architecture available for inspection?</rdfs:comment>
        <rdfs:label>RE07.3.12_IASTechnicalArchitectureAvailable</rdfs:label>
        <owl:versionInfo>page 80</owl:versionInfo>
    </owl:Class>
    


    <!-- https://savage.nps.edu/EthicalControl/ontologies/MissionExecutionOntology#RE07.3.13 -->

    <owl:Class rdf:about="https://savage.nps.edu/EthicalControl/ontologies/MissionExecutionOntology#RE07.3.13">
        <rdfs:subClassOf rdf:resource="https://savage.nps.edu/EthicalControl/ontologies/MissionExecutionOntology#DADM07.3"/>
        <rdfs:comment>Are code scanning tools used that can identify poor coding practices and common security vulnerabilities?</rdfs:comment>
        <rdfs:label>RE07.3.13_IdentifyPoorCodeSecurityVulnerabilities</rdfs:label>
        <owl:versionInfo>page 80</owl:versionInfo>
    </owl:Class>
    


    <!-- https://savage.nps.edu/EthicalControl/ontologies/MissionExecutionOntology#RE07.3.2 -->

    <owl:Class rdf:about="https://savage.nps.edu/EthicalControl/ontologies/MissionExecutionOntology#RE07.3.2">
        <rdfs:subClassOf rdf:resource="https://savage.nps.edu/EthicalControl/ontologies/MissionExecutionOntology#DADM07.3"/>
        <rdfs:comment>Are all requests for sharing of IAS algorithms documented?</rdfs:comment>
        <rdfs:label>RE07.3.2_RequestsForSharingDocumented</rdfs:label>
        <owl:versionInfo>page 79</owl:versionInfo>
    </owl:Class>
    


    <!-- https://savage.nps.edu/EthicalControl/ontologies/MissionExecutionOntology#RE07.3.3 -->

    <owl:Class rdf:about="https://savage.nps.edu/EthicalControl/ontologies/MissionExecutionOntology#RE07.3.3">
        <rdfs:subClassOf rdf:resource="https://savage.nps.edu/EthicalControl/ontologies/MissionExecutionOntology#DADM07.3"/>
        <rdfs:comment>Are there access controls and processes in place to ensure that only authorized persons may make modifications to IAS algorithms?</rdfs:comment>
        <rdfs:label>RE07.3.3_AlgorithmDevelopmentAccessControls</rdfs:label>
        <owl:versionInfo>page 79</owl:versionInfo>
    </owl:Class>
    


    <!-- https://savage.nps.edu/EthicalControl/ontologies/MissionExecutionOntology#RE07.3.4 -->

    <owl:Class rdf:about="https://savage.nps.edu/EthicalControl/ontologies/MissionExecutionOntology#RE07.3.4">
        <rdfs:subClassOf rdf:resource="https://savage.nps.edu/EthicalControl/ontologies/MissionExecutionOntology#DADM07.3"/>
        <rdfs:comment>Is the identity of all persons who accessed, or who authorized access to IAS algorithms documented?</rdfs:comment>
        <rdfs:label>RE07.3.4_IdentityAlgorithmAccessCaptured</rdfs:label>
        <owl:versionInfo>page 80</owl:versionInfo>
    </owl:Class>
    


    <!-- https://savage.nps.edu/EthicalControl/ontologies/MissionExecutionOntology#RE07.3.5 -->

    <owl:Class rdf:about="https://savage.nps.edu/EthicalControl/ontologies/MissionExecutionOntology#RE07.3.5">
        <rdfs:subClassOf rdf:resource="https://savage.nps.edu/EthicalControl/ontologies/MissionExecutionOntology#DADM07.3"/>
        <rdfs:comment>Are the current, and all previous versions of the IAS algorithms retained for inspection?</rdfs:comment>
        <rdfs:label>RE07.3.5_RetentionAlgorithmsVersioning</rdfs:label>
        <owl:versionInfo>page 80</owl:versionInfo>
    </owl:Class>
    


    <!-- https://savage.nps.edu/EthicalControl/ontologies/MissionExecutionOntology#RE07.3.6 -->

    <owl:Class rdf:about="https://savage.nps.edu/EthicalControl/ontologies/MissionExecutionOntology#RE07.3.6">
        <rdfs:subClassOf rdf:resource="https://savage.nps.edu/EthicalControl/ontologies/MissionExecutionOntology#DADM07.3"/>
        <rdfs:comment>Are all modifications to the IAS algorithms documented?</rdfs:comment>
        <rdfs:label>RE07.3.6_AlgorithmModificationsCaptured</rdfs:label>
        <owl:versionInfo>page 80</owl:versionInfo>
    </owl:Class>
    


    <!-- https://savage.nps.edu/EthicalControl/ontologies/MissionExecutionOntology#RE07.3.7 -->

    <owl:Class rdf:about="https://savage.nps.edu/EthicalControl/ontologies/MissionExecutionOntology#RE07.3.7">
        <rdfs:subClassOf rdf:resource="https://savage.nps.edu/EthicalControl/ontologies/MissionExecutionOntology#DADM07.3"/>
        <rdfs:comment>Are the IAS algorithms available for inspection immediately prior to use?</rdfs:comment>
        <rdfs:label>RE07.3.7_IASAlgorithmsAvailableInspection</rdfs:label>
        <owl:versionInfo>page 80</owl:versionInfo>
    </owl:Class>
    


    <!-- https://savage.nps.edu/EthicalControl/ontologies/MissionExecutionOntology#RE07.3.8 -->

    <owl:Class rdf:about="https://savage.nps.edu/EthicalControl/ontologies/MissionExecutionOntology#RE07.3.8">
        <rdfs:subClassOf rdf:resource="https://savage.nps.edu/EthicalControl/ontologies/MissionExecutionOntology#DADM07.3"/>
        <rdfs:comment>Is the IAS algorithm retention policy documented?</rdfs:comment>
        <rdfs:label>RE07.3.8_AlgorithmRetentionPolicyDocumented</rdfs:label>
        <owl:versionInfo>page 80</owl:versionInfo>
    </owl:Class>
    


    <!-- https://savage.nps.edu/EthicalControl/ontologies/MissionExecutionOntology#RE07.3.9 -->

    <owl:Class rdf:about="https://savage.nps.edu/EthicalControl/ontologies/MissionExecutionOntology#RE07.3.9">
        <rdfs:subClassOf rdf:resource="https://savage.nps.edu/EthicalControl/ontologies/MissionExecutionOntology#DADM07.3"/>
        <rdfs:comment>Is the nature and origin of all IAS algorithms documented?</rdfs:comment>
        <rdfs:label>RE07.3.9_AlgorithmNatureOriginDocumented</rdfs:label>
        <owl:versionInfo>page 80</owl:versionInfo>
    </owl:Class>
    


    <!-- https://savage.nps.edu/EthicalControl/ontologies/MissionExecutionOntology#RE07.4.1 -->

    <owl:Class rdf:about="https://savage.nps.edu/EthicalControl/ontologies/MissionExecutionOntology#RE07.4.1">
        <rdfs:subClassOf rdf:resource="https://savage.nps.edu/EthicalControl/ontologies/MissionExecutionOntology#DADM07.4"/>
        <rdfs:comment>Is the chain of custody for all IAS computer hardware components documented from creation to final use?</rdfs:comment>
        <rdfs:label>RE07.4.1_ComputerHardwareProvenanceDocumented</rdfs:label>
        <owl:versionInfo>page 80</owl:versionInfo>
    </owl:Class>
    


    <!-- https://savage.nps.edu/EthicalControl/ontologies/MissionExecutionOntology#RE07.4.2 -->

    <owl:Class rdf:about="https://savage.nps.edu/EthicalControl/ontologies/MissionExecutionOntology#RE07.4.2">
        <rdfs:subClassOf rdf:resource="https://savage.nps.edu/EthicalControl/ontologies/MissionExecutionOntology#DADM07.4"/>
        <rdfs:comment>Is the identity of all persons who accessed, or who authorized access to IAS computer hardware components documented?</rdfs:comment>
        <rdfs:label>RE07.4.2_ComputerHardwarePersonAccessDocumented</rdfs:label>
        <owl:versionInfo>page 80</owl:versionInfo>
    </owl:Class>
    


    <!-- https://savage.nps.edu/EthicalControl/ontologies/MissionExecutionOntology#RE07.4.3 -->

    <owl:Class rdf:about="https://savage.nps.edu/EthicalControl/ontologies/MissionExecutionOntology#RE07.4.3">
        <rdfs:subClassOf rdf:resource="https://savage.nps.edu/EthicalControl/ontologies/MissionExecutionOntology#DADM07.4"/>
        <rdfs:comment>Are there access controls and processes in place to ensure that only authorized persons may make modifications to hardware or software?</rdfs:comment>
        <rdfs:label>RE07.4.3_AccessControlsComputerHardware</rdfs:label>
        <owl:versionInfo>page 80</owl:versionInfo>
    </owl:Class>
    


    <!-- https://savage.nps.edu/EthicalControl/ontologies/MissionExecutionOntology#RE07.4.4 -->

    <owl:Class rdf:about="https://savage.nps.edu/EthicalControl/ontologies/MissionExecutionOntology#RE07.4.4">
        <rdfs:subClassOf rdf:resource="https://savage.nps.edu/EthicalControl/ontologies/MissionExecutionOntology#DADM07.4"/>
        <rdfs:comment>Are all modification and repairs to the IAS computer hardware components documented?</rdfs:comment>
        <rdfs:label>RE07.4.4_ComputerHardwareModificationRepairsLogged</rdfs:label>
        <owl:versionInfo>page 80</owl:versionInfo>
    </owl:Class>
    


    <!-- https://savage.nps.edu/EthicalControl/ontologies/MissionExecutionOntology#RE07.4.5 -->

    <owl:Class rdf:about="https://savage.nps.edu/EthicalControl/ontologies/MissionExecutionOntology#RE07.4.5">
        <rdfs:subClassOf rdf:resource="https://savage.nps.edu/EthicalControl/ontologies/MissionExecutionOntology#DADM07.4"/>
        <rdfs:comment>Are the IAS computer hardware components available for inspection immediately prior to use?</rdfs:comment>
        <rdfs:label>RE07.4.5_ComputerHardwareInspectionReady</rdfs:label>
        <owl:versionInfo>page 80</owl:versionInfo>
    </owl:Class>
    


    <!-- https://savage.nps.edu/EthicalControl/ontologies/MissionExecutionOntology#RE07.4.6 -->

    <owl:Class rdf:about="https://savage.nps.edu/EthicalControl/ontologies/MissionExecutionOntology#RE07.4.6">
        <rdfs:subClassOf rdf:resource="https://savage.nps.edu/EthicalControl/ontologies/MissionExecutionOntology#DADM07.4"/>
        <rdfs:comment>Is the nature and origin of all IAS computer hardware components documented?</rdfs:comment>
        <rdfs:label>RE07.4.6_NatureOriginComputerHardwareDocumented</rdfs:label>
        <owl:versionInfo>page 80</owl:versionInfo>
    </owl:Class>
    


    <!-- https://savage.nps.edu/EthicalControl/ontologies/MissionExecutionOntology#RE07.4.7 -->

    <owl:Class rdf:about="https://savage.nps.edu/EthicalControl/ontologies/MissionExecutionOntology#RE07.4.7">
        <rdfs:subClassOf rdf:resource="https://savage.nps.edu/EthicalControl/ontologies/MissionExecutionOntology#DADM07.4"/>
        <rdfs:comment>Does the IAS use any commercial off the shelf computer hardware components with absent or suspect provenance documentation?</rdfs:comment>
        <rdfs:label>RE07.4.7_ComputerHardwareSuspectProvenanceDocumended</rdfs:label>
        <owl:versionInfo>page 80</owl:versionInfo>
    </owl:Class>
    


    <!-- https://savage.nps.edu/EthicalControl/ontologies/MissionExecutionOntology#RE07.4.8 -->

    <owl:Class rdf:about="https://savage.nps.edu/EthicalControl/ontologies/MissionExecutionOntology#RE07.4.8">
        <rdfs:subClassOf rdf:resource="https://savage.nps.edu/EthicalControl/ontologies/MissionExecutionOntology#DADM07.4"/>
        <rdfs:comment>Is the design documentation describing the IAS computer hardware components technical architecture available for inspection?</rdfs:comment>
        <rdfs:label>RE07.4.8_ComputerHardwareTechnicalArchitectureInspectionReady</rdfs:label>
        <owl:versionInfo>page 80</owl:versionInfo>
    </owl:Class>
    


    <!-- https://savage.nps.edu/EthicalControl/ontologies/MissionExecutionOntology#RE07.5.1 -->

    <owl:Class rdf:about="https://savage.nps.edu/EthicalControl/ontologies/MissionExecutionOntology#RE07.5.1">
        <rdfs:subClassOf rdf:resource="https://savage.nps.edu/EthicalControl/ontologies/MissionExecutionOntology#DADM07.5"/>
        <rdfs:comment>Has the IAS been acquired using any waivers allowing circumvention of safety policies or regulations?</rdfs:comment>
        <rdfs:label>RE07.5.1_CircumventionSafetyPoliciesRegulations</rdfs:label>
        <owl:versionInfo>page 81</owl:versionInfo>
    </owl:Class>
    


    <!-- https://savage.nps.edu/EthicalControl/ontologies/MissionExecutionOntology#RE07.5.10 -->

    <owl:Class rdf:about="https://savage.nps.edu/EthicalControl/ontologies/MissionExecutionOntology#RE07.5.10">
        <rdfs:subClassOf rdf:resource="https://savage.nps.edu/EthicalControl/ontologies/MissionExecutionOntology#DADM07.5"/>
        <rdfs:comment>If the IAS has the potential to be considered a LAWS by DoD Directive 3000.09, has the IAS undergone the required review and approval process outlined in this policy?</rdfs:comment>
        <rdfs:label>RE07.5.10_DoDDirective300009LAWSApproval</rdfs:label>
        <owl:versionInfo>page 81</owl:versionInfo>
    </owl:Class>
    


    <!-- https://savage.nps.edu/EthicalControl/ontologies/MissionExecutionOntology#RE07.5.2 -->

    <owl:Class rdf:about="https://savage.nps.edu/EthicalControl/ontologies/MissionExecutionOntology#RE07.5.2">
        <rdfs:subClassOf rdf:resource="https://savage.nps.edu/EthicalControl/ontologies/MissionExecutionOntology#DADM07.5"/>
        <rdfs:comment>Has the IAS been acquired using any waivers allowing circumvention of ethics policies or regulations?</rdfs:comment>
        <rdfs:label>RE07.5.2_CircumventionEthicsPoliciesRegulations</rdfs:label>
        <owl:versionInfo>page 81</owl:versionInfo>
    </owl:Class>
    


    <!-- https://savage.nps.edu/EthicalControl/ontologies/MissionExecutionOntology#RE07.5.3 -->

    <owl:Class rdf:about="https://savage.nps.edu/EthicalControl/ontologies/MissionExecutionOntology#RE07.5.3">
        <rdfs:subClassOf rdf:resource="https://savage.nps.edu/EthicalControl/ontologies/MissionExecutionOntology#DADM07.5"/>
        <rdfs:comment>Has the IAS been acquired using any waivers allowing circumvention of any developmental or operational testing, verification, and validation?</rdfs:comment>
        <rdfs:label>RE07.5.3_CircumventionDevOpsVerificationValidation</rdfs:label>
        <owl:versionInfo>page 81</owl:versionInfo>
    </owl:Class>
    


    <!-- https://savage.nps.edu/EthicalControl/ontologies/MissionExecutionOntology#RE07.5.4 -->

    <owl:Class rdf:about="https://savage.nps.edu/EthicalControl/ontologies/MissionExecutionOntology#RE07.5.4">
        <rdfs:subClassOf rdf:resource="https://savage.nps.edu/EthicalControl/ontologies/MissionExecutionOntology#DADM07.5"/>
        <rdfs:comment>Has the IAS been acquired using any accelerated/rapid/other acquisition authorities that dismiss or delay risk mitigating steps otherwise present in the deliberate acquisition system?</rdfs:comment>
        <rdfs:label>RE07.5.4_CircumventionRiskDebt</rdfs:label>
        <owl:versionInfo>page 81</owl:versionInfo>
    </owl:Class>
    


    <!-- https://savage.nps.edu/EthicalControl/ontologies/MissionExecutionOntology#RE07.5.5 -->

    <owl:Class rdf:about="https://savage.nps.edu/EthicalControl/ontologies/MissionExecutionOntology#RE07.5.5">
        <rdfs:subClassOf rdf:resource="https://savage.nps.edu/EthicalControl/ontologies/MissionExecutionOntology#DADM07.5"/>
        <rdfs:comment>Are all acquisition and development-related waivers documented and available for inspection?</rdfs:comment>
        <rdfs:label>RE07.5.5_WaiversInspectionReady</rdfs:label>
        <owl:versionInfo>page 81</owl:versionInfo>
    </owl:Class>
    


    <!-- https://savage.nps.edu/EthicalControl/ontologies/MissionExecutionOntology#RE07.5.6 -->

    <owl:Class rdf:about="https://savage.nps.edu/EthicalControl/ontologies/MissionExecutionOntology#RE07.5.6">
        <rdfs:subClassOf rdf:resource="https://savage.nps.edu/EthicalControl/ontologies/MissionExecutionOntology#DADM07.5"/>
        <rdfs:comment>Is the IAS test and evaluation plan made public to the greatest extent possible (without divulging operational vulnerabilities)?</rdfs:comment>
        <rdfs:label>RE07.5.6_TestEvalutionPlanSecurelyAvailable</rdfs:label>
        <owl:versionInfo>page 81</owl:versionInfo>
    </owl:Class>
    


    <!-- https://savage.nps.edu/EthicalControl/ontologies/MissionExecutionOntology#RE07.5.7 -->

    <owl:Class rdf:about="https://savage.nps.edu/EthicalControl/ontologies/MissionExecutionOntology#RE07.5.7">
        <rdfs:subClassOf rdf:resource="https://savage.nps.edu/EthicalControl/ontologies/MissionExecutionOntology#DADM07.5"/>
        <rdfs:comment>Have the IAS developers produced ethical risk mitigation documentation for the IAS similar to the technical risk mitigation documentation already required by acquisition regulations?</rdfs:comment>
        <rdfs:label>RE07.5.7_EthicalRiskMitigationDocumentation</rdfs:label>
        <owl:versionInfo>page 81</owl:versionInfo>
    </owl:Class>
    


    <!-- https://savage.nps.edu/EthicalControl/ontologies/MissionExecutionOntology#RE07.5.8 -->

    <owl:Class rdf:about="https://savage.nps.edu/EthicalControl/ontologies/MissionExecutionOntology#RE07.5.8">
        <rdfs:subClassOf rdf:resource="https://savage.nps.edu/EthicalControl/ontologies/MissionExecutionOntology#DADM07.5"/>
        <rdfs:comment>Do IAS approval documents record any conditions of use under which the approval would be invalid or rescinded?</rdfs:comment>
        <rdfs:label>RE07.5.8_CheckInvalidApprovalDocuments</rdfs:label>
        <owl:versionInfo>page 81</owl:versionInfo>
    </owl:Class>
    


    <!-- https://savage.nps.edu/EthicalControl/ontologies/MissionExecutionOntology#RE07.5.9 -->

    <owl:Class rdf:about="https://savage.nps.edu/EthicalControl/ontologies/MissionExecutionOntology#RE07.5.9">
        <rdfs:subClassOf rdf:resource="https://savage.nps.edu/EthicalControl/ontologies/MissionExecutionOntology#DADM07.5"/>
        <rdfs:comment>Are all conditions that would require re-testing of a fielded IAS documented and made available to the end user?</rdfs:comment>
        <rdfs:label>RE07.5.9_RetestingDocumentationAvailable</rdfs:label>
        <owl:versionInfo>page 81</owl:versionInfo>
    </owl:Class>
    


    <!-- https://savage.nps.edu/EthicalControl/ontologies/MissionExecutionOntology#RE07.6.1 -->

    <owl:Class rdf:about="https://savage.nps.edu/EthicalControl/ontologies/MissionExecutionOntology#RE07.6.1">
        <rdfs:subClassOf rdf:resource="https://savage.nps.edu/EthicalControl/ontologies/MissionExecutionOntology#DADM07.6"/>
        <rdfs:comment>Are any justifications for not conducting a legal review of a new or upgraded IAS documented and publicized?</rdfs:comment>
        <rdfs:label>RE07.6.1_JustificationsMissingLegalReview</rdfs:label>
        <owl:versionInfo>page 81</owl:versionInfo>
    </owl:Class>
    


    <!-- https://savage.nps.edu/EthicalControl/ontologies/MissionExecutionOntology#RE07.6.2 -->

    <owl:Class rdf:about="https://savage.nps.edu/EthicalControl/ontologies/MissionExecutionOntology#RE07.6.2">
        <rdfs:subClassOf rdf:resource="https://savage.nps.edu/EthicalControl/ontologies/MissionExecutionOntology#DADM07.6"/>
        <rdfs:comment>Is the independence of any and all required IAS oversight bodies or regulatory authorities documented and publicized?</rdfs:comment>
        <rdfs:label>RE07.6.2_OversightBodyIndependenceChecks</rdfs:label>
        <owl:versionInfo>page 81</owl:versionInfo>
    </owl:Class>
    


    <!-- https://savage.nps.edu/EthicalControl/ontologies/MissionExecutionOntology#RE07.6.3 -->

    <owl:Class rdf:about="https://savage.nps.edu/EthicalControl/ontologies/MissionExecutionOntology#RE07.6.3">
        <rdfs:subClassOf rdf:resource="https://savage.nps.edu/EthicalControl/ontologies/MissionExecutionOntology#DADM07.6"/>
        <rdfs:comment>Have conflict of interest screenings been conducted for all persons involved in the research, development, test and evaluation processes?</rdfs:comment>
        <rdfs:label>RE07.6.3_ConflictInterestScreeningRDTEPersons</rdfs:label>
        <owl:versionInfo>page 81</owl:versionInfo>
    </owl:Class>
    


    <!-- https://savage.nps.edu/EthicalControl/ontologies/MissionExecutionOntology#RE07.6.4 -->

    <owl:Class rdf:about="https://savage.nps.edu/EthicalControl/ontologies/MissionExecutionOntology#RE07.6.4">
        <rdfs:subClassOf rdf:resource="https://savage.nps.edu/EthicalControl/ontologies/MissionExecutionOntology#DADM07.6"/>
        <rdfs:comment>Have all identified conflicts of interest been either mitigated or waived?</rdfs:comment>
        <rdfs:label>RE07.6.4_ConflictsInterestMitigationsWaived</rdfs:label>
        <owl:versionInfo>page 81</owl:versionInfo>
    </owl:Class>
    


    <!-- https://savage.nps.edu/EthicalControl/ontologies/MissionExecutionOntology#RE07.6.5 -->

    <owl:Class rdf:about="https://savage.nps.edu/EthicalControl/ontologies/MissionExecutionOntology#RE07.6.5">
        <rdfs:subClassOf rdf:resource="https://savage.nps.edu/EthicalControl/ontologies/MissionExecutionOntology#DADM07.6"/>
        <rdfs:comment>Have the justifications for conflict of interest mitigations and/or waivers been documented and publicized?</rdfs:comment>
        <rdfs:label>RE07.6.5_ConflictsJustificationsDocumentedPublished</rdfs:label>
        <owl:versionInfo>page 81</owl:versionInfo>
    </owl:Class>
    


    <!-- https://savage.nps.edu/EthicalControl/ontologies/MissionExecutionOntology#RE08.1.1 -->

    <owl:Class rdf:about="https://savage.nps.edu/EthicalControl/ontologies/MissionExecutionOntology#RE08.1.1">
        <rdfs:subClassOf rdf:resource="https://savage.nps.edu/EthicalControl/ontologies/MissionExecutionOntology#DADM08.1"/>
        <rdfs:comment>Is the collection of IAS operational data fields and their retention in an IAS operational audit log mandatory?</rdfs:comment>
        <rdfs:label>RE08.1.1_OperationalDataFieldsAuditRetention</rdfs:label>
        <owl:versionInfo>page 82</owl:versionInfo>
    </owl:Class>
    


    <!-- https://savage.nps.edu/EthicalControl/ontologies/MissionExecutionOntology#RE08.1.10 -->

    <owl:Class rdf:about="https://savage.nps.edu/EthicalControl/ontologies/MissionExecutionOntology#RE08.1.10">
        <rdfs:subClassOf rdf:resource="https://savage.nps.edu/EthicalControl/ontologies/MissionExecutionOntology#DADM08.1"/>
        <rdfs:comment>Is a procedure in place whereby individuals who have examined IAS operational audit logs and have concerns regarding the potential unethical or illegal use, can make those concerns known without fear of retaliation?</rdfs:comment>
        <rdfs:label>RE08.1.10_OperationalDataLogProcessUnthicalUseReporting</rdfs:label>
        <owl:versionInfo>page 82</owl:versionInfo>
    </owl:Class>
    


    <!-- https://savage.nps.edu/EthicalControl/ontologies/MissionExecutionOntology#RE08.1.11 -->

    <owl:Class rdf:about="https://savage.nps.edu/EthicalControl/ontologies/MissionExecutionOntology#RE08.1.11">
        <rdfs:subClassOf rdf:resource="https://savage.nps.edu/EthicalControl/ontologies/MissionExecutionOntology#DADM08.1"/>
        <rdfs:comment>Are transfers of IAS command and control documented? Operational audit log data fields</rdfs:comment>
        <rdfs:label>RE08.1.11_OperationalAuditDataC2TransferFields</rdfs:label>
        <owl:versionInfo>page 82</owl:versionInfo>
    </owl:Class>
    


    <!-- https://savage.nps.edu/EthicalControl/ontologies/MissionExecutionOntology#RE08.1.12 -->

    <owl:Class rdf:about="https://savage.nps.edu/EthicalControl/ontologies/MissionExecutionOntology#RE08.1.12">
        <rdfs:subClassOf rdf:resource="https://savage.nps.edu/EthicalControl/ontologies/MissionExecutionOntology#DADM08.1"/>
        <rdfs:comment>Does the IAS collect metadata associated with all sensed objects in its operation environment that includes object identification, confidence metrics associated with its state values (i.e., position , velocity, etc.), and historical state information?</rdfs:comment>
        <rdfs:label>RE08.1.12_OperationalEnvironmentSensedObjectMetadata</rdfs:label>
        <owl:versionInfo>page 82</owl:versionInfo>
    </owl:Class>
    


    <!-- https://savage.nps.edu/EthicalControl/ontologies/MissionExecutionOntology#RE08.1.13 -->

    <owl:Class rdf:about="https://savage.nps.edu/EthicalControl/ontologies/MissionExecutionOntology#RE08.1.13">
        <rdfs:subClassOf rdf:resource="https://savage.nps.edu/EthicalControl/ontologies/MissionExecutionOntology#DADM08.1"/>
        <rdfs:comment>Does the IAS collect time stamp metadata for all data fields and during the entire mission duration?</rdfs:comment>
        <rdfs:label>RE08.1.13_MetadataIncludesTimestamps</rdfs:label>
        <owl:versionInfo>page 82</owl:versionInfo>
    </owl:Class>
    


    <!-- https://savage.nps.edu/EthicalControl/ontologies/MissionExecutionOntology#RE08.1.14 -->

    <owl:Class rdf:about="https://savage.nps.edu/EthicalControl/ontologies/MissionExecutionOntology#RE08.1.14">
        <rdfs:subClassOf rdf:resource="https://savage.nps.edu/EthicalControl/ontologies/MissionExecutionOntology#DADM08.1"/>
        <rdfs:comment>Does the IAS collect data on the operating conditions of all critical internal systems? </rdfs:comment>
        <rdfs:label>RE08.1.14_SystemLogsCriticalInternalSystemConditions</rdfs:label>
        <owl:versionInfo>page 82</owl:versionInfo>
    </owl:Class>
    


    <!-- https://savage.nps.edu/EthicalControl/ontologies/MissionExecutionOntology#RE08.1.15 -->

    <owl:Class rdf:about="https://savage.nps.edu/EthicalControl/ontologies/MissionExecutionOntology#RE08.1.15">
        <rdfs:subClassOf rdf:resource="https://savage.nps.edu/EthicalControl/ontologies/MissionExecutionOntology#DADM08.1"/>
        <rdfs:comment>Does the IAS record all commands it receives?</rdfs:comment>
        <rdfs:label>RE08.1.15_IASRecordsC2</rdfs:label>
        <owl:versionInfo>page 83</owl:versionInfo>
    </owl:Class>
    


    <!-- https://savage.nps.edu/EthicalControl/ontologies/MissionExecutionOntology#RE08.1.16 -->

    <owl:Class rdf:about="https://savage.nps.edu/EthicalControl/ontologies/MissionExecutionOntology#RE08.1.16">
        <rdfs:subClassOf rdf:resource="https://savage.nps.edu/EthicalControl/ontologies/MissionExecutionOntology#DADM08.1"/>
        <rdfs:comment>Does the IAS record the identities of the accountable operator(s) and commander(s)?</rdfs:comment>
        <rdfs:label>RE08.1.16_IASRecordIdentitesAccountableOperatorsCommanders</rdfs:label>
        <owl:versionInfo>page 83</owl:versionInfo>
    </owl:Class>
    


    <!-- https://savage.nps.edu/EthicalControl/ontologies/MissionExecutionOntology#RE08.1.17 -->

    <owl:Class rdf:about="https://savage.nps.edu/EthicalControl/ontologies/MissionExecutionOntology#RE08.1.17">
        <rdfs:subClassOf rdf:resource="https://savage.nps.edu/EthicalControl/ontologies/MissionExecutionOntology#DADM08.1"/>
        <rdfs:comment>Does the IAS record actions taken, and decisions made by the IAS and by the human operators?</rdfs:comment>
        <rdfs:label>RE08.1.17_IASRecordsDecisions</rdfs:label>
        <owl:versionInfo>page 83</owl:versionInfo>
    </owl:Class>
    


    <!-- https://savage.nps.edu/EthicalControl/ontologies/MissionExecutionOntology#RE08.1.18 -->

    <owl:Class rdf:about="https://savage.nps.edu/EthicalControl/ontologies/MissionExecutionOntology#RE08.1.18">
        <rdfs:subClassOf rdf:resource="https://savage.nps.edu/EthicalControl/ontologies/MissionExecutionOntology#DADM08.1"/>
        <rdfs:comment>Does the IAS record the sensed actions of friendly force personnel, adversary force personnel and noncombatant persons?</rdfs:comment>
        <rdfs:label>RE08.1.18_IASRecordsSensedActionsPeople</rdfs:label>
        <owl:versionInfo>page 83</owl:versionInfo>
    </owl:Class>
    


    <!-- https://savage.nps.edu/EthicalControl/ontologies/MissionExecutionOntology#RE08.1.19 -->

    <owl:Class rdf:about="https://savage.nps.edu/EthicalControl/ontologies/MissionExecutionOntology#RE08.1.19">
        <rdfs:subClassOf rdf:resource="https://savage.nps.edu/EthicalControl/ontologies/MissionExecutionOntology#DADM08.1"/>
        <rdfs:comment>Does the IAS record all algorithms in use (to include any version number) that are utilized to produce an action/decision?</rdfs:comment>
        <rdfs:label>RE08.1.19_IASRecordsAlgorithmsUse</rdfs:label>
        <owl:versionInfo>page 83</owl:versionInfo>
    </owl:Class>
    


    <!-- https://savage.nps.edu/EthicalControl/ontologies/MissionExecutionOntology#RE08.1.2 -->

    <owl:Class rdf:about="https://savage.nps.edu/EthicalControl/ontologies/MissionExecutionOntology#RE08.1.2">
        <rdfs:subClassOf rdf:resource="https://savage.nps.edu/EthicalControl/ontologies/MissionExecutionOntology#DADM08.1"/>
        <rdfs:comment>Is the IAS instrumented with the internal and external environmental sensors needed to support the collection of all required operational audit log data fields?</rdfs:comment>
        <rdfs:label>RE08.1.2_OperationalDataSupportingSensors</rdfs:label>
        <owl:versionInfo>page 82</owl:versionInfo>
    </owl:Class>
    


    <!-- https://savage.nps.edu/EthicalControl/ontologies/MissionExecutionOntology#RE08.1.20 -->

    <owl:Class rdf:about="https://savage.nps.edu/EthicalControl/ontologies/MissionExecutionOntology#RE08.1.20">
        <rdfs:subClassOf rdf:resource="https://savage.nps.edu/EthicalControl/ontologies/MissionExecutionOntology#DADM08.1"/>
        <rdfs:comment>Does the IAS record all the training data dependencies of all algorithms in use (to include any version number) that are utilized to produce an action/decision?</rdfs:comment>
        <rdfs:label>RE08.1.20_IASRecordsTrainingDataDependencies</rdfs:label>
        <owl:versionInfo>page 83</owl:versionInfo>
    </owl:Class>
    


    <!-- https://savage.nps.edu/EthicalControl/ontologies/MissionExecutionOntology#RE08.1.21 -->

    <owl:Class rdf:about="https://savage.nps.edu/EthicalControl/ontologies/MissionExecutionOntology#RE08.1.21">
        <rdfs:subClassOf rdf:resource="https://savage.nps.edu/EthicalControl/ontologies/MissionExecutionOntology#DADM08.1"/>
        <rdfs:comment>Does the IAS record its connections to, data exchanges with, and interdependencies with, other external systems to include other IAS?</rdfs:comment>
        <rdfs:label>RE08.1.21_IASRecordsExternalsystemCommunicationsExchanges</rdfs:label>
        <owl:versionInfo>page 83</owl:versionInfo>
    </owl:Class>
    


    <!-- https://savage.nps.edu/EthicalControl/ontologies/MissionExecutionOntology#RE08.1.22 -->

    <owl:Class rdf:about="https://savage.nps.edu/EthicalControl/ontologies/MissionExecutionOntology#RE08.1.22">
        <rdfs:subClassOf rdf:resource="https://savage.nps.edu/EthicalControl/ontologies/MissionExecutionOntology#DADM08.1"/>
        <rdfs:comment>Does the IAS record the loss of data signal connections?</rdfs:comment>
        <rdfs:label>RE08.1.22_IASRecordsLossDataSignal</rdfs:label>
        <owl:versionInfo>page 83</owl:versionInfo>
    </owl:Class>
    


    <!-- https://savage.nps.edu/EthicalControl/ontologies/MissionExecutionOntology#RE08.1.23 -->

    <owl:Class rdf:about="https://savage.nps.edu/EthicalControl/ontologies/MissionExecutionOntology#RE08.1.23">
        <rdfs:subClassOf rdf:resource="https://savage.nps.edu/EthicalControl/ontologies/MissionExecutionOntology#DADM08.1"/>
        <rdfs:comment>Does the IAS record connections, data exchanges and interdependencies between its own internal subsystems?</rdfs:comment>
        <rdfs:label>RE08.1.23_IASRecordsIntersystemCommunicationsExchanges</rdfs:label>
        <owl:versionInfo>page 83</owl:versionInfo>
    </owl:Class>
    


    <!-- https://savage.nps.edu/EthicalControl/ontologies/MissionExecutionOntology#RE08.1.24 -->

    <owl:Class rdf:about="https://savage.nps.edu/EthicalControl/ontologies/MissionExecutionOntology#RE08.1.24">
        <rdfs:subClassOf rdf:resource="https://savage.nps.edu/EthicalControl/ontologies/MissionExecutionOntology#DADM08.1"/>
        <rdfs:comment>Does the IAS record data from battle damage assessments?</rdfs:comment>
        <rdfs:label>RE08.1.24_IASRecordsBDA</rdfs:label>
        <owl:versionInfo>page 83</owl:versionInfo>
    </owl:Class>
    


    <!-- https://savage.nps.edu/EthicalControl/ontologies/MissionExecutionOntology#RE08.1.25 -->

    <owl:Class rdf:about="https://savage.nps.edu/EthicalControl/ontologies/MissionExecutionOntology#RE08.1.25">
        <rdfs:subClassOf rdf:resource="https://savage.nps.edu/EthicalControl/ontologies/MissionExecutionOntology#DADM08.1"/>
        <rdfs:comment>Does the IAS record data regarding technical malfunctions and degradations of performance?</rdfs:comment>
        <rdfs:label>RE08.1.25_IASRecordsTechnicalMalfunctions</rdfs:label>
        <owl:versionInfo>page 83</owl:versionInfo>
    </owl:Class>
    


    <!-- https://savage.nps.edu/EthicalControl/ontologies/MissionExecutionOntology#RE08.1.26 -->

    <owl:Class rdf:about="https://savage.nps.edu/EthicalControl/ontologies/MissionExecutionOntology#RE08.1.26">
        <rdfs:subClassOf rdf:resource="https://savage.nps.edu/EthicalControl/ontologies/MissionExecutionOntology#DADM08.1"/>
        <rdfs:comment>Does the IAS record its position relative to all battlespace management areas, including both exclusion and inclusion areas (e.g., Notices to Airman and Mariners)?</rdfs:comment>
        <rdfs:label>RE08.1.26_IASRecordsPosition</rdfs:label>
        <owl:versionInfo>page 83</owl:versionInfo>
    </owl:Class>
    


    <!-- https://savage.nps.edu/EthicalControl/ontologies/MissionExecutionOntology#RE08.1.27 -->

    <owl:Class rdf:about="https://savage.nps.edu/EthicalControl/ontologies/MissionExecutionOntology#RE08.1.27">
        <rdfs:subClassOf rdf:resource="https://savage.nps.edu/EthicalControl/ontologies/MissionExecutionOntology#DADM08.1"/>
        <rdfs:comment>Does the IAS record the results of any risk assessments made on board during a mission and the resultant mitigation actions taken?</rdfs:comment>
        <rdfs:label>RE08.1.27_IASRecordsRiskAssessments</rdfs:label>
        <owl:versionInfo>page 83</owl:versionInfo>
    </owl:Class>
    


    <!-- https://savage.nps.edu/EthicalControl/ontologies/MissionExecutionOntology#RE08.1.3 -->

    <owl:Class rdf:about="https://savage.nps.edu/EthicalControl/ontologies/MissionExecutionOntology#RE08.1.3">
        <rdfs:subClassOf rdf:resource="https://savage.nps.edu/EthicalControl/ontologies/MissionExecutionOntology#DADM08.1"/>
        <rdfs:comment>Is the IAS equipped with sufficient data storage and/or transmission capabilities to capture and retain data at the frequency required for post-operational uses and for the entire duration of the mission?</rdfs:comment>
        <rdfs:label>RE08.1.3_AdequateStorageTransmissionOperationalAuditData</rdfs:label>
        <owl:versionInfo>page 82</owl:versionInfo>
    </owl:Class>
    


    <!-- https://savage.nps.edu/EthicalControl/ontologies/MissionExecutionOntology#RE08.1.4 -->

    <owl:Class rdf:about="https://savage.nps.edu/EthicalControl/ontologies/MissionExecutionOntology#RE08.1.4">
        <rdfs:subClassOf rdf:resource="https://savage.nps.edu/EthicalControl/ontologies/MissionExecutionOntology#DADM08.1"/>
        <rdfs:comment>Are all data descriptions understandable to non-technical persons who may use the data logs for post-operational reconstruction and analysis?</rdfs:comment>
        <rdfs:label>RE08.1.4_OperationalDataFieldsDocumentedAvailable</rdfs:label>
        <owl:versionInfo>page 82</owl:versionInfo>
    </owl:Class>
    


    <!-- https://savage.nps.edu/EthicalControl/ontologies/MissionExecutionOntology#RE08.1.5 -->

    <owl:Class rdf:about="https://savage.nps.edu/EthicalControl/ontologies/MissionExecutionOntology#RE08.1.5">
        <rdfs:subClassOf rdf:resource="https://savage.nps.edu/EthicalControl/ontologies/MissionExecutionOntology#DADM08.1"/>
        <rdfs:comment>Has the data in the operational audit log been verified to be of sufficient quality, quantity, and provenance to support any potential post-operational legal proceeding?</rdfs:comment>
        <rdfs:label>RE08.1.5_OperationalAuditDataLegallySufficient</rdfs:label>
        <owl:versionInfo>page 82</owl:versionInfo>
    </owl:Class>
    


    <!-- https://savage.nps.edu/EthicalControl/ontologies/MissionExecutionOntology#RE08.1.6 -->

    <owl:Class rdf:about="https://savage.nps.edu/EthicalControl/ontologies/MissionExecutionOntology#RE08.1.6">
        <rdfs:subClassOf rdf:resource="https://savage.nps.edu/EthicalControl/ontologies/MissionExecutionOntology#DADM08.1"/>
        <rdfs:comment>Are access controls in place to limit access to the IAS operational audit logs to authorized personal only?</rdfs:comment>
        <rdfs:label>RE08.1.6_OperationalAuditDataAccessControls</rdfs:label>
        <owl:versionInfo>page 82</owl:versionInfo>
    </owl:Class>
    


    <!-- https://savage.nps.edu/EthicalControl/ontologies/MissionExecutionOntology#RE08.1.7 -->

    <owl:Class rdf:about="https://savage.nps.edu/EthicalControl/ontologies/MissionExecutionOntology#RE08.1.7">
        <rdfs:subClassOf rdf:resource="https://savage.nps.edu/EthicalControl/ontologies/MissionExecutionOntology#DADM08.1"/>
        <rdfs:comment>Are challenges to the use of an IAS based on examination of the IAS operational audit log, and the results of those challenges recorded by the audit log data steward?</rdfs:comment>
        <rdfs:label>RE08.1.7_OperationalAuditDataStewardIssuesRecorded</rdfs:label>
        <owl:versionInfo>page 82</owl:versionInfo>
    </owl:Class>
    


    <!-- https://savage.nps.edu/EthicalControl/ontologies/MissionExecutionOntology#RE08.1.8 -->

    <owl:Class rdf:about="https://savage.nps.edu/EthicalControl/ontologies/MissionExecutionOntology#RE08.1.8">
        <rdfs:subClassOf rdf:resource="https://savage.nps.edu/EthicalControl/ontologies/MissionExecutionOntology#DADM08.1"/>
        <rdfs:comment>Are all requests for explanations or inspections of the IAS operational audit log, and the results of those inspections recorded by the audit log data steward?</rdfs:comment>
        <rdfs:label>RE08.1.8_OperationalAuditLogAccessesDocumented</rdfs:label>
        <owl:versionInfo>page 82</owl:versionInfo>
    </owl:Class>
    


    <!-- https://savage.nps.edu/EthicalControl/ontologies/MissionExecutionOntology#RE08.1.9 -->

    <owl:Class rdf:about="https://savage.nps.edu/EthicalControl/ontologies/MissionExecutionOntology#RE08.1.9">
        <rdfs:subClassOf rdf:resource="https://savage.nps.edu/EthicalControl/ontologies/MissionExecutionOntology#DADM08.1"/>
        <rdfs:comment>Is there a procedure in place to request, and approve requests, to examine the operational audit log?</rdfs:comment>
        <rdfs:label>RE08.1.9_OperationalAuditDataLogAccessProceedures</rdfs:label>
        <owl:versionInfo>page 82</owl:versionInfo>
    </owl:Class>
    


    <!-- https://savage.nps.edu/EthicalControl/ontologies/MissionExecutionOntology#RE08.2.1 -->

    <owl:Class rdf:about="https://savage.nps.edu/EthicalControl/ontologies/MissionExecutionOntology#RE08.2.1">
        <rdfs:subClassOf rdf:resource="https://savage.nps.edu/EthicalControl/ontologies/MissionExecutionOntology#DADM08.2"/>
        <rdfs:comment>Are all decisions made by the IAS traceable back to the sensor data, operator commands, algorithms and training data used?</rdfs:comment>
        <rdfs:label>RE08.2.1_DecisionsSensorDataC2AlgorithmsTrainingData</rdfs:label>
        <owl:versionInfo>page 83</owl:versionInfo>
    </owl:Class>
    


    <!-- https://savage.nps.edu/EthicalControl/ontologies/MissionExecutionOntology#RE08.2.2 -->

    <owl:Class rdf:about="https://savage.nps.edu/EthicalControl/ontologies/MissionExecutionOntology#RE08.2.2">
        <rdfs:subClassOf rdf:resource="https://savage.nps.edu/EthicalControl/ontologies/MissionExecutionOntology#DADM08.2"/>
        <rdfs:comment>Can all actions/decisions made by an IAS and the human operator who authorized the action/decision be traced back to the military objective or mission orders they were intended to support?</rdfs:comment>
        <rdfs:label>RE08.2.2_DecisionsMapObjective</rdfs:label>
        <owl:versionInfo>page 83</owl:versionInfo>
    </owl:Class>
    


    <!-- https://savage.nps.edu/EthicalControl/ontologies/MissionExecutionOntology#RE08.2.3 -->

    <owl:Class rdf:about="https://savage.nps.edu/EthicalControl/ontologies/MissionExecutionOntology#RE08.2.3">
        <rdfs:subClassOf rdf:resource="https://savage.nps.edu/EthicalControl/ontologies/MissionExecutionOntology#DADM08.2"/>
        <rdfs:comment>Can human operators retrace decision steps and interactions with the environment that resulted in an IAS action/decision of interest?</rdfs:comment>
        <rdfs:label>RE08.2.3_DecisionTraceabilityEnvironment</rdfs:label>
        <owl:versionInfo>page 83</owl:versionInfo>
    </owl:Class>
    


    <!-- https://savage.nps.edu/EthicalControl/ontologies/MissionExecutionOntology#RE08.2.4 -->

    <owl:Class rdf:about="https://savage.nps.edu/EthicalControl/ontologies/MissionExecutionOntology#RE08.2.4">
        <rdfs:subClassOf rdf:resource="https://savage.nps.edu/EthicalControl/ontologies/MissionExecutionOntology#DADM08.2"/>
        <rdfs:comment>Are the inputs from component autonomous subsystems that were used by the IAS to make decisions available for review by a human operator?</rdfs:comment>
        <rdfs:label>RE08.2.4_DecisionSubsystemInformationHumanReview</rdfs:label>
        <owl:versionInfo>page 83</owl:versionInfo>
    </owl:Class>
    


    <!-- https://savage.nps.edu/EthicalControl/ontologies/MissionExecutionOntology#RE08.3.1 -->

    <owl:Class rdf:about="https://savage.nps.edu/EthicalControl/ontologies/MissionExecutionOntology#RE08.3.1">
        <rdfs:subClassOf rdf:resource="https://savage.nps.edu/EthicalControl/ontologies/MissionExecutionOntology#DADM08.3"/>
        <rdfs:comment>Does the IAS operational audit log have a metadata field identifying the date after which retention is no longer required?</rdfs:comment>
        <rdfs:label>RE08.3.1_AuditLogPurgeDate</rdfs:label>
        <owl:versionInfo>page 84</owl:versionInfo>
    </owl:Class>
    


    <!-- https://savage.nps.edu/EthicalControl/ontologies/MissionExecutionOntology#RE08.3.2 -->

    <owl:Class rdf:about="https://savage.nps.edu/EthicalControl/ontologies/MissionExecutionOntology#RE08.3.2">
        <rdfs:subClassOf rdf:resource="https://savage.nps.edu/EthicalControl/ontologies/MissionExecutionOntology#DADM08.3"/>
        <rdfs:comment>Is IAS operational audit log data deleted automatically or manually with human oversight when its retention date is reached?</rdfs:comment>
        <rdfs:label>RE08.3.2_AuditLogPurgeMethod</rdfs:label>
        <owl:versionInfo>page 84</owl:versionInfo>
    </owl:Class>
    


    <!-- https://savage.nps.edu/EthicalControl/ontologies/MissionExecutionOntology#RE08.3.3 -->

    <owl:Class rdf:about="https://savage.nps.edu/EthicalControl/ontologies/MissionExecutionOntology#RE08.3.3">
        <rdfs:subClassOf rdf:resource="https://savage.nps.edu/EthicalControl/ontologies/MissionExecutionOntology#DADM08.3"/>
        <rdfs:comment>Are IAS operational audit logs retained beyond the statute of limitations date for any illegal acts that could possibly have been committed during an operation?</rdfs:comment>
        <rdfs:label>RE08.3.3_AuditLogRetentionStatueLegalActions</rdfs:label>
        <owl:versionInfo>page 84</owl:versionInfo>
    </owl:Class>
    


    <!-- https://savage.nps.edu/EthicalControl/ontologies/MissionExecutionOntology#RE08.3.4 -->

    <owl:Class rdf:about="https://savage.nps.edu/EthicalControl/ontologies/MissionExecutionOntology#RE08.3.4">
        <rdfs:subClassOf rdf:resource="https://savage.nps.edu/EthicalControl/ontologies/MissionExecutionOntology#DADM08.3"/>
        <rdfs:comment>Do acquisition professionals who may wish to use IAS operational audit logs to improve the performance of this, or some other IAS, have a role in deciding when the audit logs are no longer retained?</rdfs:comment>
        <rdfs:label>RE08.3.4_AuditLogExtraRetentionAcquisition</rdfs:label>
        <owl:versionInfo>page 84</owl:versionInfo>
    </owl:Class>
    


    <!-- https://savage.nps.edu/EthicalControl/ontologies/MissionExecutionOntology#RE08.3.5 -->

    <owl:Class rdf:about="https://savage.nps.edu/EthicalControl/ontologies/MissionExecutionOntology#RE08.3.5">
        <rdfs:subClassOf rdf:resource="https://savage.nps.edu/EthicalControl/ontologies/MissionExecutionOntology#DADM08.3"/>
        <rdfs:comment>Do military commanders, trainers, and doctrine writers who may wish to use IAS operational audit logs to improve future tactics, techniques and procedures have a role in deciding when the audit logs are no longer retained?</rdfs:comment>
        <rdfs:label>RE08.3.5_AuditLogExtraRetentionOthers</rdfs:label>
        <owl:versionInfo>page 84</owl:versionInfo>
    </owl:Class>
    


    <!-- https://savage.nps.edu/EthicalControl/ontologies/MissionExecutionOntology#RE08.3.6 -->

    <owl:Class rdf:about="https://savage.nps.edu/EthicalControl/ontologies/MissionExecutionOntology#RE08.3.6">
        <rdfs:subClassOf rdf:resource="https://savage.nps.edu/EthicalControl/ontologies/MissionExecutionOntology#DADM08.3"/>
        <rdfs:comment>Are data storage and transmission resources sufficient to retain all of the IAS operational audit log data created during the contemplated life cycle of the IAS?</rdfs:comment>
        <rdfs:label>RE08.3.6_DataLogStorageTransmissionSufficient</rdfs:label>
        <owl:versionInfo>page 84</owl:versionInfo>
    </owl:Class>
    


    <!-- https://savage.nps.edu/EthicalControl/ontologies/MissionExecutionOntology#RE08.3.7 -->

    <owl:Class rdf:about="https://savage.nps.edu/EthicalControl/ontologies/MissionExecutionOntology#RE08.3.7">
        <rdfs:subClassOf rdf:resource="https://savage.nps.edu/EthicalControl/ontologies/MissionExecutionOntology#DADM08.3"/>
        <rdfs:comment>Do the IAS operational audit logs require any additional handling caveats above and beyond existing document retention and destruction policies?</rdfs:comment>
        <rdfs:label>RE08.3.7_OperationalAuditLogsAdditionalHandlingCaveats</rdfs:label>
        <owl:versionInfo>page 84</owl:versionInfo>
    </owl:Class>
    


    <!-- https://savage.nps.edu/EthicalControl/ontologies/MissionExecutionOntology#RE08.3.8 -->

    <owl:Class rdf:about="https://savage.nps.edu/EthicalControl/ontologies/MissionExecutionOntology#RE08.3.8">
        <rdfs:subClassOf rdf:resource="https://savage.nps.edu/EthicalControl/ontologies/MissionExecutionOntology#DADM08.3"/>
        <rdfs:comment>Is retained IAS operational audit log data that is subsequently reused, reassessed first for its quality and continued relevancy and applicability?</rdfs:comment>
        <rdfs:label>RE08.3.8_OperationalAuditLogsQualityAssessed</rdfs:label>
        <owl:versionInfo>page 84</owl:versionInfo>
    </owl:Class>
    


    <!-- https://savage.nps.edu/EthicalControl/ontologies/MissionExecutionOntology#RE08.3.9 -->

    <owl:Class rdf:about="https://savage.nps.edu/EthicalControl/ontologies/MissionExecutionOntology#RE08.3.9">
        <rdfs:subClassOf rdf:resource="https://savage.nps.edu/EthicalControl/ontologies/MissionExecutionOntology#DADM08.3"/>
        <rdfs:comment>Are all accesses to retained IAS operational audit log data, either granted or denied, recorded by the data steward?</rdfs:comment>
        <rdfs:label>RE08.3.9_OperationalDataLogAccessRequestsRecorded</rdfs:label>
        <owl:versionInfo>page 84</owl:versionInfo>
    </owl:Class>
    


    <!-- https://savage.nps.edu/EthicalControl/ontologies/MissionExecutionOntology#RE08.4.1 -->

    <owl:Class rdf:about="https://savage.nps.edu/EthicalControl/ontologies/MissionExecutionOntology#RE08.4.1">
        <rdfs:subClassOf rdf:resource="https://savage.nps.edu/EthicalControl/ontologies/MissionExecutionOntology#DADM08.4"/>
        <rdfs:comment>Does the IAS operational audit log enable training data generation for subsequent IAS algorithm development?</rdfs:comment>
        <rdfs:label>RE08.4.1_OperationalAuditLogEnableFutureAlgorithmDevemelopment</rdfs:label>
        <owl:versionInfo>page 84</owl:versionInfo>
    </owl:Class>
    


    <!-- https://savage.nps.edu/EthicalControl/ontologies/MissionExecutionOntology#RE08.4.2 -->

    <owl:Class rdf:about="https://savage.nps.edu/EthicalControl/ontologies/MissionExecutionOntology#RE08.4.2">
        <rdfs:subClassOf rdf:resource="https://savage.nps.edu/EthicalControl/ontologies/MissionExecutionOntology#DADM08.4"/>
        <rdfs:comment>Does the IAS operational audit log enable accountability for adverse actions?</rdfs:comment>
        <rdfs:label>RE08.4.2_OperationalAuditLogEnableAccountabilityAdverseActions</rdfs:label>
        <owl:versionInfo>page 84</owl:versionInfo>
    </owl:Class>
    


    <!-- https://savage.nps.edu/EthicalControl/ontologies/MissionExecutionOntology#RE08.4.3 -->

    <owl:Class rdf:about="https://savage.nps.edu/EthicalControl/ontologies/MissionExecutionOntology#RE08.4.3">
        <rdfs:subClassOf rdf:resource="https://savage.nps.edu/EthicalControl/ontologies/MissionExecutionOntology#DADM08.4"/>
        <rdfs:comment>Does the IAS operational audit log enable further IAS refinement and testing?</rdfs:comment>
        <rdfs:label>RE08.4.3_OperationalAuditLogEnableRefinementTesting</rdfs:label>
        <owl:versionInfo>page 84</owl:versionInfo>
    </owl:Class>
    


    <!-- https://savage.nps.edu/EthicalControl/ontologies/MissionExecutionOntology#RE08.4.4 -->

    <owl:Class rdf:about="https://savage.nps.edu/EthicalControl/ontologies/MissionExecutionOntology#RE08.4.4">
        <rdfs:subClassOf rdf:resource="https://savage.nps.edu/EthicalControl/ontologies/MissionExecutionOntology#DADM08.4"/>
        <rdfs:comment>Does the IAS operational audit log enable tactics techniques and procedures development?</rdfs:comment>
        <rdfs:label>RE08.4.4_OperationalAuditLogEnableTacticsProcedures</rdfs:label>
        <owl:versionInfo>page 84</owl:versionInfo>
    </owl:Class>
    


    <!-- https://savage.nps.edu/EthicalControl/ontologies/MissionExecutionOntology#RE08.4.5 -->

    <owl:Class rdf:about="https://savage.nps.edu/EthicalControl/ontologies/MissionExecutionOntology#RE08.4.5">
        <rdfs:subClassOf rdf:resource="https://savage.nps.edu/EthicalControl/ontologies/MissionExecutionOntology#DADM08.4"/>
        <rdfs:comment>Does the IAS operational audit log enable human operator training?</rdfs:comment>
        <rdfs:label>RE08.4.5_OperationalAuditLogEnableOperatorTraining</rdfs:label>
        <owl:versionInfo>page 84</owl:versionInfo>
    </owl:Class>
    


    <!-- https://savage.nps.edu/EthicalControl/ontologies/MissionExecutionOntology#RE08.4.6 -->

    <owl:Class rdf:about="https://savage.nps.edu/EthicalControl/ontologies/MissionExecutionOntology#RE08.4.6">
        <rdfs:subClassOf rdf:resource="https://savage.nps.edu/EthicalControl/ontologies/MissionExecutionOntology#DADM08.4"/>
        <rdfs:comment>Does the IAS operational audit log enable post mission hot washes for corrective action?</rdfs:comment>
        <rdfs:label>RE08.4.6_OperationalAuditLogEnablePostMissionReview</rdfs:label>
        <owl:versionInfo>page 84</owl:versionInfo>
    </owl:Class>
    


    <!-- https://savage.nps.edu/EthicalControl/ontologies/MissionExecutionOntology#RE08.4.7 -->

    <owl:Class rdf:about="https://savage.nps.edu/EthicalControl/ontologies/MissionExecutionOntology#RE08.4.7">
        <rdfs:subClassOf rdf:resource="https://savage.nps.edu/EthicalControl/ontologies/MissionExecutionOntology#DADM08.4"/>
        <rdfs:comment>Does the IAS operational audit log enable acquisition of IAS not related to the current IAS or its mission(s)?</rdfs:comment>
        <rdfs:label>RE08.4.7_OperationalAuditLogEnableAcquisitionDifferentIAS</rdfs:label>
        <owl:versionInfo>page 84</owl:versionInfo>
    </owl:Class>
    


    <!-- https://savage.nps.edu/EthicalControl/ontologies/MissionExecutionOntology#RE08.4.8 -->

    <owl:Class rdf:about="https://savage.nps.edu/EthicalControl/ontologies/MissionExecutionOntology#RE08.4.8">
        <rdfs:subClassOf rdf:resource="https://savage.nps.edu/EthicalControl/ontologies/MissionExecutionOntology#DADM08.4"/>
        <rdfs:comment>Are the IAS operational audit logs made available for internal oversight?</rdfs:comment>
        <rdfs:label>RE08.4.8_OperationalAuditLogAvailableInternalOversight</rdfs:label>
        <owl:versionInfo>page 85</owl:versionInfo>
    </owl:Class>
    


    <!-- https://savage.nps.edu/EthicalControl/ontologies/MissionExecutionOntology#RE08.4.9 -->

    <owl:Class rdf:about="https://savage.nps.edu/EthicalControl/ontologies/MissionExecutionOntology#RE08.4.9">
        <rdfs:subClassOf rdf:resource="https://savage.nps.edu/EthicalControl/ontologies/MissionExecutionOntology#DADM08.4"/>
        <rdfs:comment>Are the IAS operational audit logs made available for external third-party oversight?</rdfs:comment>
        <rdfs:label>RE08.4.9_OperationalAuditLogAvailableExternalOversight</rdfs:label>
        <owl:versionInfo>page 85</owl:versionInfo>
    </owl:Class>
    


    <!-- https://savage.nps.edu/EthicalControl/ontologies/MissionExecutionOntology#RE09.1.1 -->

    <owl:Class rdf:about="https://savage.nps.edu/EthicalControl/ontologies/MissionExecutionOntology#RE09.1.1">
        <rdfs:subClassOf rdf:resource="https://savage.nps.edu/EthicalControl/ontologies/MissionExecutionOntology#DADM09.1"/>
        <rdfs:comment>Can the IAS alert the humans that they are interacting with an IAS and not another human?</rdfs:comment>
        <rdfs:label>RE09.1.1_SelfIdentificationIAS</rdfs:label>
        <owl:versionInfo>page 85</owl:versionInfo>
    </owl:Class>
    


    <!-- https://savage.nps.edu/EthicalControl/ontologies/MissionExecutionOntology#RE09.1.10 -->

    <owl:Class rdf:about="https://savage.nps.edu/EthicalControl/ontologies/MissionExecutionOntology#RE09.1.10">
        <rdfs:subClassOf rdf:resource="https://savage.nps.edu/EthicalControl/ontologies/MissionExecutionOntology#DADM09.1"/>
        <rdfs:comment>Is the rate of IAS false negative results known and below a previously defined and acceptable value?</rdfs:comment>
        <rdfs:label>RE09.1.10_IASFalseNegativeResults</rdfs:label>
        <owl:versionInfo>page 85</owl:versionInfo>
    </owl:Class>
    


    <!-- https://savage.nps.edu/EthicalControl/ontologies/MissionExecutionOntology#RE09.1.11 -->

    <owl:Class rdf:about="https://savage.nps.edu/EthicalControl/ontologies/MissionExecutionOntology#RE09.1.11">
        <rdfs:subClassOf rdf:resource="https://savage.nps.edu/EthicalControl/ontologies/MissionExecutionOntology#DADM09.1"/>
        <rdfs:comment>Is there an option to turn off the IAS if there are too many false alarms? Provision of shared situational awareness</rdfs:comment>
        <rdfs:label>RE09.1.11_IASOffOption</rdfs:label>
        <owl:versionInfo>page 85</owl:versionInfo>
    </owl:Class>
    


    <!-- https://savage.nps.edu/EthicalControl/ontologies/MissionExecutionOntology#RE09.1.12 -->

    <owl:Class rdf:about="https://savage.nps.edu/EthicalControl/ontologies/MissionExecutionOntology#RE09.1.12">
        <rdfs:subClassOf rdf:resource="https://savage.nps.edu/EthicalControl/ontologies/MissionExecutionOntology#DADM09.1"/>
        <rdfs:comment>Can the IAS communicate with all systems from which it must ingest data to achieve maximum situational awareness during the fog and friction of war?</rdfs:comment>
        <rdfs:label>RE09.1.12_CommunicationDuringFogOfWar</rdfs:label>
        <owl:versionInfo>page 85</owl:versionInfo>
    </owl:Class>
    


    <!-- https://savage.nps.edu/EthicalControl/ontologies/MissionExecutionOntology#RE09.1.13 -->

    <owl:Class rdf:about="https://savage.nps.edu/EthicalControl/ontologies/MissionExecutionOntology#RE09.1.13">
        <rdfs:subClassOf rdf:resource="https://savage.nps.edu/EthicalControl/ontologies/MissionExecutionOntology#DADM09.1"/>
        <rdfs:comment>Is the IAS equipped with system self‐monitoring sensors that can detect and communicate (internal) conditions that may lead to a negative outcome if not corrected?</rdfs:comment>
        <rdfs:label>RE09.1.13_SelfMonitoringSystem</rdfs:label>
        <owl:versionInfo>page 85</owl:versionInfo>
    </owl:Class>
    


    <!-- https://savage.nps.edu/EthicalControl/ontologies/MissionExecutionOntology#RE09.1.14 -->

    <owl:Class rdf:about="https://savage.nps.edu/EthicalControl/ontologies/MissionExecutionOntology#RE09.1.14">
        <rdfs:subClassOf rdf:resource="https://savage.nps.edu/EthicalControl/ontologies/MissionExecutionOntology#DADM09.1"/>
        <rdfs:comment>Can the IAS predict when operational design domain conditions and constraints might be violated and communicate the future time of the violations, the probability of occurrence and the severity to a human operator?</rdfs:comment>
        <rdfs:label>RE09.1.14_OperationalDesignVioloationPredictions</rdfs:label>
        <owl:versionInfo>page 86</owl:versionInfo>
    </owl:Class>
    


    <!-- https://savage.nps.edu/EthicalControl/ontologies/MissionExecutionOntology#RE09.1.15 -->

    <owl:Class rdf:about="https://savage.nps.edu/EthicalControl/ontologies/MissionExecutionOntology#RE09.1.15">
        <rdfs:subClassOf rdf:resource="https://savage.nps.edu/EthicalControl/ontologies/MissionExecutionOntology#DADM09.1"/>
        <rdfs:comment>Can the IAS and the human teammates effectively communicate their state, intent, and current problems to the other teammate?</rdfs:comment>
        <rdfs:label>RE09.1.15_IASHumanTeamCommunication</rdfs:label>
        <owl:versionInfo>page 86</owl:versionInfo>
    </owl:Class>
    


    <!-- https://savage.nps.edu/EthicalControl/ontologies/MissionExecutionOntology#RE09.1.16 -->

    <owl:Class rdf:about="https://savage.nps.edu/EthicalControl/ontologies/MissionExecutionOntology#RE09.1.16">
        <rdfs:subClassOf rdf:resource="https://savage.nps.edu/EthicalControl/ontologies/MissionExecutionOntology#DADM09.1"/>
        <rdfs:comment>Can the IAS communicate the current and predicted future status of fuel and ammunition levels to the human operator?</rdfs:comment>
        <rdfs:label>RE09.1.16_IASFeulAmmoLevelPredictions</rdfs:label>
        <owl:versionInfo>page 86</owl:versionInfo>
    </owl:Class>
    


    <!-- https://savage.nps.edu/EthicalControl/ontologies/MissionExecutionOntology#RE09.1.17 -->

    <owl:Class rdf:about="https://savage.nps.edu/EthicalControl/ontologies/MissionExecutionOntology#RE09.1.17">
        <rdfs:subClassOf rdf:resource="https://savage.nps.edu/EthicalControl/ontologies/MissionExecutionOntology#DADM09.1"/>
        <rdfs:comment>Can the IAS communicate its current and predicted future availability for mission execution to the human operator?</rdfs:comment>
        <rdfs:label>RE09.1.17_IASMissionExecutionAvalilabillityPrediction</rdfs:label>
        <owl:versionInfo>page 86</owl:versionInfo>
    </owl:Class>
    


    <!-- https://savage.nps.edu/EthicalControl/ontologies/MissionExecutionOntology#RE09.1.18 -->

    <owl:Class rdf:about="https://savage.nps.edu/EthicalControl/ontologies/MissionExecutionOntology#RE09.1.18">
        <rdfs:subClassOf rdf:resource="https://savage.nps.edu/EthicalControl/ontologies/MissionExecutionOntology#DADM09.1"/>
        <rdfs:comment>Can the IAS communicate (previously defined) system malfunctions to the human operator?</rdfs:comment>
        <rdfs:label>RE09.1.18_IASMalfunctionCommunication</rdfs:label>
        <owl:versionInfo>page 86</owl:versionInfo>
    </owl:Class>
    


    <!-- https://savage.nps.edu/EthicalControl/ontologies/MissionExecutionOntology#RE09.1.19 -->

    <owl:Class rdf:about="https://savage.nps.edu/EthicalControl/ontologies/MissionExecutionOntology#RE09.1.19">
        <rdfs:subClassOf rdf:resource="https://savage.nps.edu/EthicalControl/ontologies/MissionExecutionOntology#DADM09.1"/>
        <rdfs:comment>Can the IAS communicate critical messages to the human operator?</rdfs:comment>
        <rdfs:label>RE09.1.19_IASCriticalMessageCommunication</rdfs:label>
        <owl:versionInfo>page 86</owl:versionInfo>
    </owl:Class>
    


    <!-- https://savage.nps.edu/EthicalControl/ontologies/MissionExecutionOntology#RE09.1.2 -->

    <owl:Class rdf:about="https://savage.nps.edu/EthicalControl/ontologies/MissionExecutionOntology#RE09.1.2">
        <rdfs:subClassOf rdf:resource="https://savage.nps.edu/EthicalControl/ontologies/MissionExecutionOntology#DADM09.1"/>
        <rdfs:comment>Can the IAS distinguish between blue forces with human operators and other blue force IAS?</rdfs:comment>
        <rdfs:label>RE09.1.2_DistinguishBlueForceHumansIAS</rdfs:label>
        <owl:versionInfo>page 85</owl:versionInfo>
    </owl:Class>
    


    <!-- https://savage.nps.edu/EthicalControl/ontologies/MissionExecutionOntology#RE09.1.20 -->

    <owl:Class rdf:about="https://savage.nps.edu/EthicalControl/ontologies/MissionExecutionOntology#RE09.1.20">
        <rdfs:subClassOf rdf:resource="https://savage.nps.edu/EthicalControl/ontologies/MissionExecutionOntology#DADM09.1"/>
        <rdfs:comment>Can the IAS detect both sharp and gradual changes in its operational environment and provide alerts to the human operator and other systems based on criticality?</rdfs:comment>
        <rdfs:label>RE09.1.20_IASEnviromentChangeAlerts</rdfs:label>
        <owl:versionInfo>page 86</owl:versionInfo>
    </owl:Class>
    


    <!-- https://savage.nps.edu/EthicalControl/ontologies/MissionExecutionOntology#RE09.1.21 -->

    <owl:Class rdf:about="https://savage.nps.edu/EthicalControl/ontologies/MissionExecutionOntology#RE09.1.21">
        <rdfs:subClassOf rdf:resource="https://savage.nps.edu/EthicalControl/ontologies/MissionExecutionOntology#DADM09.1"/>
        <rdfs:comment>Can the IAS detect both sharp and gradual changes in its own performance and provide alerts to the human operator and other systems based on criticality?</rdfs:comment>
        <rdfs:label>RE09.1.21_IASPerformanceChangeAlerts</rdfs:label>
        <owl:versionInfo>page 86</owl:versionInfo>
    </owl:Class>
    


    <!-- https://savage.nps.edu/EthicalControl/ontologies/MissionExecutionOntology#RE09.1.22 -->

    <owl:Class rdf:about="https://savage.nps.edu/EthicalControl/ontologies/MissionExecutionOntology#RE09.1.22">
        <rdfs:subClassOf rdf:resource="https://savage.nps.edu/EthicalControl/ontologies/MissionExecutionOntology#DADM09.1"/>
        <rdfs:comment>If an IAS’s autonomous functionality fails and it must transfer command and control of itself to a human operator, will that operator have been sufficiently engaged and be able to understand the IAS’s current situation in time to safely repurpose the IAS or avert danger/loss of the IAS?</rdfs:comment>
        <rdfs:label>RE09.1.22_IASFuncitionalityFailureConcerns</rdfs:label>
        <owl:versionInfo>page 86</owl:versionInfo>
    </owl:Class>
    


    <!-- https://savage.nps.edu/EthicalControl/ontologies/MissionExecutionOntology#RE09.1.23 -->

    <owl:Class rdf:about="https://savage.nps.edu/EthicalControl/ontologies/MissionExecutionOntology#RE09.1.23">
        <rdfs:subClassOf rdf:resource="https://savage.nps.edu/EthicalControl/ontologies/MissionExecutionOntology#DADM09.1"/>
        <rdfs:comment>Can the IAS determine when it is inappropriate to interrupt a human operator with a query for assistance?</rdfs:comment>
        <rdfs:label>RE09.1.23_IASHumanAssistanceQueries</rdfs:label>
        <owl:versionInfo>page 86</owl:versionInfo>
    </owl:Class>
    


    <!-- https://savage.nps.edu/EthicalControl/ontologies/MissionExecutionOntology#RE09.1.24 -->

    <owl:Class rdf:about="https://savage.nps.edu/EthicalControl/ontologies/MissionExecutionOntology#RE09.1.24">
        <rdfs:subClassOf rdf:resource="https://savage.nps.edu/EthicalControl/ontologies/MissionExecutionOntology#DADM09.1"/>
        <rdfs:comment>Can the IAS recognize the difference between rules-based decisions and value/judgement-based decisions and query the human operator for guidance in the latter case?</rdfs:comment>
        <rdfs:label>RE09.1.24_RuleVsValueDecisionsRecognition</rdfs:label>
        <owl:versionInfo>page 86</owl:versionInfo>
    </owl:Class>
    


    <!-- https://savage.nps.edu/EthicalControl/ontologies/MissionExecutionOntology#RE09.1.25 -->

    <owl:Class rdf:about="https://savage.nps.edu/EthicalControl/ontologies/MissionExecutionOntology#RE09.1.25">
        <rdfs:subClassOf rdf:resource="https://savage.nps.edu/EthicalControl/ontologies/MissionExecutionOntology#DADM09.1"/>
        <rdfs:comment>Can the IAS recognize the difference between decisions based on deductive versus inductive vs abductive reasoning and query the human operator for guidance in the latter case?</rdfs:comment>
        <rdfs:label>RE09.1.25_DeductiveVsInductiveVsAbductiveDecisions</rdfs:label>
        <owl:versionInfo>page 86</owl:versionInfo>
    </owl:Class>
    


    <!-- https://savage.nps.edu/EthicalControl/ontologies/MissionExecutionOntology#RE09.1.26 -->

    <owl:Class rdf:about="https://savage.nps.edu/EthicalControl/ontologies/MissionExecutionOntology#RE09.1.26">
        <rdfs:subClassOf rdf:resource="https://savage.nps.edu/EthicalControl/ontologies/MissionExecutionOntology#DADM09.1"/>
        <rdfs:comment>Can the IAS upload and implement any doctrine or rules of engagement that identify predetermined situations where human guidance is a prerequisite to taking further action?</rdfs:comment>
        <rdfs:label>RE09.1.26_DoctrineWithHumanGuidanceImplementation</rdfs:label>
        <owl:versionInfo>page 86</owl:versionInfo>
    </owl:Class>
    


    <!-- https://savage.nps.edu/EthicalControl/ontologies/MissionExecutionOntology#RE09.1.27 -->

    <owl:Class rdf:about="https://savage.nps.edu/EthicalControl/ontologies/MissionExecutionOntology#RE09.1.27">
        <rdfs:subClassOf rdf:resource="https://savage.nps.edu/EthicalControl/ontologies/MissionExecutionOntology#DADM09.1"/>
        <rdfs:comment>Can the IAS identify ambiguous or incomplete instructions and request clarification from the human operator in sufficient time to be operationally effective or to prevent mistakes/mishaps?</rdfs:comment>
        <rdfs:label>RE09.1.27_IASIntructionAmbiguityIdenification</rdfs:label>
        <owl:versionInfo>page 86</owl:versionInfo>
    </owl:Class>
    


    <!-- https://savage.nps.edu/EthicalControl/ontologies/MissionExecutionOntology#RE09.1.28 -->

    <owl:Class rdf:about="https://savage.nps.edu/EthicalControl/ontologies/MissionExecutionOntology#RE09.1.28">
        <rdfs:subClassOf rdf:resource="https://savage.nps.edu/EthicalControl/ontologies/MissionExecutionOntology#DADM09.1"/>
        <rdfs:comment>Can the IAS detect anomalies and seek human guidance when its programming says that it is under attack, but the political situation is completely benign?</rdfs:comment>
        <rdfs:label>RE09.1.28_AnomalyDetectionAndHumanGuidance</rdfs:label>
        <owl:versionInfo>page 86</owl:versionInfo>
    </owl:Class>
    


    <!-- https://savage.nps.edu/EthicalControl/ontologies/MissionExecutionOntology#RE09.1.3 -->

    <owl:Class rdf:about="https://savage.nps.edu/EthicalControl/ontologies/MissionExecutionOntology#RE09.1.3">
        <rdfs:subClassOf rdf:resource="https://savage.nps.edu/EthicalControl/ontologies/MissionExecutionOntology#DADM09.1"/>
        <rdfs:comment>Will continued reliance on the IAS cause human operator skills to diminish such that they can no longer back up the IAS in the event that the IAS becomes unavailable?</rdfs:comment>
        <rdfs:label>RE09.1.3_IASRelianceDiminishHumanSkills</rdfs:label>
        <owl:versionInfo>page 85</owl:versionInfo>
    </owl:Class>
    


    <!-- https://savage.nps.edu/EthicalControl/ontologies/MissionExecutionOntology#RE09.1.4 -->

    <owl:Class rdf:about="https://savage.nps.edu/EthicalControl/ontologies/MissionExecutionOntology#RE09.1.4">
        <rdfs:subClassOf rdf:resource="https://savage.nps.edu/EthicalControl/ontologies/MissionExecutionOntology#DADM09.1"/>
        <rdfs:comment>Can the IAS make decisions when incapacitated human operators cannot?</rdfs:comment>
        <rdfs:label>RE09.1.4_CanIASMakeDecisionsWhenHumanCannot</rdfs:label>
        <owl:versionInfo>page 85</owl:versionInfo>
    </owl:Class>
    


    <!-- https://savage.nps.edu/EthicalControl/ontologies/MissionExecutionOntology#RE09.1.5 -->

    <owl:Class rdf:about="https://savage.nps.edu/EthicalControl/ontologies/MissionExecutionOntology#RE09.1.5">
        <rdfs:subClassOf rdf:resource="https://savage.nps.edu/EthicalControl/ontologies/MissionExecutionOntology#DADM09.1"/>
        <rdfs:comment>What types of decisions is the IAS allowed to make or delegate?</rdfs:comment>
        <rdfs:label>RE09.1.5_DecisionsIASCanMake</rdfs:label>
        <owl:versionInfo>page 85</owl:versionInfo>
    </owl:Class>
    


    <!-- https://savage.nps.edu/EthicalControl/ontologies/MissionExecutionOntology#RE09.1.6 -->

    <owl:Class rdf:about="https://savage.nps.edu/EthicalControl/ontologies/MissionExecutionOntology#RE09.1.6">
        <rdfs:subClassOf rdf:resource="https://savage.nps.edu/EthicalControl/ontologies/MissionExecutionOntology#DADM09.1"/>
        <rdfs:comment>Can the IAS detect when the human operator is under too much stress to make a sound decision and unilaterally make decisions without human oversight that normally would require it?</rdfs:comment>
        <rdfs:label>RE09.1.6_HumanStressDetection</rdfs:label>
        <owl:versionInfo>page 85</owl:versionInfo>
    </owl:Class>
    


    <!-- https://savage.nps.edu/EthicalControl/ontologies/MissionExecutionOntology#RE09.1.7 -->

    <owl:Class rdf:about="https://savage.nps.edu/EthicalControl/ontologies/MissionExecutionOntology#RE09.1.7">
        <rdfs:subClassOf rdf:resource="https://savage.nps.edu/EthicalControl/ontologies/MissionExecutionOntology#DADM09.1"/>
        <rdfs:comment>Can the IAS provide explanations of its actions and/or predictions that are understandable by the human operator?</rdfs:comment>
        <rdfs:label>RE09.1.7_HumanUnderstandableIASExplanations</rdfs:label>
        <owl:versionInfo>page 85</owl:versionInfo>
    </owl:Class>
    


    <!-- https://savage.nps.edu/EthicalControl/ontologies/MissionExecutionOntology#RE09.1.8 -->

    <owl:Class rdf:about="https://savage.nps.edu/EthicalControl/ontologies/MissionExecutionOntology#RE09.1.8">
        <rdfs:subClassOf rdf:resource="https://savage.nps.edu/EthicalControl/ontologies/MissionExecutionOntology#DADM09.1"/>
        <rdfs:comment>Can the IAS detect human user complacency?</rdfs:comment>
        <rdfs:label>RE09.1.8_HumanComplacencyDetection</rdfs:label>
        <owl:versionInfo>page 85</owl:versionInfo>
    </owl:Class>
    


    <!-- https://savage.nps.edu/EthicalControl/ontologies/MissionExecutionOntology#RE09.1.9 -->

    <owl:Class rdf:about="https://savage.nps.edu/EthicalControl/ontologies/MissionExecutionOntology#RE09.1.9">
        <rdfs:subClassOf rdf:resource="https://savage.nps.edu/EthicalControl/ontologies/MissionExecutionOntology#DADM09.1"/>
        <rdfs:comment>Is the rate of IAS false positive results known and below a previously defined and acceptable value?</rdfs:comment>
        <rdfs:label>RE09.1.9_IASFalsePositiveResults</rdfs:label>
        <owl:versionInfo>page 85</owl:versionInfo>
    </owl:Class>
    


    <!-- https://savage.nps.edu/EthicalControl/ontologies/MissionExecutionOntology#RE09.2.1 -->

    <owl:Class rdf:about="https://savage.nps.edu/EthicalControl/ontologies/MissionExecutionOntology#RE09.2.1">
        <rdfs:subClassOf rdf:resource="https://savage.nps.edu/EthicalControl/ontologies/MissionExecutionOntology#DADM09.2"/>
        <rdfs:comment>Can the IAS detect and respond appropriately to conforming and non-conforming human behaviors?</rdfs:comment>
        <rdfs:label>RE09.2.1_IASHumanConformityResponse</rdfs:label>
        <owl:versionInfo>page 87</owl:versionInfo>
    </owl:Class>
    


    <!-- https://savage.nps.edu/EthicalControl/ontologies/MissionExecutionOntology#RE09.2.2 -->

    <owl:Class rdf:about="https://savage.nps.edu/EthicalControl/ontologies/MissionExecutionOntology#RE09.2.2">
        <rdfs:subClassOf rdf:resource="https://savage.nps.edu/EthicalControl/ontologies/MissionExecutionOntology#DADM09.2"/>
        <rdfs:comment>Can the IAS identify an instruction from a human operator that violates its preprogrammed definitions of the Law of Armed Conflict, policy, or rules of engagement, not carry out the instruction, and provide a reason to the human operator for not doing so?</rdfs:comment>
        <rdfs:label>RE09.2.2_HumanInstructionLawViolationDetection</rdfs:label>
        <owl:versionInfo>page 87</owl:versionInfo>
    </owl:Class>
    


    <!-- https://savage.nps.edu/EthicalControl/ontologies/MissionExecutionOntology#RE09.2.3 -->

    <owl:Class rdf:about="https://savage.nps.edu/EthicalControl/ontologies/MissionExecutionOntology#RE09.2.3">
        <rdfs:subClassOf rdf:resource="https://savage.nps.edu/EthicalControl/ontologies/MissionExecutionOntology#DADM09.2"/>
        <rdfs:comment>Can an IAS decision to not carry out an instruction that violates its preprogrammed definition of the Law of Armed Conflict, policy, or rules of engagement be overridden by the human operator or some other commander?</rdfs:comment>
        <rdfs:label>RE09.2.3_HumanCommanderIASDecisionOverriding</rdfs:label>
        <owl:versionInfo>page 87</owl:versionInfo>
    </owl:Class>
    


    <!-- https://savage.nps.edu/EthicalControl/ontologies/MissionExecutionOntology#RE09.2.4 -->

    <owl:Class rdf:about="https://savage.nps.edu/EthicalControl/ontologies/MissionExecutionOntology#RE09.2.4">
        <rdfs:subClassOf rdf:resource="https://savage.nps.edu/EthicalControl/ontologies/MissionExecutionOntology#DADM09.2"/>
        <rdfs:comment>Can the IAS request mission re–planning if planned mission execution violates mission success criteria, or other operational constraints (such as the crossing of a geographic border), and report detected violations to the human operator?</rdfs:comment>
        <rdfs:label>RE09.2.4_MissionCorrectionAbility</rdfs:label>
        <owl:versionInfo>page 87</owl:versionInfo>
    </owl:Class>
    


    <!-- https://savage.nps.edu/EthicalControl/ontologies/MissionExecutionOntology#RE09.2.5 -->

    <owl:Class rdf:about="https://savage.nps.edu/EthicalControl/ontologies/MissionExecutionOntology#RE09.2.5">
        <rdfs:subClassOf rdf:resource="https://savage.nps.edu/EthicalControl/ontologies/MissionExecutionOntology#DADM09.2"/>
        <rdfs:comment>Can the IAS perform arbitration between competing mission and navigation objectives based on constraints configured by the human operator?</rdfs:comment>
        <rdfs:label>RE09.2.5_IASArbitrationBetweenCompetingObjectives</rdfs:label>
        <owl:versionInfo>page 87</owl:versionInfo>
    </owl:Class>
    


    <!-- https://savage.nps.edu/EthicalControl/ontologies/MissionExecutionOntology#RE09.2.6 -->

    <owl:Class rdf:about="https://savage.nps.edu/EthicalControl/ontologies/MissionExecutionOntology#RE09.2.6">
        <rdfs:subClassOf rdf:resource="https://savage.nps.edu/EthicalControl/ontologies/MissionExecutionOntology#DADM09.2"/>
        <rdfs:comment>Can the IAS detect situations that fall beyond its narrow application domain that subsequently require it to contact a human operator for additional guidance?</rdfs:comment>
        <rdfs:label>RE09.2.6_NarrowDomainSituationDetection</rdfs:label>
        <owl:versionInfo>page 87</owl:versionInfo>
    </owl:Class>
    


    <!-- https://savage.nps.edu/EthicalControl/ontologies/MissionExecutionOntology#RE09.3.1 -->

    <owl:Class rdf:about="https://savage.nps.edu/EthicalControl/ontologies/MissionExecutionOntology#RE09.3.1">
        <rdfs:subClassOf rdf:resource="https://savage.nps.edu/EthicalControl/ontologies/MissionExecutionOntology#DADM09.3"/>
        <rdfs:comment>Can the IAS determine the optimal frequency of how often they must query humans for commands and ensure that they do not miss any commands?</rdfs:comment>
        <rdfs:label>RE09.3.1_IASHumanQueryFrequency</rdfs:label>
        <owl:versionInfo>page 87</owl:versionInfo>
    </owl:Class>
    


    <!-- https://savage.nps.edu/EthicalControl/ontologies/MissionExecutionOntology#RE09.3.2 -->

    <owl:Class rdf:about="https://savage.nps.edu/EthicalControl/ontologies/MissionExecutionOntology#RE09.3.2">
        <rdfs:subClassOf rdf:resource="https://savage.nps.edu/EthicalControl/ontologies/MissionExecutionOntology#DADM09.3"/>
        <rdfs:comment>Can the IAS communicate with the human using natural language, gestures or haptics to ease and to accelerate information exchanges with human operators?</rdfs:comment>
        <rdfs:label>RE09.3.2_IASHumanLikeCommunications</rdfs:label>
        <owl:versionInfo>page 87</owl:versionInfo>
    </owl:Class>
    


    <!-- https://savage.nps.edu/EthicalControl/ontologies/MissionExecutionOntology#RE09.3.3 -->

    <owl:Class rdf:about="https://savage.nps.edu/EthicalControl/ontologies/MissionExecutionOntology#RE09.3.3">
        <rdfs:subClassOf rdf:resource="https://savage.nps.edu/EthicalControl/ontologies/MissionExecutionOntology#DADM09.3"/>
        <rdfs:comment>Can the IAS monitor the attentional focus, cognitive load, and task status of the human operator, and only communicate information that does not overburden the human operator with unnecessary or irrelevant information or tasks?</rdfs:comment>
        <rdfs:label>RE09.3.3_IASHumanCognitiveLoadMonitoring</rdfs:label>
        <owl:versionInfo>page 87</owl:versionInfo>
    </owl:Class>
    


    <!-- https://savage.nps.edu/EthicalControl/ontologies/MissionExecutionOntology#RE09.3.4 -->

    <owl:Class rdf:about="https://savage.nps.edu/EthicalControl/ontologies/MissionExecutionOntology#RE09.3.4">
        <rdfs:subClassOf rdf:resource="https://savage.nps.edu/EthicalControl/ontologies/MissionExecutionOntology#DADM09.3"/>
        <rdfs:comment>Can the IAS detect the emotional and physical state of the human operator to maximize efficiency of communications and activities?</rdfs:comment>
        <rdfs:label>RE09.3.4_IASHumanEmotionPhysicalStateDetection</rdfs:label>
        <owl:versionInfo>page 87</owl:versionInfo>
    </owl:Class>
    


    <!-- https://savage.nps.edu/EthicalControl/ontologies/MissionExecutionOntology#RE09.3.5 -->

    <owl:Class rdf:about="https://savage.nps.edu/EthicalControl/ontologies/MissionExecutionOntology#RE09.3.5">
        <rdfs:subClassOf rdf:resource="https://savage.nps.edu/EthicalControl/ontologies/MissionExecutionOntology#DADM09.3"/>
        <rdfs:comment>Can the IAS support human–machine joint training to allow an understanding to develop between the human operator and the IAS regarding team objectives, platform roles, co–dependency relationships, and mutual expectations for competence, dependability, predictability, and timeliness?</rdfs:comment>
        <rdfs:label>RE09.3.5_HumanMachineJointTraining</rdfs:label>
        <owl:versionInfo>page 87</owl:versionInfo>
    </owl:Class>
    


    <!-- https://savage.nps.edu/EthicalControl/ontologies/MissionExecutionOntology#RE09.3.6 -->

    <owl:Class rdf:about="https://savage.nps.edu/EthicalControl/ontologies/MissionExecutionOntology#RE09.3.6">
        <rdfs:subClassOf rdf:resource="https://savage.nps.edu/EthicalControl/ontologies/MissionExecutionOntology#DADM09.3"/>
        <rdfs:comment>Is the delegation of actions explicitly represented in the dialogue between the human and the machine?</rdfs:comment>
        <rdfs:label>RE09.3.6_HumanMachineActionDelegations</rdfs:label>
        <owl:versionInfo>page 87</owl:versionInfo>
    </owl:Class>
    


    <!-- https://savage.nps.edu/EthicalControl/ontologies/MissionExecutionOntology#RE09.3.7 -->

    <owl:Class rdf:about="https://savage.nps.edu/EthicalControl/ontologies/MissionExecutionOntology#RE09.3.7">
        <rdfs:subClassOf rdf:resource="https://savage.nps.edu/EthicalControl/ontologies/MissionExecutionOntology#DADM09.3"/>
        <rdfs:comment>Can the human modify the conditions placed on the delegated actions and/or decisions of the machine?</rdfs:comment>
        <rdfs:label>RE09.3.7_HumanDelegationModificationCriteria</rdfs:label>
        <owl:versionInfo>page 88</owl:versionInfo>
    </owl:Class>
    


    <!-- https://savage.nps.edu/EthicalControl/ontologies/MissionExecutionOntology#RE09.3.8 -->

    <owl:Class rdf:about="https://savage.nps.edu/EthicalControl/ontologies/MissionExecutionOntology#RE09.3.8">
        <rdfs:subClassOf rdf:resource="https://savage.nps.edu/EthicalControl/ontologies/MissionExecutionOntology#DADM09.3"/>
        <rdfs:comment>Is there monitoring and documentation that the machine is acting within its prescribed boundaries?</rdfs:comment>
        <rdfs:label>RE09.3.8_MachineActionMonitoringAndDocumentation</rdfs:label>
        <owl:versionInfo>page 88</owl:versionInfo>
    </owl:Class>
    


    <!-- https://savage.nps.edu/EthicalControl/ontologies/MissionExecutionOntology#RE10.1.1 -->

    <owl:Class rdf:about="https://savage.nps.edu/EthicalControl/ontologies/MissionExecutionOntology#RE10.1.1">
        <rdfs:subClassOf rdf:resource="https://savage.nps.edu/EthicalControl/ontologies/MissionExecutionOntology#DADM10.1"/>
        <rdfs:comment>Did the IAS test and evaluation procedure receive an already-trained IAS, or is the IAS to be tested also to be trained in the replicated operational environment?</rdfs:comment>
        <rdfs:label>RE10.1.1_TrainedReplicatedOperationalEnvironments</rdfs:label>
        <owl:versionInfo>page 88</owl:versionInfo>
    </owl:Class>
    


    <!-- https://savage.nps.edu/EthicalControl/ontologies/MissionExecutionOntology#RE10.1.10 -->

    <owl:Class rdf:about="https://savage.nps.edu/EthicalControl/ontologies/MissionExecutionOntology#RE10.1.10">
        <rdfs:subClassOf rdf:resource="https://savage.nps.edu/EthicalControl/ontologies/MissionExecutionOntology#DADM10.1"/>
        <rdfs:comment>Is there ongoing test and evaluation after fielding to evaluate the ability of the IAS to adapt to new, unexpected circumstances, or new input data?</rdfs:comment>
        <rdfs:label>RE10.1.10_TestEvaluationOngoingNewUnexpectedCircumstances</rdfs:label>
        <owl:versionInfo>page 88</owl:versionInfo>
    </owl:Class>
    


    <!-- https://savage.nps.edu/EthicalControl/ontologies/MissionExecutionOntology#RE10.1.11 -->

    <owl:Class rdf:about="https://savage.nps.edu/EthicalControl/ontologies/MissionExecutionOntology#RE10.1.11">
        <rdfs:subClassOf rdf:resource="https://savage.nps.edu/EthicalControl/ontologies/MissionExecutionOntology#DADM10.1"/>
        <rdfs:comment>Does the IAS possess measurable and testable autonomous capabilities?</rdfs:comment>
        <rdfs:label>RE10.1.11_TestEvaluationMeasurableTestableAutonomousCapabilities</rdfs:label>
        <owl:versionInfo>page 88</owl:versionInfo>
    </owl:Class>
    


    <!-- https://savage.nps.edu/EthicalControl/ontologies/MissionExecutionOntology#RE10.1.12 -->

    <owl:Class rdf:about="https://savage.nps.edu/EthicalControl/ontologies/MissionExecutionOntology#RE10.1.12">
        <rdfs:subClassOf rdf:resource="https://savage.nps.edu/EthicalControl/ontologies/MissionExecutionOntology#DADM10.1"/>
        <rdfs:comment>Have members of the AI and safety engineering research communities with expertise in the potential safety or failure risks from loss of command and control been consulted?</rdfs:comment>
        <rdfs:label>RE10.1.12_C2SafetyEngineersConsulted</rdfs:label>
        <owl:versionInfo>page 88</owl:versionInfo>
    </owl:Class>
    


    <!-- https://savage.nps.edu/EthicalControl/ontologies/MissionExecutionOntology#RE10.1.13 -->

    <owl:Class rdf:about="https://savage.nps.edu/EthicalControl/ontologies/MissionExecutionOntology#RE10.1.13">
        <rdfs:subClassOf rdf:resource="https://savage.nps.edu/EthicalControl/ontologies/MissionExecutionOntology#DADM10.1"/>
        <rdfs:comment>Was the operational testing and verification witnessed by an independent third party (non-DOD) such as the Underwriter’s Laboratory or operational test and evaluation personnel from another federal agency?</rdfs:comment>
        <rdfs:label>RE10.1.13_IndependentThirdPartyTestingVerification</rdfs:label>
        <owl:versionInfo>page 89</owl:versionInfo>
    </owl:Class>
    


    <!-- https://savage.nps.edu/EthicalControl/ontologies/MissionExecutionOntology#RE10.1.2 -->

    <owl:Class rdf:about="https://savage.nps.edu/EthicalControl/ontologies/MissionExecutionOntology#RE10.1.2">
        <rdfs:subClassOf rdf:resource="https://savage.nps.edu/EthicalControl/ontologies/MissionExecutionOntology#DADM10.1"/>
        <rdfs:comment>Did the IAS test and evaluation procedure test all components for the presence of autonomous capabilities?</rdfs:comment>
        <rdfs:label>RE10.1.2_TestEvaluationAutonomous</rdfs:label>
        <owl:versionInfo>page 88</owl:versionInfo>
    </owl:Class>
    


    <!-- https://savage.nps.edu/EthicalControl/ontologies/MissionExecutionOntology#RE10.1.3 -->

    <owl:Class rdf:about="https://savage.nps.edu/EthicalControl/ontologies/MissionExecutionOntology#RE10.1.3">
        <rdfs:subClassOf rdf:resource="https://savage.nps.edu/EthicalControl/ontologies/MissionExecutionOntology#DADM10.1"/>
        <rdfs:comment>Did the IAS test and evaluation procedure record all test results to make them available for inspection and oversight?</rdfs:comment>
        <rdfs:label>RE10.1.3_TestEvaluationResultsInspectionOversight</rdfs:label>
        <owl:versionInfo>page 88</owl:versionInfo>
    </owl:Class>
    


    <!-- https://savage.nps.edu/EthicalControl/ontologies/MissionExecutionOntology#RE10.1.4 -->

    <owl:Class rdf:about="https://savage.nps.edu/EthicalControl/ontologies/MissionExecutionOntology#RE10.1.4">
        <rdfs:subClassOf rdf:resource="https://savage.nps.edu/EthicalControl/ontologies/MissionExecutionOntology#DADM10.1"/>
        <rdfs:comment>Did the IAS test and evaluation procedure use traditional model checking that may be unsuited for the IAS?</rdfs:comment>
        <rdfs:label>RE10.1.4_TestEvaluationResultsUnsuitableModelTesting</rdfs:label>
        <owl:versionInfo>page 88</owl:versionInfo>
    </owl:Class>
    


    <!-- https://savage.nps.edu/EthicalControl/ontologies/MissionExecutionOntology#RE10.1.5 -->

    <owl:Class rdf:about="https://savage.nps.edu/EthicalControl/ontologies/MissionExecutionOntology#RE10.1.5">
        <rdfs:subClassOf rdf:resource="https://savage.nps.edu/EthicalControl/ontologies/MissionExecutionOntology#DADM10.1"/>
        <rdfs:comment>Did operational testing provide authorized and certified conditions for use of IAS?</rdfs:comment>
        <rdfs:label>RE10.1.5_TestEvaluationAuthorizedCertifiedConditions</rdfs:label>
        <owl:versionInfo>page 88</owl:versionInfo>
    </owl:Class>
    


    <!-- https://savage.nps.edu/EthicalControl/ontologies/MissionExecutionOntology#RE10.1.6 -->

    <owl:Class rdf:about="https://savage.nps.edu/EthicalControl/ontologies/MissionExecutionOntology#RE10.1.6">
        <rdfs:subClassOf rdf:resource="https://savage.nps.edu/EthicalControl/ontologies/MissionExecutionOntology#DADM10.1"/>
        <rdfs:comment>Did the IAS test and evaluation procedure use simulations to push the system to its breaking point so that the boundaries between success and failure were tested and verified in a representative operational environment?</rdfs:comment>
        <rdfs:label>RE10.1.6_TestEvaluationSimulationEdgeCaseBoundaries</rdfs:label>
        <owl:versionInfo>page 88</owl:versionInfo>
    </owl:Class>
    


    <!-- https://savage.nps.edu/EthicalControl/ontologies/MissionExecutionOntology#RE10.1.7 -->

    <owl:Class rdf:about="https://savage.nps.edu/EthicalControl/ontologies/MissionExecutionOntology#RE10.1.7">
        <rdfs:subClassOf rdf:resource="https://savage.nps.edu/EthicalControl/ontologies/MissionExecutionOntology#DADM10.1"/>
        <rdfs:comment>Did the IAS test and evaluation procedure utilize an environment (e.g., Live Virtual Constructive environment) that best captures the behaviors that may emerge under real-world operational conditions?</rdfs:comment>
        <rdfs:label>RE10.1.7_TestEvaluationResultsLVCEnvironment</rdfs:label>
        <owl:versionInfo>page 88</owl:versionInfo>
    </owl:Class>
    


    <!-- https://savage.nps.edu/EthicalControl/ontologies/MissionExecutionOntology#RE10.1.8 -->

    <owl:Class rdf:about="https://savage.nps.edu/EthicalControl/ontologies/MissionExecutionOntology#RE10.1.8">
        <rdfs:subClassOf rdf:resource="https://savage.nps.edu/EthicalControl/ontologies/MissionExecutionOntology#DADM10.1"/>
        <rdfs:comment>Were components or sub-components of the IAS available for testing and fleet concept of employment and experimentation?</rdfs:comment>
        <rdfs:label>RE10.1.8_TestEvaluationSubcomponentResults</rdfs:label>
        <owl:versionInfo>page 88</owl:versionInfo>
    </owl:Class>
    


    <!-- https://savage.nps.edu/EthicalControl/ontologies/MissionExecutionOntology#RE10.1.9 -->

    <owl:Class rdf:about="https://savage.nps.edu/EthicalControl/ontologies/MissionExecutionOntology#RE10.1.9">
        <rdfs:subClassOf rdf:resource="https://savage.nps.edu/EthicalControl/ontologies/MissionExecutionOntology#DADM10.1"/>
        <rdfs:comment>Has the threshold been identified for adequate test and evaluation of autonomous capabilities with respect to their manned counterparts, and with respect to the risk of not having any autonomous systems?</rdfs:comment>
        <rdfs:label>RE10.1.9_TestEvaluationAutonomousResults</rdfs:label>
        <owl:versionInfo>page 88</owl:versionInfo>
    </owl:Class>
    


    <!-- https://savage.nps.edu/EthicalControl/ontologies/MissionExecutionOntology#RE10.2.1 -->

    <owl:Class rdf:about="https://savage.nps.edu/EthicalControl/ontologies/MissionExecutionOntology#RE10.2.1">
        <rdfs:subClassOf rdf:resource="https://savage.nps.edu/EthicalControl/ontologies/MissionExecutionOntology#DADM10.2"/>
        <rdfs:comment>Did the IAS test and evaluation procedure use simulations adequately representative of the contemplated operational environment and document all operational parameters that would cause it to be used in an environment that the simulation did not faithfully replicate?</rdfs:comment>
        <rdfs:label>RE10.2.1_TestEvaluationComplexSimulation</rdfs:label>
        <owl:versionInfo>page 89</owl:versionInfo>
    </owl:Class>
    


    <!-- https://savage.nps.edu/EthicalControl/ontologies/MissionExecutionOntology#RE10.2.10 -->

    <owl:Class rdf:about="https://savage.nps.edu/EthicalControl/ontologies/MissionExecutionOntology#RE10.2.10">
        <rdfs:subClassOf rdf:resource="https://savage.nps.edu/EthicalControl/ontologies/MissionExecutionOntology#DADM10.2"/>
        <rdfs:comment>Did the IAS test and evaluation procedure consider how an IAS might overwrite all or part of its original software as a result of exposure to new training data, such that the procedure must be repeated on the new software baseline?</rdfs:comment>
        <rdfs:label>RE10.2.10_TestEvaluationChangesNewTrainingData</rdfs:label>
        <owl:versionInfo>page 89</owl:versionInfo>
    </owl:Class>
    


    <!-- https://savage.nps.edu/EthicalControl/ontologies/MissionExecutionOntology#RE10.2.11 -->

    <owl:Class rdf:about="https://savage.nps.edu/EthicalControl/ontologies/MissionExecutionOntology#RE10.2.11">
        <rdfs:subClassOf rdf:resource="https://savage.nps.edu/EthicalControl/ontologies/MissionExecutionOntology#DADM10.2"/>
        <rdfs:comment>Did the IAS test and evaluation procedure consider whether the data stream providing instructions to the IAS is vulnerable to hacking or &quot;in flight&quot; hijacking?</rdfs:comment>
        <rdfs:label>RE10.2.11_TestEvaluationC2Hijacking</rdfs:label>
        <owl:versionInfo>page 89</owl:versionInfo>
    </owl:Class>
    


    <!-- https://savage.nps.edu/EthicalControl/ontologies/MissionExecutionOntology#RE10.2.12 -->

    <owl:Class rdf:about="https://savage.nps.edu/EthicalControl/ontologies/MissionExecutionOntology#RE10.2.12">
        <rdfs:subClassOf rdf:resource="https://savage.nps.edu/EthicalControl/ontologies/MissionExecutionOntology#DADM10.2"/>
        <rdfs:comment>Did the IAS test and evaluation procedure consider infiltration into the industrial supply chain?</rdfs:comment>
        <rdfs:label>RE10.2.12_TestEvaluationInfiltrationIndustrialSupplyChain</rdfs:label>
        <owl:versionInfo>page 90</owl:versionInfo>
    </owl:Class>
    


    <!-- https://savage.nps.edu/EthicalControl/ontologies/MissionExecutionOntology#RE10.2.13 -->

    <owl:Class rdf:about="https://savage.nps.edu/EthicalControl/ontologies/MissionExecutionOntology#RE10.2.13">
        <rdfs:subClassOf rdf:resource="https://savage.nps.edu/EthicalControl/ontologies/MissionExecutionOntology#DADM10.2"/>
        <rdfs:comment>Did the IAS test and evaluation procedure utilize virtual twin models to test the IAS in simulated environments to predict how it will interact with IAS and non-autonomous systems from neutral nations, allied nations and from other services?</rdfs:comment>
        <rdfs:label>RE10.2.13_TestEvaluationDigitalTwinsExternalSystems</rdfs:label>
        <owl:versionInfo>page 90</owl:versionInfo>
    </owl:Class>
    


    <!-- https://savage.nps.edu/EthicalControl/ontologies/MissionExecutionOntology#RE10.2.14 -->

    <owl:Class rdf:about="https://savage.nps.edu/EthicalControl/ontologies/MissionExecutionOntology#RE10.2.14">
        <rdfs:subClassOf rdf:resource="https://savage.nps.edu/EthicalControl/ontologies/MissionExecutionOntology#DADM10.2"/>
        <rdfs:comment>Did the IAS development include an AI-developed capability to conduct planning where there will be a need to design test plans in a timely manner to assure thorough testing while being able to predict certain behaviors with these systems (e.g., Autonomous Systems Test (AST) Planning)?</rdfs:comment>
        <rdfs:label>RE10.2.14_DevelopmentConductPlanning</rdfs:label>
        <owl:versionInfo>page 90</owl:versionInfo>
    </owl:Class>
    


    <!-- https://savage.nps.edu/EthicalControl/ontologies/MissionExecutionOntology#RE10.2.15 -->

    <owl:Class rdf:about="https://savage.nps.edu/EthicalControl/ontologies/MissionExecutionOntology#RE10.2.15">
        <rdfs:subClassOf rdf:resource="https://savage.nps.edu/EthicalControl/ontologies/MissionExecutionOntology#DADM10.2"/>
        <rdfs:comment>Did the IAS development include an AI-developed capability that will guarantee safety during testing through the use of immersion technologies to adapt tests to best suit IAS cognitive capabilities (e.g., conducting AST Execution &amp; Control)?</rdfs:comment>
        <rdfs:label>RE10.2.15_DevelopmentGuarenteeSafety</rdfs:label>
        <owl:versionInfo>page 90</owl:versionInfo>
    </owl:Class>
    


    <!-- https://savage.nps.edu/EthicalControl/ontologies/MissionExecutionOntology#RE10.2.16 -->

    <owl:Class rdf:about="https://savage.nps.edu/EthicalControl/ontologies/MissionExecutionOntology#RE10.2.16">
        <rdfs:subClassOf rdf:resource="https://savage.nps.edu/EthicalControl/ontologies/MissionExecutionOntology#DADM10.2"/>
        <rdfs:comment>Did the IAS development include an AI-developed capability to conduct assessments (e.g., Autonomous System Performance Assessment) to capture how IAS interact with existing and newly fielded manned and unmanned systems in realistic operational environments?</rdfs:comment>
        <rdfs:label>RE10.2.16_DevelopmentConductAssessments</rdfs:label>
        <owl:versionInfo>page 90</owl:versionInfo>
    </owl:Class>
    


    <!-- https://savage.nps.edu/EthicalControl/ontologies/MissionExecutionOntology#RE10.2.17 -->

    <owl:Class rdf:about="https://savage.nps.edu/EthicalControl/ontologies/MissionExecutionOntology#RE10.2.17">
        <rdfs:subClassOf rdf:resource="https://savage.nps.edu/EthicalControl/ontologies/MissionExecutionOntology#DADM10.2"/>
        <rdfs:comment>Can functional components be tested in the replicated environment while assessing reliability and identification of vulnerabilities?</rdfs:comment>
        <rdfs:label>RE10.2.17_FunctionalComponentTestingReplicatedEnvironment</rdfs:label>
        <owl:versionInfo>page 90</owl:versionInfo>
    </owl:Class>
    


    <!-- https://savage.nps.edu/EthicalControl/ontologies/MissionExecutionOntology#RE10.2.18 -->

    <owl:Class rdf:about="https://savage.nps.edu/EthicalControl/ontologies/MissionExecutionOntology#RE10.2.18">
        <rdfs:subClassOf rdf:resource="https://savage.nps.edu/EthicalControl/ontologies/MissionExecutionOntology#DADM10.2"/>
        <rdfs:comment>Can human-IAS interaction be measured in the replicated environment while assessing reliability and identification of vulnerabilities?</rdfs:comment>
        <rdfs:label>RE10.2.18_HumanInteractionMeasuredreplicatedEnvironment</rdfs:label>
        <owl:versionInfo>page 90</owl:versionInfo>
    </owl:Class>
    


    <!-- https://savage.nps.edu/EthicalControl/ontologies/MissionExecutionOntology#RE10.2.2 -->

    <owl:Class rdf:about="https://savage.nps.edu/EthicalControl/ontologies/MissionExecutionOntology#RE10.2.2">
        <rdfs:subClassOf rdf:resource="https://savage.nps.edu/EthicalControl/ontologies/MissionExecutionOntology#DADM10.2"/>
        <rdfs:comment>Did the IAS test and evaluation procedure use simulated or otherwise artificially generated data to replicate the contemplated operational environment?</rdfs:comment>
        <rdfs:label>RE10.2.2_TestEvaluationSimulatedDataCoverage</rdfs:label>
        <owl:versionInfo>page 89</owl:versionInfo>
    </owl:Class>
    


    <!-- https://savage.nps.edu/EthicalControl/ontologies/MissionExecutionOntology#RE10.2.3 -->

    <owl:Class rdf:about="https://savage.nps.edu/EthicalControl/ontologies/MissionExecutionOntology#RE10.2.3">
        <rdfs:subClassOf rdf:resource="https://savage.nps.edu/EthicalControl/ontologies/MissionExecutionOntology#DADM10.2"/>
        <rdfs:comment>Has the relevance of the IAS training data to the contemplated operational environment been validated?</rdfs:comment>
        <rdfs:label>RE10.2.3_TrainingDataEnvironmentValidation</rdfs:label>
        <owl:versionInfo>page 89</owl:versionInfo>
    </owl:Class>
    


    <!-- https://savage.nps.edu/EthicalControl/ontologies/MissionExecutionOntology#RE10.2.4 -->

    <owl:Class rdf:about="https://savage.nps.edu/EthicalControl/ontologies/MissionExecutionOntology#RE10.2.4">
        <rdfs:subClassOf rdf:resource="https://savage.nps.edu/EthicalControl/ontologies/MissionExecutionOntology#DADM10.2"/>
        <rdfs:comment>Has any use of simulated data been validated against real-world data? Breadth of testing in the replicated environment</rdfs:comment>
        <rdfs:label>RE10.2.4_SimulatedDataValidatedRealWorldData</rdfs:label>
        <owl:versionInfo>page 89</owl:versionInfo>
    </owl:Class>
    


    <!-- https://savage.nps.edu/EthicalControl/ontologies/MissionExecutionOntology#RE10.2.5 -->

    <owl:Class rdf:about="https://savage.nps.edu/EthicalControl/ontologies/MissionExecutionOntology#RE10.2.5">
        <rdfs:subClassOf rdf:resource="https://savage.nps.edu/EthicalControl/ontologies/MissionExecutionOntology#DADM10.2"/>
        <rdfs:comment>Did the IAS test and evaluation procedure subject the system to adversarial machine learning attacks to identify potential attack vectors?</rdfs:comment>
        <rdfs:label>RE10.2.5_TestEvaluationAdversarialMachineLearningAttacks</rdfs:label>
        <owl:versionInfo>page 89</owl:versionInfo>
    </owl:Class>
    


    <!-- https://savage.nps.edu/EthicalControl/ontologies/MissionExecutionOntology#RE10.2.6 -->

    <owl:Class rdf:about="https://savage.nps.edu/EthicalControl/ontologies/MissionExecutionOntology#RE10.2.6">
        <rdfs:subClassOf rdf:resource="https://savage.nps.edu/EthicalControl/ontologies/MissionExecutionOntology#DADM10.2"/>
        <rdfs:comment>Did the IAS test and evaluation procedure limit the replicated environment to what the IAS will encounter in the contemplated operational environment and document all parameters that would cause it to be used in an environment test and evaluation did not faithfully replicate?</rdfs:comment>
        <rdfs:label>RE10.2.6_TestEvaluationLimitedReplicatedEnvironment</rdfs:label>
        <owl:versionInfo>page 89</owl:versionInfo>
    </owl:Class>
    


    <!-- https://savage.nps.edu/EthicalControl/ontologies/MissionExecutionOntology#RE10.2.7 -->

    <owl:Class rdf:about="https://savage.nps.edu/EthicalControl/ontologies/MissionExecutionOntology#RE10.2.7">
        <rdfs:subClassOf rdf:resource="https://savage.nps.edu/EthicalControl/ontologies/MissionExecutionOntology#DADM10.2"/>
        <rdfs:comment>Did the IAS test and evaluation procedure consider interactions with human operators using a fully representative sample of all potential human operators?</rdfs:comment>
        <rdfs:label>RE10.2.7_TestEvaluationHumanInteractionRepresentative</rdfs:label>
        <owl:versionInfo>page 89</owl:versionInfo>
    </owl:Class>
    


    <!-- https://savage.nps.edu/EthicalControl/ontologies/MissionExecutionOntology#RE10.2.8 -->

    <owl:Class rdf:about="https://savage.nps.edu/EthicalControl/ontologies/MissionExecutionOntology#RE10.2.8">
        <rdfs:subClassOf rdf:resource="https://savage.nps.edu/EthicalControl/ontologies/MissionExecutionOntology#DADM10.2"/>
        <rdfs:comment>Did the IAS test and evaluation procedure use computer models to generate thousands of data-based scenarios to anticipate and analyze any emergent behavior?</rdfs:comment>
        <rdfs:label>RE10.2.8_TestEvaluationEmergentBehaviorExploration</rdfs:label>
        <owl:versionInfo>page 89</owl:versionInfo>
    </owl:Class>
    


    <!-- https://savage.nps.edu/EthicalControl/ontologies/MissionExecutionOntology#RE10.2.9 -->

    <owl:Class rdf:about="https://savage.nps.edu/EthicalControl/ontologies/MissionExecutionOntology#RE10.2.9">
        <rdfs:subClassOf rdf:resource="https://savage.nps.edu/EthicalControl/ontologies/MissionExecutionOntology#DADM10.2"/>
        <rdfs:comment>Did the IAS test and evaluation procedure consider how an IAS might overwrite all or part of its original software as a result of exposure to new sensor data, such that the procedure must be repeated on the new software baseline?</rdfs:comment>
        <rdfs:label>RE10.2.9_TestEvaluationChangesNewSensorData</rdfs:label>
        <owl:versionInfo>page 89</owl:versionInfo>
    </owl:Class>
    


    <!-- https://savage.nps.edu/EthicalControl/ontologies/MissionExecutionOntology#RE10.3.1 -->

    <owl:Class rdf:about="https://savage.nps.edu/EthicalControl/ontologies/MissionExecutionOntology#RE10.3.1">
        <rdfs:subClassOf rdf:resource="https://savage.nps.edu/EthicalControl/ontologies/MissionExecutionOntology#DADM10.3"/>
        <rdfs:comment>Did the IAS test and evaluation procedure push the system to its breaking point so that this/these points are known to the operators?</rdfs:comment>
        <rdfs:label>RE10.3.1_TestEvaluationBreakPointTesting</rdfs:label>
        <owl:versionInfo>page 90</owl:versionInfo>
    </owl:Class>
    


    <!-- https://savage.nps.edu/EthicalControl/ontologies/MissionExecutionOntology#RE10.3.2 -->

    <owl:Class rdf:about="https://savage.nps.edu/EthicalControl/ontologies/MissionExecutionOntology#RE10.3.2">
        <rdfs:subClassOf rdf:resource="https://savage.nps.edu/EthicalControl/ontologies/MissionExecutionOntology#DADM10.3"/>
        <rdfs:comment>Did the IAS test and evaluation procedure utilize red team attacks (kinetic and cyber) to capture the full range of behaviors that might emerge under real-world operational conditions?</rdfs:comment>
        <rdfs:label>RE10.3.2_TestEvaluationRedTeamTesting</rdfs:label>
        <owl:versionInfo>page 90</owl:versionInfo>
    </owl:Class>
    


    <!-- https://savage.nps.edu/EthicalControl/ontologies/MissionExecutionOntology#RE10.3.3 -->

    <owl:Class rdf:about="https://savage.nps.edu/EthicalControl/ontologies/MissionExecutionOntology#RE10.3.3">
        <rdfs:subClassOf rdf:resource="https://savage.nps.edu/EthicalControl/ontologies/MissionExecutionOntology#DADM10.3"/>
        <rdfs:comment>Did the IAS test and evaluation procedure utilize red team attacks specifically designed to drive the system into inappropriate behaviors?</rdfs:comment>
        <rdfs:label>RE10.3.3_TestEvaluationInappropriateBehaviorProbingTesting</rdfs:label>
        <owl:versionInfo>page 90</owl:versionInfo>
    </owl:Class>
    


    <!-- https://savage.nps.edu/EthicalControl/ontologies/MissionExecutionOntology#RE11.1.1 -->

    <owl:Class rdf:about="https://savage.nps.edu/EthicalControl/ontologies/MissionExecutionOntology#RE11.1.1">
        <rdfs:subClassOf rdf:resource="https://savage.nps.edu/EthicalControl/ontologies/MissionExecutionOntology#DADM11.1"/>
        <rdfs:comment>Have all senior policy and decision makers, on scene commanders, scientists, engineers, acquisition officials, legal counsels, operators and supported troops received training in the Law of Armed Conflict, IAS ethics principles, and current rules of engagement?</rdfs:comment>
        <rdfs:label>RE11.1.1_BaselineLegalEthicalTraining</rdfs:label>
        <owl:versionInfo>page 90</owl:versionInfo>
    </owl:Class>
    


    <!-- https://savage.nps.edu/EthicalControl/ontologies/MissionExecutionOntology#RE11.1.2 -->

    <owl:Class rdf:about="https://savage.nps.edu/EthicalControl/ontologies/MissionExecutionOntology#RE11.1.2">
        <rdfs:subClassOf rdf:resource="https://savage.nps.edu/EthicalControl/ontologies/MissionExecutionOntology#DADM11.1"/>
        <rdfs:comment>Can human operators with the power to override IAS use during an operation recognize legally and ethically questionable decisions and actions?</rdfs:comment>
        <rdfs:label>RE11.1.2_RecognitionLegallyEthicallQuestionableDecisionsActions</rdfs:label>
        <owl:versionInfo>page 91</owl:versionInfo>
    </owl:Class>
    


    <!-- https://savage.nps.edu/EthicalControl/ontologies/MissionExecutionOntology#RE11.1.3 -->

    <owl:Class rdf:about="https://savage.nps.edu/EthicalControl/ontologies/MissionExecutionOntology#RE11.1.3">
        <rdfs:subClassOf rdf:resource="https://savage.nps.edu/EthicalControl/ontologies/MissionExecutionOntology#DADM11.1"/>
        <rdfs:comment>Do all commanders and users that possess current proficiency certifications to operate the IAS, fully understand how the IAS processes ethical dilemma scenarios?</rdfs:comment>
        <rdfs:label>RE11.1.3_UnderstandingEthicalDilemmaScenarios</rdfs:label>
        <owl:versionInfo>page 91</owl:versionInfo>
    </owl:Class>
    


    <!-- https://savage.nps.edu/EthicalControl/ontologies/MissionExecutionOntology#RE11.2.1 -->

    <owl:Class rdf:about="https://savage.nps.edu/EthicalControl/ontologies/MissionExecutionOntology#RE11.2.1">
        <rdfs:subClassOf rdf:resource="https://savage.nps.edu/EthicalControl/ontologies/MissionExecutionOntology#DADM11.2"/>
        <rdfs:comment>Do training and education requirements exist for IAS as part of the certification process for the deploying forces that may employ them?</rdfs:comment>
        <rdfs:label>RE11.2.1_CertificationProcessEducationTrainingRequirements</rdfs:label>
        <owl:versionInfo>page 91</owl:versionInfo>
    </owl:Class>
    


    <!-- https://savage.nps.edu/EthicalControl/ontologies/MissionExecutionOntology#RE11.2.2 -->

    <owl:Class rdf:about="https://savage.nps.edu/EthicalControl/ontologies/MissionExecutionOntology#RE11.2.2">
        <rdfs:subClassOf rdf:resource="https://savage.nps.edu/EthicalControl/ontologies/MissionExecutionOntology#DADM11.2"/>
        <rdfs:comment>Are IAS training, education, and qualification certifications required and recorded for all personnel?</rdfs:comment>
        <rdfs:label>RE11.2.2_CertificationsTrainingEducationRecorded</rdfs:label>
        <owl:versionInfo>page 91</owl:versionInfo>
    </owl:Class>
    


    <!-- https://savage.nps.edu/EthicalControl/ontologies/MissionExecutionOntology#RE11.2.3 -->

    <owl:Class rdf:about="https://savage.nps.edu/EthicalControl/ontologies/MissionExecutionOntology#RE11.2.3">
        <rdfs:subClassOf rdf:resource="https://savage.nps.edu/EthicalControl/ontologies/MissionExecutionOntology#DADM11.2"/>
        <rdfs:comment>Does the commander’s legal staff monitor the laws, ethics policies and regulations that govern the use of the IAS to ensure current training, education, and qualification certifications are compliant with them?</rdfs:comment>
        <rdfs:label>RE11.2.3_LegalMonitorLawsPoliciesRegulations</rdfs:label>
        <owl:versionInfo>page 91</owl:versionInfo>
    </owl:Class>
    


    <!-- https://savage.nps.edu/EthicalControl/ontologies/MissionExecutionOntology#RE11.2.4 -->

    <owl:Class rdf:about="https://savage.nps.edu/EthicalControl/ontologies/MissionExecutionOntology#RE11.2.4">
        <rdfs:subClassOf rdf:resource="https://savage.nps.edu/EthicalControl/ontologies/MissionExecutionOntology#DADM11.2"/>
        <rdfs:comment>Does the commander’s legal staff have a sufficient technical understanding of IAS?</rdfs:comment>
        <rdfs:label>RE11.2.4_LegalTechnicalUnderstanding</rdfs:label>
        <owl:versionInfo>page 91</owl:versionInfo>
    </owl:Class>
    


    <!-- https://savage.nps.edu/EthicalControl/ontologies/MissionExecutionOntology#RE11.2.5 -->

    <owl:Class rdf:about="https://savage.nps.edu/EthicalControl/ontologies/MissionExecutionOntology#RE11.2.5">
        <rdfs:subClassOf rdf:resource="https://savage.nps.edu/EthicalControl/ontologies/MissionExecutionOntology#DADM11.2"/>
        <rdfs:comment>Are all legal reviews double checked by technical and procurement officials to ensure that they are based on a sound technical understanding of the IAS?</rdfs:comment>
        <rdfs:label>RE11.2.5_LegalReviewsTechnicalProcurementSoundness</rdfs:label>
        <owl:versionInfo>page 91</owl:versionInfo>
    </owl:Class>
    


    <!-- https://savage.nps.edu/EthicalControl/ontologies/MissionExecutionOntology#RE11.3.1 -->

    <owl:Class rdf:about="https://savage.nps.edu/EthicalControl/ontologies/MissionExecutionOntology#RE11.3.1">
        <rdfs:subClassOf rdf:resource="https://savage.nps.edu/EthicalControl/ontologies/MissionExecutionOntology#DADM11.3"/>
        <rdfs:comment>Do all commanders and users understand the difference between general and narrow artificial intelligence?</rdfs:comment>
        <rdfs:label>RE11.3.1_UnderstandingGeneralNarrowModels</rdfs:label>
        <owl:versionInfo>page 91</owl:versionInfo>
    </owl:Class>
    


    <!-- https://savage.nps.edu/EthicalControl/ontologies/MissionExecutionOntology#RE11.3.10 -->

    <owl:Class rdf:about="https://savage.nps.edu/EthicalControl/ontologies/MissionExecutionOntology#RE11.3.10">
        <rdfs:subClassOf rdf:resource="https://savage.nps.edu/EthicalControl/ontologies/MissionExecutionOntology#DADM11.3"/>
        <rdfs:comment>Can all commanders and users determine the degree of autonomy needed in different operational environments and understand the risk mitigation tactics, techniques, procedures and technologies available to them?</rdfs:comment>
        <rdfs:label>RE11.3.10_DegreeAutonomyTTPs</rdfs:label>
        <owl:versionInfo>page 92</owl:versionInfo>
    </owl:Class>
    


    <!-- https://savage.nps.edu/EthicalControl/ontologies/MissionExecutionOntology#RE11.3.11 -->

    <owl:Class rdf:about="https://savage.nps.edu/EthicalControl/ontologies/MissionExecutionOntology#RE11.3.11">
        <rdfs:subClassOf rdf:resource="https://savage.nps.edu/EthicalControl/ontologies/MissionExecutionOntology#DADM11.3"/>
        <rdfs:comment>Can the commanders discern the consequences of the IAS limitations? Understanding the role of data</rdfs:comment>
        <rdfs:label>RE11.3.11_UnderstandingIASLimitationsDataContext</rdfs:label>
        <owl:versionInfo>page 92</owl:versionInfo>
    </owl:Class>
    


    <!-- https://savage.nps.edu/EthicalControl/ontologies/MissionExecutionOntology#RE11.3.12 -->

    <owl:Class rdf:about="https://savage.nps.edu/EthicalControl/ontologies/MissionExecutionOntology#RE11.3.12">
        <rdfs:subClassOf rdf:resource="https://savage.nps.edu/EthicalControl/ontologies/MissionExecutionOntology#DADM11.3"/>
        <rdfs:comment>Do all commanders and users understand the dependence of IAS on training data and the new attack vectors this dependency opens up to the enemy?</rdfs:comment>
        <rdfs:label>RE11.3.12_UnderstandingTrainingDataAttackVectors</rdfs:label>
        <owl:versionInfo>page 92</owl:versionInfo>
    </owl:Class>
    


    <!-- https://savage.nps.edu/EthicalControl/ontologies/MissionExecutionOntology#RE11.3.13 -->

    <owl:Class rdf:about="https://savage.nps.edu/EthicalControl/ontologies/MissionExecutionOntology#RE11.3.13">
        <rdfs:subClassOf rdf:resource="https://savage.nps.edu/EthicalControl/ontologies/MissionExecutionOntology#DADM11.3"/>
        <rdfs:comment>Do all commanders and users understand the difference between training data, input data and feedback data?</rdfs:comment>
        <rdfs:label>RE11.3.13_UnderstandingTrainTestValidateDatasets</rdfs:label>
        <owl:versionInfo>page 92</owl:versionInfo>
    </owl:Class>
    


    <!-- https://savage.nps.edu/EthicalControl/ontologies/MissionExecutionOntology#RE11.3.2 -->

    <owl:Class rdf:about="https://savage.nps.edu/EthicalControl/ontologies/MissionExecutionOntology#RE11.3.2">
        <rdfs:subClassOf rdf:resource="https://savage.nps.edu/EthicalControl/ontologies/MissionExecutionOntology#DADM11.3"/>
        <rdfs:comment>Do all commanders and users understand the concept of &quot;brittleness&quot; with respect to narrow artificial intelligence applications?</rdfs:comment>
        <rdfs:label>RE11.3.2_UnderstandingModelBrittleness</rdfs:label>
        <owl:versionInfo>page 91</owl:versionInfo>
    </owl:Class>
    


    <!-- https://savage.nps.edu/EthicalControl/ontologies/MissionExecutionOntology#RE11.3.3 -->

    <owl:Class rdf:about="https://savage.nps.edu/EthicalControl/ontologies/MissionExecutionOntology#RE11.3.3">
        <rdfs:subClassOf rdf:resource="https://savage.nps.edu/EthicalControl/ontologies/MissionExecutionOntology#DADM11.3"/>
        <rdfs:comment>Do all commanders and users know how to evaluate when IAS are, and are not, necessary to achieving the military objective?</rdfs:comment>
        <rdfs:label>RE11.3.3_UnderstandingIASOperationallyNecessary</rdfs:label>
        <owl:versionInfo>page 91</owl:versionInfo>
    </owl:Class>
    


    <!-- https://savage.nps.edu/EthicalControl/ontologies/MissionExecutionOntology#RE11.3.4 -->

    <owl:Class rdf:about="https://savage.nps.edu/EthicalControl/ontologies/MissionExecutionOntology#RE11.3.4">
        <rdfs:subClassOf rdf:resource="https://savage.nps.edu/EthicalControl/ontologies/MissionExecutionOntology#DADM11.3"/>
        <rdfs:comment>Do all commanders and users know the technical limitations of IAS?</rdfs:comment>
        <rdfs:label>RE11.3.4_UnderstandingIASTechnicalLimitations</rdfs:label>
        <owl:versionInfo>page 91</owl:versionInfo>
    </owl:Class>
    


    <!-- https://savage.nps.edu/EthicalControl/ontologies/MissionExecutionOntology#RE11.3.5 -->

    <owl:Class rdf:about="https://savage.nps.edu/EthicalControl/ontologies/MissionExecutionOntology#RE11.3.5">
        <rdfs:subClassOf rdf:resource="https://savage.nps.edu/EthicalControl/ontologies/MissionExecutionOntology#DADM11.3"/>
        <rdfs:comment>Do all commanders and users know the limitations of IAS imposed by the operational environment?</rdfs:comment>
        <rdfs:label>RE11.3.5_UnderstandingEnvironmentOperationalLimitationsIAS</rdfs:label>
        <owl:versionInfo>page 91</owl:versionInfo>
    </owl:Class>
    


    <!-- https://savage.nps.edu/EthicalControl/ontologies/MissionExecutionOntology#RE11.3.6 -->

    <owl:Class rdf:about="https://savage.nps.edu/EthicalControl/ontologies/MissionExecutionOntology#RE11.3.6">
        <rdfs:subClassOf rdf:resource="https://savage.nps.edu/EthicalControl/ontologies/MissionExecutionOntology#DADM11.3"/>
        <rdfs:comment>Do all commanders and users know the limitations of IAS imposed by the data environment?</rdfs:comment>
        <rdfs:label>RE11.3.6_UnderstandingDataEnvironmentLimitationsIAS</rdfs:label>
        <owl:versionInfo>page 91</owl:versionInfo>
    </owl:Class>
    


    <!-- https://savage.nps.edu/EthicalControl/ontologies/MissionExecutionOntology#RE11.3.7 -->

    <owl:Class rdf:about="https://savage.nps.edu/EthicalControl/ontologies/MissionExecutionOntology#RE11.3.7">
        <rdfs:subClassOf rdf:resource="https://savage.nps.edu/EthicalControl/ontologies/MissionExecutionOntology#DADM11.3"/>
        <rdfs:comment>Do all commanders and users know how to distinguish between components that do and do not possess autonomous capabilities?</rdfs:comment>
        <rdfs:label>RE11.3.7_UnderstandingComponentsAutonomousCapabilities</rdfs:label>
        <owl:versionInfo>page 91</owl:versionInfo>
    </owl:Class>
    


    <!-- https://savage.nps.edu/EthicalControl/ontologies/MissionExecutionOntology#RE11.3.8 -->

    <owl:Class rdf:about="https://savage.nps.edu/EthicalControl/ontologies/MissionExecutionOntology#RE11.3.8">
        <rdfs:subClassOf rdf:resource="https://savage.nps.edu/EthicalControl/ontologies/MissionExecutionOntology#DADM11.3"/>
        <rdfs:comment>Do all commanders and users understand the degrees of autonomy and their impact on IAS capabilities and limitations?</rdfs:comment>
        <rdfs:label>RE11.3.8_UnderstandingDegreeAutonomyIASCapabilitesLimitations</rdfs:label>
        <owl:versionInfo>page 91</owl:versionInfo>
    </owl:Class>
    


    <!-- https://savage.nps.edu/EthicalControl/ontologies/MissionExecutionOntology#RE11.3.9 -->

    <owl:Class rdf:about="https://savage.nps.edu/EthicalControl/ontologies/MissionExecutionOntology#RE11.3.9">
        <rdfs:subClassOf rdf:resource="https://savage.nps.edu/EthicalControl/ontologies/MissionExecutionOntology#DADM11.3"/>
        <rdfs:comment>Do all commanders and users know how to conduct a risk assessment for the use of IAS?</rdfs:comment>
        <rdfs:label>RE11.3.9_UnderstandingConductRiskAssessmentIAS</rdfs:label>
        <owl:versionInfo>page 92</owl:versionInfo>
    </owl:Class>
    


    <!-- https://savage.nps.edu/EthicalControl/ontologies/MissionExecutionOntology#RE11.4.1 -->

    <owl:Class rdf:about="https://savage.nps.edu/EthicalControl/ontologies/MissionExecutionOntology#RE11.4.1">
        <rdfs:subClassOf rdf:resource="https://savage.nps.edu/EthicalControl/ontologies/MissionExecutionOntology#DADM11.4"/>
        <rdfs:comment>Do all commanders and users understand the difference between inductive, deductive, and abductive reasoning, and the limitations of algorithms in each?</rdfs:comment>
        <rdfs:label>RE11.4.1_UnderstandingReasoningMethodsLimitations</rdfs:label>
        <owl:versionInfo>page 92</owl:versionInfo>
    </owl:Class>
    


    <!-- https://savage.nps.edu/EthicalControl/ontologies/MissionExecutionOntology#RE11.4.2 -->

    <owl:Class rdf:about="https://savage.nps.edu/EthicalControl/ontologies/MissionExecutionOntology#RE11.4.2">
        <rdfs:subClassOf rdf:resource="https://savage.nps.edu/EthicalControl/ontologies/MissionExecutionOntology#DADM11.4"/>
        <rdfs:comment>Do all commanders and users understand the different types of machine learning (supervised, unsupervised, reinforcement) used by the IAS and the operational environments amenable to each?</rdfs:comment>
        <rdfs:label>RE11.4.2_UnderstandingMLUsedIAS</rdfs:label>
        <owl:versionInfo>page 92</owl:versionInfo>
    </owl:Class>
    


    <!-- https://savage.nps.edu/EthicalControl/ontologies/MissionExecutionOntology#RE11.5.1 -->

    <owl:Class rdf:about="https://savage.nps.edu/EthicalControl/ontologies/MissionExecutionOntology#RE11.5.1">
        <rdfs:subClassOf rdf:resource="https://savage.nps.edu/EthicalControl/ontologies/MissionExecutionOntology#DADM11.5"/>
        <rdfs:comment>Can all commanders and users recognize a data poisoning attack?</rdfs:comment>
        <rdfs:label>RE11.5.1_RecognizeDataPoisoningAttack</rdfs:label>
        <owl:versionInfo>page 92</owl:versionInfo>
    </owl:Class>
    


    <!-- https://savage.nps.edu/EthicalControl/ontologies/MissionExecutionOntology#RE11.5.2 -->

    <owl:Class rdf:about="https://savage.nps.edu/EthicalControl/ontologies/MissionExecutionOntology#RE11.5.2">
        <rdfs:subClassOf rdf:resource="https://savage.nps.edu/EthicalControl/ontologies/MissionExecutionOntology#DADM11.5"/>
        <rdfs:comment>Can all commanders and users recognize an instance of &quot;reward function gaming?&quot;</rdfs:comment>
        <rdfs:label>RE11.5.2_RecognizeRewardGamingMalfunction</rdfs:label>
        <owl:versionInfo>page 92</owl:versionInfo>
    </owl:Class>
    


    <!-- https://savage.nps.edu/EthicalControl/ontologies/MissionExecutionOntology#RE11.5.3 -->

    <owl:Class rdf:about="https://savage.nps.edu/EthicalControl/ontologies/MissionExecutionOntology#RE11.5.3">
        <rdfs:subClassOf rdf:resource="https://savage.nps.edu/EthicalControl/ontologies/MissionExecutionOntology#DADM11.5"/>
        <rdfs:comment>Can all commanders and users recognize an instance of &quot;adversarial spoofing?&quot;</rdfs:comment>
        <rdfs:label>RE11.5.3_RecognizeAdversarialSpoofing</rdfs:label>
        <owl:versionInfo>page 92</owl:versionInfo>
    </owl:Class>
    


    <!-- https://savage.nps.edu/EthicalControl/ontologies/MissionExecutionOntology#RE11.5.4 -->

    <owl:Class rdf:about="https://savage.nps.edu/EthicalControl/ontologies/MissionExecutionOntology#RE11.5.4">
        <rdfs:subClassOf rdf:resource="https://savage.nps.edu/EthicalControl/ontologies/MissionExecutionOntology#DADM11.5"/>
        <rdfs:comment>Can all commanders and users recognize an instance of &quot;catastrophic forgetting?&quot;</rdfs:comment>
        <rdfs:label>RE11.5.4_RecognizeCatastrophicForgetting</rdfs:label>
        <owl:versionInfo>page 92</owl:versionInfo>
    </owl:Class>
    


    <!-- https://savage.nps.edu/EthicalControl/ontologies/MissionExecutionOntology#RE11.5.5 -->

    <owl:Class rdf:about="https://savage.nps.edu/EthicalControl/ontologies/MissionExecutionOntology#RE11.5.5">
        <rdfs:subClassOf rdf:resource="https://savage.nps.edu/EthicalControl/ontologies/MissionExecutionOntology#DADM11.5"/>
        <rdfs:comment>Can all commanders and users recognize an instance of &quot;concept drift?&quot;</rdfs:comment>
        <rdfs:label>RE11.5.5_RecognizeConceptDrift</rdfs:label>
        <owl:versionInfo>page 92</owl:versionInfo>
    </owl:Class>
    


    <!-- https://savage.nps.edu/EthicalControl/ontologies/MissionExecutionOntology#RE11.5.6 -->

    <owl:Class rdf:about="https://savage.nps.edu/EthicalControl/ontologies/MissionExecutionOntology#RE11.5.6">
        <rdfs:subClassOf rdf:resource="https://savage.nps.edu/EthicalControl/ontologies/MissionExecutionOntology#DADM11.5"/>
        <rdfs:comment>Can all commanders and users recognize an instance of &quot;model inversion?&quot;</rdfs:comment>
        <rdfs:label>RE11.5.6_RecognizeModelInversion</rdfs:label>
        <owl:versionInfo>page 92</owl:versionInfo>
    </owl:Class>
    


    <!-- https://savage.nps.edu/EthicalControl/ontologies/MissionExecutionOntology#RE11.5.7 -->

    <owl:Class rdf:about="https://savage.nps.edu/EthicalControl/ontologies/MissionExecutionOntology#RE11.5.7">
        <rdfs:subClassOf rdf:resource="https://savage.nps.edu/EthicalControl/ontologies/MissionExecutionOntology#DADM11.5"/>
        <rdfs:comment>Can all commanders and users recognize a &quot;deep fake?&quot;</rdfs:comment>
        <rdfs:label>RE11.5.7_RecognizeDeepFake</rdfs:label>
        <owl:versionInfo>page 92</owl:versionInfo>
    </owl:Class>
    


    <!-- https://savage.nps.edu/EthicalControl/ontologies/MissionExecutionOntology#RE11.5.8 -->

    <owl:Class rdf:about="https://savage.nps.edu/EthicalControl/ontologies/MissionExecutionOntology#RE11.5.8">
        <rdfs:subClassOf rdf:resource="https://savage.nps.edu/EthicalControl/ontologies/MissionExecutionOntology#DADM11.5"/>
        <rdfs:comment>Can all commanders and users recognize an instance of reprogramming by unauthorized users?</rdfs:comment>
        <rdfs:label>RE11.5.8_RecognizeUnauthorizedReprogramming</rdfs:label>
        <owl:versionInfo>page 92</owl:versionInfo>
    </owl:Class>
    


    <!-- https://savage.nps.edu/EthicalControl/ontologies/MissionExecutionOntology#RE11.5.9 -->

    <owl:Class rdf:about="https://savage.nps.edu/EthicalControl/ontologies/MissionExecutionOntology#RE11.5.9">
        <rdfs:subClassOf rdf:resource="https://savage.nps.edu/EthicalControl/ontologies/MissionExecutionOntology#DADM11.5"/>
        <rdfs:comment>Can all commanders and users recognize a system that is &quot;tightly coupled?&quot;</rdfs:comment>
        <rdfs:label>RE11.5.9_RecognizeTightlyCoupledSystem</rdfs:label>
        <owl:versionInfo>page 92</owl:versionInfo>
    </owl:Class>
    


    <!-- https://savage.nps.edu/EthicalControl/ontologies/MissionExecutionOntology#RE12.1.1 -->

    <owl:Class rdf:about="https://savage.nps.edu/EthicalControl/ontologies/MissionExecutionOntology#RE12.1.1">
        <rdfs:subClassOf rdf:resource="https://savage.nps.edu/EthicalControl/ontologies/MissionExecutionOntology#DADM12.1"/>
        <rdfs:comment>Can the commander reduce the mission duration such that the IAS risk mitigation conditions and planning factors will be, or can reasonably be expected to be, uniformly consistent?</rdfs:comment>
        <rdfs:label>RE12.1.1_DurationLimitedUniformlyConsistent</rdfs:label>
        <owl:versionInfo>page 93</owl:versionInfo>
    </owl:Class>
    


    <!-- https://savage.nps.edu/EthicalControl/ontologies/MissionExecutionOntology#RE12.1.2 -->

    <owl:Class rdf:about="https://savage.nps.edu/EthicalControl/ontologies/MissionExecutionOntology#RE12.1.2">
        <rdfs:subClassOf rdf:resource="https://savage.nps.edu/EthicalControl/ontologies/MissionExecutionOntology#DADM12.1"/>
        <rdfs:comment>Does the target selection that the human operator provides the IAS have an expiration time within the duration of the mission, such that the human operator will be alerted to select and verify new targets after the expiration time has expired?</rdfs:comment>
        <rdfs:label>RE12.1.2_TargetTimeouts</rdfs:label>
        <owl:versionInfo>page 93</owl:versionInfo>
    </owl:Class>
    


    <!-- https://savage.nps.edu/EthicalControl/ontologies/MissionExecutionOntology#RE12.1.3 -->

    <owl:Class rdf:about="https://savage.nps.edu/EthicalControl/ontologies/MissionExecutionOntology#RE12.1.3">
        <rdfs:subClassOf rdf:resource="https://savage.nps.edu/EthicalControl/ontologies/MissionExecutionOntology#DADM12.1"/>
        <rdfs:comment>Is the commander able to alter the degree of autonomy of the IAS during long missions based on whether it is in a loitering mode, or an active task execution mode?</rdfs:comment>
        <rdfs:label>RE12.1.3_AlterableDegreeAutonomy</rdfs:label>
        <owl:versionInfo>page 93</owl:versionInfo>
    </owl:Class>
    


    <!-- https://savage.nps.edu/EthicalControl/ontologies/MissionExecutionOntology#RE12.1.4 -->

    <owl:Class rdf:about="https://savage.nps.edu/EthicalControl/ontologies/MissionExecutionOntology#RE12.1.4">
        <rdfs:subClassOf rdf:resource="https://savage.nps.edu/EthicalControl/ontologies/MissionExecutionOntology#DADM12.1"/>
        <rdfs:comment>Is the reliability of communications links commensurate with both the duration and the geographic extent of the mission?</rdfs:comment>
        <rdfs:label>RE12.1.4_CommsReliabilityDurationGeographicMissionExtent</rdfs:label>
        <owl:versionInfo>page 93</owl:versionInfo>
    </owl:Class>
    


    <!-- https://savage.nps.edu/EthicalControl/ontologies/MissionExecutionOntology#RE12.1.5 -->

    <owl:Class rdf:about="https://savage.nps.edu/EthicalControl/ontologies/MissionExecutionOntology#RE12.1.5">
        <rdfs:subClassOf rdf:resource="https://savage.nps.edu/EthicalControl/ontologies/MissionExecutionOntology#DADM12.1"/>
        <rdfs:comment>Can the IAS compare risk mitigation and planning factors provided to it at the beginning of a long mission, and compare these to sensed conditions just prior to an action/decision and abort the action if they are different?</rdfs:comment>
        <rdfs:label>RE12.1.5_ComparisonChangingMissionParameters</rdfs:label>
        <owl:versionInfo>page 93</owl:versionInfo>
    </owl:Class>
    


    <!-- https://savage.nps.edu/EthicalControl/ontologies/MissionExecutionOntology#RE12.2.1 -->

    <owl:Class rdf:about="https://savage.nps.edu/EthicalControl/ontologies/MissionExecutionOntology#RE12.2.1">
        <rdfs:subClassOf rdf:resource="https://savage.nps.edu/EthicalControl/ontologies/MissionExecutionOntology#DADM12.2"/>
        <rdfs:comment>Can the commander reduce the expanse of the operational environment to an area where risk mitigation conditions and planning factors are known to be, or are reasonably expected to be, uniformly consistent?</rdfs:comment>
        <rdfs:label>RE12.2.1_ExpanseLimitedUniformlyConsistent</rdfs:label>
        <owl:versionInfo>page 93</owl:versionInfo>
    </owl:Class>
    


    <!-- https://savage.nps.edu/EthicalControl/ontologies/MissionExecutionOntology#RE12.2.2 -->

    <owl:Class rdf:about="https://savage.nps.edu/EthicalControl/ontologies/MissionExecutionOntology#RE12.2.2">
        <rdfs:subClassOf rdf:resource="https://savage.nps.edu/EthicalControl/ontologies/MissionExecutionOntology#DADM12.2"/>
        <rdfs:comment>Can the commander subdivide a large operational area into smaller ones where risk mitigation conditions and planning factors are known to be, or are reasonably expected to be, uniformly consistent, and assign one IAS to each area, with each IAS specifically programmed to address the conditions unique to each subsection?</rdfs:comment>
        <rdfs:label>RE12.2.2_MissionOperationalAreaDividedUniformlyConsistent</rdfs:label>
        <owl:versionInfo>page 93</owl:versionInfo>
    </owl:Class>
    


    <!-- https://savage.nps.edu/EthicalControl/ontologies/MissionExecutionOntology#RE12.2.3 -->

    <owl:Class rdf:about="https://savage.nps.edu/EthicalControl/ontologies/MissionExecutionOntology#RE12.2.3">
        <rdfs:subClassOf rdf:resource="https://savage.nps.edu/EthicalControl/ontologies/MissionExecutionOntology#DADM12.2"/>
        <rdfs:comment>Is the IAS equipped with a capability that tailors its approved degree of autonomy and authorized actions based on geographical location?</rdfs:comment>
        <rdfs:label>RE12.2.3_LocationBasedDegreeAutonomy</rdfs:label>
        <owl:versionInfo>page 93</owl:versionInfo>
    </owl:Class>
    


    <!-- https://savage.nps.edu/EthicalControl/ontologies/MissionExecutionOntology#RE12.2.4 -->

    <owl:Class rdf:about="https://savage.nps.edu/EthicalControl/ontologies/MissionExecutionOntology#RE12.2.4">
        <rdfs:subClassOf rdf:resource="https://savage.nps.edu/EthicalControl/ontologies/MissionExecutionOntology#DADM12.2"/>
        <rdfs:comment>If a target is verified within a geographic location but transits outside it later in time, can the IAS still engage, or does it immediately cease action?</rdfs:comment>
        <rdfs:label>RE12.2.4_IASRecognizedDisplacedWillCease</rdfs:label>
        <owl:versionInfo>page 93</owl:versionInfo>
    </owl:Class>
    


    <!-- https://savage.nps.edu/EthicalControl/ontologies/MissionExecutionOntology#RE12.2.5 -->

    <owl:Class rdf:about="https://savage.nps.edu/EthicalControl/ontologies/MissionExecutionOntology#RE12.2.5">
        <rdfs:subClassOf rdf:resource="https://savage.nps.edu/EthicalControl/ontologies/MissionExecutionOntology#DADM12.2"/>
        <rdfs:comment>Is the IAS equipped with a capability that tailors its approved degree of autonomy and authorized actions based on its distance from a human operator?</rdfs:comment>
        <rdfs:label>RE12.2.5_DistanceBasedDegreeAutonomy</rdfs:label>
        <owl:versionInfo>page 93</owl:versionInfo>
    </owl:Class>
    


    <!-- https://savage.nps.edu/EthicalControl/ontologies/MissionExecutionOntology#RE12.2.6 -->

    <owl:Class rdf:about="https://savage.nps.edu/EthicalControl/ontologies/MissionExecutionOntology#RE12.2.6">
        <rdfs:subClassOf rdf:resource="https://savage.nps.edu/EthicalControl/ontologies/MissionExecutionOntology#DADM12.2"/>
        <rdfs:comment>Can the IAS recognize when it is assigned an area of regard too large for reliable autonomous operation?</rdfs:comment>
        <rdfs:label>RE12.2.6_IASReportAORTooLarge</rdfs:label>
        <owl:versionInfo>page 93</owl:versionInfo>
    </owl:Class>
    


    <!-- https://savage.nps.edu/EthicalControl/ontologies/MissionExecutionOntology#RE12.2.7 -->

    <owl:Class rdf:about="https://savage.nps.edu/EthicalControl/ontologies/MissionExecutionOntology#RE12.2.7">
        <rdfs:subClassOf rdf:resource="https://savage.nps.edu/EthicalControl/ontologies/MissionExecutionOntology#DADM12.2"/>
        <rdfs:comment>Can the IAS recognize when it has been assigned to an area of regard where the fundamental risk mitigation conditions are not uniformly consistent?</rdfs:comment>
        <rdfs:label>RE12.2.7_IASReportAsymetricRiskAreas</rdfs:label>
        <owl:versionInfo>page 94</owl:versionInfo>
    </owl:Class>
    


    <!-- https://savage.nps.edu/EthicalControl/ontologies/MissionExecutionOntology#RE12.3.1 -->

    <owl:Class rdf:about="https://savage.nps.edu/EthicalControl/ontologies/MissionExecutionOntology#RE12.3.1">
        <rdfs:subClassOf rdf:resource="https://savage.nps.edu/EthicalControl/ontologies/MissionExecutionOntology#DADM12.3"/>
        <rdfs:comment>Is the IAS equipped with a switch that will disable its autonomous functionalities after a predetermined set time has elapsed?</rdfs:comment>
        <rdfs:label>RE12.3.1_AutonomousFunctionTimeout</rdfs:label>
        <owl:versionInfo>page 94</owl:versionInfo>
    </owl:Class>
    


    <!-- https://savage.nps.edu/EthicalControl/ontologies/MissionExecutionOntology#RE12.3.2 -->

    <owl:Class rdf:about="https://savage.nps.edu/EthicalControl/ontologies/MissionExecutionOntology#RE12.3.2">
        <rdfs:subClassOf rdf:resource="https://savage.nps.edu/EthicalControl/ontologies/MissionExecutionOntology#DADM12.3"/>
        <rdfs:comment>Is the IAS equipped with a geo-fence switch that will disable its autonomous functionalities if it strays from an authorized operational area?</rdfs:comment>
        <rdfs:label>RE12.3.2_AutonomousDisengageOutsideGeofence</rdfs:label>
        <owl:versionInfo>page 94</owl:versionInfo>
    </owl:Class>
    


    <!-- https://savage.nps.edu/EthicalControl/ontologies/MissionExecutionOntology#RE12.3.3 -->

    <owl:Class rdf:about="https://savage.nps.edu/EthicalControl/ontologies/MissionExecutionOntology#RE12.3.3">
        <rdfs:subClassOf rdf:resource="https://savage.nps.edu/EthicalControl/ontologies/MissionExecutionOntology#DADM12.3"/>
        <rdfs:comment>If risk is reduced with increased mission time or expanded geographic range, can the human operator increase autonomous capabilities of the IAS as needed?</rdfs:comment>
        <rdfs:label>RE12.3.3_AutonomyModeChangedOverTime</rdfs:label>
        <owl:versionInfo>page 94</owl:versionInfo>
    </owl:Class>
    


    <!-- https://savage.nps.edu/EthicalControl/ontologies/MissionExecutionOntology#RE12.3.4 -->

    <owl:Class rdf:about="https://savage.nps.edu/EthicalControl/ontologies/MissionExecutionOntology#RE12.3.4">
        <rdfs:subClassOf rdf:resource="https://savage.nps.edu/EthicalControl/ontologies/MissionExecutionOntology#DADM12.3"/>
        <rdfs:comment>Is the commander notified if they have an IAS with a disablement switch that has been overridden by higher authority?</rdfs:comment>
        <rdfs:label>RE12.3.4_CommanderNotifiedHigherAuthorityOverride</rdfs:label>
        <owl:versionInfo>page 94</owl:versionInfo>
    </owl:Class>
    


    <!-- https://savage.nps.edu/EthicalControl/ontologies/MissionExecutionOntology#RE12.3.5 -->

    <owl:Class rdf:about="https://savage.nps.edu/EthicalControl/ontologies/MissionExecutionOntology#RE12.3.5">
        <rdfs:subClassOf rdf:resource="https://savage.nps.edu/EthicalControl/ontologies/MissionExecutionOntology#DADM12.3"/>
        <rdfs:comment>Is the IAS equipped with a disablement switch that can selectively disable only certain functions or subsystems?</rdfs:comment>
        <rdfs:label>RE12.3.5_IASDisablementSystemGranularity</rdfs:label>
        <owl:versionInfo>page 94</owl:versionInfo>
    </owl:Class>
    


    <!-- https://savage.nps.edu/EthicalControl/ontologies/MissionExecutionOntology#RE12.3.6 -->

    <owl:Class rdf:about="https://savage.nps.edu/EthicalControl/ontologies/MissionExecutionOntology#RE12.3.6">
        <rdfs:subClassOf rdf:resource="https://savage.nps.edu/EthicalControl/ontologies/MissionExecutionOntology#DADM12.3"/>
        <rdfs:comment>Is the IAS equipped with a &quot;soft&quot; disablement switch that disables autonomous functionality but can be reversed if certain predetermined conditions are detected or an override authorization is received?</rdfs:comment>
        <rdfs:label>RE12.3.6_AutonomyConditionalReengagement</rdfs:label>
        <owl:versionInfo>page 94</owl:versionInfo>
    </owl:Class>
    


    <!-- https://savage.nps.edu/EthicalControl/ontologies/MissionExecutionOntology#RE12.3.7 -->

    <owl:Class rdf:about="https://savage.nps.edu/EthicalControl/ontologies/MissionExecutionOntology#RE12.3.7">
        <rdfs:subClassOf rdf:resource="https://savage.nps.edu/EthicalControl/ontologies/MissionExecutionOntology#DADM12.3"/>
        <rdfs:comment>If the IAS is disabled, can it safely and securely return to a predetermined location? </rdfs:comment>
        <rdfs:label>RE12.3.7_IASAttemptRTB</rdfs:label>
        <owl:versionInfo>page 94</owl:versionInfo>
    </owl:Class>
    


    <!-- https://savage.nps.edu/EthicalControl/ontologies/MissionExecutionOntology#RE13.1.1 -->

    <owl:Class rdf:about="https://savage.nps.edu/EthicalControl/ontologies/MissionExecutionOntology#RE13.1.1">
        <rdfs:subClassOf rdf:resource="https://savage.nps.edu/EthicalControl/ontologies/MissionExecutionOntology#DADM13.1"/>
        <rdfs:comment>Does the IAS potentially affect the rights enumerated in the first ten amendments to the US Constitution (the Bill of Rights)?</rdfs:comment>
        <rdfs:label>RE13.1.1_IASAffectBillOfRights</rdfs:label>
        <owl:versionInfo>page 94</owl:versionInfo>
    </owl:Class>
    


    <!-- https://savage.nps.edu/EthicalControl/ontologies/MissionExecutionOntology#RE13.1.2 -->

    <owl:Class rdf:about="https://savage.nps.edu/EthicalControl/ontologies/MissionExecutionOntology#RE13.1.2">
        <rdfs:subClassOf rdf:resource="https://savage.nps.edu/EthicalControl/ontologies/MissionExecutionOntology#DADM13.1"/>
        <rdfs:comment>Does the IAS potentially affect the rights enumerated in the Civil Rights Act of 1964, the Equal Protection Clause of the U.S. Constitution and all subsequent enactments?</rdfs:comment>
        <rdfs:label>RE13.1.2_IASAffectCivilEqualConstitutionRights</rdfs:label>
        <owl:versionInfo>page 94</owl:versionInfo>
    </owl:Class>
    


    <!-- https://savage.nps.edu/EthicalControl/ontologies/MissionExecutionOntology#RE13.1.3 -->

    <owl:Class rdf:about="https://savage.nps.edu/EthicalControl/ontologies/MissionExecutionOntology#RE13.1.3">
        <rdfs:subClassOf rdf:resource="https://savage.nps.edu/EthicalControl/ontologies/MissionExecutionOntology#DADM13.1"/>
        <rdfs:comment>Does the IAS potentially affect the rights enumerated in the European Union General Data Protection Regulation or the US Privacy Statutes regarding collection, transmission and safeguarding of personal data?</rdfs:comment>
        <rdfs:label>RE13.1.3_IASAffectEuropeanUSPersonalData</rdfs:label>
        <owl:versionInfo>page 94</owl:versionInfo>
    </owl:Class>
    


    <!-- https://savage.nps.edu/EthicalControl/ontologies/MissionExecutionOntology#RE13.1.4 -->

    <owl:Class rdf:about="https://savage.nps.edu/EthicalControl/ontologies/MissionExecutionOntology#RE13.1.4">
        <rdfs:subClassOf rdf:resource="https://savage.nps.edu/EthicalControl/ontologies/MissionExecutionOntology#DADM13.1"/>
        <rdfs:comment>Does the IAS potentially affect due process?</rdfs:comment>
        <rdfs:label>RE13.1.4_IASAffectDueProcess</rdfs:label>
        <owl:versionInfo>page 94</owl:versionInfo>
    </owl:Class>
    


    <!-- https://savage.nps.edu/EthicalControl/ontologies/MissionExecutionOntology#RE13.1.5 -->

    <owl:Class rdf:about="https://savage.nps.edu/EthicalControl/ontologies/MissionExecutionOntology#RE13.1.5">
        <rdfs:subClassOf rdf:resource="https://savage.nps.edu/EthicalControl/ontologies/MissionExecutionOntology#DADM13.1"/>
        <rdfs:comment>Does the IAS potentially affect agreements to not retain personally identifiable information after termination of IAS use?</rdfs:comment>
        <rdfs:label>RE13.1.5_IASAffectPIIAgreements</rdfs:label>
        <owl:versionInfo>page 94</owl:versionInfo>
    </owl:Class>
    


    <!-- https://savage.nps.edu/EthicalControl/ontologies/MissionExecutionOntology#RE13.1.6 -->

    <owl:Class rdf:about="https://savage.nps.edu/EthicalControl/ontologies/MissionExecutionOntology#RE13.1.6">
        <rdfs:subClassOf rdf:resource="https://savage.nps.edu/EthicalControl/ontologies/MissionExecutionOntology#DADM13.1"/>
        <rdfs:comment>Does the IAS potentially affect the &quot;dictates of public conscience?&quot;</rdfs:comment>
        <rdfs:label>RE13.1.6_IASAffectDictatesPublicConscience</rdfs:label>
        <owl:versionInfo>page 94</owl:versionInfo>
    </owl:Class>
    


    <!-- https://savage.nps.edu/EthicalControl/ontologies/MissionExecutionOntology#RE13.1.7 -->

    <owl:Class rdf:about="https://savage.nps.edu/EthicalControl/ontologies/MissionExecutionOntology#RE13.1.7">
        <rdfs:subClassOf rdf:resource="https://savage.nps.edu/EthicalControl/ontologies/MissionExecutionOntology#DADM13.1"/>
        <rdfs:comment>Does the IAS potentially affect the establishment of mass surveillance capabilities in an area where there is an expectation of privacy?</rdfs:comment>
        <rdfs:label>RE13.1.7_IASAffectMassSurveillancePrivacyExpectation</rdfs:label>
        <owl:versionInfo>page 95</owl:versionInfo>
    </owl:Class>
    


    <!-- https://savage.nps.edu/EthicalControl/ontologies/MissionExecutionOntology#RE13.2.1 -->

    <owl:Class rdf:about="https://savage.nps.edu/EthicalControl/ontologies/MissionExecutionOntology#RE13.2.1">
        <rdfs:subClassOf rdf:resource="https://savage.nps.edu/EthicalControl/ontologies/MissionExecutionOntology#DADM13.2"/>
        <rdfs:comment>Are potentially affected persons notified that the IAS is in use?</rdfs:comment>
        <rdfs:label>RE13.2.1_IASUseRequiresNotification</rdfs:label>
        <owl:versionInfo>page 95</owl:versionInfo>
    </owl:Class>
    


    <!-- https://savage.nps.edu/EthicalControl/ontologies/MissionExecutionOntology#RE13.2.10 -->

    <owl:Class rdf:about="https://savage.nps.edu/EthicalControl/ontologies/MissionExecutionOntology#RE13.2.10">
        <rdfs:subClassOf rdf:resource="https://savage.nps.edu/EthicalControl/ontologies/MissionExecutionOntology#DADM13.2"/>
        <rdfs:comment>Are potentially affected persons made aware when sensitive personal information is collected and retained by the IAS?</rdfs:comment>
        <rdfs:label>RE13.2.10_IASPotentiallyAffectedPersonsAwareSensitivePersonalInformation</rdfs:label>
        <owl:versionInfo>page 95</owl:versionInfo>
    </owl:Class>
    


    <!-- https://savage.nps.edu/EthicalControl/ontologies/MissionExecutionOntology#RE13.2.11 -->

    <owl:Class rdf:about="https://savage.nps.edu/EthicalControl/ontologies/MissionExecutionOntology#RE13.2.11">
        <rdfs:subClassOf rdf:resource="https://savage.nps.edu/EthicalControl/ontologies/MissionExecutionOntology#DADM13.2"/>
        <rdfs:comment>Are potentially affected persons notified when their personal data is destroyed after IAS use?</rdfs:comment>
        <rdfs:label>RE13.2.11_IASPotentiallyAffectedPersonsNotifiedPersonalDataDestroyed</rdfs:label>
        <owl:versionInfo>page 95</owl:versionInfo>
    </owl:Class>
    


    <!-- https://savage.nps.edu/EthicalControl/ontologies/MissionExecutionOntology#RE13.2.12 -->

    <owl:Class rdf:about="https://savage.nps.edu/EthicalControl/ontologies/MissionExecutionOntology#RE13.2.12">
        <rdfs:subClassOf rdf:resource="https://savage.nps.edu/EthicalControl/ontologies/MissionExecutionOntology#DADM13.2"/>
        <rdfs:comment>Are potentially affected persons made aware of retention policies and schedules for personal data?</rdfs:comment>
        <rdfs:label>RE13.2.12_IASPotentiallyAffectedPersonsAwareRetentionPoliciesPersonalData</rdfs:label>
        <owl:versionInfo>page 95</owl:versionInfo>
    </owl:Class>
    


    <!-- https://savage.nps.edu/EthicalControl/ontologies/MissionExecutionOntology#RE13.2.13 -->

    <owl:Class rdf:about="https://savage.nps.edu/EthicalControl/ontologies/MissionExecutionOntology#RE13.2.13">
        <rdfs:subClassOf rdf:resource="https://savage.nps.edu/EthicalControl/ontologies/MissionExecutionOntology#DADM13.2"/>
        <rdfs:comment>Are potentially affected persons allowed to deny the disclosure of their personal data to third parties?</rdfs:comment>
        <rdfs:label>RE13.2.13_IASPotentiallyAffectedPersonsCanControlThirdPartyDisclosure</rdfs:label>
        <owl:versionInfo>page 95</owl:versionInfo>
    </owl:Class>
    


    <!-- https://savage.nps.edu/EthicalControl/ontologies/MissionExecutionOntology#RE13.2.14 -->

    <owl:Class rdf:about="https://savage.nps.edu/EthicalControl/ontologies/MissionExecutionOntology#RE13.2.14">
        <rdfs:subClassOf rdf:resource="https://savage.nps.edu/EthicalControl/ontologies/MissionExecutionOntology#DADM13.2"/>
        <rdfs:comment>Are potentially affected persons made aware of personal data protection policies and measures?</rdfs:comment>
        <rdfs:label>RE13.2.14_IASPotentiallyAffectedPersonsPersonalDataProtectionPoliciesMeasures</rdfs:label>
        <owl:versionInfo>page 95</owl:versionInfo>
    </owl:Class>
    


    <!-- https://savage.nps.edu/EthicalControl/ontologies/MissionExecutionOntology#RE13.2.15 -->

    <owl:Class rdf:about="https://savage.nps.edu/EthicalControl/ontologies/MissionExecutionOntology#RE13.2.15">
        <rdfs:subClassOf rdf:resource="https://savage.nps.edu/EthicalControl/ontologies/MissionExecutionOntology#DADM13.2"/>
        <rdfs:comment>Are potentially affected persons notified of the purpose of the IAS that is trained using their personal data?</rdfs:comment>
        <rdfs:label>RE13.2.15_IASPotentiallyAffectedPersonsNotifiedTrainingPersonalData</rdfs:label>
        <owl:versionInfo>page 95</owl:versionInfo>
    </owl:Class>
    


    <!-- https://savage.nps.edu/EthicalControl/ontologies/MissionExecutionOntology#RE13.2.16 -->

    <owl:Class rdf:about="https://savage.nps.edu/EthicalControl/ontologies/MissionExecutionOntology#RE13.2.16">
        <rdfs:subClassOf rdf:resource="https://savage.nps.edu/EthicalControl/ontologies/MissionExecutionOntology#DADM13.2"/>
        <rdfs:comment>Are potentially affected persons informed when they are interacting with an IAS and not a human being?</rdfs:comment>
        <rdfs:label>RE13.2.16_IASPotentiallyAffectedPersonsInformedInteractingIAS</rdfs:label>
        <owl:versionInfo>page 96</owl:versionInfo>
    </owl:Class>
    


    <!-- https://savage.nps.edu/EthicalControl/ontologies/MissionExecutionOntology#RE13.2.17 -->

    <owl:Class rdf:about="https://savage.nps.edu/EthicalControl/ontologies/MissionExecutionOntology#RE13.2.17">
        <rdfs:subClassOf rdf:resource="https://savage.nps.edu/EthicalControl/ontologies/MissionExecutionOntology#DADM13.2"/>
        <rdfs:comment>Are potentially affected persons made aware of the demographic, professional and intellectual diversity of the staff that developed the IAS?</rdfs:comment>
        <rdfs:label>RE13.2.17_IASPotentiallyAffectedPersonsMadeAwareDemographicProfessionalIntellectualDiversity</rdfs:label>
        <owl:versionInfo>page 96</owl:versionInfo>
    </owl:Class>
    


    <!-- https://savage.nps.edu/EthicalControl/ontologies/MissionExecutionOntology#RE13.2.18 -->

    <owl:Class rdf:about="https://savage.nps.edu/EthicalControl/ontologies/MissionExecutionOntology#RE13.2.18">
        <rdfs:subClassOf rdf:resource="https://savage.nps.edu/EthicalControl/ontologies/MissionExecutionOntology#DADM13.2"/>
        <rdfs:comment>Are potentially affected persons made aware of negative determinations made by an IAS and given an opportunity to challenge those determinations to a human arbitrator?</rdfs:comment>
        <rdfs:label>RE13.2.18_IASPotentiallyAffectedPersonsChallengeNegativeDeterminations</rdfs:label>
        <owl:versionInfo>page 96</owl:versionInfo>
    </owl:Class>
    


    <!-- https://savage.nps.edu/EthicalControl/ontologies/MissionExecutionOntology#RE13.2.19 -->

    <owl:Class rdf:about="https://savage.nps.edu/EthicalControl/ontologies/MissionExecutionOntology#RE13.2.19">
        <rdfs:subClassOf rdf:resource="https://savage.nps.edu/EthicalControl/ontologies/MissionExecutionOntology#DADM13.2"/>
        <rdfs:comment>Are potentially affected persons informed as to what policies, laws, regulations, and/or rules governed the use of the IAS?</rdfs:comment>
        <rdfs:label>RE13.2.19_IASPotentiallyAffectedPersonsInformedPolicyLawRegsRules</rdfs:label>
        <owl:versionInfo>page 96</owl:versionInfo>
    </owl:Class>
    


    <!-- https://savage.nps.edu/EthicalControl/ontologies/MissionExecutionOntology#RE13.2.2 -->

    <owl:Class rdf:about="https://savage.nps.edu/EthicalControl/ontologies/MissionExecutionOntology#RE13.2.2">
        <rdfs:subClassOf rdf:resource="https://savage.nps.edu/EthicalControl/ontologies/MissionExecutionOntology#DADM13.2"/>
        <rdfs:comment>Are potentially affected persons allowed to monitor the use of the IAS?</rdfs:comment>
        <rdfs:label>RE13.2.2_IASPotentiallyAffectedPersonsAllowedMonitorUse</rdfs:label>
        <owl:versionInfo>page 95</owl:versionInfo>
    </owl:Class>
    


    <!-- https://savage.nps.edu/EthicalControl/ontologies/MissionExecutionOntology#RE13.2.20 -->

    <owl:Class rdf:about="https://savage.nps.edu/EthicalControl/ontologies/MissionExecutionOntology#RE13.2.20">
        <rdfs:subClassOf rdf:resource="https://savage.nps.edu/EthicalControl/ontologies/MissionExecutionOntology#DADM13.2"/>
        <rdfs:comment>Are potentially affected persons informed as to the test and evaluation procedures used to validate the IAS?</rdfs:comment>
        <rdfs:label>RE13.2.20_IASPotentiallyAffectedPersonsTestValidationProcedures</rdfs:label>
        <owl:versionInfo>page 96</owl:versionInfo>
    </owl:Class>
    


    <!-- https://savage.nps.edu/EthicalControl/ontologies/MissionExecutionOntology#RE13.2.21 -->

    <owl:Class rdf:about="https://savage.nps.edu/EthicalControl/ontologies/MissionExecutionOntology#RE13.2.21">
        <rdfs:subClassOf rdf:resource="https://savage.nps.edu/EthicalControl/ontologies/MissionExecutionOntology#DADM13.2"/>
        <rdfs:comment>Are potentially affected persons informed when the IAS is repurposed for use from some other, unrelated original purpose?</rdfs:comment>
        <rdfs:label>RE13.2.21_IASPotentiallyAffectedPersonsInformedRepurpose</rdfs:label>
        <owl:versionInfo>page 96</owl:versionInfo>
    </owl:Class>
    


    <!-- https://savage.nps.edu/EthicalControl/ontologies/MissionExecutionOntology#RE13.2.22 -->

    <owl:Class rdf:about="https://savage.nps.edu/EthicalControl/ontologies/MissionExecutionOntology#RE13.2.22">
        <rdfs:subClassOf rdf:resource="https://savage.nps.edu/EthicalControl/ontologies/MissionExecutionOntology#DADM13.2"/>
        <rdfs:comment>Are potentially affected persons made aware when the perpetuation of a bias by an IAS has been discovered?</rdfs:comment>
        <rdfs:label>RE13.2.22_IASPotentiallyAffectedPersonsNotificationPerpetuationBias</rdfs:label>
        <owl:versionInfo>page 96</owl:versionInfo>
    </owl:Class>
    


    <!-- https://savage.nps.edu/EthicalControl/ontologies/MissionExecutionOntology#RE13.2.23 -->

    <owl:Class rdf:about="https://savage.nps.edu/EthicalControl/ontologies/MissionExecutionOntology#RE13.2.23">
        <rdfs:subClassOf rdf:resource="https://savage.nps.edu/EthicalControl/ontologies/MissionExecutionOntology#DADM13.2"/>
        <rdfs:comment>Are potentially affected persons advised that IAS use can have adverse effects, even though they are unintended?</rdfs:comment>
        <rdfs:label>RE13.2.23_IASPotentiallyAffectedPersonsAdvisedUnintendedAdverseEffects</rdfs:label>
        <owl:versionInfo>page 96</owl:versionInfo>
    </owl:Class>
    


    <!-- https://savage.nps.edu/EthicalControl/ontologies/MissionExecutionOntology#RE13.2.3 -->

    <owl:Class rdf:about="https://savage.nps.edu/EthicalControl/ontologies/MissionExecutionOntology#RE13.2.3">
        <rdfs:subClassOf rdf:resource="https://savage.nps.edu/EthicalControl/ontologies/MissionExecutionOntology#DADM13.2"/>
        <rdfs:comment>Are potentially affected persons allowed to opt in or opt out of the use of the IAS?</rdfs:comment>
        <rdfs:label>RE13.2.3_IASPotentiallyAffectedPersonsAllowedOptIn</rdfs:label>
        <owl:versionInfo>page 95</owl:versionInfo>
    </owl:Class>
    


    <!-- https://savage.nps.edu/EthicalControl/ontologies/MissionExecutionOntology#RE13.2.4 -->

    <owl:Class rdf:about="https://savage.nps.edu/EthicalControl/ontologies/MissionExecutionOntology#RE13.2.4">
        <rdfs:subClassOf rdf:resource="https://savage.nps.edu/EthicalControl/ontologies/MissionExecutionOntology#DADM13.2"/>
        <rdfs:comment>Are potentially affected persons made aware of the opportunities to, and the procedures for, requesting access to IAS source code for inspection purposes?</rdfs:comment>
        <rdfs:label>RE13.2.4_IASPotentiallyAffectedPersonsAllowedMonitorUse</rdfs:label>
        <owl:versionInfo>page 95</owl:versionInfo>
    </owl:Class>
    


    <!-- https://savage.nps.edu/EthicalControl/ontologies/MissionExecutionOntology#RE13.2.5 -->

    <owl:Class rdf:about="https://savage.nps.edu/EthicalControl/ontologies/MissionExecutionOntology#RE13.2.5">
        <rdfs:subClassOf rdf:resource="https://savage.nps.edu/EthicalControl/ontologies/MissionExecutionOntology#DADM13.2"/>
        <rdfs:comment>Are potentially affected persons aware of the opportunities to, and the procedures for, requesting access to IAS concepts of operations and standard operating procedures for inspection purposes?</rdfs:comment>
        <rdfs:label>RE13.2.5_IASPotentiallyAffectedPersonsAwareSOPConops</rdfs:label>
        <owl:versionInfo>page 95</owl:versionInfo>
    </owl:Class>
    


    <!-- https://savage.nps.edu/EthicalControl/ontologies/MissionExecutionOntology#RE13.2.6 -->

    <owl:Class rdf:about="https://savage.nps.edu/EthicalControl/ontologies/MissionExecutionOntology#RE13.2.6">
        <rdfs:subClassOf rdf:resource="https://savage.nps.edu/EthicalControl/ontologies/MissionExecutionOntology#DADM13.2"/>
        <rdfs:comment>Are potentially affected persons aware of the opportunities to, and the procedures for, requesting access to IAS training data for inspection purposes?</rdfs:comment>
        <rdfs:label>RE13.2.6_IASPotentiallyAffectedPersonsAwareAccessTrainingDataInspection</rdfs:label>
        <owl:versionInfo>page 95</owl:versionInfo>
    </owl:Class>
    


    <!-- https://savage.nps.edu/EthicalControl/ontologies/MissionExecutionOntology#RE13.2.7 -->

    <owl:Class rdf:about="https://savage.nps.edu/EthicalControl/ontologies/MissionExecutionOntology#RE13.2.7">
        <rdfs:subClassOf rdf:resource="https://savage.nps.edu/EthicalControl/ontologies/MissionExecutionOntology#DADM13.2"/>
        <rdfs:comment>Are potentially affected persons advised that IAS use can have adverse impacts based on age, race, color, ethnicity, sex, religion, national origin, gender, gender identity, sexual orientation, familial status, biometric information, or disability status or economic class?</rdfs:comment>
        <rdfs:label>RE13.2.7_IASPotentiallyAffectedPersonsAdvisedAdverseImpacts</rdfs:label>
        <owl:versionInfo>page 95</owl:versionInfo>
    </owl:Class>
    


    <!-- https://savage.nps.edu/EthicalControl/ontologies/MissionExecutionOntology#RE13.2.8 -->

    <owl:Class rdf:about="https://savage.nps.edu/EthicalControl/ontologies/MissionExecutionOntology#RE13.2.8">
        <rdfs:subClassOf rdf:resource="https://savage.nps.edu/EthicalControl/ontologies/MissionExecutionOntology#DADM13.2"/>
        <rdfs:comment>Are potentially affected persons advised that IAS use can have adverse impacts based on membership in a group that enjoys legally protected status?</rdfs:comment>
        <rdfs:label>RE13.2.8_IASPotentiallyAffectedPersonsAdviseAdverseLegallyProtectedGroup</rdfs:label>
        <owl:versionInfo>page 95</owl:versionInfo>
    </owl:Class>
    


    <!-- https://savage.nps.edu/EthicalControl/ontologies/MissionExecutionOntology#RE13.2.9 -->

    <owl:Class rdf:about="https://savage.nps.edu/EthicalControl/ontologies/MissionExecutionOntology#RE13.2.9">
        <rdfs:subClassOf rdf:resource="https://savage.nps.edu/EthicalControl/ontologies/MissionExecutionOntology#DADM13.2"/>
        <rdfs:comment>Are potentially affected persons advised that IAS use can adversely impact their access to housing, education, employment, insurance, credit, or access to places of public accommodation?</rdfs:comment>
        <rdfs:label>RE13.2.9_IASPotentiallyAffectedPersonsAdviseAdverseImpactOpportunity</rdfs:label>
        <owl:versionInfo>page 95</owl:versionInfo>
    </owl:Class>
    


    <!-- https://savage.nps.edu/EthicalControl/ontologies/MissionExecutionOntology#RE13.3.1.1 -->

    <owl:Class rdf:about="https://savage.nps.edu/EthicalControl/ontologies/MissionExecutionOntology#RE13.3.1.1">
        <rdfs:subClassOf rdf:resource="https://savage.nps.edu/EthicalControl/ontologies/MissionExecutionOntology#DADM13.3.1"/>
        <rdfs:comment>Does the demographic makeup of the IAS development team reflect that of the population(s) potentially affected by use of the IAS?</rdfs:comment>
        <rdfs:label>RE13.3.1.1_DemographicsMirroredDevelopmentIAS</rdfs:label>
        <owl:versionInfo>page 96</owl:versionInfo>
    </owl:Class>
    


    <!-- https://savage.nps.edu/EthicalControl/ontologies/MissionExecutionOntology#RE13.3.1.10 -->

    <owl:Class rdf:about="https://savage.nps.edu/EthicalControl/ontologies/MissionExecutionOntology#RE13.3.1.10">
        <rdfs:subClassOf rdf:resource="https://savage.nps.edu/EthicalControl/ontologies/MissionExecutionOntology#DADM13.3.1"/>
        <rdfs:comment>Do development teams look for synthetic training data generated from models that are potentially subject to bias?</rdfs:comment>
        <rdfs:label>RE13.3.1.10_DevelopmentTeamsIdentifyBiasSyntheticTrainingData</rdfs:label>
        <owl:versionInfo>page 97</owl:versionInfo>
    </owl:Class>
    


    <!-- https://savage.nps.edu/EthicalControl/ontologies/MissionExecutionOntology#RE13.3.1.11 -->

    <owl:Class rdf:about="https://savage.nps.edu/EthicalControl/ontologies/MissionExecutionOntology#RE13.3.1.11">
        <rdfs:subClassOf rdf:resource="https://savage.nps.edu/EthicalControl/ontologies/MissionExecutionOntology#DADM13.3.1"/>
        <rdfs:comment>Do development teams validate potentially biased synthetic data against real data?</rdfs:comment>
        <rdfs:label>RE13.3.1.11_DevelopmentTeamsCheckSynthicVSRealDataBias</rdfs:label>
        <owl:versionInfo>page 97</owl:versionInfo>
    </owl:Class>
    


    <!-- https://savage.nps.edu/EthicalControl/ontologies/MissionExecutionOntology#RE13.3.1.12 -->

    <owl:Class rdf:about="https://savage.nps.edu/EthicalControl/ontologies/MissionExecutionOntology#RE13.3.1.12">
        <rdfs:subClassOf rdf:resource="https://savage.nps.edu/EthicalControl/ontologies/MissionExecutionOntology#DADM13.3.1"/>
        <rdfs:comment>Do development teams look for bias seeping into the training data during the data collection process?</rdfs:comment>
        <rdfs:label>RE13.3.1.12_DevelopmentTeamsIdentifyBiasTrainingDataCollection</rdfs:label>
        <owl:versionInfo>page 97</owl:versionInfo>
    </owl:Class>
    


    <!-- https://savage.nps.edu/EthicalControl/ontologies/MissionExecutionOntology#RE13.3.1.13 -->

    <owl:Class rdf:about="https://savage.nps.edu/EthicalControl/ontologies/MissionExecutionOntology#RE13.3.1.13">
        <rdfs:subClassOf rdf:resource="https://savage.nps.edu/EthicalControl/ontologies/MissionExecutionOntology#DADM13.3.1"/>
        <rdfs:comment>Do development teams look for &quot;Simpson’s paradox,&quot; where fusing data introduces new bias to the IAS?</rdfs:comment>
        <rdfs:label>RE13.3.1.13_DevelopmentTeamsIdentifySimpsonsParadoxDataFusion</rdfs:label>
        <owl:versionInfo>page 97</owl:versionInfo>
    </owl:Class>
    


    <!-- https://savage.nps.edu/EthicalControl/ontologies/MissionExecutionOntology#RE13.3.1.14 -->

    <owl:Class rdf:about="https://savage.nps.edu/EthicalControl/ontologies/MissionExecutionOntology#RE13.3.1.14">
        <rdfs:subClassOf rdf:resource="https://savage.nps.edu/EthicalControl/ontologies/MissionExecutionOntology#DADM13.3.1"/>
        <rdfs:comment>Do development teams look for &quot;technological solutionism,&quot; the perception that technology will lead to only positive solutions?</rdfs:comment>
        <rdfs:label>RE13.3.1.14_DevelopmentTeamsIdentifyTechnologicalSolutionism</rdfs:label>
        <owl:versionInfo>page 97</owl:versionInfo>
    </owl:Class>
    


    <!-- https://savage.nps.edu/EthicalControl/ontologies/MissionExecutionOntology#RE13.3.1.15 -->

    <owl:Class rdf:about="https://savage.nps.edu/EthicalControl/ontologies/MissionExecutionOntology#RE13.3.1.15">
        <rdfs:subClassOf rdf:resource="https://savage.nps.edu/EthicalControl/ontologies/MissionExecutionOntology#DADM13.3.1"/>
        <rdfs:comment>Do development teams look for representation bias where the training data is not a representative reflection of the affected population?</rdfs:comment>
        <rdfs:label>RE13.3.1.15_DevelopmentTeamsIdentifyRepresentationBias</rdfs:label>
        <owl:versionInfo>page 97</owl:versionInfo>
    </owl:Class>
    


    <!-- https://savage.nps.edu/EthicalControl/ontologies/MissionExecutionOntology#RE13.3.1.16 -->

    <owl:Class rdf:about="https://savage.nps.edu/EthicalControl/ontologies/MissionExecutionOntology#RE13.3.1.16">
        <rdfs:subClassOf rdf:resource="https://savage.nps.edu/EthicalControl/ontologies/MissionExecutionOntology#DADM13.3.1"/>
        <rdfs:comment>Do development teams look for omitted variable bias where the operational environment contains a variable not present in the models used to develop the IAS?</rdfs:comment>
        <rdfs:label>RE13.3.1.16_DevelopmentTeamsIdentifyOmittedVariableBias</rdfs:label>
        <owl:versionInfo>page 97</owl:versionInfo>
    </owl:Class>
    


    <!-- https://savage.nps.edu/EthicalControl/ontologies/MissionExecutionOntology#RE13.3.1.17 -->

    <owl:Class rdf:about="https://savage.nps.edu/EthicalControl/ontologies/MissionExecutionOntology#RE13.3.1.17">
        <rdfs:subClassOf rdf:resource="https://savage.nps.edu/EthicalControl/ontologies/MissionExecutionOntology#DADM13.3.1"/>
        <rdfs:comment>Do development teams look for social or behavior bias where the affected person’s reactions to the IAS influences IAS actions/decisions?</rdfs:comment>
        <rdfs:label>RE13.3.1.17_DevelopmentTeamsIdentifySocialBehaviorBias</rdfs:label>
        <owl:versionInfo>page 97</owl:versionInfo>
    </owl:Class>
    


    <!-- https://savage.nps.edu/EthicalControl/ontologies/MissionExecutionOntology#RE13.3.1.18 -->

    <owl:Class rdf:about="https://savage.nps.edu/EthicalControl/ontologies/MissionExecutionOntology#RE13.3.1.18">
        <rdfs:subClassOf rdf:resource="https://savage.nps.edu/EthicalControl/ontologies/MissionExecutionOntology#DADM13.3.1"/>
        <rdfs:comment>Do development teams look for ranking bias where the IAS actions or decisions are based on a small number of heavily weighted results and not on all available information?</rdfs:comment>
        <rdfs:label>RE13.3.1.18_DevelopmentTeamsIdentifyRankingBias</rdfs:label>
        <owl:versionInfo>page 97</owl:versionInfo>
    </owl:Class>
    


    <!-- https://savage.nps.edu/EthicalControl/ontologies/MissionExecutionOntology#RE13.3.1.19 -->

    <owl:Class rdf:about="https://savage.nps.edu/EthicalControl/ontologies/MissionExecutionOntology#RE13.3.1.19">
        <rdfs:subClassOf rdf:resource="https://savage.nps.edu/EthicalControl/ontologies/MissionExecutionOntology#DADM13.3.1"/>
        <rdfs:comment>Do development teams look for aggregation bias where the IAS requires multiple models to fairly represent all sub-groups within the parent group population?</rdfs:comment>
        <rdfs:label>RE13.3.1.19_DevelopmentTeamsIdentifyAggregationBiasMultiModel</rdfs:label>
        <owl:versionInfo>page 97</owl:versionInfo>
    </owl:Class>
    


    <!-- https://savage.nps.edu/EthicalControl/ontologies/MissionExecutionOntology#RE13.3.1.2 -->

    <owl:Class rdf:about="https://savage.nps.edu/EthicalControl/ontologies/MissionExecutionOntology#RE13.3.1.2">
        <rdfs:subClassOf rdf:resource="https://savage.nps.edu/EthicalControl/ontologies/MissionExecutionOntology#DADM13.3.1"/>
        <rdfs:comment>When it is not possible or practicable to assemble a development team with a demographic makeup reflective of the potentially affected population, do team members have access to training materials that educate them on the cultures and characteristics of those populations?</rdfs:comment>
        <rdfs:label>RE13.3.1.2_TeamAccessTrainingBalanceDemographics</rdfs:label>
        <owl:versionInfo>page 96</owl:versionInfo>
    </owl:Class>
    


    <!-- https://savage.nps.edu/EthicalControl/ontologies/MissionExecutionOntology#RE13.3.1.20 -->

    <owl:Class rdf:about="https://savage.nps.edu/EthicalControl/ontologies/MissionExecutionOntology#RE13.3.1.20">
        <rdfs:subClassOf rdf:resource="https://savage.nps.edu/EthicalControl/ontologies/MissionExecutionOntology#DADM13.3.1"/>
        <rdfs:comment>Do development teams look for evaluation bias where IAS models may be erroneously validated?</rdfs:comment>
        <rdfs:label>RE13.3.1.20_DevelopmentTeamsIdentifyEvaluationBias</rdfs:label>
        <owl:versionInfo>page 97</owl:versionInfo>
    </owl:Class>
    


    <!-- https://savage.nps.edu/EthicalControl/ontologies/MissionExecutionOntology#RE13.3.1.21 -->

    <owl:Class rdf:about="https://savage.nps.edu/EthicalControl/ontologies/MissionExecutionOntology#RE13.3.1.21">
        <rdfs:subClassOf rdf:resource="https://savage.nps.edu/EthicalControl/ontologies/MissionExecutionOntology#DADM13.3.1"/>
        <rdfs:comment>Do development teams look for temporal bias where the operational context changes, perhaps imperceptibly, so that initial assumptions about the environment, and the training data chosen to represent it, are no longer valid?</rdfs:comment>
        <rdfs:label>RE13.3.1.21_DevelopmentTeamsIdentifyTemoralBias</rdfs:label>
        <owl:versionInfo>page 97</owl:versionInfo>
    </owl:Class>
    


    <!-- https://savage.nps.edu/EthicalControl/ontologies/MissionExecutionOntology#RE13.3.1.22 -->

    <owl:Class rdf:about="https://savage.nps.edu/EthicalControl/ontologies/MissionExecutionOntology#RE13.3.1.22">
        <rdfs:subClassOf rdf:resource="https://savage.nps.edu/EthicalControl/ontologies/MissionExecutionOntology#DADM13.3.1"/>
        <rdfs:comment>Do development teams look for automation bias where human operators tend to reflexively accept decisions made by an automated system?</rdfs:comment>
        <rdfs:label>RE13.3.1.22_DevelopmentTeamsIdentifyAutomationBias</rdfs:label>
        <owl:versionInfo>page 97</owl:versionInfo>
    </owl:Class>
    


    <!-- https://savage.nps.edu/EthicalControl/ontologies/MissionExecutionOntology#RE13.3.1.23 -->

    <owl:Class rdf:about="https://savage.nps.edu/EthicalControl/ontologies/MissionExecutionOntology#RE13.3.1.23">
        <rdfs:subClassOf rdf:resource="https://savage.nps.edu/EthicalControl/ontologies/MissionExecutionOntology#DADM13.3.1"/>
        <rdfs:comment>Do development teams look for assimilation bias where human operators tend to modify information to fit into pre-existing analytical frameworks?</rdfs:comment>
        <rdfs:label>RE13.3.1.23_DevelopmentTeamsIdentifyAssimilationBias</rdfs:label>
        <owl:versionInfo>page 97</owl:versionInfo>
    </owl:Class>
    


    <!-- https://savage.nps.edu/EthicalControl/ontologies/MissionExecutionOntology#RE13.3.1.24 -->

    <owl:Class rdf:about="https://savage.nps.edu/EthicalControl/ontologies/MissionExecutionOntology#RE13.3.1.24">
        <rdfs:subClassOf rdf:resource="https://savage.nps.edu/EthicalControl/ontologies/MissionExecutionOntology#DADM13.3.1"/>
        <rdfs:comment>Do development teams look for confirmation bias where developers gather training data that reaffirm conclusions they’ve already made?</rdfs:comment>
        <rdfs:label>RE13.3.1.24_DevelopmentTeamsIdentifyConfirmationBias</rdfs:label>
        <owl:versionInfo>page 97</owl:versionInfo>
    </owl:Class>
    


    <!-- https://savage.nps.edu/EthicalControl/ontologies/MissionExecutionOntology#RE13.3.1.25 -->

    <owl:Class rdf:about="https://savage.nps.edu/EthicalControl/ontologies/MissionExecutionOntology#RE13.3.1.25">
        <rdfs:subClassOf rdf:resource="https://savage.nps.edu/EthicalControl/ontologies/MissionExecutionOntology#DADM13.3.1"/>
        <rdfs:comment>Do development teams look for simplification bias where human operators tend to simplify phenomena they encounter?</rdfs:comment>
        <rdfs:label>RE13.3.1.25_DevelopmentTeamsIdentifySimplificationBias</rdfs:label>
        <owl:versionInfo>page 98</owl:versionInfo>
    </owl:Class>
    


    <!-- https://savage.nps.edu/EthicalControl/ontologies/MissionExecutionOntology#RE13.3.1.26 -->

    <owl:Class rdf:about="https://savage.nps.edu/EthicalControl/ontologies/MissionExecutionOntology#RE13.3.1.26">
        <rdfs:subClassOf rdf:resource="https://savage.nps.edu/EthicalControl/ontologies/MissionExecutionOntology#DADM13.3.1"/>
        <rdfs:comment>Do development teams look for activity bias where training data comes from a system’s most active users, rather than less active or inactive users?</rdfs:comment>
        <rdfs:label>RE13.3.1.26_DevelopmentTeamsIdentifyActivityBias</rdfs:label>
        <owl:versionInfo>page 98</owl:versionInfo>
    </owl:Class>
    


    <!-- https://savage.nps.edu/EthicalControl/ontologies/MissionExecutionOntology#RE13.3.1.27 -->

    <owl:Class rdf:about="https://savage.nps.edu/EthicalControl/ontologies/MissionExecutionOntology#RE13.3.1.27">
        <rdfs:subClassOf rdf:resource="https://savage.nps.edu/EthicalControl/ontologies/MissionExecutionOntology#DADM13.3.1"/>
        <rdfs:comment>Do development teams look for annotator bias where developers rely on automation as a heuristic replacement for their own information seeking and processing?</rdfs:comment>
        <rdfs:label>RE13.3.1.27_DevelopmentTeamsIdentifyAnnotatorBias</rdfs:label>
        <owl:versionInfo>page 98</owl:versionInfo>
    </owl:Class>
    


    <!-- https://savage.nps.edu/EthicalControl/ontologies/MissionExecutionOntology#RE13.3.1.28 -->

    <owl:Class rdf:about="https://savage.nps.edu/EthicalControl/ontologies/MissionExecutionOntology#RE13.3.1.28">
        <rdfs:subClassOf rdf:resource="https://savage.nps.edu/EthicalControl/ontologies/MissionExecutionOntology#DADM13.3.1"/>
        <rdfs:comment>Do development teams look for content production bias where nonexistent differences in the data result from structural, lexical, semantic or syntactic differences in use by developers?</rdfs:comment>
        <rdfs:label>RE13.3.1.28_DevelopmentTeamsIdentifyContentProductionBias</rdfs:label>
        <owl:versionInfo>page 98</owl:versionInfo>
    </owl:Class>
    


    <!-- https://savage.nps.edu/EthicalControl/ontologies/MissionExecutionOntology#RE13.3.1.29 -->

    <owl:Class rdf:about="https://savage.nps.edu/EthicalControl/ontologies/MissionExecutionOntology#RE13.3.1.29">
        <rdfs:subClassOf rdf:resource="https://savage.nps.edu/EthicalControl/ontologies/MissionExecutionOntology#DADM13.3.1"/>
        <rdfs:comment>Do development teams look for exclusion bias where specific groups of user populations are excluded from testing and subsequent analyses?</rdfs:comment>
        <rdfs:label>RE13.3.1.29_DevelopmentTeamsIdentifyExclusionBias</rdfs:label>
        <owl:versionInfo>page 98</owl:versionInfo>
    </owl:Class>
    


    <!-- https://savage.nps.edu/EthicalControl/ontologies/MissionExecutionOntology#RE13.3.1.3 -->

    <owl:Class rdf:about="https://savage.nps.edu/EthicalControl/ontologies/MissionExecutionOntology#RE13.3.1.3">
        <rdfs:subClassOf rdf:resource="https://savage.nps.edu/EthicalControl/ontologies/MissionExecutionOntology#DADM13.3.1"/>
        <rdfs:comment>Do development teams look for unintended biases in the training data?</rdfs:comment>
        <rdfs:label>RE13.3.1.3_DevelopmentTeamsUnintendedBiasesTrainingData</rdfs:label>
        <owl:versionInfo>page 96</owl:versionInfo>
    </owl:Class>
    


    <!-- https://savage.nps.edu/EthicalControl/ontologies/MissionExecutionOntology#RE13.3.1.30 -->

    <owl:Class rdf:about="https://savage.nps.edu/EthicalControl/ontologies/MissionExecutionOntology#RE13.3.1.30">
        <rdfs:subClassOf rdf:resource="https://savage.nps.edu/EthicalControl/ontologies/MissionExecutionOntology#DADM13.3.1"/>
        <rdfs:comment>Do development teams look for feedback loop bias where an algorithm learns from user behavior and feeds that behavior back into the model?</rdfs:comment>
        <rdfs:label>RE13.3.1.30_DevelopmentTeamsIdentifyFeedbackLoopBias</rdfs:label>
        <owl:versionInfo>page 98</owl:versionInfo>
    </owl:Class>
    


    <!-- https://savage.nps.edu/EthicalControl/ontologies/MissionExecutionOntology#RE13.3.1.31 -->

    <owl:Class rdf:about="https://savage.nps.edu/EthicalControl/ontologies/MissionExecutionOntology#RE13.3.1.31">
        <rdfs:subClassOf rdf:resource="https://savage.nps.edu/EthicalControl/ontologies/MissionExecutionOntology#DADM13.3.1"/>
        <rdfs:comment>Do development teams look for funding bias where biased results are reported in order to support or satisfy a funding agency or financial supporter?</rdfs:comment>
        <rdfs:label>RE13.3.1.31_DevelopmentTeamsIdentifyFundingBias</rdfs:label>
        <owl:versionInfo>page 98</owl:versionInfo>
    </owl:Class>
    


    <!-- https://savage.nps.edu/EthicalControl/ontologies/MissionExecutionOntology#RE13.3.1.32 -->

    <owl:Class rdf:about="https://savage.nps.edu/EthicalControl/ontologies/MissionExecutionOntology#RE13.3.1.32">
        <rdfs:subClassOf rdf:resource="https://savage.nps.edu/EthicalControl/ontologies/MissionExecutionOntology#DADM13.3.1"/>
        <rdfs:comment>Do development teams look for historical bias where models are trained on past and potentially biased decisions?</rdfs:comment>
        <rdfs:label>RE13.3.1.32_DevelopmentTeamsIdentifyHistoricalBias</rdfs:label>
        <owl:versionInfo>page 98</owl:versionInfo>
    </owl:Class>
    


    <!-- https://savage.nps.edu/EthicalControl/ontologies/MissionExecutionOntology#RE13.3.1.33 -->

    <owl:Class rdf:about="https://savage.nps.edu/EthicalControl/ontologies/MissionExecutionOntology#RE13.3.1.33">
        <rdfs:subClassOf rdf:resource="https://savage.nps.edu/EthicalControl/ontologies/MissionExecutionOntology#DADM13.3.1"/>
        <rdfs:comment>Do development teams look for mirror imaging bias where an IAS is developed to counter an adversary force (such as in a military application) and the developers assume that members of the adversary force have the same cultural, ethical, and cognitive characteristics of members of their own force?</rdfs:comment>
        <rdfs:label>RE13.3.1.33_DevelopmentTeamsIdentifyMirrorImageBias</rdfs:label>
        <owl:versionInfo>page 98</owl:versionInfo>
    </owl:Class>
    


    <!-- https://savage.nps.edu/EthicalControl/ontologies/MissionExecutionOntology#RE13.3.1.34 -->

    <owl:Class rdf:about="https://savage.nps.edu/EthicalControl/ontologies/MissionExecutionOntology#RE13.3.1.34">
        <rdfs:subClassOf rdf:resource="https://savage.nps.edu/EthicalControl/ontologies/MissionExecutionOntology#DADM13.3.1"/>
        <rdfs:comment>Do development teams look for inherited bias where tools that are built with machine learning are used to generate inputs for other machine learning algorithms?</rdfs:comment>
        <rdfs:label>RE13.3.1.34_DevelopmentTeamsIdentifyInheritedBias</rdfs:label>
        <owl:versionInfo>page 98</owl:versionInfo>
    </owl:Class>
    


    <!-- https://savage.nps.edu/EthicalControl/ontologies/MissionExecutionOntology#RE13.3.1.35 -->

    <owl:Class rdf:about="https://savage.nps.edu/EthicalControl/ontologies/MissionExecutionOntology#RE13.3.1.35">
        <rdfs:subClassOf rdf:resource="https://savage.nps.edu/EthicalControl/ontologies/MissionExecutionOntology#DADM13.3.1"/>
        <rdfs:comment>Do development teams look for interpretation bias where users interpret algorithmic outputs according to their internalized biases and views?</rdfs:comment>
        <rdfs:label>RE13.3.1.35_DevelopmentTeamsIdentifyInterpretationBias</rdfs:label>
        <owl:versionInfo>page 98</owl:versionInfo>
    </owl:Class>
    


    <!-- https://savage.nps.edu/EthicalControl/ontologies/MissionExecutionOntology#RE13.3.1.36 -->

    <owl:Class rdf:about="https://savage.nps.edu/EthicalControl/ontologies/MissionExecutionOntology#RE13.3.1.36">
        <rdfs:subClassOf rdf:resource="https://savage.nps.edu/EthicalControl/ontologies/MissionExecutionOntology#DADM13.3.1"/>
        <rdfs:comment>Do development teams look for linking bias where network attributes obtained from user connections, activities, or interactions differ and misrepresent the true behavior of the users?</rdfs:comment>
        <rdfs:label>RE13.3.1.36_DevelopmentTeamsIdentifyLinkingBias</rdfs:label>
        <owl:versionInfo>page 98</owl:versionInfo>
    </owl:Class>
    


    <!-- https://savage.nps.edu/EthicalControl/ontologies/MissionExecutionOntology#RE13.3.1.37 -->

    <owl:Class rdf:about="https://savage.nps.edu/EthicalControl/ontologies/MissionExecutionOntology#RE13.3.1.37">
        <rdfs:subClassOf rdf:resource="https://savage.nps.edu/EthicalControl/ontologies/MissionExecutionOntology#DADM13.3.1"/>
        <rdfs:comment>Do development teams look for loss of situational awareness bias where human- machine teaming leads to humans being unaware of their situation such that, when command and control of a system is given to them, they are unprepared to assume their duties?</rdfs:comment>
        <rdfs:label>RE13.3.1.37_DevelopmentTeamsIdentifyLossSituationalAwarenessBias</rdfs:label>
        <owl:versionInfo>page 98</owl:versionInfo>
    </owl:Class>
    


    <!-- https://savage.nps.edu/EthicalControl/ontologies/MissionExecutionOntology#RE13.3.1.38 -->

    <owl:Class rdf:about="https://savage.nps.edu/EthicalControl/ontologies/MissionExecutionOntology#RE13.3.1.38">
        <rdfs:subClassOf rdf:resource="https://savage.nps.edu/EthicalControl/ontologies/MissionExecutionOntology#DADM13.3.1"/>
        <rdfs:comment>Do development teams look for modal confusion bias where modal interfaces confuse human operators, who misunderstand which mode the system is using, taking actions which are correct for a different mode but incorrect for their current situation?</rdfs:comment>
        <rdfs:label>RE13.3.1.38_DevelopmentTeamsIdentifyModalConfusionBias</rdfs:label>
        <owl:versionInfo>page 98</owl:versionInfo>
    </owl:Class>
    


    <!-- https://savage.nps.edu/EthicalControl/ontologies/MissionExecutionOntology#RE13.3.1.39 -->

    <owl:Class rdf:about="https://savage.nps.edu/EthicalControl/ontologies/MissionExecutionOntology#RE13.3.1.39">
        <rdfs:subClassOf rdf:resource="https://savage.nps.edu/EthicalControl/ontologies/MissionExecutionOntology#DADM13.3.1"/>
        <rdfs:comment>Do development teams look for ranking bias where top-ranked information is perceived to be more important than lower ranking information?</rdfs:comment>
        <rdfs:label>RE13.3.1.39_DevelopmentTeamsIdentifyRankingBias</rdfs:label>
        <owl:versionInfo>page 99</owl:versionInfo>
    </owl:Class>
    


    <!-- https://savage.nps.edu/EthicalControl/ontologies/MissionExecutionOntology#RE13.3.1.4 -->

    <owl:Class rdf:about="https://savage.nps.edu/EthicalControl/ontologies/MissionExecutionOntology#RE13.3.1.4">
        <rdfs:subClassOf rdf:resource="https://savage.nps.edu/EthicalControl/ontologies/MissionExecutionOntology#DADM13.3.1"/>
        <rdfs:comment>Do development teams look for unintended biases in the IAS algorithms?</rdfs:comment>
        <rdfs:label>RE13.3.1.4_DevelopmentTeamsUnintendedIASAlgorithms</rdfs:label>
        <owl:versionInfo>page 96</owl:versionInfo>
    </owl:Class>
    


    <!-- https://savage.nps.edu/EthicalControl/ontologies/MissionExecutionOntology#RE13.3.1.40 -->

    <owl:Class rdf:about="https://savage.nps.edu/EthicalControl/ontologies/MissionExecutionOntology#RE13.3.1.40">
        <rdfs:subClassOf rdf:resource="https://savage.nps.edu/EthicalControl/ontologies/MissionExecutionOntology#DADM13.3.1"/>
        <rdfs:comment>Do development teams look for sampling bias where non-random sampling of subgroups, causing trends estimated for one population to not be generalizable to data collected from a new population?</rdfs:comment>
        <rdfs:label>RE13.3.1.40_DevelopmentTeamsIdentifySamplingBias</rdfs:label>
        <owl:versionInfo>page 99</owl:versionInfo>
    </owl:Class>
    


    <!-- https://savage.nps.edu/EthicalControl/ontologies/MissionExecutionOntology#RE13.3.1.41 -->

    <owl:Class rdf:about="https://savage.nps.edu/EthicalControl/ontologies/MissionExecutionOntology#RE13.3.1.41">
        <rdfs:subClassOf rdf:resource="https://savage.nps.edu/EthicalControl/ontologies/MissionExecutionOntology#DADM13.3.1"/>
        <rdfs:comment>Do development teams look for training data bias where algorithms are trained on one type of data and do not extrapolate beyond those data?</rdfs:comment>
        <rdfs:label>RE13.3.1.41_DevelopmentTeamsIdentifyTrainingDataBias</rdfs:label>
        <owl:versionInfo>page 99</owl:versionInfo>
    </owl:Class>
    


    <!-- https://savage.nps.edu/EthicalControl/ontologies/MissionExecutionOntology#RE13.3.1.42 -->

    <owl:Class rdf:about="https://savage.nps.edu/EthicalControl/ontologies/MissionExecutionOntology#RE13.3.1.42">
        <rdfs:subClassOf rdf:resource="https://savage.nps.edu/EthicalControl/ontologies/MissionExecutionOntology#DADM13.3.1"/>
        <rdfs:comment>Do development teams look for uncertainty bias where predictive algorithms favor groups that are better represented in the training data, since there will be less uncertainty associated with those predictions?</rdfs:comment>
        <rdfs:label>RE13.3.1.42_DevelopmentTeamsIdentifyUncertaintyBias</rdfs:label>
        <owl:versionInfo>page 99</owl:versionInfo>
    </owl:Class>
    


    <!-- https://savage.nps.edu/EthicalControl/ontologies/MissionExecutionOntology#RE13.3.1.5 -->

    <owl:Class rdf:about="https://savage.nps.edu/EthicalControl/ontologies/MissionExecutionOntology#RE13.3.1.5">
        <rdfs:subClassOf rdf:resource="https://savage.nps.edu/EthicalControl/ontologies/MissionExecutionOntology#DADM13.3.1"/>
        <rdfs:comment>Do development teams consider cultural biases in coalition and allied IAS and across joint services?</rdfs:comment>
        <rdfs:label>RE13.3.1.5_DevelopmentTeamsConsiderCulturalBiases</rdfs:label>
        <owl:versionInfo>page 96</owl:versionInfo>
    </owl:Class>
    


    <!-- https://savage.nps.edu/EthicalControl/ontologies/MissionExecutionOntology#RE13.3.1.6 -->

    <owl:Class rdf:about="https://savage.nps.edu/EthicalControl/ontologies/MissionExecutionOntology#RE13.3.1.6">
        <rdfs:subClassOf rdf:resource="https://savage.nps.edu/EthicalControl/ontologies/MissionExecutionOntology#DADM13.3.1"/>
        <rdfs:comment>Do development teams look for &quot;data hubris&quot; by attempting to identify the underlying causal mechanisms in their models so that spurious correlations identified by the IAS are not taken to be actual causal relationships?</rdfs:comment>
        <rdfs:label>RE13.3.1.6_DevelopmentTeamsConsiderSpuriousCorrelations</rdfs:label>
        <owl:versionInfo>page 96</owl:versionInfo>
    </owl:Class>
    


    <!-- https://savage.nps.edu/EthicalControl/ontologies/MissionExecutionOntology#RE13.3.1.7 -->

    <owl:Class rdf:about="https://savage.nps.edu/EthicalControl/ontologies/MissionExecutionOntology#RE13.3.1.7">
        <rdfs:subClassOf rdf:resource="https://savage.nps.edu/EthicalControl/ontologies/MissionExecutionOntology#DADM13.3.1"/>
        <rdfs:comment>Do development teams look for bias introduced by IAS interaction with human operators?</rdfs:comment>
        <rdfs:label>RE13.3.1.7_DevelopmentTeamsIdentifyBiasIASHumanOperators</rdfs:label>
        <owl:versionInfo>page 96</owl:versionInfo>
    </owl:Class>
    


    <!-- https://savage.nps.edu/EthicalControl/ontologies/MissionExecutionOntology#RE13.3.1.8 -->

    <owl:Class rdf:about="https://savage.nps.edu/EthicalControl/ontologies/MissionExecutionOntology#RE13.3.1.8">
        <rdfs:subClassOf rdf:resource="https://savage.nps.edu/EthicalControl/ontologies/MissionExecutionOntology#DADM13.3.1"/>
        <rdfs:comment>Do development teams look for bias introduced by IAS ingest of sensor data in the operational environment?</rdfs:comment>
        <rdfs:label>RE13.3.1.8_DevelopmentTeamsIdentifyBiasIASOpEnvSensor</rdfs:label>
        <owl:versionInfo>page 97</owl:versionInfo>
    </owl:Class>
    


    <!-- https://savage.nps.edu/EthicalControl/ontologies/MissionExecutionOntology#RE13.3.1.9 -->

    <owl:Class rdf:about="https://savage.nps.edu/EthicalControl/ontologies/MissionExecutionOntology#RE13.3.1.9">
        <rdfs:subClassOf rdf:resource="https://savage.nps.edu/EthicalControl/ontologies/MissionExecutionOntology#DADM13.3.1"/>
        <rdfs:comment>Do development teams look for &quot;black box&quot; decision-making algorithms that make it difficult or impossible to detect bias?</rdfs:comment>
        <rdfs:label>RE13.3.1.9_DevelopmentTeamsIdentifyBlackBoxDecisionMakingBias</rdfs:label>
        <owl:versionInfo>page 97</owl:versionInfo>
    </owl:Class>
    


    <!-- https://savage.nps.edu/EthicalControl/ontologies/MissionExecutionOntology#RE13.3.2.1 -->

    <owl:Class rdf:about="https://savage.nps.edu/EthicalControl/ontologies/MissionExecutionOntology#RE13.3.2.1">
        <rdfs:subClassOf rdf:resource="https://savage.nps.edu/EthicalControl/ontologies/MissionExecutionOntology#DADM13.3.2"/>
        <rdfs:comment>Are IAS results revisited using human-on-the-loop oversight to look for biased results and rights violations that the IAS is not capable of identifying?</rdfs:comment>
        <rdfs:label>RE13.3.2.1_IASResultsRevisited</rdfs:label>
        <owl:versionInfo>page 99</owl:versionInfo>
    </owl:Class>
    


    <!-- https://savage.nps.edu/EthicalControl/ontologies/MissionExecutionOntology#RE13.3.2.2 -->

    <owl:Class rdf:about="https://savage.nps.edu/EthicalControl/ontologies/MissionExecutionOntology#RE13.3.2.2">
        <rdfs:subClassOf rdf:resource="https://savage.nps.edu/EthicalControl/ontologies/MissionExecutionOntology#DADM13.3.2"/>
        <rdfs:comment>Are human-on-the-loop oversight functions conducted by a group of persons representative of the population(s) potentially affected by the IAS?</rdfs:comment>
        <rdfs:label>RE13.3.2.2_IASOversightPersonsRepresentative</rdfs:label>
        <owl:versionInfo>page 99</owl:versionInfo>
    </owl:Class>
    


    <!-- https://savage.nps.edu/EthicalControl/ontologies/MissionExecutionOntology#RE13.3.2.3 -->

    <owl:Class rdf:about="https://savage.nps.edu/EthicalControl/ontologies/MissionExecutionOntology#RE13.3.2.3">
        <rdfs:subClassOf rdf:resource="https://savage.nps.edu/EthicalControl/ontologies/MissionExecutionOntology#DADM13.3.2"/>
        <rdfs:comment>Is IAS use eliminated or curtailed when oversight groups discover bias or rights violations?</rdfs:comment>
        <rdfs:label>RE13.3.2.3_IASUseRestrictedDiscoveryBiasRightsViolation</rdfs:label>
        <owl:versionInfo>page 99</owl:versionInfo>
    </owl:Class>
    


    <!-- https://savage.nps.edu/EthicalControl/ontologies/MissionExecutionOntology#RE13.3.2.4 -->

    <owl:Class rdf:about="https://savage.nps.edu/EthicalControl/ontologies/MissionExecutionOntology#RE13.3.2.4">
        <rdfs:subClassOf rdf:resource="https://savage.nps.edu/EthicalControl/ontologies/MissionExecutionOntology#DADM13.3.2"/>
        <rdfs:comment>When oversight groups discover bias or rights violations in one IAS, do they then look for the same bias in other IAS that have used all or part of the training data or algorithms used by the biased IAS?</rdfs:comment>
        <rdfs:label>RE13.3.2.4_IASBiasRightsDiscoveryDrivesEnterpriseModelUpdates</rdfs:label>
        <owl:versionInfo>page 99</owl:versionInfo>
    </owl:Class>
    


    <!-- https://savage.nps.edu/EthicalControl/ontologies/MissionExecutionOntology#RE13.3.2.5 -->

    <owl:Class rdf:about="https://savage.nps.edu/EthicalControl/ontologies/MissionExecutionOntology#RE13.3.2.5">
        <rdfs:subClassOf rdf:resource="https://savage.nps.edu/EthicalControl/ontologies/MissionExecutionOntology#DADM13.3.2"/>
        <rdfs:comment>When oversight groups discover bias or rights violations in one IAS, do they ensure that a replacement or revision does not reproduce the same negative outcome, or introduce a new negative outcome?</rdfs:comment>
        <rdfs:label>RE13.3.2.5_IASBiasRightsDiscoveryEnterpriseModelUpdatesConfirmation</rdfs:label>
        <owl:versionInfo>page 99</owl:versionInfo>
    </owl:Class>
    


    <!-- https://savage.nps.edu/EthicalControl/ontologies/MissionExecutionOntology#RE13.3.2.6 -->

    <owl:Class rdf:about="https://savage.nps.edu/EthicalControl/ontologies/MissionExecutionOntology#RE13.3.2.6">
        <rdfs:subClassOf rdf:resource="https://savage.nps.edu/EthicalControl/ontologies/MissionExecutionOntology#DADM13.3.2"/>
        <rdfs:comment>Are oversight groups familiar with &quot;reviewer’s bias,&quot; where the reviewers may be susceptible to introducing their own sets of expertise, experiences, and biases into evaluations?</rdfs:comment>
        <rdfs:label>RE13.3.2.6_OversightReviewersBiasFamiliarity</rdfs:label>
        <owl:versionInfo>page 99</owl:versionInfo>
    </owl:Class>
    


    <!-- https://savage.nps.edu/EthicalControl/ontologies/MissionExecutionOntology#ROE -->

    <owl:Class rdf:about="https://savage.nps.edu/EthicalControl/ontologies/MissionExecutionOntology#ROE">
        <rdfs:subClassOf rdf:resource="https://savage.nps.edu/EthicalControl/ontologies/MissionExecutionOntology#DADM_Abbreviations"/>
        <rdfs:label>Rules of Engagement (ROE)</rdfs:label>
        <owl:versionInfo>page 100</owl:versionInfo>
    </owl:Class>
    


    <!-- https://savage.nps.edu/EthicalControl/ontologies/MissionExecutionOntology#Reference01_DoDD3000.09 -->

    <owl:Class rdf:about="https://savage.nps.edu/EthicalControl/ontologies/MissionExecutionOntology#Reference01_DoDD3000.09">
        <rdfs:subClassOf rdf:resource="https://savage.nps.edu/EthicalControl/ontologies/MissionExecutionOntology#DADM_References"/>
        <rdfs:comment>TODO: Get description from reference document and put it here

DOD Directive 3000.09. May 8, 2017. Autonomy in Weapon Systems. https://www.esd.whs.mil/Portals/54/Documents/DD/issuances/dodd/300009p.pdf</rdfs:comment>
        <owl:versionInfo>page 101</owl:versionInfo>
    </owl:Class>
    


    <!-- https://savage.nps.edu/EthicalControl/ontologies/MissionExecutionOntology#Reference02_DoDD5000.01 -->

    <owl:Class rdf:about="https://savage.nps.edu/EthicalControl/ontologies/MissionExecutionOntology#Reference02_DoDD5000.01">
        <rdfs:subClassOf rdf:resource="https://savage.nps.edu/EthicalControl/ontologies/MissionExecutionOntology#DADM_References"/>
        <rdfs:comment>TODO: Get description from reference document and put it here

DOD Directive 5000.01. Sept. 9, 2020. The Defense Acquisition System. Office of the Under Secretary of Defense for Acquisition and Sustainment. https://www.esd.whs.mil/Portals/54/Documents/DD/issuances/dodd/500001p.pdf?ver=2020-09-09-160307-310</rdfs:comment>
        <rdfs:comment>pg 101</rdfs:comment>
    </owl:Class>
    


    <!-- https://savage.nps.edu/EthicalControl/ontologies/MissionExecutionOntology#Reference03_DoDD2311.01 -->

    <owl:Class rdf:about="https://savage.nps.edu/EthicalControl/ontologies/MissionExecutionOntology#Reference03_DoDD2311.01">
        <rdfs:subClassOf rdf:resource="https://savage.nps.edu/EthicalControl/ontologies/MissionExecutionOntology#DADM_References"/>
        <rdfs:comment>TODO: Get description from reference document and put it here

DOD Directive 2311.01. July 2, 2020. DOD Law of War Program. https://www.esd.whs.mil/Portals/54/Documents/DD/issuances/dodd/231101p.pdf?ver=2020-07-02-143157-007</rdfs:comment>
        <rdfs:comment>pg 101</rdfs:comment>
    </owl:Class>
    


    <!-- https://savage.nps.edu/EthicalControl/ontologies/MissionExecutionOntology#Reference04_DoDD3000.03E -->

    <owl:Class rdf:about="https://savage.nps.edu/EthicalControl/ontologies/MissionExecutionOntology#Reference04_DoDD3000.03E">
        <rdfs:subClassOf rdf:resource="https://savage.nps.edu/EthicalControl/ontologies/MissionExecutionOntology#DADM_References"/>
        <rdfs:comment>TODO: Get description from reference document and put it here

DOD Directive 3000.03E. August 31, 2018. DOD Executive Agent for Non-Lethal Weapons (NLW) and NLW Policy. https://www.esd.whs.mil/Portals/54/Documents/DD/issuances/dodd/300003p.pdf?ver=2017-09-27-125836-647</rdfs:comment>
        <owl:versionInfo>page 101</owl:versionInfo>
    </owl:Class>
    


    <!-- https://savage.nps.edu/EthicalControl/ontologies/MissionExecutionOntology#Reference05_DepSECDEF -->

    <owl:Class rdf:about="https://savage.nps.edu/EthicalControl/ontologies/MissionExecutionOntology#Reference05_DepSECDEF">
        <rdfs:subClassOf rdf:resource="https://savage.nps.edu/EthicalControl/ontologies/MissionExecutionOntology#DADM_References"/>
        <rdfs:comment>TODO: Get description from reference document and put it here

Kathleen Hicks, Deputy Secretary of Defense. May 26, 2021. Memorandum for Senior Pentagon Leadership, Commanders of the Combatant Commands, Defense Agencies, and DOD Field Activities. Subject: Implementing Responsible Artificial Intelligence in the Department of Defense. https://media.defense.gov/2021/May/27/2002730593/-1/-1/0/IMPLEMENTING-RESPONSIBLE-ARTIFICIAL-INTELLIGENCE-IN-THE-DEPARTMENT-OF-DEFENSE.PDF</rdfs:comment>
        <owl:versionInfo>page 101</owl:versionInfo>
    </owl:Class>
    


    <!-- https://savage.nps.edu/EthicalControl/ontologies/MissionExecutionOntology#Reference06_DoDEthicsAI -->

    <owl:Class rdf:about="https://savage.nps.edu/EthicalControl/ontologies/MissionExecutionOntology#Reference06_DoDEthicsAI">
        <rdfs:subClassOf rdf:resource="https://savage.nps.edu/EthicalControl/ontologies/MissionExecutionOntology#DADM_References"/>
        <rdfs:comment>TODO: Get description from reference document and put it here

&quot;DOD Adopts Ethical Principles for Artificial Intelligence.&quot; Department of Defense Press Release. Feb. 24, 2020. https://www.defense.gov/Newsroom/Releases/Release/Article/2091996/dod-adopts-ethical-principles-for-artificial-intelligence/.</rdfs:comment>
        <owl:versionInfo>page 101</owl:versionInfo>
    </owl:Class>
    


    <!-- https://savage.nps.edu/EthicalControl/ontologies/MissionExecutionOntology#Reference07_ArmyOfNone -->

    <owl:Class rdf:about="https://savage.nps.edu/EthicalControl/ontologies/MissionExecutionOntology#Reference07_ArmyOfNone">
        <rdfs:subClassOf rdf:resource="https://savage.nps.edu/EthicalControl/ontologies/MissionExecutionOntology#DADM_References"/>
        <rdfs:comment>TODO: Get description from reference document and put it here

Scharre, Paul. 2018. Army of None: Autonomous Weapons and the Future of War. New York: W.W. Norton &amp; Company.</rdfs:comment>
        <owl:versionInfo>page 101</owl:versionInfo>
    </owl:Class>
    


    <!-- https://savage.nps.edu/EthicalControl/ontologies/MissionExecutionOntology#Reference08_StopKillerRobots -->

    <owl:Class rdf:about="https://savage.nps.edu/EthicalControl/ontologies/MissionExecutionOntology#Reference08_StopKillerRobots">
        <rdfs:subClassOf rdf:resource="https://savage.nps.edu/EthicalControl/ontologies/MissionExecutionOntology#DADM_References"/>
        <rdfs:comment>TODO: Get description from reference document and put it here

&quot;Campaign to Stop Killer Robots.&quot; https://www.stopkillerrobots.org/learn/</rdfs:comment>
        <owl:versionInfo>page 101</owl:versionInfo>
    </owl:Class>
    


    <!-- https://savage.nps.edu/EthicalControl/ontologies/MissionExecutionOntology#Reference09_OUSDEthicsAI -->

    <owl:Class rdf:about="https://savage.nps.edu/EthicalControl/ontologies/MissionExecutionOntology#Reference09_OUSDEthicsAI">
        <rdfs:subClassOf rdf:resource="https://savage.nps.edu/EthicalControl/ontologies/MissionExecutionOntology#DADM_References"/>
        <rdfs:comment>TODO: Get description from reference document and put it here

Work, Robert O. &quot;Keynote Address to the Policy and Ethics of Intelligent Autonomous Systems: Technical Exchange Meeting.&quot; (Used with permission), Autonomy Community of Interest, Office of the Secretary of Defense, March 4. 2021.</rdfs:comment>
        <owl:versionInfo>page 101</owl:versionInfo>
    </owl:Class>
    


    <!-- https://savage.nps.edu/EthicalControl/ontologies/MissionExecutionOntology#Reference10_DAUKPP -->

    <owl:Class rdf:about="https://savage.nps.edu/EthicalControl/ontologies/MissionExecutionOntology#Reference10_DAUKPP">
        <rdfs:subClassOf rdf:resource="https://savage.nps.edu/EthicalControl/ontologies/MissionExecutionOntology#DADM_References"/>
        <rdfs:comment>TODO: Get description from reference document and put it here

&quot;Key Performance Parameter.&quot; Defense Acquisition University Glossary. https://www.dau.edu/glossary/Pages/Glossary.aspx#!both|K|27793</rdfs:comment>
        <owl:versionInfo>page 101</owl:versionInfo>
    </owl:Class>
    


    <!-- https://savage.nps.edu/EthicalControl/ontologies/MissionExecutionOntology#Reference11_FAR35.017 -->

    <owl:Class rdf:about="https://savage.nps.edu/EthicalControl/ontologies/MissionExecutionOntology#Reference11_FAR35.017">
        <rdfs:subClassOf rdf:resource="https://savage.nps.edu/EthicalControl/ontologies/MissionExecutionOntology#DADM_References"/>
        <rdfs:comment>TODO: Get description from reference document and put it here

Federal Acquisition Regulations Sec. 35.017. Federally Funded Research and Development Centers. https://www.acquisition.gov/far/35.017</rdfs:comment>
        <owl:versionInfo>page 101</owl:versionInfo>
    </owl:Class>
    


    <!-- https://savage.nps.edu/EthicalControl/ontologies/MissionExecutionOntology#Reference12_FFRDC -->

    <owl:Class rdf:about="https://savage.nps.edu/EthicalControl/ontologies/MissionExecutionOntology#Reference12_FFRDC">
        <rdfs:subClassOf rdf:resource="https://savage.nps.edu/EthicalControl/ontologies/MissionExecutionOntology#DADM_References"/>
        <rdfs:comment>TODO: Get description from reference document and put it here

Federally Funded Research and Development Centers. https://www.law.cornell.edu/cfr/text/48/35.017</rdfs:comment>
        <owl:versionInfo>page 101</owl:versionInfo>
    </owl:Class>
    


    <!-- https://savage.nps.edu/EthicalControl/ontologies/MissionExecutionOntology#Reference13_DASNAIStrategy -->

    <owl:Class rdf:about="https://savage.nps.edu/EthicalControl/ontologies/MissionExecutionOntology#Reference13_DASNAIStrategy">
        <rdfs:subClassOf rdf:resource="https://savage.nps.edu/EthicalControl/ontologies/MissionExecutionOntology#DADM_References"/>
        <rdfs:comment>TODO: Get description from reference document and put it here

Joan L. Johnson, Deputy Assistant Secretary of the Navy, Research, Development, Test and Evaluation, and Chief of Naval Research RADM Lorin C. Selby. July 2, 2021. Department of the Navy, Science and Technology Strategy for Intelligent Autonomous Systems. https://nps.edu/web/slamr/-/intelligent-autonomous-systems-science-and-technology-strategy-issued.</rdfs:comment>
        <owl:versionInfo>page 101</owl:versionInfo>
    </owl:Class>
    


    <!-- https://savage.nps.edu/EthicalControl/ontologies/MissionExecutionOntology#Reference14_SECNAVCNOCMC -->

    <owl:Class rdf:about="https://savage.nps.edu/EthicalControl/ontologies/MissionExecutionOntology#Reference14_SECNAVCNOCMC">
        <rdfs:subClassOf rdf:resource="https://savage.nps.edu/EthicalControl/ontologies/MissionExecutionOntology#DADM_References"/>
        <rdfs:comment>TODO: Get description from reference document and put it here

Thomas W. Harker, Secretary of the Navy (Acting), Admiral Michal M. Gilday Chief of Naval Operations, and General David H. Berger Commandant of the Marine Corps. March 16, 2021. &quot;Department of the Navy Unmanned Campaign Framework.&quot; https://www.navy.mil/Portals/1/Strategic/20210315%20Unmanned%20Campaign_Final_LowRes.pdf?ver=LtCZ-BPlWki6vCBTdgtDMA%3d%3d</rdfs:comment>
        <owl:versionInfo>page 101</owl:versionInfo>
    </owl:Class>
    


    <!-- https://savage.nps.edu/EthicalControl/ontologies/MissionExecutionOntology#Reference15_JPUB1.02 -->

    <owl:Class rdf:about="https://savage.nps.edu/EthicalControl/ontologies/MissionExecutionOntology#Reference15_JPUB1.02">
        <rdfs:subClassOf rdf:resource="https://savage.nps.edu/EthicalControl/ontologies/MissionExecutionOntology#DADM_References"/>
        <rdfs:comment>TODO: Get description from reference document and put it here

Joint Publication 1-02. Nov. 8, 2010 (as amended through Feb. 8, 2016). Department of Defense Dictionary of Military and Associated Terms. https://www.jcs.mil/Portals/36/Documents/Doctrine/pubs/dictionary.pdf?ver=QkmPX3lFZqhMjdEGeSoB4A%3d%3d</rdfs:comment>
        <owl:versionInfo>page 102</owl:versionInfo>
    </owl:Class>
    


    <!-- https://savage.nps.edu/EthicalControl/ontologies/MissionExecutionOntology#Reference16_JPUB5.01 -->

    <owl:Class rdf:about="https://savage.nps.edu/EthicalControl/ontologies/MissionExecutionOntology#Reference16_JPUB5.01">
        <rdfs:subClassOf rdf:resource="https://savage.nps.edu/EthicalControl/ontologies/MissionExecutionOntology#DADM_References"/>
        <rdfs:comment>TODO: Get description from reference document and put it here

Joint Publication 5-01. Dec. 1, 2020. Joint Planning. https://www.jcs.mil/Portals/36/Documents/Doctrine/pubs/jp5_0.pdf?ver=us_fQ_pGS_u65ateysmAng%3d%3d</rdfs:comment>
        <owl:versionInfo>page 102</owl:versionInfo>
    </owl:Class>
    


    <!-- https://savage.nps.edu/EthicalControl/ontologies/MissionExecutionOntology#Reference17_SECNAV5000.2F -->

    <owl:Class rdf:about="https://savage.nps.edu/EthicalControl/ontologies/MissionExecutionOntology#Reference17_SECNAV5000.2F">
        <rdfs:subClassOf rdf:resource="https://savage.nps.edu/EthicalControl/ontologies/MissionExecutionOntology#DADM_References"/>
        <rdfs:comment>TODO: Get description from reference document and put it here

Secretary of the Navy Instruction 5000.2F. March 26, 2019. Defense Acquisition System and Joint Capabilities Integration and Development System Implementation. https://www.secnav.navy.mil/doni/Directives/05000%20General%20Management%20Security%20and%20Safety%20Services/05-00%20General%20Admin%20and%20Management%20Support/5000.2F.pdf</rdfs:comment>
        <owl:versionInfo>page 102</owl:versionInfo>
    </owl:Class>
    


    <!-- https://savage.nps.edu/EthicalControl/ontologies/MissionExecutionOntology#Reference18_USNWC_Sparrow -->

    <owl:Class rdf:about="https://savage.nps.edu/EthicalControl/ontologies/MissionExecutionOntology#Reference18_USNWC_Sparrow">
        <rdfs:subClassOf rdf:resource="https://savage.nps.edu/EthicalControl/ontologies/MissionExecutionOntology#DADM_References"/>
        <rdfs:comment>TODO: Get description from reference document and put it here

Sparrow, Robert. 2015. &quot;Twenty Seconds to Comply: Autonomous Weapon Systems and the Recognition of Surrender.&quot; International Law Studies 91: 699-728. https://digital-commons.usnwc.edu/cgi/viewcontent.cgi?article=1413&amp;context=ils.</rdfs:comment>
        <owl:versionInfo>page 102</owl:versionInfo>
    </owl:Class>
    


    <!-- https://savage.nps.edu/EthicalControl/ontologies/MissionExecutionOntology#Reference19_OGCDoDLawOfWar -->

    <owl:Class rdf:about="https://savage.nps.edu/EthicalControl/ontologies/MissionExecutionOntology#Reference19_OGCDoDLawOfWar">
        <rdfs:subClassOf rdf:resource="https://savage.nps.edu/EthicalControl/ontologies/MissionExecutionOntology#DADM_References"/>
        <rdfs:comment>TODO: Get description from reference document and put it here

Office of the General Counsel, Department of Defense. June 2015. Department of Defense Law of War Manual. https://dod.defense.gov/Portals/1/Documents/law_war_manual15.pdf</rdfs:comment>
        <owl:versionInfo>page 102</owl:versionInfo>
    </owl:Class>
    


    <!-- https://savage.nps.edu/EthicalControl/ontologies/MissionExecutionOntology#Reference20_DAUGuidebook -->

    <owl:Class rdf:about="https://savage.nps.edu/EthicalControl/ontologies/MissionExecutionOntology#Reference20_DAUGuidebook">
        <rdfs:subClassOf rdf:resource="https://savage.nps.edu/EthicalControl/ontologies/MissionExecutionOntology#DADM_References"/>
        <rdfs:comment>TODO: Get description from reference document and put it here

&quot;Defense Acquisition Guidebook, Chapter 8.&quot; Defense Acquisition University. https://www.dau.edu/guidebooks/Shared%20Documents/Chapter%208%20Test%20and%20Evaluation.pdf</rdfs:comment>
        <owl:versionInfo>page 102</owl:versionInfo>
    </owl:Class>
    


    <!-- https://savage.nps.edu/EthicalControl/ontologies/MissionExecutionOntology#Reference21_AnnualReportOTE -->

    <owl:Class rdf:about="https://savage.nps.edu/EthicalControl/ontologies/MissionExecutionOntology#Reference21_AnnualReportOTE">
        <rdfs:subClassOf rdf:resource="https://savage.nps.edu/EthicalControl/ontologies/MissionExecutionOntology#DADM_References"/>
        <rdfs:comment>TODO: Get description from reference document and put it here

Behler, Robert F. FY 2020 Annual Report to Congress. Director, Opertional Test and Evaluation. https://www.dote.osd.mil/Portals/97/pub/reports/FY2020/other/2020DOTEAnnualReport.pdf?ver=rvLsaCQ_njLmPDrNIFJBWQ%3d%3d.</rdfs:comment>
        <owl:versionInfo>page 102</owl:versionInfo>
    </owl:Class>
    


    <!-- https://savage.nps.edu/EthicalControl/ontologies/MissionExecutionOntology#Reference22_SURFDEVRON1 -->

    <owl:Class rdf:about="https://savage.nps.edu/EthicalControl/ontologies/MissionExecutionOntology#Reference22_SURFDEVRON1">
        <rdfs:subClassOf rdf:resource="https://savage.nps.edu/EthicalControl/ontologies/MissionExecutionOntology#DADM_References"/>
        <rdfs:comment>TODO: Get description from reference document and put it here

&quot;Surface Development Squadron One (SURFDEVRON 1).&quot; https://www.surfpac.navy.mil/surfdevron1/</rdfs:comment>
        <owl:versionInfo>page 102</owl:versionInfo>
    </owl:Class>
    


    <!-- https://savage.nps.edu/EthicalControl/ontologies/MissionExecutionOntology#Reference23_UUVRON1 -->

    <owl:Class rdf:about="https://savage.nps.edu/EthicalControl/ontologies/MissionExecutionOntology#Reference23_UUVRON1">
        <rdfs:subClassOf rdf:resource="https://savage.nps.edu/EthicalControl/ontologies/MissionExecutionOntology#DADM_References"/>
        <rdfs:comment>TODO:  Get description from reference document and put it here

&quot;Unmanned Underwater Vehicle Squadron One (UUVRON 1).&quot; https://www.csp.navy.mil/csds5/Detachments/Detachment-Unmanned-Undersea-Vehicles/.</rdfs:comment>
        <owl:versionInfo>page 102</owl:versionInfo>
    </owl:Class>
    


    <!-- https://savage.nps.edu/EthicalControl/ontologies/MissionExecutionOntology#Reference24_OPNAV5400 -->

    <owl:Class rdf:about="https://savage.nps.edu/EthicalControl/ontologies/MissionExecutionOntology#Reference24_OPNAV5400">
        <rdfs:subClassOf rdf:resource="https://savage.nps.edu/EthicalControl/ontologies/MissionExecutionOntology#DADM_References"/>
        <rdfs:comment>TODO:  Get description from reference document and put it here

OPNAV Notice 5400. August 20, 2020. Establish Commanding Officer, Unmanned Carrier Launched Multi-role Squadron One Zero. https://www.secnav.navy.mil/doni/Directives/05000%20General%20Management%20Security%20and%20Safety%20Services/05-400%20Organization%20and%20Functional%20Support%20Services/5400.2288%20(20).pdf</rdfs:comment>
        <owl:versionInfo>page 102</owl:versionInfo>
    </owl:Class>
    


    <!-- https://savage.nps.edu/EthicalControl/ontologies/MissionExecutionOntology#Reference25_NATO -->

    <owl:Class rdf:about="https://savage.nps.edu/EthicalControl/ontologies/MissionExecutionOntology#Reference25_NATO">
        <rdfs:subClassOf rdf:resource="https://savage.nps.edu/EthicalControl/ontologies/MissionExecutionOntology#DADM_References"/>
        <rdfs:comment>TODO:  Get description from reference document and put it here

Bosch, Karel van den, and Adelbert Bronkhorst. Human-AI Cooperation to Benefit Military Decision Making. North Atlantic Treaty Organization. STO-MP-IST-160. https://www.google.com/url?sa=t&amp;rct=j&amp;q=&amp;esrc=s&amp;source=web&amp;cd=&amp;ved=2ahUKEwj3qcTugtTyAhWCv54KHTbyCIIQFnoECBwQAQ&amp;url=https%3A%2F%2Fwww.sto.nato.int%2Fpublications%2FSTO%2520Meeting%2520Proceedings%2FSTO-MP-IST-160%2FMP-IST-160-S3-1.pdf&amp;usg=AOvVaw2kiRBQmXTFyA19rlG1ZZaE.</rdfs:comment>
        <owl:versionInfo>page 102</owl:versionInfo>
    </owl:Class>
    


    <!-- https://savage.nps.edu/EthicalControl/ontologies/MissionExecutionOntology#Reference26_DoNCIODARPA -->

    <owl:Class rdf:about="https://savage.nps.edu/EthicalControl/ontologies/MissionExecutionOntology#Reference26_DoNCIODARPA">
        <rdfs:subClassOf rdf:resource="https://savage.nps.edu/EthicalControl/ontologies/MissionExecutionOntology#DADM_References"/>
        <rdfs:comment>TODO:  Get description from reference document and put it here

DARPA News. &quot;Creating Cross-Domain Kill Webs in Real Time.&quot; CHIPS: The Department of the Navy&apos;s Information Technology Magazine. Sept. 21, 2020. https://www.doncio.navy.mil/chips/ArticleDetails.aspx?ID=13872.</rdfs:comment>
        <owl:versionInfo>page 102</owl:versionInfo>
    </owl:Class>
    


    <!-- https://savage.nps.edu/EthicalControl/ontologies/MissionExecutionOntology#Reference27_USNTacticalCloud -->

    <owl:Class rdf:about="https://savage.nps.edu/EthicalControl/ontologies/MissionExecutionOntology#Reference27_USNTacticalCloud">
        <rdfs:subClassOf rdf:resource="https://savage.nps.edu/EthicalControl/ontologies/MissionExecutionOntology#DADM_References"/>
        <rdfs:comment>TODO:  Get description from reference document and put it here

Dalton, Andy. &quot;The Navy&apos;s New Cloud Network Forms a Tactical &apos;Kill Web&apos;.&quot; Engadget. May 19, 2016. https://www.engadget.com/2016-05-19-us-navy-tactical-cloud-network-kill-web.html.</rdfs:comment>
        <owl:versionInfo>page 102</owl:versionInfo>
    </owl:Class>
    


    <!-- https://savage.nps.edu/EthicalControl/ontologies/MissionExecutionOntology#Reference28_KillWeb -->

    <owl:Class rdf:about="https://savage.nps.edu/EthicalControl/ontologies/MissionExecutionOntology#Reference28_KillWeb">
        <rdfs:subClassOf rdf:resource="https://savage.nps.edu/EthicalControl/ontologies/MissionExecutionOntology#DADM_References"/>
        <rdfs:comment>TODO:  Get description from reference document and put it here

Osborn, Kris. &quot;Kill Web: Why the U.S. Military Sees Speed as the Ultimate Weapon.&quot; The National Interest. Dec. 20, 2020. https://nationalinterest.org/blog/buzz/kill-web-why-us-military-sees-speed-ultimate-weapon-174769.</rdfs:comment>
        <owl:versionInfo>page 102</owl:versionInfo>
    </owl:Class>
    


    <!-- https://savage.nps.edu/EthicalControl/ontologies/MissionExecutionOntology#Reference29_TFRoleOfAutonomy -->

    <owl:Class rdf:about="https://savage.nps.edu/EthicalControl/ontologies/MissionExecutionOntology#Reference29_TFRoleOfAutonomy">
        <rdfs:subClassOf rdf:resource="https://savage.nps.edu/EthicalControl/ontologies/MissionExecutionOntology#DADM_References"/>
        <rdfs:comment>TODO:  Get description from reference document and put it here

Murphy, Robin, and James Shields. &quot;Task Force on the Role of Autonomy in the DoD Systems.&quot; Jun. 2012. https://sites.nationalacademies.org/cs/groups/pgasite/documents/webpage/pga_082152.pdf.</rdfs:comment>
        <owl:versionInfo>page 102</owl:versionInfo>
    </owl:Class>
    


    <!-- https://savage.nps.edu/EthicalControl/ontologies/MissionExecutionOntology#Reference30_JPUB1.04 -->

    <owl:Class rdf:about="https://savage.nps.edu/EthicalControl/ontologies/MissionExecutionOntology#Reference30_JPUB1.04">
        <rdfs:subClassOf rdf:resource="https://savage.nps.edu/EthicalControl/ontologies/MissionExecutionOntology#DADM_References"/>
        <rdfs:comment>Joint Publication 1-04. August 2, 2016. Legal Support to Military Operations. https://www.jcs.mil/Portals/36/Documents/Doctrine/pubs/jp1_04.pdf</rdfs:comment>
        <owl:versionInfo>page 103</owl:versionInfo>
    </owl:Class>
    


    <!-- https://savage.nps.edu/EthicalControl/ontologies/MissionExecutionOntology#Reference31_DNI -->

    <owl:Class rdf:about="https://savage.nps.edu/EthicalControl/ontologies/MissionExecutionOntology#Reference31_DNI">
        <rdfs:subClassOf rdf:resource="https://savage.nps.edu/EthicalControl/ontologies/MissionExecutionOntology#DADM_References"/>
        <rdfs:comment>Dan Coats, Director of National Intelligence, and Principal Deputy Director of National Intelligence Susan Gordon. Jan. 16, 2019. The AIM Initiative: A Strategy for Augmenting Intelligence Using Machines. Office of the Director of National Intellegence. https://www.dni.gov/files/ODNI/documents/AIM-Strategy.pdf</rdfs:comment>
    </owl:Class>
    


    <!-- https://savage.nps.edu/EthicalControl/ontologies/MissionExecutionOntology#Reference32_BrittlenessAI -->

    <owl:Class rdf:about="https://savage.nps.edu/EthicalControl/ontologies/MissionExecutionOntology#Reference32_BrittlenessAI">
        <rdfs:subClassOf rdf:resource="https://savage.nps.edu/EthicalControl/ontologies/MissionExecutionOntology#DADM_References"/>
        <rdfs:comment>Cummings, M. L. The Surprising Brittleness of AI. Women Corporate Directors. https://www.womencorporatedirectors.org/WCD/News/JAN-Feb2020/Reality%20Light.pdf.</rdfs:comment>
    </owl:Class>
    


    <!-- https://savage.nps.edu/EthicalControl/ontologies/MissionExecutionOntology#Reference33_CJCSI5123.01H -->

    <owl:Class rdf:about="https://savage.nps.edu/EthicalControl/ontologies/MissionExecutionOntology#Reference33_CJCSI5123.01H">
        <rdfs:subClassOf rdf:resource="https://savage.nps.edu/EthicalControl/ontologies/MissionExecutionOntology#DADM_References"/>
        <rdfs:comment>Chairman of the Joint Chiefs of Staff Instruction (CJCSI) 5123.01H. August 31, 2018. Charter of the Joint Requirements Oversight Council (JROC) and Implementation of the Joint Capabilities Inetegration and Development System (JCIDS) https://www.jcs.mil/Portals/36/Documents/Library/Instructions/CJCSI%205123.01H.pdf?ver=2018-10-26-163922-137</rdfs:comment>
    </owl:Class>
    


    <!-- https://savage.nps.edu/EthicalControl/ontologies/MissionExecutionOntology#Reference34_USNIWarPlanOrange -->

    <owl:Class rdf:about="https://savage.nps.edu/EthicalControl/ontologies/MissionExecutionOntology#Reference34_USNIWarPlanOrange">
        <rdfs:subClassOf rdf:resource="https://savage.nps.edu/EthicalControl/ontologies/MissionExecutionOntology#DADM_References"/>
        <rdfs:comment>Miller, Edward S. 1991. War Plan Orange: The U.S. Strategy to Defeat Japan, 1897–1945. Annapolis, Maryland: United States Naval Institute Press.</rdfs:comment>
    </owl:Class>
    


    <!-- https://savage.nps.edu/EthicalControl/ontologies/MissionExecutionOntology#Reference35_USNWC_Letendre -->

    <owl:Class rdf:about="https://savage.nps.edu/EthicalControl/ontologies/MissionExecutionOntology#Reference35_USNWC_Letendre">
        <rdfs:subClassOf rdf:resource="https://savage.nps.edu/EthicalControl/ontologies/MissionExecutionOntology#DADM_References"/>
        <rdfs:comment>Letendre, Linell A. 2020. &quot;Lethal Autonomous Weapon Systems: Translating Geek Speak for Lawyers.&quot; International Law Studies 96: 274-294. https://digital-commons.usnwc.edu/cgi/viewcontent.cgi?article=2925&amp;context=ils.</rdfs:comment>
    </owl:Class>
    


    <!-- https://savage.nps.edu/EthicalControl/ontologies/MissionExecutionOntology#Reference36_JAIC -->

    <owl:Class rdf:about="https://savage.nps.edu/EthicalControl/ontologies/MissionExecutionOntology#Reference36_JAIC">
        <rdfs:subClassOf rdf:resource="https://savage.nps.edu/EthicalControl/ontologies/MissionExecutionOntology#DADM_References"/>
        <rdfs:comment>JAIC Public Affairs. &quot;Enabling AI Data Readiness in the Department of Defense.&quot; April 1, 2021. https://www.ai.mil/blog_04_01_21_enabling_ai_data_readiness_in_the_dod.html</rdfs:comment>
        <owl:versionInfo>page 103</owl:versionInfo>
    </owl:Class>
    


    <!-- https://savage.nps.edu/EthicalControl/ontologies/MissionExecutionOntology#Reference37_ACLU_Ruane -->

    <owl:Class rdf:about="https://savage.nps.edu/EthicalControl/ontologies/MissionExecutionOntology#Reference37_ACLU_Ruane">
        <rdfs:subClassOf rdf:resource="https://savage.nps.edu/EthicalControl/ontologies/MissionExecutionOntology#DADM_References"/>
        <rdfs:comment>Ruane, Kate (American Civil Liberties Union), Face Recognition Technology Moratorium Coalition Letter, Feb. 16, 2021. https://www.aclu.org/sites/default/files/field_document/02.16.2021_coalition_letter_requesting_federal_moratorium_on_facial_recognition.pdf.</rdfs:comment>
        <owl:versionInfo>page 103</owl:versionInfo>
    </owl:Class>
    


    <!-- https://savage.nps.edu/EthicalControl/ontologies/MissionExecutionOntology#Reference38_EUMassSurveillance -->

    <owl:Class rdf:about="https://savage.nps.edu/EthicalControl/ontologies/MissionExecutionOntology#Reference38_EUMassSurveillance">
        <rdfs:subClassOf rdf:resource="https://savage.nps.edu/EthicalControl/ontologies/MissionExecutionOntology#DADM_References"/>
        <rdfs:comment>Jakubowska, Ella, and Diego Narajo. May 13, 2020. Ban Biometric Mass Surveillance: A Set of Fundamental Rights Demands for the European Commission and EU Member States. European Digital Rights. https://edri.org/our-work/blog-ban-biometric-mass-surveillance/.</rdfs:comment>
        <owl:versionInfo>page 103</owl:versionInfo>
    </owl:Class>
    


    <!-- https://savage.nps.edu/EthicalControl/ontologies/MissionExecutionOntology#Reference39_AINow_Richardson -->

    <owl:Class rdf:about="https://savage.nps.edu/EthicalControl/ontologies/MissionExecutionOntology#Reference39_AINow_Richardson">
        <rdfs:subClassOf rdf:resource="https://savage.nps.edu/EthicalControl/ontologies/MissionExecutionOntology#DADM_References"/>
        <rdfs:comment>Richardson, Rashida. Dec. 2019. Confronting Black Boxes: A Shadow Report of the New York City Automated Decision System Task Force. AI Now Institute. https://ainowinstitute.org/ads-shadowreport-2019.pdf.</rdfs:comment>
        <owl:versionInfo>page 103</owl:versionInfo>
    </owl:Class>
    


    <!-- https://savage.nps.edu/EthicalControl/ontologies/MissionExecutionOntology#Reference40_WarOnTheRocks -->

    <owl:Class rdf:about="https://savage.nps.edu/EthicalControl/ontologies/MissionExecutionOntology#Reference40_WarOnTheRocks">
        <rdfs:subClassOf rdf:resource="https://savage.nps.edu/EthicalControl/ontologies/MissionExecutionOntology#DADM_References"/>
        <rdfs:comment>Stumborg, Michael F. &quot;See You in a Month: AI&apos;s Long Data Tail.&quot; War on the Rocks. Oct. 17, 2019. https://warontherocks.com/2019/10/see-you-in-a-month-ais-long-data-tail/.</rdfs:comment>
        <owl:versionInfo>page 103</owl:versionInfo>
    </owl:Class>
    


    <!-- https://savage.nps.edu/EthicalControl/ontologies/MissionExecutionOntology#Reference41_JCOS_UJTL -->

    <owl:Class rdf:about="https://savage.nps.edu/EthicalControl/ontologies/MissionExecutionOntology#Reference41_JCOS_UJTL">
        <rdfs:subClassOf rdf:resource="https://savage.nps.edu/EthicalControl/ontologies/MissionExecutionOntology#DADM_References"/>
        <rdfs:comment>Joint Chiefs of Staff. May 24, 2021. &quot;Universal Joint Task List.&quot; https://www.jcs.mil/Doctrine/Joint-Training/UJTL/.</rdfs:comment>
        <owl:versionInfo>page 103</owl:versionInfo>
    </owl:Class>
    


    <!-- https://savage.nps.edu/EthicalControl/ontologies/MissionExecutionOntology#Reference42_USPOR_Zhang -->

    <owl:Class rdf:about="https://savage.nps.edu/EthicalControl/ontologies/MissionExecutionOntology#Reference42_USPOR_Zhang">
        <rdfs:subClassOf rdf:resource="https://savage.nps.edu/EthicalControl/ontologies/MissionExecutionOntology#DADM_References"/>
        <rdfs:comment>Zhang, Baobao, and Allan Dafoe. Jan. 2019. Artificial Intelligence: American Attitudes and Trends. Center for the Governance of AI, Future of Humanity Institute, University of Oxford. https://governanceai.github.io/US-Public-Opinion-Report-Jan-2019/executive-summary.html.</rdfs:comment>
        <owl:versionInfo>page 103</owl:versionInfo>
    </owl:Class>
    


    <!-- https://savage.nps.edu/EthicalControl/ontologies/MissionExecutionOntology#Reference43_GoogleMaven -->

    <owl:Class rdf:about="https://savage.nps.edu/EthicalControl/ontologies/MissionExecutionOntology#Reference43_GoogleMaven">
        <rdfs:subClassOf rdf:resource="https://savage.nps.edu/EthicalControl/ontologies/MissionExecutionOntology#DADM_References"/>
        <rdfs:comment>Mitchell, Billy. &quot;Google’s Departure from Project Maven Was a ‘Little Bit of a Canary in a Coal Mine’.&quot; FedScoop. Nov. 5, 2019. https://www.fedscoop.com/google-project-maven-canary-coal-mine/.</rdfs:comment>
        <owl:versionInfo>page 103</owl:versionInfo>
    </owl:Class>
    


    <!-- https://savage.nps.edu/EthicalControl/ontologies/MissionExecutionOntology#Reference44_PoliceMagIED -->

    <owl:Class rdf:about="https://savage.nps.edu/EthicalControl/ontologies/MissionExecutionOntology#Reference44_PoliceMagIED">
        <rdfs:subClassOf rdf:resource="https://savage.nps.edu/EthicalControl/ontologies/MissionExecutionOntology#DADM_References"/>
        <rdfs:comment>Corderre, Michael, and Michael Register. &quot;Fighting Back Against IEDs.&quot; Police Magazine. Sept. 17, 2009. https://www.policemag.com/340191/fighting-back-against-ieds.</rdfs:comment>
        <owl:versionInfo>page 103</owl:versionInfo>
    </owl:Class>
    


    <!-- https://savage.nps.edu/EthicalControl/ontologies/MissionExecutionOntology#Reference45_UNMAS -->

    <owl:Class rdf:about="https://savage.nps.edu/EthicalControl/ontologies/MissionExecutionOntology#Reference45_UNMAS">
        <rdfs:subClassOf rdf:resource="https://savage.nps.edu/EthicalControl/ontologies/MissionExecutionOntology#DADM_References"/>
        <rdfs:comment>&quot;Improvised Explosive Device Lexicon.&quot; United Nations Mine Action Service. https://unmas.org/sites/default/files/unmas_ied_lexicon_0.pdf.</rdfs:comment>
        <owl:versionInfo>page 103</owl:versionInfo>
    </owl:Class>
    


    <!-- https://savage.nps.edu/EthicalControl/ontologies/MissionExecutionOntology#Reference46_ICRedCross -->

    <owl:Class rdf:about="https://savage.nps.edu/EthicalControl/ontologies/MissionExecutionOntology#Reference46_ICRedCross">
        <rdfs:subClassOf rdf:resource="https://savage.nps.edu/EthicalControl/ontologies/MissionExecutionOntology#DADM_References"/>
        <rdfs:comment>International Committee of the Red Cross. March 2016. Autonomous Weapon Systems: Implications of Increasing Autonomy in the Critical Functions of Weapons. https://icrcndresourcecentre.org/wp-content/uploads/2017/11/4283_002_Autonomus-Weapon-Systems_WEB.pdf.</rdfs:comment>
        <owl:versionInfo>page 103</owl:versionInfo>
    </owl:Class>
    


    <!-- https://savage.nps.edu/EthicalControl/ontologies/MissionExecutionOntology#Reference47_IPRAW -->

    <owl:Class rdf:about="https://savage.nps.edu/EthicalControl/ontologies/MissionExecutionOntology#Reference47_IPRAW">
        <rdfs:subClassOf rdf:resource="https://savage.nps.edu/EthicalControl/ontologies/MissionExecutionOntology#DADM_References"/>
        <rdfs:comment>International Panel on the Regulation of Autonomous Weapons. May 2020. A Path Toward the Regulation of LAWS. https://www.ipraw.org/wp-content/uploads/2020/05/iPRAW-Briefing_Path-to-Regulation_May2020.pdf</rdfs:comment>
        <owl:versionInfo>page 104</owl:versionInfo>
    </owl:Class>
    


    <!-- https://savage.nps.edu/EthicalControl/ontologies/MissionExecutionOntology#Reference48_DoDPrinciplesCEWS -->

    <owl:Class rdf:about="https://savage.nps.edu/EthicalControl/ontologies/MissionExecutionOntology#Reference48_DoDPrinciplesCEWS">
        <rdfs:subClassOf rdf:resource="https://savage.nps.edu/EthicalControl/ontologies/MissionExecutionOntology#DADM_References"/>
        <rdfs:comment>Work, Robert O. April 2021. Principles for the Combat Employment of Weapon Systems with Autonomous Functionalities. Center for a New American Security. https://www.cnas.org/publications/reports/proposed-dod-principles-for-the-combat-employment-of-weapon-systems-with-autonomous-functionalities</rdfs:comment>
        <owl:versionInfo>page 104</owl:versionInfo>
    </owl:Class>
    


    <!-- https://savage.nps.edu/EthicalControl/ontologies/MissionExecutionOntology#Reference49_TamingKillerRobots -->

    <owl:Class rdf:about="https://savage.nps.edu/EthicalControl/ontologies/MissionExecutionOntology#Reference49_TamingKillerRobots">
        <rdfs:subClassOf rdf:resource="https://savage.nps.edu/EthicalControl/ontologies/MissionExecutionOntology#DADM_References"/>
        <rdfs:comment>Cook, Adam. 2019. Taming Killer Robots: Giving Meaning to the &quot;Meaningful Human Control&quot; Standard for Lethal Autonomous Weapons Systems. Air University Press, Curtis E. LeMay Center for Doctrine Development and Education. JAG School Paper, no. 1. https://media.defense.gov/2019/Jun/18/2002146749/-1/-1/0/JP_001_COOK_TAMING_KILLER_ROBOTS.PDF</rdfs:comment>
        <owl:versionInfo>page 104</owl:versionInfo>
    </owl:Class>
    


    <!-- https://savage.nps.edu/EthicalControl/ontologies/MissionExecutionOntology#RehearsalConstraint -->

    <owl:Class rdf:about="https://savage.nps.edu/EthicalControl/ontologies/MissionExecutionOntology#RehearsalConstraint">
        <rdfs:subClassOf rdf:resource="https://savage.nps.edu/EthicalControl/ontologies/MissionExecutionOntology#DADM_Constraints"/>
    </owl:Class>
    


    <!-- https://savage.nps.edu/EthicalControl/ontologies/MissionExecutionOntology#RuleOfEngagementConstraint -->

    <owl:Class rdf:about="https://savage.nps.edu/EthicalControl/ontologies/MissionExecutionOntology#RuleOfEngagementConstraint">
        <rdfs:subClassOf rdf:resource="https://savage.nps.edu/EthicalControl/ontologies/MissionExecutionOntology#OperationalConstraint"/>
    </owl:Class>
    


    <!-- https://savage.nps.edu/EthicalControl/ontologies/MissionExecutionOntology#SJA -->

    <owl:Class rdf:about="https://savage.nps.edu/EthicalControl/ontologies/MissionExecutionOntology#SJA">
        <rdfs:subClassOf rdf:resource="https://savage.nps.edu/EthicalControl/ontologies/MissionExecutionOntology#DADM_Abbreviations"/>
        <rdfs:label>Staff Judge Advocate (SJA)</rdfs:label>
        <owl:versionInfo>page 100</owl:versionInfo>
    </owl:Class>
    


    <!-- https://savage.nps.edu/EthicalControl/ontologies/MissionExecutionOntology#SME -->

    <owl:Class rdf:about="https://savage.nps.edu/EthicalControl/ontologies/MissionExecutionOntology#SME">
        <rdfs:subClassOf rdf:resource="https://savage.nps.edu/EthicalControl/ontologies/MissionExecutionOntology#DADM_Abbreviations"/>
        <rdfs:label>Subject Matter Expert (SME)</rdfs:label>
        <owl:versionInfo>page 100</owl:versionInfo>
    </owl:Class>
    


    <!-- https://savage.nps.edu/EthicalControl/ontologies/MissionExecutionOntology#SUCCESS -->

    <owl:Class rdf:about="https://savage.nps.edu/EthicalControl/ontologies/MissionExecutionOntology#SUCCESS">
        <rdfs:subClassOf rdf:resource="https://savage.nps.edu/EthicalControl/ontologies/MissionExecutionOntology#EndCondition"/>
        <rdfs:comment>The SUCCESS EndCondition indicates that a Goal instance completed and succeeded in meeting all associated IntendedOutcome requirements.</rdfs:comment>
    </owl:Class>
    


    <!-- https://savage.nps.edu/EthicalControl/ontologies/MissionExecutionOntology#SYSCOM -->

    <owl:Class rdf:about="https://savage.nps.edu/EthicalControl/ontologies/MissionExecutionOntology#SYSCOM">
        <rdfs:subClassOf rdf:resource="https://savage.nps.edu/EthicalControl/ontologies/MissionExecutionOntology#DADM_Abbreviations"/>
        <rdfs:label>Systems Command (SYSCOM)</rdfs:label>
        <owl:versionInfo>page 100</owl:versionInfo>
    </owl:Class>
    


    <!-- https://savage.nps.edu/EthicalControl/ontologies/MissionExecutionOntology#TTP -->

    <owl:Class rdf:about="https://savage.nps.edu/EthicalControl/ontologies/MissionExecutionOntology#TTP">
        <rdfs:subClassOf rdf:resource="https://savage.nps.edu/EthicalControl/ontologies/MissionExecutionOntology#DADM_Abbreviations"/>
        <rdfs:label>Tactics Techniques Procedures (TTP)</rdfs:label>
        <owl:versionInfo>page 100</owl:versionInfo>
    </owl:Class>
    


    <!-- https://savage.nps.edu/EthicalControl/ontologies/MissionExecutionOntology#TemporalConstraint -->

    <owl:Class rdf:about="https://savage.nps.edu/EthicalControl/ontologies/MissionExecutionOntology#TemporalConstraint">
        <rdfs:subClassOf rdf:resource="https://savage.nps.edu/EthicalControl/ontologies/MissionExecutionOntology#OperationalConstraint"/>
        <rdfs:subClassOf rdf:resource="https://savage.nps.edu/EthicalControl/ontologies/MissionExecutionOntology#PolicyConstraint"/>
    </owl:Class>
    


    <!-- https://savage.nps.edu/EthicalControl/ontologies/MissionExecutionOntology#UJTL -->

    <owl:Class rdf:about="https://savage.nps.edu/EthicalControl/ontologies/MissionExecutionOntology#UJTL">
        <rdfs:subClassOf rdf:resource="https://savage.nps.edu/EthicalControl/ontologies/MissionExecutionOntology#DADM_Abbreviations"/>
        <rdfs:label>Universal Joint Task List (UJTL)</rdfs:label>
        <owl:versionInfo>page 100</owl:versionInfo>
    </owl:Class>
    


    <!-- https://savage.nps.edu/EthicalControl/ontologies/MissionExecutionOntology#USPolicy -->

    <owl:Class rdf:about="https://savage.nps.edu/EthicalControl/ontologies/MissionExecutionOntology#USPolicy">
        <rdfs:subClassOf rdf:resource="https://savage.nps.edu/EthicalControl/ontologies/MissionExecutionOntology#LegalConstraint"/>
    </owl:Class>
    


    <!-- https://savage.nps.edu/EthicalControl/ontologies/MissionExecutionOntology#UxS -->

    <owl:Class rdf:about="https://savage.nps.edu/EthicalControl/ontologies/MissionExecutionOntology#UxS">
        <rdfs:subClassOf rdf:resource="https://savage.nps.edu/EthicalControl/ontologies/MissionExecutionOntology#DADM_Abbreviations"/>
        <rdfs:label>Unmanned System (UxS)</rdfs:label>
        <owl:versionInfo>page 100</owl:versionInfo>
    </owl:Class>
    


    <!-- https://savage.nps.edu/EthicalControl/ontologies/MissionExecutionOntology#Vehicle -->

    <owl:Class rdf:about="https://savage.nps.edu/EthicalControl/ontologies/MissionExecutionOntology#Vehicle">
        <rdfs:subClassOf>
            <owl:Restriction>
                <owl:onProperty rdf:resource="https://savage.nps.edu/EthicalControl/ontologies/MissionExecutionOntology#canAchieve"/>
                <owl:allValuesFrom rdf:resource="https://savage.nps.edu/EthicalControl/ontologies/MissionExecutionOntology#IntendedOutcome"/>
            </owl:Restriction>
        </rdfs:subClassOf>
        <rdfs:subClassOf>
            <owl:Restriction>
                <owl:onProperty rdf:resource="https://savage.nps.edu/EthicalControl/ontologies/MissionExecutionOntology#canIdentify"/>
                <owl:allValuesFrom rdf:resource="https://savage.nps.edu/EthicalControl/ontologies/MissionExecutionOntology#DADM_Constraints"/>
            </owl:Restriction>
        </rdfs:subClassOf>
        <rdfs:subClassOf>
            <owl:Restriction>
                <owl:onProperty rdf:resource="https://savage.nps.edu/EthicalControl/ontologies/MissionExecutionOntology#canMeet"/>
                <owl:allValuesFrom rdf:resource="https://savage.nps.edu/EthicalControl/ontologies/MissionExecutionOntology#Goal"/>
            </owl:Restriction>
        </rdfs:subClassOf>
        <rdfs:subClassOf>
            <owl:Restriction>
                <owl:onProperty rdf:resource="https://savage.nps.edu/EthicalControl/ontologies/MissionExecutionOntology#canPerform"/>
                <owl:allValuesFrom rdf:resource="https://savage.nps.edu/EthicalControl/ontologies/MissionExecutionOntology#Mission"/>
            </owl:Restriction>
        </rdfs:subClassOf>
        <rdfs:subClassOf>
            <owl:Restriction>
                <owl:onProperty rdf:resource="https://savage.nps.edu/EthicalControl/ontologies/MissionExecutionOntology#hasFeature"/>
                <owl:allValuesFrom rdf:resource="https://savage.nps.edu/EthicalControl/ontologies/MissionExecutionOntology#VehicleFeature"/>
            </owl:Restriction>
        </rdfs:subClassOf>
        <rdfs:comment>A Vehicle is a physical device for performing a Mission, requiring the Vehicle to be able to meet Mission goals, under associated Contraints, using VehicleFeature instances that can meet assigned IntendedOutcome instances by being able to measure conformance to the associated Constraints.</rdfs:comment>
    </owl:Class>
    <owl:Axiom>
        <owl:annotatedSource rdf:resource="https://savage.nps.edu/EthicalControl/ontologies/MissionExecutionOntology#Vehicle"/>
        <owl:annotatedProperty rdf:resource="http://www.w3.org/2000/01/rdf-schema#subClassOf"/>
        <owl:annotatedTarget>
            <owl:Restriction>
                <owl:onProperty rdf:resource="https://savage.nps.edu/EthicalControl/ontologies/MissionExecutionOntology#hasFeature"/>
                <owl:allValuesFrom rdf:resource="https://savage.nps.edu/EthicalControl/ontologies/MissionExecutionOntology#VehicleFeature"/>
            </owl:Restriction>
        </owl:annotatedTarget>
        <rdfs:comment>A Vehicle can have 0 or more VehicleFeatures.</rdfs:comment>
        <rdfs:comment>isPerformableBy and canPerform are inversely equivalent.</rdfs:comment>
        <rdfs:label>V1</rdfs:label>
        <rdfs:label>V2</rdfs:label>
    </owl:Axiom>
    


    <!-- https://savage.nps.edu/EthicalControl/ontologies/MissionExecutionOntology#VehicleFeature -->

    <owl:Class rdf:about="https://savage.nps.edu/EthicalControl/ontologies/MissionExecutionOntology#VehicleFeature">
        <rdfs:subClassOf>
            <owl:Restriction>
                <owl:onProperty rdf:resource="https://savage.nps.edu/EthicalControl/ontologies/MissionExecutionOntology#canFulfill"/>
                <owl:allValuesFrom rdf:resource="https://savage.nps.edu/EthicalControl/ontologies/MissionExecutionOntology#IntendedOutcome"/>
            </owl:Restriction>
        </rdfs:subClassOf>
        <rdfs:subClassOf>
            <owl:Restriction>
                <owl:onProperty rdf:resource="https://savage.nps.edu/EthicalControl/ontologies/MissionExecutionOntology#canMeasure"/>
                <owl:allValuesFrom rdf:resource="https://savage.nps.edu/EthicalControl/ontologies/MissionExecutionOntology#EndCondition"/>
            </owl:Restriction>
        </rdfs:subClassOf>
        <rdfs:comment>A VehicleFeature is a capability associated with a Vehicle that is able to fulfill IntendedOutcome instances required by Goals in a Mission, and is able to test the conditions defined in each Mission or Goal Constraint to determine if an exception to the constraint will occur.</rdfs:comment>
    </owl:Class>
    <owl:Axiom>
        <owl:annotatedSource rdf:resource="https://savage.nps.edu/EthicalControl/ontologies/MissionExecutionOntology#VehicleFeature"/>
        <owl:annotatedProperty rdf:resource="http://www.w3.org/2000/01/rdf-schema#subClassOf"/>
        <owl:annotatedTarget>
            <owl:Restriction>
                <owl:onProperty rdf:resource="https://savage.nps.edu/EthicalControl/ontologies/MissionExecutionOntology#canFulfill"/>
                <owl:allValuesFrom rdf:resource="https://savage.nps.edu/EthicalControl/ontologies/MissionExecutionOntology#IntendedOutcome"/>
            </owl:Restriction>
        </owl:annotatedTarget>
        <rdfs:comment>A VehicleFeature may be able to fulfill 0 or more GoalRequirements.</rdfs:comment>
        <rdfs:label>F1</rdfs:label>
    </owl:Axiom>
    <owl:Axiom>
        <owl:annotatedSource rdf:resource="https://savage.nps.edu/EthicalControl/ontologies/MissionExecutionOntology#VehicleFeature"/>
        <owl:annotatedProperty rdf:resource="http://www.w3.org/2000/01/rdf-schema#subClassOf"/>
        <owl:annotatedTarget>
            <owl:Restriction>
                <owl:onProperty rdf:resource="https://savage.nps.edu/EthicalControl/ontologies/MissionExecutionOntology#canMeasure"/>
                <owl:allValuesFrom rdf:resource="https://savage.nps.edu/EthicalControl/ontologies/MissionExecutionOntology#EndCondition"/>
            </owl:Restriction>
        </owl:annotatedTarget>
        <rdfs:comment>A VehicleFeature may be able to test 0 or more constraints.</rdfs:comment>
        <rdfs:label>F2</rdfs:label>
    </owl:Axiom>
    


    <!-- https://savage.nps.edu/EthicalControl/ontologies/MissionExecutionOntology#R&amp;D -->

    <owl:Class rdf:about="https://savage.nps.edu/EthicalControl/ontologies/MissionExecutionOntology#R&amp;D">
        <rdfs:subClassOf rdf:resource="https://savage.nps.edu/EthicalControl/ontologies/MissionExecutionOntology#DADM_Abbreviations"/>
        <rdfs:label>Research &amp; Development (R&amp;D)</rdfs:label>
        <owl:versionInfo>page 100</owl:versionInfo>
    </owl:Class>
    


    <!-- https://savage.nps.edu/EthicalControl/ontologies/MissionExecutionOntology#T&amp;E -->

    <owl:Class rdf:about="https://savage.nps.edu/EthicalControl/ontologies/MissionExecutionOntology#T&amp;E">
        <rdfs:subClassOf rdf:resource="https://savage.nps.edu/EthicalControl/ontologies/MissionExecutionOntology#DADM_Abbreviations"/>
        <rdfs:label>Test and Evaluation (T&amp;E)</rdfs:label>
        <owl:versionInfo>page 100</owl:versionInfo>
    </owl:Class>
    


    <!-- 
    ///////////////////////////////////////////////////////////////////////////////////////
    //
    // Annotations
    //
    ///////////////////////////////////////////////////////////////////////////////////////
     -->

    <rdf:Description rdf:about="http://www.w3.org/2002/07/owl#topObjectProperty">
        <owl:versionInfo rdf:datatype="http://www.w3.org/2001/XMLSchema#decimal">3.1</owl:versionInfo>
    </rdf:Description>
    


    <!-- 
    ///////////////////////////////////////////////////////////////////////////////////////
    //
    // General axioms
    //
    ///////////////////////////////////////////////////////////////////////////////////////
     -->

    <rdf:Description>
        <rdf:type rdf:resource="http://www.w3.org/2002/07/owl#AllDisjointClasses"/>
        <owl:members rdf:parseType="Collection">
            <rdf:Description rdf:about="https://savage.nps.edu/EthicalControl/ontologies/MissionExecutionOntology#DADM_Constraints"/>
            <rdf:Description rdf:about="https://savage.nps.edu/EthicalControl/ontologies/MissionExecutionOntology#EndCondition"/>
            <rdf:Description rdf:about="https://savage.nps.edu/EthicalControl/ontologies/MissionExecutionOntology#Goal"/>
            <rdf:Description rdf:about="https://savage.nps.edu/EthicalControl/ontologies/MissionExecutionOntology#IntendedOutcome"/>
            <rdf:Description rdf:about="https://savage.nps.edu/EthicalControl/ontologies/MissionExecutionOntology#Mission"/>
            <rdf:Description rdf:about="https://savage.nps.edu/EthicalControl/ontologies/MissionExecutionOntology#Vehicle"/>
            <rdf:Description rdf:about="https://savage.nps.edu/EthicalControl/ontologies/MissionExecutionOntology#VehicleFeature"/>
        </owl:members>
    </rdf:Description>
    <rdf:Description>
        <rdf:type rdf:resource="http://www.w3.org/2002/07/owl#AllDisjointClasses"/>
        <owl:members rdf:parseType="Collection">
            <rdf:Description rdf:about="https://savage.nps.edu/EthicalControl/ontologies/MissionExecutionOntology#EXCEPTION"/>
            <rdf:Description rdf:about="https://savage.nps.edu/EthicalControl/ontologies/MissionExecutionOntology#FAILURE"/>
            <rdf:Description rdf:about="https://savage.nps.edu/EthicalControl/ontologies/MissionExecutionOntology#SUCCESS"/>
        </owl:members>
    </rdf:Description>
</rdf:RDF>



<!-- Generated by the OWL API (version 4.5.9.2019-02-01T07:24:44Z) https://github.com/owlcs/owlapi -->

